@prefix : <http://pi.pauwel.be/voc/buildingelement#> .
@prefix vs: <http://www.w3.org/2003/06/sw-vocab-status/ns#> .
@prefix beo: <http://pi.pauwel.be/voc/buildingelement#> .
@prefix dce: <http://purl.org/dc/elements/1.1/> .
@prefix ifc: <http://www.buildingsmart-tech.org/ifcOWL/IFC4_ADD2#> .
@prefix owl: <http://www.w3.org/2002/07/owl#> .
@prefix rdf: <http://www.w3.org/1999/02/22-rdf-syntax-ns#> .
@prefix xml: <http://www.w3.org/XML/1998/namespace> .
@prefix xsd: <http://www.w3.org/2001/XMLSchema#> .
@prefix foaf: <http://xmlns.com/foaf/0.1/> .
@prefix rdfs: <http://www.w3.org/2000/01/rdf-schema#> .
@prefix vann: <http://purl.org/vocab/vann/> .
@prefix voaf: <http://purl.org/vocommons/voaf#> .
@prefix dcterms: <http://purl.org/dc/terms/> .
@base <http://pi.pauwel.be/voc/buildingelement> .

<http://pi.pauwel.be/voc/buildingelement> rdf:type owl:Ontology ;
                                           dce:Language "en" ;
                                           dce:description "The Building Element Ontology provides an ontology based on the IfcBuildingElement subtree in the IFC specification, containing a taxonomy of classes that allow to define common building elements."@en ;
                                           dce:modified "December 27th 2018" ;
                                           dce:title "Building Element Ontology" ;
                                           dcterms:creator [ rdf:type foaf:Person ;
                                                             foaf:name "Pieter Pauwels"
                                                           ] ;
                                           dcterms:description "The Building Element Ontology provides an ontology based on the IfcBuildingElement subtree in the IFC specification, containing a taxonomy of classes that allow to define common building elements."@en ;
                                           dcterms:issued "2018-12-27"^^xsd:date ;
                                           dcterms:license <https://creativecommons.org/licenses/by/1.0/> ;
                                           dcterms:title "Building Element Ontology"@en ;
                                           vann:preferredNamespacePrefix "beo" ;
                                           vann:preferredNamespaceUri beo: ;
                                           owl:versionInfo "December 27th 2018" ,
                                                           "v0.1.0" .

#################################################################
#    Annotation properties
#################################################################

###  http://purl.org/dc/elements/1.1/Language
dce:Language rdf:type owl:AnnotationProperty .


###  http://purl.org/dc/elements/1.1/description
dce:description rdf:type owl:AnnotationProperty .


###  http://purl.org/dc/elements/1.1/modified
dce:modified rdf:type owl:AnnotationProperty .


###  http://purl.org/dc/elements/1.1/title
dce:title rdf:type owl:AnnotationProperty .


###  http://purl.org/dc/terms/contributor
dcterms:contributor rdf:type owl:AnnotationProperty .


###  http://purl.org/dc/terms/creator
dcterms:creator rdf:type owl:AnnotationProperty .


###  http://purl.org/dc/terms/description
dcterms:description rdf:type owl:AnnotationProperty .


###  http://purl.org/dc/terms/issued
dcterms:issued rdf:type owl:AnnotationProperty .


###  http://purl.org/dc/terms/license
dcterms:license rdf:type owl:AnnotationProperty .


###  http://purl.org/dc/terms/modified
dcterms:modified rdf:type owl:AnnotationProperty .


###  http://purl.org/dc/terms/title
dcterms:title rdf:type owl:AnnotationProperty .


###  http://purl.org/vocab/vann/preferredNamespacePrefix
vann:preferredNamespacePrefix rdf:type owl:AnnotationProperty .


###  http://purl.org/vocab/vann/preferredNamespaceUri
vann:preferredNamespaceUri rdf:type owl:AnnotationProperty .


###  http://www.w3.org/2003/06/sw-vocab-status/ns#term_status
vs:term_status rdf:type owl:AnnotationProperty .


#################################################################
#    Data properties
#################################################################

###  http://xmlns.com/foaf/0.1/name
foaf:name rdf:type owl:DatatypeProperty .


#################################################################
#    Classes
#################################################################

###  http://pi.pauwel.be/voc/buildingelement#Beam
beo:Beam rdf:type owl:Class ;
         rdfs:subClassOf beo:BuildingElement ;
         rdfs:comment "A horizontal, or nearly horizontal, structural member that is capable of withstanding load primarily by resisting bending. It represents such a member from an architectural point of view. It is not required to be load bearing."@en ,
                      "A standard beam usually used horizontally."@nb-no ,
                      "http://bsdd.buildingsmart.org/#concept/details/3zXEi0qSCHuO00025QrE$V"@en ;
         rdfs:label "Balk"@nl ,
                    "Beam"@en ,
                    "Bjælke"@da ,
                    "balken"@de-de ,
                    "biegeträger"@de-de ,
                    "bjelke"@nb-no ,
                    "poutre"@fr-fr ;
         rdfs:seeAlso ifc:IfcBeam .


###  http://pi.pauwel.be/voc/buildingelement#Beam-BEAM
beo:Beam-BEAM rdf:type owl:Class ;
              rdfs:subClassOf beo:Beam ;
              rdfs:comment "A horizontal, or nearly horizontal, structural member that is capable of withstanding load primarily by resisting bending. It represents such a member from an architectural point of view. It is not required to be load bearing."@en ,
                           "A standard beam usually used horizontally."@nb-no ,
                           "http://bsdd.buildingsmart.org/#concept/details/0KKIHMGYH7H8MAfgxbrxuV"@en ;
              rdfs:label "Beam"@en ,
                         "balk"@nl-nl ,
                         "balken"@de-de ,
                         "biegeträger"@de-de ,
                         "bjelke"@nb-no ,
                         "ligger"@nl-nl ,
                         "poutre"@fr-fr ;
              rdfs:seeAlso ifc:IfcBeamEnumType .


###  http://pi.pauwel.be/voc/buildingelement#Beam-HOLLOWCORE
beo:Beam-HOLLOWCORE rdf:type owl:Class ;
                    rdfs:subClassOf beo:Beam ;
                    rdfs:comment "Platte mit rechteckigem Querschnitt, in der auf voller Länge in Längsrichtung kreisrunde oder ovale Hohlräume (Aussparungen) verlaufen"@de-de ,
                                 "dalle de section rectangulaire comportant des vides longitudinaux sur toute leur longueur ou des vides de forme ovale"@fr-fr ,
                                 "http://bsdd.buildingsmart.org/#concept/details/2gzZKHqELB$gPVKajRAFXc"@en ,
                                 "losa de sección rectangular con huecos circulares o óvales para toda su longitud"@es-es ,
                                 "monolithic prestressed or reinforced elements with a constant overall depth divided into an upper and lower flange, linked by vertical webs, so constituting cores as longitudinal voids the cross section of which is constant and presents one vertical axis."@en ,
                                 "prostokątna płyta z okrągłymi lub owalnymi przestrzeniami na całej długości"@pl-pl ,
                                 "rectangular section slab with full-length longitudinal circular or oval shaped voids"@en-gb ,
                                 "rectangular section slab with full-length longitudinal circular or oval shaped voids."@en ,
                                 "rektangulärt bjälklag med längsgående cirkelformade eller ovalformade tomrum längs med hela bjälklaget"@sv-se ,
                                 "rektangulært element med hulrum i fuld længde i langsgående, cirkulær eller oval form"@dk-dk ,
                                 "rektangulært element med langsgående sirkulære eller ovale hulrom i full lengde"@nb-no ,
                                 "suorakaiteenmuotoinen laattaelementti, jossa on koko pituudeltaan pyöreitä tai ovaalinmuotoisia onteloita/tyhjätiloja"@fi-fi ,
                                 "плоча с правоъгълно сечение и кухини по цялата дължина с надлъжна кръгла или овална форма "@bg-bg ;
                    rdfs:label "Pre-cast Hollow Core Slab"@en ,
                               "dalle alvéolée préfabriquée en béton"@fr-fr ,
                               "förtillverkade betongprodukter - håldäcksplattor"@sv-se ,
                               "hulldekke"@nb-no ,
                               "hulldekkeelement"@nb-no ,
                               "lastre alveolari precompresse"@it-it ,
                               "losa alveolar prefabricada"@es-es ,
                               "ontelolaatta"@fi-fi ,
                               "pre-cast hollow core slab"@en-gb ,
                               "prefabrikkert hulldekke"@nb-no ,
                               "prefabrykowana płyta kanałowa stropowa"@pl-pl ,
                               "præfabrikeret huldækelement"@dk-dk ,
                               "werkseitig hergestellte Hohlplatte"@de-de ,
                               "готови плочи с кухини"@bg-bg ;
                    rdfs:seeAlso ifc:IfcBeamEnumType .


###  http://pi.pauwel.be/voc/buildingelement#Beam-JOIST
beo:Beam-JOIST rdf:type owl:Class ;
               rdfs:subClassOf beo:Beam ;
               rdfs:comment "http://bsdd.buildingsmart.org/#concept/details/1_zkjNhS95oA5oDSSTnEvO"@en ;
               rdfs:label "Joiste"@en ,
                          "tilpasset bjelke"@nb-no ;
               rdfs:seeAlso ifc:IfcBeamEnumType .


###  http://pi.pauwel.be/voc/buildingelement#Beam-LINTEL
beo:Beam-LINTEL rdf:type owl:Class ;
                rdfs:subClassOf beo:Beam ;
                rdfs:comment "http://bsdd.buildingsmart.org/#concept/details/1PivEYC0575QGoaAFjN8c9"@en ;
                rdfs:label "Lintel"@en ,
                           "overdekking"@nb-no ;
                rdfs:seeAlso ifc:IfcBeamEnumType .


###  http://pi.pauwel.be/voc/buildingelement#Beam-SPANDREL
beo:Beam-SPANDREL rdf:type owl:Class ;
                  rdfs:subClassOf beo:Beam ;
                  rdfs:comment "http://bsdd.buildingsmart.org/#concept/details/2$vr6UW$f3SwHilnemEZoH"@en ;
                  rdfs:label "Spandrel"@en ,
                             "brystning"@nb-no ;
                  rdfs:seeAlso ifc:IfcBeamEnumType .


###  http://pi.pauwel.be/voc/buildingelement#Beam-T_BEAM
beo:Beam-T_BEAM rdf:type owl:Class ;
                rdfs:subClassOf beo:Beam ;
                rdfs:comment "http://bsdd.buildingsmart.org/#concept/details/1o9Up6wBr339DlpjWIWE$l"@en ;
                rdfs:label "T_Beam"@en ,
                           "t_bjelke"@nb-no ;
                rdfs:seeAlso ifc:IfcBeamEnumType .


###  http://pi.pauwel.be/voc/buildingelement#BuildingElement
beo:BuildingElement rdf:type owl:Class ;
                    rdfs:subClassOf <https://schema.org/Product>, <http://purl.org/goodrelations/v1#SomeItems> ;
                    rdfs:comment "Bauelement"@de-de ,
                                 "Comprises all elements that are primarily part of the construction of a building, i.e., its structural and space separating system. Building elements are all physically existent and tangible things."@en ,
                                 "http://bsdd.buildingsmart.org/#concept/details/2AFYKXkEn7RxYuvbduGfUV"@en ;
                    rdfs:label "Bauteil"@de-de ,
                               "Building Element"@en ,
                               "Elément de construction"@fr-fr ;
                    rdfs:seeAlso ifc:IfcBuildingElement .


###  http://pi.pauwel.be/voc/buildingelement#BuildingElementPart
beo:BuildingElementPart rdf:type owl:Class ;
                        rdfs:subClassOf beo:ElementComponent ;
                        rdfs:comment "http://bsdd.buildingsmart.org/#concept/details/3v2S1DH0r50BHIhWE6QHMZ"@en ,
                                     "ifcbuildingelementpart represents major components as subordinate parts of a building element. typical usage examples include precast concrete sandwich walls, where the layers may have different geometry representations. in this case the layered material representation does not sufficiently describe the element. each layer is represented by an own instance of the ifcbuildingelementpart with its own geometry description. the kind of building element part is further specified by a corresponding instance of ifcbuildingelementparttype, referred to by ifcreldefinesbytype."@en ;
                        rdfs:label "Building Element Part"@en ,
                                   "Teil eines Bauelements"@de-de ,
                                   "partie d'élément de construction"@fr-fr ;
                        rdfs:seeAlso ifc:IfcBuildingElementPart .


###  http://pi.pauwel.be/voc/buildingelement#BuildingElementPart-INSULATION
beo:BuildingElementPart-INSULATION rdf:type owl:Class ;
                                   rdfs:subClassOf beo:BuildingElementPart ;
                                   rdfs:comment "http://bsdd.buildingsmart.org/#concept/details/2CF$o8Mgv2_xbw_kioa_YW"@en ;
                                   rdfs:label "Insulation"@en ,
                                              "isolasjon"@nb-no ;
                                   rdfs:seeAlso ifc:IfcBuildingElementPartEnumType .


###  http://pi.pauwel.be/voc/buildingelement#BuildingElementPart-PRECASTPANEL
beo:BuildingElementPart-PRECASTPANEL rdf:type owl:Class ;
                                     rdfs:subClassOf beo:BuildingElementPart ;
                                     rdfs:comment "http://bsdd.buildingsmart.org/#concept/details/0pt2K5QIXB89suCXlsQZw$"@en ;
                                     rdfs:label "Precast Panel"@en ;
                                     rdfs:seeAlso ifc:IfcBuildingElementPartEnumType .


###  http://pi.pauwel.be/voc/buildingelement#Chimney
beo:Chimney rdf:type owl:Class ;
            rdfs:subClassOf beo:BuildingElement ;
            rdfs:comment "A vertical structure of brick, masonry, or steel that carries exhaust gases or steam away from a fire, engine, etc."@en ,
                         "Typically vertical, or as near as vertical, parts of the construction of a building and part of the building fabric. Often constructed by pre-cast or insitu concrete, today seldom by bricks."@en ,
                         "http://bsdd.buildingsmart.org/#concept/details/0xE4A0qSaHuO00025QrE$V"@en ,
                         "konstruksjon bestående av én eller flere vegger som omslutter én eller flere røykkanaler"@nb-no ,
                         "structure consisting of a wall or walls enclosing  a flue or flues"@en ;
            rdfs:label "Abgasanlage"@de-de ,
                       "Abgassanlage"@de-de ,
                       "Chimney"@en ,
                       "Schoorsteen"@nl ,
                       "Schoorsteen"@nl-nl ,
                       "Schornstein"@de-de ,
                       "Skorsten"@da ,
                       "cheminée"@fr-fr ,
                       "conduit de fumée"@fr-fr ,
                       "pipe"@nb-no ,
                       "skorstein"@nb-no ;
            rdfs:seeAlso ifc:IfcChimney .


###  http://pi.pauwel.be/voc/buildingelement#Column
beo:Column rdf:type owl:Class ;
           rdfs:subClassOf beo:BuildingElement ;
           rdfs:comment "A vertical structural member which often is aligned with a structural grid intersection. It represents a vertical, or nearly vertical, structural member that transmits, through compression, the weight of the structure above to other structural elements below. It represents such a member from an architectural point of view. It is not required to be load bearing."@en ,
                        "http://bsdd.buildingsmart.org/#concept/details/1CDOE0qSeHuO00025QrE$V"@en ;
           rdfs:label "Column"@en ,
                      "Kolom"@nl ,
                      "Stütze / Pfeiler"@de-de ,
                      "Søjle"@da ,
                      "poteau"@fr-fr ;
           rdfs:seeAlso ifc:IfcColumn .


###  http://pi.pauwel.be/voc/buildingelement#Column-COLUMN
beo:Column-COLUMN rdf:type owl:Class ;
                  rdfs:subClassOf beo:Column ;
                  rdfs:comment "A vertical structural member which often is aligned with a structural grid intersection. It represents a vertical, or nearly vertical, structural member that transmits, through compression, the weight of the structure above to other structural elements below. It represents such a member from an architectural point of view. It is not required to be load bearing."@en ,
                               "Søyle"@nb-no ,
                               "http://bsdd.buildingsmart.org/#concept/details/1k5QL8XejA8v7H3XePklst"@en ;
                  rdfs:label "Column"@en ,
                             "Druckstab"@de-de ,
                             "Stütze"@de-de ,
                             "poteau"@fr-fr ;
                  rdfs:seeAlso ifc:IfcColumnEnumType .


###  http://pi.pauwel.be/voc/buildingelement#Column-PILASTER
beo:Column-PILASTER rdf:type owl:Class ;
                    rdfs:subClassOf beo:Column ;
                    rdfs:comment "Pilaster"@nb-no ,
                                 "http://bsdd.buildingsmart.org/#concept/details/08F4W56in3zeQ$ucplQrmF"@en ,
                                 "http://bsdd.buildingsmart.org/#concept/details/312dw0BS8Htm00025QrE$V"@en ,
                                 "vertikalt fremspring på vegg"@nb-no ;
                    rdfs:label "Pilaster"@en ,
                               "Pilaster"@nl-nl ;
                    rdfs:seeAlso ifc:IfcColumnEnumType .


###  http://pi.pauwel.be/voc/buildingelement#Covering
beo:Covering rdf:type owl:Class ;
             rdfs:subClassOf beo:BuildingElement ;
             rdfs:comment "An element which covers some part of another element and is fully dependent on that other element."@en ,
                          "http://bsdd.buildingsmart.org/#concept/details/3uBPs0qSyHuO00025QrE$V"@en ;
             rdfs:label "Bekleidung / Belag"@de-de ,
                        "Covering"@en ,
                        "kledning / belegg"@nb-no ,
                        "revêtement"@fr-fr ;
             rdfs:seeAlso ifc:IfcCovering .


###  http://pi.pauwel.be/voc/buildingelement#Covering-CEILING
beo:Covering-CEILING rdf:type owl:Class ;
                     rdfs:subClassOf beo:Covering ;
                     rdfs:comment "http://bsdd.buildingsmart.org/#concept/details/05pSAVKa99GQlGChUhmlv1"@en ;
                     rdfs:label "Ceiling"@en ,
                                "tak"@nb-no ;
                     rdfs:seeAlso ifc:IfcCoveringEnumType .


###  http://pi.pauwel.be/voc/buildingelement#Covering-CLADDING
beo:Covering-CLADDING rdf:type owl:Class ;
                      rdfs:subClassOf beo:Covering ;
                      rdfs:comment "http://bsdd.buildingsmart.org/#concept/details/0MKWgDXdn9OfqhAzFzvTUH"@en ;
                      rdfs:label "Cladding"@en ,
                                 "kledning"@nb-no ;
                      rdfs:seeAlso ifc:IfcCoveringEnumType .


###  http://pi.pauwel.be/voc/buildingelement#Covering-FLOORING
beo:Covering-FLOORING rdf:type owl:Class ;
                      rdfs:subClassOf beo:Covering ;
                      rdfs:comment "http://bsdd.buildingsmart.org/#concept/details/1MZNPRnDz1jOV_XCmntitl"@en ;
                      rdfs:label "Flooring"@en ,
                                 "gulv"@nb-no ;
                      rdfs:seeAlso ifc:IfcCoveringEnumType .


###  http://pi.pauwel.be/voc/buildingelement#Covering-INSULATION
beo:Covering-INSULATION rdf:type owl:Class ;
                        rdfs:subClassOf beo:Covering ;
                        rdfs:comment "http://bsdd.buildingsmart.org/#concept/details/0m_WyU8An7RAFjJPRPQn1j"@en ;
                        rdfs:label "Insulation"@en ,
                                   "isolasjon"@nb-no ;
                        rdfs:seeAlso ifc:IfcCoveringEnumType .


###  http://pi.pauwel.be/voc/buildingelement#Covering-MEMBRANE
beo:Covering-MEMBRANE rdf:type owl:Class ;
                      rdfs:subClassOf beo:Covering ;
                      rdfs:comment "http://bsdd.buildingsmart.org/#concept/details/3vHSkCoT0Hsm00051Mm008"@en ,
                                   "vanntett og/eller damptett lag som er festet til sluket i gulvet, på gulvet eller på taket"@nb-no ,
                                   """watertight and/or damp proof layer attached to the gully either in the floor or on the floor or
roof"""@en ;
                      rdfs:label "Dichtungsbahn"@de-de ,
                                 "Membrane"@en ,
                                 "film d'étanchéité"@fr-fr ,
                                 "membran"@nb-no ;
                      rdfs:seeAlso ifc:IfcCoveringEnumType .


###  http://pi.pauwel.be/voc/buildingelement#Covering-MOLDING
beo:Covering-MOLDING rdf:type owl:Class ;
                     rdfs:subClassOf beo:Covering ;
                     rdfs:comment "http://bsdd.buildingsmart.org/#concept/details/0rO5hENaL0Sx5ncSZm5QWi"@en ,
                                  "http://bsdd.buildingsmart.org/#concept/details/39P8INeF1DvPcZnWFCA0jO"@en ;
                     rdfs:label "Gesims"@de-de ,
                                "Matériau de la moulure"@fr-fr ,
                                "Molding"@en ,
                                "gerikt"@nb-no ,
                                "taklist"@nb-no ;
                     rdfs:seeAlso ifc:IfcCoveringEnumType .


###  http://pi.pauwel.be/voc/buildingelement#Covering-ROOFING
beo:Covering-ROOFING rdf:type owl:Class ;
                     rdfs:subClassOf beo:Covering ;
                     rdfs:comment "http://bsdd.buildingsmart.org/#concept/details/1roIuYcU5AxfQM_Wf18q7t"@en ;
                     rdfs:label "Roofing"@en ,
                                "takdekke"@nb-no ,
                                "taktekking"@nb-no ;
                     rdfs:seeAlso ifc:IfcCoveringEnumType .


###  http://pi.pauwel.be/voc/buildingelement#Covering-SKIRTINGBOARD
beo:Covering-SKIRTINGBOARD rdf:type owl:Class ;
                           rdfs:subClassOf beo:Covering ;
                           rdfs:comment "http://bsdd.buildingsmart.org/#concept/details/0rhD2N_cvFRRnqQ6pRM9aE"@en ;
                           rdfs:label "Matériau de la plinthe"@fr-fr ,
                                      "Skirting Board"@en ,
                                      "Sockelleiste"@de-de ,
                                      "skirtingboard"@en ,
                                      "幅木材"@ja-jp ;
                           rdfs:seeAlso ifc:IfcCoveringEnumType .


###  http://pi.pauwel.be/voc/buildingelement#Covering-SLEEVING
beo:Covering-SLEEVING rdf:type owl:Class ;
                      rdfs:subClassOf beo:Covering ;
                      rdfs:comment "http://bsdd.buildingsmart.org/#concept/details/2mox_rbmb43xWuIkQmJqW1"@en ;
                      rdfs:label "Sleeving"@en ,
                                 "strømpe"@nb-no ;
                      rdfs:seeAlso ifc:IfcCoveringEnumType .


###  http://pi.pauwel.be/voc/buildingelement#Covering-WRAPPING
beo:Covering-WRAPPING rdf:type owl:Class ;
                      rdfs:subClassOf beo:Covering ;
                      rdfs:comment "http://bsdd.buildingsmart.org/#concept/details/16XES3__TAdwQ57Ox4T_V8"@en ;
                      rdfs:label "Wrapping"@en ,
                                 "innkledning"@nb-no ;
                      rdfs:seeAlso ifc:IfcCoveringEnumType .


###  http://pi.pauwel.be/voc/buildingelement#CurtainWall
beo:CurtainWall rdf:type owl:Class ;
                rdfs:subClassOf beo:BuildingElement ;
                rdfs:comment "An exterior wall of a building which is an assembly of components, hung from the edge of the floor/roof structure rather than bearing on a floor. "@en ,
                             "Vertikale und horizontale Bauteile, die untereinander verbunden und mit dem Tragwerk des Gebäudes verankert sind sowie gefüllt sind, um eine raumabschließende, durchgehende Außenschicht zu bilden, die alleine oder gemeinsam mit der übrigen Baukonstruktion, alle normalen Funktionen einer Außenwand bietet, jedoch keine lastabtragenden Funktionen erfüllt"@de-de ,
                             "elementi strutturali verticali e orizzontali, collegati assieme e ancorati alla struttura di supporto dell'edificio e tamponati, a formare una pelle di chiusura continua che fornisce, da sola o in congiunzione con la costruzione, tutte le normali funzioni di un muro esterno, ma non assume nessuna delle caratteristiche portanti della struttura dell'edificio"@it-it ,
                             "elementos estructurales verticales y horizontales, conectados entre sí y anclados a la estructura portante del edificio y rellenados, para formar un conjunto de piel continua que proporciona, por sí mismo o conjuntamente con la construcción del edificio, todas las funciones normales de una pared externa, pero no se hace cargo de ninguna de las características portantes de la estructura del edificio"@es-es ,
                             "http://bsdd.buildingsmart.org/#concept/details/1nBFK0qT0HuO00025QrE$V"@en ,
                             "les éléments de structure verticaux et horizontaux reliés ensemble et ancrés sur la structure portante du bâtiment et remplis pour former un espace renfermant une peau continue qui fournit, par elle-même ou en combinaison avec la construction du bâtiment, toutes les fonctions normales d'un mur extérieur, mais n'emprunte aucune des caractéristiques de résistance à la charge de la structure du bâtiment"@fr-fr ,
                             "lodrette og vandrette bygningselementer, der er bundet sammen og forankret til bygningens bærende konstruktion og fyldt, så de danner en fortløbende inddækning, der i sig selv eller sammen med bygningskonstruktionen leverer alle en ydermurs normale funktioner, men som ikke påtager sig nogen af bygningskonstruktionens bærende egenskaber"@dk-dk ,
                             "pionowe i poziome elementy konstrukcyjne, połączone ze sobą i zakotwiczone w konstrukcji nośnej budynku i w zabudowie typu plomba, tworzące przestrzeń obejmującą ciągłą warstwę, która zapewnia, samodzielnie lub w połączeniu z konstrukcją budynku, wszystkie normalne funkcje ściany zewnętrznej, ale nie spełnia żadnej funkcji nośnej dla konstrukcji budynku"@pl-pl ,
                             "pysty- ja vaakasuuntaisia rakenneosia, toisiinsa liitettyinä ja rakennuksen kantavaan rakenteeseen kiinnitettynä, täydennettynä muodostamaan suojaavan yhtenäisen pintatilan, jolla on sellaisenaan tai yhdessä rakennuksen kanssa kaikki ulkoisen seinän normaalit toimintaominaisuudet, mutta jota ei käytetä kantavana rakenteena"@fi-fi ,
                             "utvendig, ikkebærende veggkonstruksjon forankret til bygningens hovedbærekonstruksjon. påhengsvegger bygges vanligvis av et rammeverk av metall, tre eller PVC med vertikale og horisontale komponenter som overfører påhengsveggens egenvekt og eventuelle vindkrefter til bygningens bærekonstruksjon"@nb-no ,
                             "vertical and horizontal structural members, connected together and anchored to the supporting structure of the building and infilled, to form a space enclosing continuous skin, which provides, by itself or in conjunction with the building construction, all the normal functions of an external wall, but does not take on any of the load bearing characteristics of the building structure"@en ,
                             "vertikala och horisontella byggnadsdelar som har sammanfogats och förankrats vid byggnadens stödkonstruktion och isolerats, för att skapa en inhägnad med kontinuerlig yta som, av sig själv eller tillsammans med byggnadskonstruktionen, erbjuder alla funktioner som en yttervägg vanligtvis har, men som inte har några av byggnadskonstruktionens bärande egenskaper"@sv-se ,
                             "вертикални и хоризонтални конструктивни елементи, свързани помежду си, закрепени към основната конструкция на сградата и запълнени, за да образуват непрекъсната ограждаща пространството обвивка, която осигурява, самостоятелно или съвместно с конструкцията на сградата, всички изисквани функции към една външна стена, но без да изпълнява никакви функции свързани с носимоспособността на сградната конструкция"@bg-bg ;
                rdfs:label "Curtain Wall"@en ,
                           "Gordijngevel"@nl ,
                           "Gordijngevel"@nl-nl ,
                           "Mur rideau"@fr-fr ,
                           "Vorhangfassade"@de-de ,
                           "Vorhangfassadenbausatz"@de-de ,
                           "julkisivujärjestelmä"@fi-fi ,
                           "påhengsvegg"@nb-no ,
                           "sats till utfackningsväggar"@sv-se ,
                           "zestaw ściany osłonowej"@pl-pl ,
                           "монтажни модули за окачени фасади"@bg-bg ;
                rdfs:seeAlso ifc:IfcCurtainWall .


###  http://pi.pauwel.be/voc/buildingelement#DiscreteAccessory
beo:DiscreteAccessory rdf:type owl:Class ;
                      rdfs:subClassOf beo:ElementComponent ;
                      rdfs:comment "A representation of different kinds of accessories included in or added to elements."@en ,
                                   "http://bsdd.buildingsmart.org/#concept/details/0W7W20qT8HuO00025QrE$V"@en ;
                      rdfs:label "Accessoire composé"@fr-fr ,
                                 "Discrete Accessory"@en ,
                                 "Zusatzgerät / Einbauteil"@de-de ;
                      rdfs:seeAlso ifc:IfcDiscreteAccessory .


###  http://pi.pauwel.be/voc/buildingelement#DiscreteAccessory-ANCHORPLATE
beo:DiscreteAccessory-ANCHORPLATE rdf:type owl:Class ;
                                  rdfs:subClassOf beo:DiscreteAccessory ;
                                  rdfs:comment "http://bsdd.buildingsmart.org/#concept/details/1XD5ysVrvF$haI5OgtznWi"@en ;
                                  rdfs:label "Anchor Plate"@en ;
                                  rdfs:seeAlso ifc:IfcDiscreteAccessoryEnumType .


###  http://pi.pauwel.be/voc/buildingelement#DiscreteAccessory-BRACKET
beo:DiscreteAccessory-BRACKET rdf:type owl:Class ;
                              rdfs:subClassOf beo:DiscreteAccessory ;
                              rdfs:comment "An artefact which is projecting from the side of a wall or other structure intended to support some other artefacts.        "@en ,
                                           "Brakkett for utstyr"@nb-no ,
                                           "Innstøpningsbrakett"@nb-no ,
                                           "http://bsdd.buildingsmart.org/#concept/details/3EGCgYGC9F3PmaQ821Ax2u"@en ,
                                           "http://bsdd.buildingsmart.org/#concept/details/3vHPwWoT0Hsm00051Mm008"@en ,
                                           "http://bsdd.buildingsmart.org/#concept/details/3vHcVCoT0Hsm00051Mm008"@en ;
                              rdfs:label "Bracket"@en ,
                                         "Console"@nl-nl ,
                                         "Winkellasche"@de-de ,
                                         "bracket for innerwall"@en ,
                                         "brakett"@nb-no ,
                                         "brakett innervegg"@nb-no ,
                                         "console"@en ,
                                         "crochet"@fr-fr ,
                                         "innervegg"@nb-no ,
                                         "innerveggbrakett"@nb-no ,
                                         "innstøpningsbrakett"@nb-no ;
                              rdfs:seeAlso ifc:IfcDiscreteAccessoryEnumType .


###  http://pi.pauwel.be/voc/buildingelement#DiscreteAccessory-SHOE
beo:DiscreteAccessory-SHOE rdf:type owl:Class ;
                           rdfs:subClassOf beo:DiscreteAccessory ;
                           rdfs:comment "http://bsdd.buildingsmart.org/#concept/details/1i44itooP5F9e53Jc$HR0o"@en ;
                           rdfs:label "Shoe" ,
                                      "søylesko"@nb-no ;
                           rdfs:seeAlso ifc:IfcDiscreteAccessoryEnumType .


###  http://pi.pauwel.be/voc/buildingelement#Door
beo:Door rdf:type owl:Class ;
         rdfs:subClassOf beo:BuildingElement ;
         rdfs:comment "Bygningsdel som dekker en åpning i utvendig eller innvendig vegg, og som kan åpnes eller stenges for passasje."@nb-no ,
                      "En åpning i en barriære med et dørblad som kan lukke åpningen og en ramme som holder dørbladet."@nb-no ,
                      "a complete unit consisting of a door frame and a door leaf or leaves, supplied with the essential hardware and wheatherseal, as a product from a single source"@en ,
                      "construction for closing an opening intended primarily for access or egress or both. Typically consisting of a panel that swings on hinges or that slides or rotates"@en ,
                      "http://bsdd.buildingsmart.org/#concept/details/3vHRQ8oT0Hsm00051Mm008"@en ;
         rdfs:label "Deur"@nl-nl ,
                    "Door"@en ,
                    "Dør"@da ,
                    "Tür"@de-de ,
                    "Türeinheit"@de-de ,
                    "dør"@nb-no ,
                    "dør med karm"@nb-no ,
                    "porte"@fr-fr ;
         rdfs:seeAlso ifc:IfcDoor .


###  http://pi.pauwel.be/voc/buildingelement#Door-DOOR
beo:Door-DOOR rdf:type owl:Class ;
              rdfs:subClassOf beo:Door ;
              rdfs:comment "A standard door usually within a wall opening, as a door panel in a curtain wall, or as a \"free standing\" door."@en ,
                           "Bygningsdel som dekker en åpning i utvendig eller innvendig vegg, og som kan åpnes eller stenges for passasje."@nb-no ,
                           "En åpning i en barriære med et dørblad som kan lukke åpningen og en ramme som holder dørbladet."@nb-no ,
                           "a complete unit consisting of a door frame and a door leaf or leaves, supplied with the essential hardware and wheatherseal, as a product from a single source"@en ,
                           "construction for closing an opening intended primarily for access or egress or both. Typically consisting of a panel that swings on hinges or that slides or rotates"@en ,
                           "http://bsdd.buildingsmart.org/#concept/details/2reX7MzyDDPP8OCoYtmU7d"@en ;
              rdfs:label "Deur"@nl-nl ,
                         "Door"@en ,
                         "Tür"@de-de ,
                         "Türeinheit"@de-de ,
                         "bloc-porte"@fr-fr ,
                         "deur"@nl-nl ,
                         "dør"@nb-no ,
                         "dør med karm"@nb-no ,
                         "porte"@fr-fr ;
              rdfs:seeAlso ifc:IfcDoorEnumType .


###  http://pi.pauwel.be/voc/buildingelement#Door-GATE
beo:Door-GATE rdf:type owl:Class ;
              rdfs:subClassOf beo:Door ;
              rdfs:comment """Det engelske ordet 'gate' og det franske ordet 'portail' refererer til produkter utenfor bygninger, for eksempel i innhegninger, gjerder osv.
Det tyske ordet 'Tor' refererer til alle produkter for å stenge åpninger, som tillater passering av kjøretøyer."""@nb-no ,
                           "a movable barrier, usually on hinges, closing an opening in a fence, wall, or other enclosure"@en ,
                           "http://bsdd.buildingsmart.org/#concept/details/3C6qVkdNfEGOKvZBfksYwB"@en ,
                           "innretning for å lukke en åpning som er beregnet for passering av kjøretøyer og personer"@nb-no ;
              rdfs:label "Gate"@en ,
                         "Hek"@nl-nl ,
                         "Poort"@nl-nl ,
                         "Tor"@de-de ,
                         "fermeture"@fr-fr ,
                         "port"@nb-no ;
              rdfs:seeAlso ifc:IfcDoorEnumType .


###  http://pi.pauwel.be/voc/buildingelement#Door-TRAPDOOR
beo:Door-TRAPDOOR rdf:type owl:Class ;
                  rdfs:subClassOf beo:Door ;
                  rdfs:comment "http://bsdd.buildingsmart.org/#concept/details/3_T7f4cxzB_ur2vAtd6pJe"@en ;
                  rdfs:label "Roof Hatch"@en ,
                             "Trap Door"@en ,
                             "takluke"@nb-no ;
                  rdfs:seeAlso ifc:IfcDoorEnumType .


###  http://pi.pauwel.be/voc/buildingelement#ElementComponent
beo:ElementComponent rdf:type owl:Class ;
                     rdfs:subClassOf <https://schema.org/Product> ;
                     rdfs:comment "A representation for minor items included in, added to or connecting to or between elements, which usually are not of interest from the overall building structure viewpoint. However, these small parts may have vital and load carrying functions within the construction. These items do not provide any actual space boundaries. Typical examples include different kinds of fasteners and various accessories."@en ,
                                  "http://bsdd.buildingsmart.org/#concept/details/2pKpW0qSeHuO00025QrE$V"@en ;
                     rdfs:label "Composant d'élément"@fr-fr ,
                                "Element Component"@en ,
                                "Elementenbestandteil"@de-de ;
                     rdfs:seeAlso ifc:IfcElementComponent .


###  http://pi.pauwel.be/voc/buildingelement#Fastener
beo:Fastener rdf:type owl:Class ;
             rdfs:subClassOf beo:ElementComponent ;
             rdfs:comment "Jointing component that is used to operate a door, window, shutter, gate or drawer ."@en ,
                          "Representations of fixing parts which are used as fasteners to connect or join elements with other elements. "@en ,
                          "http://bsdd.buildingsmart.org/#concept/details/2$v8e0qUGHuO00025QrE$V"@en ;
             rdfs:label "Befestigungsmittel"@de-de ,
                        "Elément d'assemblage"@fr-fr ,
                        "Fastener"@en ,
                        "festeinnretning"@nb-no ;
             rdfs:seeAlso ifc:IfcFastener .


###  http://pi.pauwel.be/voc/buildingelement#Fastener-GLUE
beo:Fastener-GLUE rdf:type owl:Class ;
                  rdfs:subClassOf beo:Fastener ;
                  rdfs:comment "bindemedel eller bindemedelslösning för hopfogning av fasta material"@sv-se ,
                               "binder or binder solution for joining solid materials"@en ,
                               "http://bsdd.buildingsmart.org/#concept/details/097NQ9z4T7eOn7nJCQC0yI"@en ;
                  rdfs:label "Glue"@en ,
                             "lim"@nb-no ,
                             "lim"@sv-se ;
                  rdfs:seeAlso ifc:IfcFastenerEnumType .


###  http://pi.pauwel.be/voc/buildingelement#Fastener-MORTAR
beo:Fastener-MORTAR rdf:type owl:Class ;
                    rdfs:subClassOf beo:Fastener ;
                    rdfs:comment "http://bsdd.buildingsmart.org/#concept/details/0dS2xSsC1BbvRjM1MIjNn5"@en ;
                    rdfs:label "Mortar"@en ,
                               "mørtel"@nb-no ;
                    rdfs:seeAlso ifc:IfcFastenerEnumType .


###  http://pi.pauwel.be/voc/buildingelement#Fastener-WELD
beo:Fastener-WELD rdf:type owl:Class ;
                  rdfs:subClassOf beo:Fastener ;
                  rdfs:comment "a weld seam between parts of metallic material or other suitable materials"@en ,
                               "a weld seam between parts of metallic material or other suitable materials"@en-gb ,
                               "http://bsdd.buildingsmart.org/#concept/details/01DZw_Z2b4CwKEwBQ9ERPZ"@en ;
                  rdfs:label "Weld"@en ,
                             "sveis"@nb-no ;
                  rdfs:seeAlso ifc:IfcFastenerEnumType .


###  http://pi.pauwel.be/voc/buildingelement#Footing
beo:Footing rdf:type owl:Class ;
            rdfs:subClassOf beo:BuildingElement ;
            rdfs:comment "A part of the foundation of a structure that spreads and transmits the load to the soil. Also characterized as shallow foundation, where the loads are transferred to the ground near the surface."@en ,
                         "Flachgründung"@de-de ,
                         "http://bsdd.buildingsmart.org/#concept/details/2vyAW0qUWHuO00025QrE$V"@en ;
            rdfs:label "Footing"@en ,
                       "Fundament"@de-de ,
                       "Funderingsvoet"@nl-nl ,
                       "fondation"@fr-fr ;
            rdfs:seeAlso ifc:IfcFooting .


###  http://pi.pauwel.be/voc/buildingelement#Footing-CAISSON_FOUNDATION
beo:Footing-CAISSON_FOUNDATION rdf:type owl:Class ;
                               rdfs:subClassOf beo:Footing ;
                               rdfs:comment "http://bsdd.buildingsmart.org/#concept/details/0MGkpmTGDFC80qy7qA0W2w"@en ;
                               rdfs:label "Caisson Foundation"@en ,
                                          "senkekasse til fundament"@nb-no ;
                               rdfs:seeAlso ifc:IfcFootingEnumType .


###  http://pi.pauwel.be/voc/buildingelement#Footing-FOOTING_BEAM
beo:Footing-FOOTING_BEAM rdf:type owl:Class ;
                         rdfs:subClassOf beo:Footing ;
                         rdfs:comment "http://bsdd.buildingsmart.org/#concept/details/3hRbiifMvFOgC3tEfSPD8X"@en ;
                         rdfs:label "Footing Beam"@en ;
                         rdfs:seeAlso ifc:IfcFootingEnumType .


###  http://pi.pauwel.be/voc/buildingelement#Footing-PAD_FOOTING
beo:Footing-PAD_FOOTING rdf:type owl:Class ;
                        rdfs:subClassOf beo:Footing ;
                        rdfs:comment "http://bsdd.buildingsmart.org/#concept/details/1XJ0TK6AbBfxMCQLLkdnDr"@en ;
                        rdfs:label "Pad Footing"@en ;
                        rdfs:seeAlso ifc:IfcFootingEnumType .


###  http://pi.pauwel.be/voc/buildingelement#Footing-PILE_CAP
beo:Footing-PILE_CAP rdf:type owl:Class ;
                     rdfs:subClassOf beo:Footing ;
                     rdfs:comment "http://bsdd.buildingsmart.org/#concept/details/3$LxhKMZjFuBdi75OQXj0L"@en ;
                     rdfs:label "Pile Cap"@en ;
                     rdfs:seeAlso ifc:IfcFootingEnumType .


###  http://pi.pauwel.be/voc/buildingelement#Footing-STRIP_FOOTING
beo:Footing-STRIP_FOOTING rdf:type owl:Class ;
                          rdfs:subClassOf beo:Footing ;
                          rdfs:comment "http://bsdd.buildingsmart.org/#concept/details/0mDEbMPpzB9B_vQTUHZLHe"@en ;
                          rdfs:label "Strip Footing"@en ,
                                     "platefundament"@nb-no ;
                          rdfs:seeAlso ifc:IfcFootingEnumType .


###  http://pi.pauwel.be/voc/buildingelement#MechanicalFastener
beo:MechanicalFastener rdf:type owl:Class ;
                       rdfs:subClassOf beo:ElementComponent ;
                       rdfs:comment "A fastener connecting building elements mechanically. A single instance may represent one or many of actual mechanical fasteners, for example an array of bolts or a row of nails."@en ,
                                    "http://bsdd.buildingsmart.org/#concept/details/2$KV20qV0HuO00025QrE$V"@en ;
                       rdfs:label "Mechanical Fastener"@en ,
                                  "MechanicalFastener" ,
                                  "Mechanisches Befestigungsmittel"@de-de ,
                                  "mekanisk festemiddel"@nb-no ;
                       rdfs:seeAlso ifc:IfcMechanicalFastener .


###  http://pi.pauwel.be/voc/buildingelement#MechanicalFastener-ANCHORBOLT
beo:MechanicalFastener-ANCHORBOLT rdf:type owl:Class ;
                                  rdfs:subClassOf beo:MechanicalFastener ;
                                  rdfs:comment "http://bsdd.buildingsmart.org/#concept/details/3NJqge3HD7du28Nje_S1Yv"@en ;
                                  rdfs:label "Anchor Bolt"@en ,
                                             "mekanisk ankerbolt"@nb-no ;
                                  rdfs:seeAlso ifc:IfcMechanicalFastenerEnumType .


###  http://pi.pauwel.be/voc/buildingelement#MechanicalFastener-BOLT
beo:MechanicalFastener-BOLT rdf:type owl:Class ;
                            rdfs:subClassOf beo:MechanicalFastener ;
                            rdfs:comment "a threaded cylindrical rod that engages with a similarly threaded hole in a nut or any other part to form a fastener. the mechanical fastener often also includes one or more washers and one or more nuts."@en ,
                                         "http://bsdd.buildingsmart.org/#concept/details/2yfVRHZ2X7heCLVLk0oVBK"@en ;
                            rdfs:label "Bolt"@en ,
                                       "mekanisk festemiddel - bolt"@nb-no ;
                            rdfs:seeAlso ifc:IfcMechanicalFastenerEnumType .


###  http://pi.pauwel.be/voc/buildingelement#MechanicalFastener-DOWEL
beo:MechanicalFastener-DOWEL rdf:type owl:Class ;
                             rdfs:subClassOf beo:MechanicalFastener ;
                             rdfs:comment "Dybel"@nb-no ,
                                          "http://bsdd.buildingsmart.org/#concept/details/2jZSkKNyPBMwSeeMxlYWrc"@en ,
                                          "http://bsdd.buildingsmart.org/#concept/details/3vHOxEoT0Hsm00051Mm008"@en ,
                                          "rod protruding from the toe of the sheet pile, used for fixing sheet piles to the bed-rock"@en ,
                                          "stag som stikker ut fra foten av spuntnålen, og som brukes for å feste spunten til fjell"@nb-no ;
                             rdfs:label "Dowel" ,
                                        "Felsdübel"@de-de ,
                                        "dowel"@en ,
                                        "dybel"@nb-no ,
                                        "goujon pour rocher"@fr-fr ,
                                        "rock dowel"@en ;
                             rdfs:seeAlso ifc:IfcMechanicalFastenerEnumType .


###  http://pi.pauwel.be/voc/buildingelement#MechanicalFastener-NAIL
beo:MechanicalFastener-NAIL rdf:type owl:Class ;
                            rdfs:subClassOf beo:MechanicalFastener ;
                            rdfs:comment "http://bsdd.buildingsmart.org/#concept/details/1WICu7sp12cQ$$2QCHf$DB"@en ;
                            rdfs:label "Nail"@en ,
                                       "spiker"@nb-no ;
                            rdfs:seeAlso ifc:IfcMechanicalFastenerEnumType .


###  http://pi.pauwel.be/voc/buildingelement#MechanicalFastener-NAILPLATE
beo:MechanicalFastener-NAILPLATE rdf:type owl:Class ;
                                 rdfs:subClassOf beo:MechanicalFastener ;
                                 rdfs:comment "http://bsdd.buildingsmart.org/#concept/details/26FDcCBjH3BOLZTZb29fxk"@en ;
                                 rdfs:label "Nail Plate"@en ,
                                            "spikerplate"@nb-no ;
                                 rdfs:seeAlso ifc:IfcMechanicalFastenerEnumType .


###  http://pi.pauwel.be/voc/buildingelement#MechanicalFastener-RIVET
beo:MechanicalFastener-RIVET rdf:type owl:Class ;
                             rdfs:subClassOf beo:MechanicalFastener ;
                             rdfs:comment "http://bsdd.buildingsmart.org/#concept/details/1zynxAt3H1eAVfmukRcO4R"@en ;
                             rdfs:label "Rivet"@en ,
                                        "nagle"@nb-no ;
                             rdfs:seeAlso ifc:IfcMechanicalFastenerEnumType .


###  http://pi.pauwel.be/voc/buildingelement#MechanicalFastener-SCREW
beo:MechanicalFastener-SCREW rdf:type owl:Class ;
                             rdfs:subClassOf beo:MechanicalFastener ;
                             rdfs:comment "http://bsdd.buildingsmart.org/#concept/details/2NLmoal3LAGxceh8SPCvI7"@en ;
                             rdfs:label "Screw"@en ,
                                        "skrue"@nb-no ;
                             rdfs:seeAlso ifc:IfcMechanicalFastenerEnumType .


###  http://pi.pauwel.be/voc/buildingelement#MechanicalFastener-SHEARCONNECTOR
beo:MechanicalFastener-SHEARCONNECTOR rdf:type owl:Class ;
                                      rdfs:subClassOf beo:MechanicalFastener ;
                                      rdfs:comment "http://bsdd.buildingsmart.org/#concept/details/0sHCCoroj0pesEpqdsmtRT"@en ;
                                      rdfs:label "Shear Connector"@en ;
                                      rdfs:seeAlso ifc:IfcMechanicalFastenerEnumType .


###  http://pi.pauwel.be/voc/buildingelement#MechanicalFastener-STAPLE
beo:MechanicalFastener-STAPLE rdf:type owl:Class ;
                              rdfs:subClassOf beo:MechanicalFastener ;
                              rdfs:comment "http://bsdd.buildingsmart.org/#concept/details/3ugeBu3lP8WANu_d7DFAtv"@en ;
                              rdfs:label "Staple"@en ,
                                         "stift"@nb-no ;
                              rdfs:seeAlso ifc:IfcMechanicalFastenerEnumType .


###  http://pi.pauwel.be/voc/buildingelement#MechanicalFastener-STUDSHEARCONNECTOR
beo:MechanicalFastener-STUDSHEARCONNECTOR rdf:type owl:Class ;
                                          rdfs:subClassOf beo:MechanicalFastener ;
                                          rdfs:comment "http://bsdd.buildingsmart.org/#concept/details/2VmXuOwNvFIxXMT91lYI9q"@en ;
                                          rdfs:label "Stud Shear Connector"@en ;
                                          rdfs:seeAlso ifc:IfcMechanicalFastenerEnumType .


###  http://pi.pauwel.be/voc/buildingelement#Member
beo:Member rdf:type owl:Class ;
           rdfs:subClassOf beo:BuildingElement ;
           rdfs:comment "A structural member designed to carry loads between or beyond points of support. It is not required to be load bearing.  A linear architectural or structural element that cannot be expressed more specifically as either a beam or column."@en ,
                        "http://bsdd.buildingsmart.org/#concept/details/11GXc0qV4HuO00025QrE$V"@en ;
           rdfs:label "Member"@en ,
                      "Membre"@fr-fr ,
                      "Stab / Stabträger"@de-de ,
                      "konstruksjonsdel"@nb-no ;
           rdfs:seeAlso ifc:IfcMember .


###  http://pi.pauwel.be/voc/buildingelement#Member-BRACE
beo:Member-BRACE rdf:type owl:Class ;
                 rdfs:subClassOf beo:Member ;
                 rdfs:comment "http://bsdd.buildingsmart.org/#concept/details/0ccYVvWMX5jwoOSredVplR"@en ;
                 rdfs:label "Brace"@en ,
                            "avstiver"@nb-no ;
                 rdfs:seeAlso ifc:IfcMemberEnumType .


###  http://pi.pauwel.be/voc/buildingelement#Member-CHORD
beo:Member-CHORD rdf:type owl:Class ;
                 rdfs:subClassOf beo:Member ;
                 rdfs:comment "http://bsdd.buildingsmart.org/#concept/details/1_qCPXQ3j1VBh_PCDSM2PC"@en ;
                 rdfs:label "Chord"@en ,
                            "gurt"@nb-no ;
                 rdfs:seeAlso ifc:IfcMemberEnumType .


###  http://pi.pauwel.be/voc/buildingelement#Member-COLLAR
beo:Member-COLLAR rdf:type owl:Class ;
                  rdfs:subClassOf beo:Member ;
                  rdfs:comment "http://bsdd.buildingsmart.org/#concept/details/1r9F5o8Pv9mPKppdGc$YOw"@en ;
                  rdfs:label "Collar"@en ,
                             "krage"@nb-no ;
                  rdfs:seeAlso ifc:IfcMemberEnumType .


###  http://pi.pauwel.be/voc/buildingelement#Member-MEMBER
beo:Member-MEMBER rdf:type owl:Class ;
                  rdfs:subClassOf beo:Member ;
                  rdfs:comment "A structural member designed to carry loads between or beyond points of support. It is not required to be load bearing.  A linear architectural or structural element that cannot be expressed more specifically as either a beam or column."@en ,
                               "http://bsdd.buildingsmart.org/#concept/details/11GXc0qV4HuO00025QrE$V"@en ;
                  rdfs:label "Member"@en ,
                             "Membre"@fr-fr ,
                             "Stab / Stabträger"@de-de ,
                             "konstruksjonsdel"@nb-no ;
                  rdfs:seeAlso ifc:IfcMemberEnumType .


###  http://pi.pauwel.be/voc/buildingelement#Member-MULLION
beo:Member-MULLION rdf:type owl:Class ;
                   rdfs:subClassOf beo:Member ;
                   rdfs:comment "http://bsdd.buildingsmart.org/#concept/details/2H6TZXz1vEFOlOdhLv3CD7"@en ;
                   rdfs:label "Mullion"@en ,
                              "midtstolpe"@nb-no ;
                   rdfs:seeAlso ifc:IfcMemberEnumType .


###  http://pi.pauwel.be/voc/buildingelement#Member-PLATE
beo:Member-PLATE rdf:type owl:Class ;
                 rdfs:subClassOf beo:Member ;
                 rdfs:comment "A planar and often flat part with constant thickness. May carry loads between or beyond points of support, or provide stiffening. "@en ,
                              "http://bsdd.buildingsmart.org/#concept/details/3zdC5dewn4ROXxRERahlnc"@en ;
                 rdfs:label "Plate"@en ,
                            "Platte / Paneel"@de-de ,
                            "plaque"@fr-fr ,
                            "plate"@nb-no ,
                            "platevarmeveksler"@nb-no ;
                 rdfs:seeAlso ifc:IfcMemberEnumType .


###  http://pi.pauwel.be/voc/buildingelement#Member-POST
beo:Member-POST rdf:type owl:Class ;
                rdfs:subClassOf beo:Member ;
                rdfs:comment "a linear member (usually used vertically) within a roof structure to support purlins"@en ,
                             "a linear member (usually used vertically) within a roof structure to support purlins"@en-gb ,
                             "http://bsdd.buildingsmart.org/#concept/details/3pLJTABEHCJeV4uMg1OJxY"@en ;
                rdfs:label "Post" ,
                           "stolpe"@nb-no ;
                rdfs:seeAlso ifc:IfcMemberEnumType .


###  http://pi.pauwel.be/voc/buildingelement#Member-PURLIN
beo:Member-PURLIN rdf:type owl:Class ;
                  rdfs:subClassOf beo:Member ;
                  rdfs:comment "http://bsdd.buildingsmart.org/#concept/details/2ClC__ZBT6lgGn9bEtyKAq"@en ;
                  rdfs:label "Purlin" ,
                             "takås"@nb-no ;
                  rdfs:seeAlso ifc:IfcMemberEnumType .


###  http://pi.pauwel.be/voc/buildingelement#Member-RAFTER
beo:Member-RAFTER rdf:type owl:Class ;
                  rdfs:subClassOf beo:Member ;
                  rdfs:comment "http://bsdd.buildingsmart.org/#concept/details/14MOjpDn1DYfI9uAgvn_Mm"@en ,
                               "sperre"@nb-no ;
                  rdfs:label "Rafter"@en ;
                  rdfs:seeAlso ifc:IfcMemberEnumType .


###  http://pi.pauwel.be/voc/buildingelement#Member-STRINGER
beo:Member-STRINGER rdf:type owl:Class ;
                    rdfs:subClassOf beo:Member ;
                    rdfs:comment "http://bsdd.buildingsmart.org/#concept/details/31phWfaoDEDwTkU1_cQp7G"@en ;
                    rdfs:label "Stringer"@en ,
                               "vange"@nb-no ;
                    rdfs:seeAlso ifc:IfcMemberEnumType .


###  http://pi.pauwel.be/voc/buildingelement#Member-STRUT
beo:Member-STRUT rdf:type owl:Class ;
                 rdfs:subClassOf beo:Member ;
                 rdfs:comment "http://bsdd.buildingsmart.org/#concept/details/0F1OouH1f9rPC$dWa4xYLb"@en ;
                 rdfs:label "Strut"@en ,
                            "trykkstav"@nb-no ;
                 rdfs:seeAlso ifc:IfcMemberEnumType .


###  http://pi.pauwel.be/voc/buildingelement#Member-STUD
beo:Member-STUD rdf:type owl:Class ;
                rdfs:subClassOf beo:Member ;
                rdfs:comment "http://bsdd.buildingsmart.org/#concept/details/14DS4URKP2au1B2s5ghLFp"@en ;
                rdfs:label "Stud"@en ,
                           "stender"@nb-no ;
                rdfs:seeAlso ifc:IfcMemberEnumType .


###  http://pi.pauwel.be/voc/buildingelement#Pile
beo:Pile rdf:type owl:Class ;
         rdfs:subClassOf beo:BuildingElement ;
         rdfs:comment "A vertical structural member of timber, concrete, or steel, driven into the earth as a foundation or support for a structure for the transfer of actions. "@en ,
                      "En stråle av tømmer, betong eller stål, drevet ned i jorden som fundament eller støtte til en struktur."@nb-no ,
                      "http://bsdd.buildingsmart.org/#concept/details/3vHXEAoT0Hsm00051Mm008"@en ,
                      "slankt bærende element i grunnen for overføring av laster. I denne europeiske standarden er slankhetsforholdet ikke begrenset"@nb-no ;
         rdfs:label "Fundament / Tiefgründung"@de-de ,
                    "Pfahl"@de-de ,
                    "Pile"@en ,
                    "pel"@nb-no ,
                    "pele"@nb-no ,
                    "pieu"@fr-fr ,
                    "pæl"@nb-no ;
         rdfs:seeAlso ifc:IfcPile .


###  http://pi.pauwel.be/voc/buildingelement#Pile-BORED
beo:Pile-BORED rdf:type owl:Class ;
               rdfs:subClassOf beo:Pile ;
               rdfs:comment "http://bsdd.buildingsmart.org/#concept/details/1INEbwMtrBy9rKhAuvXYmq"@en ;
               rdfs:label "Bored Pile"@en ,
                          "boret pel"@nb-no ;
               rdfs:seeAlso ifc:IfcPileEnumType .


###  http://pi.pauwel.be/voc/buildingelement#Pile-COHESION
beo:Pile-COHESION rdf:type owl:Class ;
                  rdfs:subClassOf beo:Pile ;
                  rdfs:comment "http://bsdd.buildingsmart.org/#concept/details/3xzAjG3Uv5qeCDRxYCXd4d"@en ;
                  rdfs:label "Cohesion Pile"@en ,
                             "kohesjon pel"@nb-no ;
                  rdfs:seeAlso ifc:IfcPileEnumType .


###  http://pi.pauwel.be/voc/buildingelement#Pile-DRIVEN
beo:Pile-DRIVEN rdf:type owl:Class ;
                rdfs:subClassOf beo:Pile ;
                rdfs:comment "http://bsdd.buildingsmart.org/#concept/details/2Qg5YD6TD299EHtweCaOOy"@en ;
                rdfs:label "Driven Pile"@en ,
                           "rammet pel"@nb-no ;
                rdfs:seeAlso ifc:IfcPileEnumType .


###  http://pi.pauwel.be/voc/buildingelement#Pile-FRICTION
beo:Pile-FRICTION rdf:type owl:Class ;
                  rdfs:subClassOf beo:Pile ;
                  rdfs:comment "http://bsdd.buildingsmart.org/#concept/details/3LgOubO_D3EhcElUZP9dMe"@en ;
                  rdfs:label "Friction Pile"@en ,
                             "friksjonspele"@nb-no ;
                  rdfs:seeAlso ifc:IfcPileEnumType .


###  http://pi.pauwel.be/voc/buildingelement#Pile-JETGROUTING
beo:Pile-JETGROUTING rdf:type owl:Class ;
                     rdfs:subClassOf beo:Pile ;
                     rdfs:comment "http://bsdd.buildingsmart.org/#concept/details/1tI0jqBjHEmADWyrGGYig6"@en ;
                     rdfs:label "Jet Grouting Pile"@en ;
                     rdfs:seeAlso ifc:IfcPileEnumType .


###  http://pi.pauwel.be/voc/buildingelement#Pile-SUPPORT
beo:Pile-SUPPORT rdf:type owl:Class ;
                 rdfs:subClassOf beo:Pile ;
                 rdfs:comment "http://bsdd.buildingsmart.org/#concept/details/3qZud6iazFjOZ3wK3WoQch"@en ;
                 rdfs:label "Support"@en ,
                            "støtte"@nb-no ;
                 rdfs:seeAlso ifc:IfcPileEnumType .


###  http://pi.pauwel.be/voc/buildingelement#Plate
beo:Plate rdf:type owl:Class ;
          rdfs:subClassOf beo:BuildingElement ;
          rdfs:comment "A planar and often flat part with constant thickness. May carry loads between or beyond points of support, or provide stiffening. "@en ,
                       "http://bsdd.buildingsmart.org/#concept/details/3z14Y0qVCHuO00025QrE$V"@en ;
          rdfs:label "Plate"@en ,
                     "Platte / Paneel"@de-de ,
                     "plaque"@fr-fr ,
                     "plate"@nb-no ;
          rdfs:seeAlso ifc:IfcPlate .


###  http://pi.pauwel.be/voc/buildingelement#Plate-CURTAIN_PANEL
beo:Plate-CURTAIN_PANEL rdf:type owl:Class ;
                        rdfs:subClassOf beo:Plate ;
                        rdfs:comment "a planar element within a curtain wall, often consisting of a frame with fixed glazing"@en ,
                                     "a planar element within a curtain wall, often consisting of a frame with fixed glazing"@en-gb ,
                                     "http://bsdd.buildingsmart.org/#concept/details/2N7mbvPFL0QRlf$nLuQE0U"@en ;
                        rdfs:label "Curtain Panel"@en ,
                                   "skjermpanel"@nb-no ;
                        rdfs:seeAlso ifc:IfcPlateEnumType .


###  http://pi.pauwel.be/voc/buildingelement#Plate-SHEET
beo:Plate-SHEET rdf:type owl:Class ;
                rdfs:subClassOf beo:Plate ;
                rdfs:comment "http://bsdd.buildingsmart.org/#concept/details/2C4D8j05v51eRokWOWtlju"@en ;
                rdfs:label "Sheet"@en ;
                rdfs:seeAlso ifc:IfcPlateEnumType .


###  http://pi.pauwel.be/voc/buildingelement#Railing
beo:Railing rdf:type owl:Class ;
            rdfs:subClassOf beo:BuildingElement ;
            rdfs:comment "A frame assembly adjacent to human circulation spaces and at some space boundaries where it is used in line of walls or to compliment walls. Designed to aid humans, either as an optional physical support, or to prevent injury by falling."@en ,
                         "http://bsdd.buildingsmart.org/#concept/details/02irk0qVyHuO00025QrE$V"@en ;
            rdfs:label "Garde corps"@fr-fr ,
                       "Geländer"@de-de ,
                       "Gelænder"@da ,
                       "Hekwerk"@nl-nl ,
                       "Leuning"@nl ,
                       "Railing"@en ,
                       "Reling"@nl-nl ,
                       "garde-corps"@fr-fr ,
                       "rekkverk"@nb-no ;
            rdfs:seeAlso ifc:IfcRailing .


###  http://pi.pauwel.be/voc/buildingelement#Railing-BALUSTRADE
beo:Railing-BALUSTRADE rdf:type owl:Class ;
                       rdfs:subClassOf beo:Railing ;
                       rdfs:comment "A balustrade is a separation construction alongside the edges of floors, roofs, stairs and ramps, protecting against falling into the deep."@en ,
                                    "http://bsdd.buildingsmart.org/#concept/details/0ZHKicPyL9l8uyCir_Dsef"@en ,
                                    "http://bsdd.buildingsmart.org/#concept/details/30Ez0HE6XAHQh6wJkRK6T$"@en ;
                       rdfs:label "Balustrade"@en ,
                                  "Geländer"@de-de ,
                                  "Hekwerk"@nl-nl ,
                                  "balustrader"@nb-no ,
                                  "rekkverk"@nb-no ;
                       rdfs:seeAlso ifc:IfcRailingEnumType .


###  http://pi.pauwel.be/voc/buildingelement#Railing-GUARDRAIL
beo:Railing-GUARDRAIL rdf:type owl:Class ;
                      rdfs:subClassOf beo:Railing ;
                      rdfs:comment "A frame assembly adjacent to human circulation spaces and at some space boundaries where it is used in line of walls or to compliment walls. Designed to aid humans, either as an optional physical support, or to prevent injury by falling."@en ,
                                   "http://bsdd.buildingsmart.org/#concept/details/2804vLstn5DfaH_vxv53w3"@en ;
                      rdfs:label "Garde corps"@fr-fr ,
                                 "Geländer"@de-de ,
                                 "Guardrail"@en ,
                                 "garde-corps"@fr-fr ,
                                 "rekkverk"@nb-no ;
                      rdfs:seeAlso ifc:IfcRailingEnumType .


###  http://pi.pauwel.be/voc/buildingelement#Railing-HANDRAIL
beo:Railing-HANDRAIL rdf:type owl:Class ;
                     rdfs:subClassOf beo:Railing ;
                     rdfs:comment "Håndlister, typisk i korridorer"@nb-no ,
                                  "http://bsdd.buildingsmart.org/#concept/details/3vHRZWoT0Hsm00051Mm008"@en ;
                     rdfs:label "Handlauf"@de-de ,
                                "Handrail"@en ,
                                "håndlist"@nb-no ,
                                "main courante"@fr-fr ;
                     rdfs:seeAlso ifc:IfcRailingEnumType .


###  http://pi.pauwel.be/voc/buildingelement#Ramp
beo:Ramp rdf:type owl:Class ;
         rdfs:subClassOf beo:BuildingElement ;
         rdfs:comment "A vertical passageway which provides a human circulation link between one floor level and another floor level at a different elevation. Normally does not include steps."@en ,
                      "Rampe"@nb-no ,
                      "http://bsdd.buildingsmart.org/#concept/details/0kpjo0qVyHuO00025QrE$V"@en ;
         rdfs:label "Helling"@nl ,
                    "Ramp"@en ,
                    "Rampe"@da ,
                    "Rampe"@de-de ,
                    "Rampe"@fr-fr ,
                    "helling"@nl-nl ,
                    "hellingbaan"@nl-nl ,
                    "rampe"@nb-no ,
                    "skråplan"@nb-no ;
         rdfs:seeAlso ifc:IfcRamp .


###  http://pi.pauwel.be/voc/buildingelement#Ramp-HALF_TURN_RAMP
beo:Ramp-HALF_TURN_RAMP rdf:type owl:Class ;
                        rdfs:subClassOf beo:Ramp ;
                        rdfs:comment "http://bsdd.buildingsmart.org/#concept/details/1hJB5FgjL4_v2TrvOBjmzz"@en ;
                        rdfs:label "Half Turn Ramp"@en ,
                                   "halv omdreining rampe"@nb-no ;
                        rdfs:seeAlso ifc:IfcRampEnumType .


###  http://pi.pauwel.be/voc/buildingelement#Ramp-QUARTER_TURN_RAMP
beo:Ramp-QUARTER_TURN_RAMP rdf:type owl:Class ;
                           rdfs:subClassOf beo:Ramp ;
                           rdfs:comment "http://bsdd.buildingsmart.org/#concept/details/1FZ7G8CAP2UxmW6fnuOOfQ"@en ;
                           rdfs:label "Quarter Turn Ramp"@en ,
                                      "rampe med en sving"@nb-no ;
                           rdfs:seeAlso ifc:IfcRampEnumType .


###  http://pi.pauwel.be/voc/buildingelement#Ramp-SPIRAL_RAMP
beo:Ramp-SPIRAL_RAMP rdf:type owl:Class ;
                     rdfs:subClassOf beo:Ramp ;
                     rdfs:comment "http://bsdd.buildingsmart.org/#concept/details/2__YGgu4XCN9NmT3LhvE6V"@en ;
                     rdfs:label "Spiral Ramp"@en ;
                     rdfs:seeAlso ifc:IfcRampEnumType .


###  http://pi.pauwel.be/voc/buildingelement#Ramp-STRAIGHT_RUN_RAMP
beo:Ramp-STRAIGHT_RUN_RAMP rdf:type owl:Class ;
                           rdfs:subClassOf beo:Ramp ;
                           rdfs:comment "http://bsdd.buildingsmart.org/#concept/details/1SYNqJ72H64g7EG2vm8VJu"@en ;
                           rdfs:label "Straight Run Ramp"@en ;
                           rdfs:seeAlso ifc:IfcRampEnumType .


###  http://pi.pauwel.be/voc/buildingelement#Ramp-TWO_QUARTER_TURN_RAMP
beo:Ramp-TWO_QUARTER_TURN_RAMP rdf:type owl:Class ;
                               rdfs:subClassOf beo:Ramp ;
                               rdfs:comment "http://bsdd.buildingsmart.org/#concept/details/2wUjACPhnDyAgFiGarLaek"@en ;
                               rdfs:label "Two Quarter Turn Ramp"@en ,
                                          "rampe med to svinger"@nb-no ;
                               rdfs:seeAlso ifc:IfcRampEnumType .


###  http://pi.pauwel.be/voc/buildingelement#Ramp-TWO_STRAIGHT_RUN_RAMP
beo:Ramp-TWO_STRAIGHT_RUN_RAMP rdf:type owl:Class ;
                               rdfs:subClassOf beo:Ramp ;
                               rdfs:comment "http://bsdd.buildingsmart.org/#concept/details/2skPwOQSH1Ex7UR3SpDGbT"@en ;
                               rdfs:label "Two Straight Run Ramp"@en ;
                               rdfs:seeAlso ifc:IfcRampEnumType .


###  http://pi.pauwel.be/voc/buildingelement#RampFlight
beo:RampFlight rdf:type owl:Class ;
               rdfs:subClassOf beo:BuildingElement ;
               rdfs:comment "A single inclined segment, or several inclined segments that are connected by a horizontal segment, referred to as a landing. "@en ,
                            "http://bsdd.buildingsmart.org/#concept/details/1kbSG0qVyHuO00025QrE$V"@en ;
               rdfs:label "Ramp Flight"@en ,
                          "Rampenlauf"@de-de ,
                          "Volée"@fr-fr ,
                          "rampe"@nb-no ;
               rdfs:seeAlso ifc:IfcRampFlight .


###  http://pi.pauwel.be/voc/buildingelement#RampFlight-SPIRAL
beo:RampFlight-SPIRAL rdf:type owl:Class ;
                      rdfs:subClassOf beo:RampFlight ;
                      rdfs:comment "http://bsdd.buildingsmart.org/#concept/details/0CDsSbmyb4GA$0xajhCLYB"@en ;
                      rdfs:label "Spiral"@en ,
                                 "spiral"@nb-no ,
                                 "vindel"@nb-no ;
                      rdfs:seeAlso ifc:IfcRampFlightEnumType .


###  http://pi.pauwel.be/voc/buildingelement#RampFlight-STRAIGHT
beo:RampFlight-STRAIGHT rdf:type owl:Class ;
                        rdfs:subClassOf beo:RampFlight ;
                        rdfs:comment "http://bsdd.buildingsmart.org/#concept/details/0fyv31IoL8mwvU9TcZR2FC"@en ;
                        rdfs:label "Straight"@en ,
                                   "rett"@nb-no ;
                        rdfs:seeAlso ifc:IfcRampFlightEnumType .


###  http://pi.pauwel.be/voc/buildingelement#ReinforcingBar
beo:ReinforcingBar rdf:type owl:Class ;
                   rdfs:subClassOf beo:ReinforcingElement ;
                   rdfs:comment "a reinforcing bar is usually made of steel with manufactured deformations in the surface, and used in concrete and masonry construction to provide additional strength. a single instance of this class may represent one or many of actual rebars, for example a row of rebars."@en ,
                                "http://bsdd.buildingsmart.org/#concept/details/1zlbN6A$z4r8Er6nWNbSMZ"@en ;
                   rdfs:label "Bewehrungsstab"@de-de ,
                              "Reinforcing Bar"@en ,
                              "armeringsstang"@nb-no ,
                              "barre d'armature"@fr-fr ;
                   rdfs:seeAlso ifc:IfcReinforcingBar .


###  http://pi.pauwel.be/voc/buildingelement#ReinforcingBar-ANCHORING
beo:ReinforcingBar-ANCHORING rdf:type owl:Class ;
                             rdfs:subClassOf beo:ReinforcingBar ;
                             rdfs:comment "http://bsdd.buildingsmart.org/#concept/details/3X1mNZzk542ez6g92TTVdH"@en ;
                             rdfs:label "Anchoring"@en ;
                             rdfs:seeAlso ifc:IfcReinforcingBarEnumType .


###  http://pi.pauwel.be/voc/buildingelement#ReinforcingBar-EDGE
beo:ReinforcingBar-EDGE rdf:type owl:Class ;
                        rdfs:subClassOf beo:ReinforcingBar ;
                        rdfs:comment "http://bsdd.buildingsmart.org/#concept/details/0tRGNh1sv19OvGghikeGYQ"@en ;
                        rdfs:label "Edge"@en ;
                        rdfs:seeAlso ifc:IfcReinforcingBarEnumType .


###  http://pi.pauwel.be/voc/buildingelement#ReinforcingBar-LIGATURE
beo:ReinforcingBar-LIGATURE rdf:type owl:Class ;
                            rdfs:subClassOf beo:ReinforcingBar ;
                            rdfs:comment "http://bsdd.buildingsmart.org/#concept/details/09DzOB3qT10AwjdzYLo1LA"@en ;
                            rdfs:label "Ligature"@en ;
                            rdfs:seeAlso ifc:IfcReinforcingBarEnumType .


###  http://pi.pauwel.be/voc/buildingelement#ReinforcingBar-MAIN
beo:ReinforcingBar-MAIN rdf:type owl:Class ;
                        rdfs:subClassOf beo:ReinforcingBar ;
                        rdfs:comment "http://bsdd.buildingsmart.org/#concept/details/0ZDnwDkMT9fhTxjjLnIpAX"@en ;
                        rdfs:label "Main"@en ;
                        rdfs:seeAlso ifc:IfcReinforcingBarEnumType .


###  http://pi.pauwel.be/voc/buildingelement#ReinforcingBar-PUNCHING
beo:ReinforcingBar-PUNCHING rdf:type owl:Class ;
                            rdfs:subClassOf beo:ReinforcingBar ;
                            rdfs:comment "http://bsdd.buildingsmart.org/#concept/details/1RO$_IvNP7eQABna$VzMm_"@en ;
                            rdfs:label "Punching"@en ;
                            rdfs:seeAlso ifc:IfcReinforcingBarEnumType .


###  http://pi.pauwel.be/voc/buildingelement#ReinforcingBar-RING
beo:ReinforcingBar-RING rdf:type owl:Class ;
                        rdfs:subClassOf beo:ReinforcingBar ;
                        rdfs:comment "http://bsdd.buildingsmart.org/#concept/details/2zA8DFnW5B8hiBjIlXcktx"@en ;
                        rdfs:label "Ring"@en ;
                        rdfs:seeAlso ifc:IfcReinforcingBarEnumType .


###  http://pi.pauwel.be/voc/buildingelement#ReinforcingBar-SHEAR
beo:ReinforcingBar-SHEAR rdf:type owl:Class ;
                         rdfs:subClassOf beo:ReinforcingBar ;
                         rdfs:comment "http://bsdd.buildingsmart.org/#concept/details/220Wv8D4n11hjTIo_DzfBR"@en ;
                         rdfs:label "Shear"@en ,
                                    "skive"@nb-no ;
                         rdfs:seeAlso ifc:IfcReinforcingBarEnumType .


###  http://pi.pauwel.be/voc/buildingelement#ReinforcingBar-STUD
beo:ReinforcingBar-STUD rdf:type owl:Class ;
                        rdfs:subClassOf beo:ReinforcingBar ;
                        rdfs:comment "http://bsdd.buildingsmart.org/#concept/details/3cWXnrQEvAfRCh9LjK26$R"@en ;
                        rdfs:label "Stud"@en ,
                                   "stender"@nb-no ;
                        rdfs:seeAlso ifc:IfcReinforcingBarEnumType .


###  http://pi.pauwel.be/voc/buildingelement#ReinforcingElement
beo:ReinforcingElement rdf:type owl:Class ;
                       rdfs:subClassOf beo:ElementComponent ;
                       rdfs:comment "a reinforcing element represents bars, wires, strands, meshes, tendons, and other components embedded in concrete in such a manner that the reinforcement and the concrete act together in resisting forces."@en ,
                                    "http://bsdd.buildingsmart.org/#concept/details/1aiY$$Wf98m8a5cp3Hzgdu"@en ;
                       rdfs:label "Bewehrung"@de-de ,
                                  "Reinforcing Element"@en ,
                                  "elément d'armature"@fr-fr ;
                       rdfs:seeAlso ifc:IfcReinforcingElement .


###  http://pi.pauwel.be/voc/buildingelement#ReinforcingMesh
beo:ReinforcingMesh rdf:type owl:Class ;
                    rdfs:subClassOf beo:ReinforcingElement ;
                    rdfs:comment "a reinforcing mesh is a series of longitudinal and transverse wires or bars of various gauges, arranged at right angles to each other and welded at all points of intersection; usually used for concrete slab reinforcement. it is also known as welded wire fabric. in scope are plane meshes as well as bent meshes."@en ,
                                 "http://bsdd.buildingsmart.org/#concept/details/3R4n2h6wn67Q4clocrGT7J"@en ;
                    rdfs:label "Bewehrungsmatte"@de-de ,
                               "Reinforcing Mesh"@en ,
                               "treillis"@fr-fr ;
                    rdfs:seeAlso ifc:IfcReinforcingMesh .


###  http://pi.pauwel.be/voc/buildingelement#Roof
beo:Roof rdf:type owl:Class ;
         rdfs:subClassOf beo:BuildingElement ;
         rdfs:comment "A covering of the top part of a building. Protects the building against the effects of weather."@en ,
                      "http://bsdd.buildingsmart.org/#concept/details/2Iyg00qW4HuO00025QrE$V"@en ;
         rdfs:label "Dach"@de-de ,
                    "Dak"@nl ,
                    "Roof"@en ,
                    "Tag"@da ,
                    "toiture"@fr-fr ;
         rdfs:seeAlso ifc:IfcRoof .


###  http://pi.pauwel.be/voc/buildingelement#Roof-BARREL_ROOF
beo:Roof-BARREL_ROOF rdf:type owl:Class ;
                     rdfs:subClassOf beo:Roof ;
                     rdfs:comment "http://bsdd.buildingsmart.org/#concept/details/172RLdein1b8WIbTtDLVbc"@en ;
                     rdfs:label "Barrel Roof"@en ;
                     rdfs:seeAlso ifc:IfcRoofEnumType .


###  http://pi.pauwel.be/voc/buildingelement#Roof-BUTTERFLY_ROOF
beo:Roof-BUTTERFLY_ROOF rdf:type owl:Class ;
                        rdfs:subClassOf beo:Roof ;
                        rdfs:comment "http://bsdd.buildingsmart.org/#concept/details/2W6yLK2r968h2TWfGC2xWu"@en ;
                        rdfs:label "Butterfly Roof"@en ;
                        rdfs:seeAlso ifc:IfcRoofEnumType .


###  http://pi.pauwel.be/voc/buildingelement#Roof-DOME_ROOF
beo:Roof-DOME_ROOF rdf:type owl:Class ;
                   rdfs:subClassOf beo:Roof ;
                   rdfs:comment "http://bsdd.buildingsmart.org/#concept/details/3UcE2aJPP4ewOoRn29unfZ"@en ;
                   rdfs:label "Dome Roof"@en ,
                              "kuppeltak"@nb-no ;
                   rdfs:seeAlso ifc:IfcRoofEnumType .


###  http://pi.pauwel.be/voc/buildingelement#Roof-FLAT_ROOF
beo:Roof-FLAT_ROOF rdf:type owl:Class ;
                   rdfs:subClassOf beo:Roof ;
                   rdfs:comment "http://bsdd.buildingsmart.org/#concept/details/3IeKrtrMz2SQN7qpJt82e5"@en ;
                   rdfs:label "Flat Roof"@en ,
                              "flatt tak"@nb-no ;
                   rdfs:seeAlso ifc:IfcRoofEnumType .


###  http://pi.pauwel.be/voc/buildingelement#Roof-FREEFORM
beo:Roof-FREEFORM rdf:type owl:Class ;
                  rdfs:subClassOf beo:Roof ;
                  rdfs:comment "http://bsdd.buildingsmart.org/#concept/details/2KVHvK7iXAEfKlD5hGIFEc"@en ;
                  rdfs:label "Free Form Roof"@en ,
                             "friform tak"@nb-no ;
                  rdfs:seeAlso ifc:IfcRoofEnumType .


###  http://pi.pauwel.be/voc/buildingelement#Roof-GABLE_ROOF
beo:Roof-GABLE_ROOF rdf:type owl:Class ;
                    rdfs:subClassOf beo:Roof ;
                    rdfs:comment "http://bsdd.buildingsmart.org/#concept/details/0gHJNRNhz6LOTHVbnW$nEj"@en ;
                    rdfs:label "Gable Roof"@en ,
                               "gavl"@nb-no ;
                    rdfs:seeAlso ifc:IfcRoofEnumType .


###  http://pi.pauwel.be/voc/buildingelement#Roof-GAMBREL_ROOF
beo:Roof-GAMBREL_ROOF rdf:type owl:Class ;
                      rdfs:subClassOf beo:Roof ;
                      rdfs:comment "http://bsdd.buildingsmart.org/#concept/details/2BnDhKP1HF3vXxnwqccewa"@en ;
                      rdfs:label "Gambrel Roof"@en ,
                                 "gambrel tak"@nb-no ;
                      rdfs:seeAlso ifc:IfcRoofEnumType .


###  http://pi.pauwel.be/voc/buildingelement#Roof-HIPPED_GABLE_ROOF
beo:Roof-HIPPED_GABLE_ROOF rdf:type owl:Class ;
                           rdfs:subClassOf beo:Roof ;
                           rdfs:comment "http://bsdd.buildingsmart.org/#concept/details/3Su_2ncLX1Oes0r3fNr4uE"@en ;
                           rdfs:label "Hipped Gable Roof"@en ,
                                      "valm/saltak"@nb-no ;
                           rdfs:seeAlso ifc:IfcRoofEnumType .


###  http://pi.pauwel.be/voc/buildingelement#Roof-HIP_ROOF
beo:Roof-HIP_ROOF rdf:type owl:Class ;
                  rdfs:subClassOf beo:Roof ;
                  rdfs:comment "http://bsdd.buildingsmart.org/#concept/details/0waejMcyT3zwP6nRClvfSx"@en ;
                  rdfs:label "Hip Roof"@en ,
                             "valmtak"@nb-no ;
                  rdfs:seeAlso ifc:IfcRoofEnumType .


###  http://pi.pauwel.be/voc/buildingelement#Roof-MANSARD_ROOF
beo:Roof-MANSARD_ROOF rdf:type owl:Class ;
                      rdfs:subClassOf beo:Roof ;
                      rdfs:comment "http://bsdd.buildingsmart.org/#concept/details/1hB_MPg3j35vRsm_vutjD2"@en ;
                      rdfs:label "Mansard Roof"@en ,
                                 "mansardtak"@nb-no ;
                      rdfs:seeAlso ifc:IfcRoofEnumType .


###  http://pi.pauwel.be/voc/buildingelement#Roof-PAVILION_ROOF
beo:Roof-PAVILION_ROOF rdf:type owl:Class ;
                       rdfs:subClassOf beo:Roof ;
                       rdfs:comment "http://bsdd.buildingsmart.org/#concept/details/11Ltv09Eb7lRJW184fZ9gF"@en ;
                       rdfs:label "Pavilion Roof"@en ,
                                  "paviljongtak"@nb-no ;
                       rdfs:seeAlso ifc:IfcRoofEnumType .


###  http://pi.pauwel.be/voc/buildingelement#Roof-RAINBOW_ROOF
beo:Roof-RAINBOW_ROOF rdf:type owl:Class ;
                      rdfs:subClassOf beo:Roof ;
                      rdfs:comment "http://bsdd.buildingsmart.org/#concept/details/1MnaPoqUb0L8PGqS6yHzbq"@en ;
                      rdfs:label "Rainbow Roof"@en ,
                                 "buetak"@nb-no ;
                      rdfs:seeAlso ifc:IfcRoofEnumType .


###  http://pi.pauwel.be/voc/buildingelement#Roof-SHED_ROOF
beo:Roof-SHED_ROOF rdf:type owl:Class ;
                   rdfs:subClassOf beo:Roof ;
                   rdfs:comment "http://bsdd.buildingsmart.org/#concept/details/3GsCyHvinDMPWmecHluOEq"@en ;
                   rdfs:label "Shed Roof"@en ,
                              "pulttak"@nb-no ;
                   rdfs:seeAlso ifc:IfcRoofEnumType .


###  http://pi.pauwel.be/voc/buildingelement#ShadingDevice
beo:ShadingDevice rdf:type owl:Class ;
                  rdfs:subClassOf beo:BuildingElement ;
                  rdfs:comment """Purpose built devices to protect from the sunlight, from natural light, or screening them from view. Shading devices can form part of the facade or can be mounted inside the building, they can be fixed or operable.
"""@en ,
                               "http://bsdd.buildingsmart.org/#concept/details/11vQg0qWSHuO00025QrE$V"@en ;
                  rdfs:label "Afskærmningsanordning"@da ,
                             "Shading Device"@en ,
                             "Sonnenschutz festeingebaut"@de-de ,
                             "Zonnewering"@nl ,
                             "protection solaire"@fr-fr ,
                             "skjermingstype"@nb-no ;
                  rdfs:seeAlso ifc:IfcShadingDevice .


###  http://pi.pauwel.be/voc/buildingelement#ShadingDevice-AWNING
beo:ShadingDevice-AWNING rdf:type owl:Class ;
                         rdfs:subClassOf beo:ShadingDevice ;
                         rdfs:comment "a rooflike shelter of canvas or other material extending over a doorway, from the top of a window, over a deck, etc., in order to provide protection, as from the sun"@en ,
                                      "http://bsdd.buildingsmart.org/#concept/details/3NoPxSKmL7yQEzPT8cmssT"@en ,
                                      "product made of fabric/material, located externally, above, in front of, or within an opening and extending in a horizontal and/or sloping and/or vertical plane"@en ,
                                      "produkt laget av stoff/materiale som plasseres utvendig over, foran eller i en åpning, og som stikker ut i et horisontalt og/eller skrånende og/eller vertikalt plan"@nb-no ;
                         rdfs:label "Awning"@en ,
                                    "Zonwering"@nl-nl ,
                                    "markise"@nb-no ,
                                    "solskjerming"@nb-no .


###  http://pi.pauwel.be/voc/buildingelement#ShadingDevice-JALOUSIE
beo:ShadingDevice-JALOUSIE rdf:type owl:Class ;
                           rdfs:subClassOf beo:ShadingDevice ;
                           rdfs:comment "Solavskjerming, Persienner"@nb-no ,
                                        "http://bsdd.buildingsmart.org/#concept/details/1$w9Dw6W9DJvD2GfuZFMSR"@en ,
                                        "http://bsdd.buildingsmart.org/#concept/details/3vHLsWoT0Hsm00051Mm008"@en ,
                                        "product consisting of horizontal slats which can be tilted. it may be retracted by raising and stacking the slats."@en ;
                           rdfs:label "Jalousie"@de-de ,
                                      "Jalousie"@en ,
                                      "blinds"@en ,
                                      "lamell"@nb-no ,
                                      "persienne"@nb-no ,
                                      "persienner"@nb-no ,
                                      "sjalusi"@nb-no ,
                                      "stores vénetiens"@fr-fr ,
                                      "sun shading device"@en ,
                                      "venetian blind"@en ;
                           rdfs:seeAlso ifc:IfcShadingDeviceEnumType .


###  http://pi.pauwel.be/voc/buildingelement#ShadingDevice-SHUTTER
beo:ShadingDevice-SHUTTER rdf:type owl:Class ;
                          rdfs:subClassOf beo:ShadingDevice ;
                          rdfs:comment "An artefact which is a part of an assembly that can be moved from a position where it permits contact, to a position where it becomes a part of the enclosure or partition shielding the fixed contacts.                "@en ,
                                       "Movable component installed in an opening or duct to form a barrier for security purposes; used to control the passage of heat or light or to delay the spread of fire, smoke or gases."@en ,
                                       "Solavskjerming, Solgardin"@nb-no ,
                                       "Sun-shading device"@en ,
                                       "http://bsdd.buildingsmart.org/#concept/details/0w_lVI8P10c9rjT$RsNEVr"@en ,
                                       "http://bsdd.buildingsmart.org/#concept/details/27f2fkTV50YwB1IZgMURLa"@en ,
                                       "http://bsdd.buildingsmart.org/#concept/details/3vHUzKoT0Hsm00051Mm008"@en ,
                                       "product installed either internally or externally to provide additional covering and/or protection to an opening"@en ;
                          rdfs:label "Abschluß"@de-de ,
                                     "Shutter"@en ,
                                     "fermeture"@fr-fr ,
                                     "markise"@nb-no ,
                                     "skodde"@nb-no ,
                                     "solgardin"@nb-no ;
                          rdfs:seeAlso ifc:IfcShadingDeviceEnumType .


###  http://pi.pauwel.be/voc/buildingelement#Slab
beo:Slab rdf:type owl:Class ;
         rdfs:subClassOf beo:BuildingElement ;
         rdfs:comment """A component of the construction that normally encloses a space vertically. May provide the lower support (floor) or upper construction (roof slab) in any space in a building.
Only the core or constructional part of this construction is considered to be a slab. The upper finish (flooring, roofing) and the lower finish (ceiling, suspended ceiling) are considered to be coverings. """@en ,
                      "http://bsdd.buildingsmart.org/#concept/details/3pXDk0qWSHuO00025QrE$V"@en ;
         rdfs:label "Decke / Dachfläche / Bodenplatte"@de-de ,
                    "Dæk"@da ,
                    "Plaat"@nl ,
                    "Slab"@en ,
                    "dalle"@fr-fr ,
                    "dekke"@nb-no ;
         rdfs:seeAlso ifc:IfcSlab .


###  http://pi.pauwel.be/voc/buildingelement#Slab-BASESLAB
beo:Slab-BASESLAB rdf:type owl:Class ;
                  rdfs:subClassOf beo:Slab ;
                  rdfs:comment "http://bsdd.buildingsmart.org/#concept/details/1hBroEIeL9neS3mSSGZiyC"@en ;
                  rdfs:label "Base Slab" ,
                             "støpt fundament"@nb-no ;
                  rdfs:seeAlso ifc:IfcSlabEnumType .


###  http://pi.pauwel.be/voc/buildingelement#Slab-FLOOR
beo:Slab-FLOOR rdf:type owl:Class ;
               rdfs:subClassOf beo:Slab ;
               rdfs:comment "http://bsdd.buildingsmart.org/#concept/details/0jBALpJIv7vvlWkbd9HdCx"@en ;
               rdfs:label "Floor"@en ,
                          "dekke"@nb-no ,
                          "gulv"@nb-no ;
               rdfs:seeAlso ifc:IfcSlabEnumType .


###  http://pi.pauwel.be/voc/buildingelement#Slab-LANDING
beo:Slab-LANDING rdf:type owl:Class ;
                 rdfs:subClassOf beo:Slab ;
                 rdfs:comment "http://bsdd.buildingsmart.org/#concept/details/3tQbZvvrfA8OUjU1kc2rUZ"@en ;
                 rdfs:label "Landing"@en ,
                            "repo"@nb-no ;
                 rdfs:seeAlso ifc:IfcSlabEnumType .


###  http://pi.pauwel.be/voc/buildingelement#Slab-ROOF
beo:Slab-ROOF rdf:type owl:Class ;
              rdfs:subClassOf beo:Slab ;
              rdfs:comment "A covering of the top part of a building. Protects the building against the effects of weather."@en ,
                           "http://bsdd.buildingsmart.org/#concept/details/3Hvwx39_rCaRS49F4qRGBb"@en ;
              rdfs:label "Dach"@de-de ,
                         "Roof"@en ,
                         "flatt tak"@nb-no ,
                         "toiture"@fr-fr ;
              rdfs:seeAlso ifc:IfcSlabEnumType .


###  http://pi.pauwel.be/voc/buildingelement#Stair
beo:Stair rdf:type owl:Class ;
          rdfs:subClassOf beo:BuildingElement ;
          rdfs:comment "A vertical passageway allowing occupants to walk (step) from one floor level to another floor level at a different elevation. May include a landing as an intermediate floor slab."@en ,
                       "http://bsdd.buildingsmart.org/#concept/details/3DhWM0qWmHuO00025QrE$V"@en ;
          rdfs:label "Stair"@en ,
                     "Trap"@nl ,
                     "Trap"@nl-nl ,
                     "Trappe"@da ,
                     "Trapslag"@nl-nl ,
                     "Treppe"@de-de ,
                     "escalier"@fr-fr ,
                     "trapp"@nb-no ;
          rdfs:seeAlso ifc:IfcStair .


###  http://pi.pauwel.be/voc/buildingelement#Stair-CURVED_RUN_STAIR
beo:Stair-CURVED_RUN_STAIR rdf:type owl:Class ;
                           rdfs:subClassOf beo:Stair ;
                           rdfs:comment "a stair extending from one level to another without turns or winders. the stair is consisting of one curved flight."@en ,
                                        "http://bsdd.buildingsmart.org/#concept/details/1lkxIX8Gj23Bi50H2qpZB9"@en ;
                           rdfs:label "Curved Run Stair"@en ;
                           rdfs:seeAlso ifc:IfcStairEnumType .


###  http://pi.pauwel.be/voc/buildingelement#Stair-DOUBLE_RETURN_STAIR
beo:Stair-DOUBLE_RETURN_STAIR rdf:type owl:Class ;
                              rdfs:subClassOf beo:Stair ;
                              rdfs:comment "a stair having one straight flight to a wide quarterspace landing, and two side flights from that landing into opposite directions. the stair is making a 90° turn. the direction of traffic is determined by the walking line."@en ,
                                           "http://bsdd.buildingsmart.org/#concept/details/3NNCQTceL7Uf8ZhJf40gs9"@en ;
                              rdfs:label "Double Return Stair"@en ;
                              rdfs:seeAlso ifc:IfcStairEnumType .


###  http://pi.pauwel.be/voc/buildingelement#Stair-HALF_TURN_STAIR
beo:Stair-HALF_TURN_STAIR rdf:type owl:Class ;
                          rdfs:subClassOf beo:Stair ;
                          rdfs:comment "a stair making a 180° turn, consisting of two straight flights connected by a halfspace landing. the orientation of the turn is determined by the walking line."@en ,
                                       "http://bsdd.buildingsmart.org/#concept/details/3YmaH1onP90PM6kEWHUjFv"@en ;
                          rdfs:label "Half Turn Stair"@en ;
                          rdfs:seeAlso ifc:IfcStairEnumType .


###  http://pi.pauwel.be/voc/buildingelement#Stair-HALF_WINDING_STAIR
beo:Stair-HALF_WINDING_STAIR rdf:type owl:Class ;
                             rdfs:subClassOf beo:Stair ;
                             rdfs:comment "http://bsdd.buildingsmart.org/#concept/details/0Vw081Hfz1AQne1V5CsfUA"@en ;
                             rdfs:label "Half Winding Stair"@en ;
                             rdfs:seeAlso ifc:IfcStairEnumType .


###  http://pi.pauwel.be/voc/buildingelement#Stair-QUARTER_TURN_STAIR
beo:Stair-QUARTER_TURN_STAIR rdf:type owl:Class ;
                             rdfs:subClassOf beo:Stair ;
                             rdfs:comment "a stair making a 90° turn, consisting of two straight flights connected by a quarterspace landing. the direction of the turn is determined by the walking line."@en ,
                                          "http://bsdd.buildingsmart.org/#concept/details/1IEbbDJDHAFQb9SZweXH3x"@en ;
                             rdfs:label "Quarter Turn Stair"@en ;
                             rdfs:seeAlso ifc:IfcStairEnumType .


###  http://pi.pauwel.be/voc/buildingelement#Stair-QUARTER_WINDING_STAIR
beo:Stair-QUARTER_WINDING_STAIR rdf:type owl:Class ;
                                rdfs:subClassOf beo:Stair ;
                                rdfs:comment "http://bsdd.buildingsmart.org/#concept/details/3PzSNWl5T1EgMXH$Tn6uuQ"@en ;
                                rdfs:label "Quarter Winding Stair"@en ;
                                rdfs:seeAlso ifc:IfcStairEnumType .


###  http://pi.pauwel.be/voc/buildingelement#Stair-SPIRAL_STAIR
beo:Stair-SPIRAL_STAIR rdf:type owl:Class ;
                       rdfs:subClassOf beo:Stair ;
                       rdfs:comment "http://bsdd.buildingsmart.org/#concept/details/0UwQe$TXP47AhE5k0mZzCe"@en ;
                       rdfs:label "Spiral Stair"@en ;
                       rdfs:seeAlso ifc:IfcStairEnumType .


###  http://pi.pauwel.be/voc/buildingelement#Stair-STRAIGHT_RUN_STAIR
beo:Stair-STRAIGHT_RUN_STAIR rdf:type owl:Class ;
                             rdfs:subClassOf beo:Stair ;
                             rdfs:comment "http://bsdd.buildingsmart.org/#concept/details/3p4WSJmK96Oe6HXE$jmWWy"@en ;
                             rdfs:label "Straight Run Stair"@en ;
                             rdfs:seeAlso ifc:IfcStairEnumType .


###  http://pi.pauwel.be/voc/buildingelement#Stair-THREE_QUARTER_TURN_STAIR
beo:Stair-THREE_QUARTER_TURN_STAIR rdf:type owl:Class ;
                                   rdfs:subClassOf beo:Stair ;
                                   rdfs:comment "http://bsdd.buildingsmart.org/#concept/details/2jTG3NRNHCyhbsMbwK38v5"@en ;
                                   rdfs:label "Three Quarter Turn Stair"@en ;
                                   rdfs:seeAlso ifc:IfcStairEnumType .


###  http://pi.pauwel.be/voc/buildingelement#Stair-THREE_QUARTER_WINDING_STAIR
beo:Stair-THREE_QUARTER_WINDING_STAIR rdf:type owl:Class ;
                                      rdfs:subClassOf beo:Stair ;
                                      rdfs:comment "http://bsdd.buildingsmart.org/#concept/details/0rPjGYk_LFnOayZFsJg3tr"@en ;
                                      rdfs:label "Three Quarter Winding Stair"@en ;
                                      rdfs:seeAlso ifc:IfcStairEnumType .


###  http://pi.pauwel.be/voc/buildingelement#Stair-TWO_CURVED_RUN_STAIR
beo:Stair-TWO_CURVED_RUN_STAIR rdf:type owl:Class ;
                               rdfs:subClassOf beo:Stair ;
                               rdfs:comment "http://bsdd.buildingsmart.org/#concept/details/0cSo1dkGL8NunRzp$sQsTc"@en ;
                               rdfs:label "Two Curved Run Stair"@en ;
                               rdfs:seeAlso ifc:IfcStairEnumType .


###  http://pi.pauwel.be/voc/buildingelement#Stair-TWO_QUARTER_TURN_STAIR
beo:Stair-TWO_QUARTER_TURN_STAIR rdf:type owl:Class ;
                                 rdfs:subClassOf beo:Stair ;
                                 rdfs:comment "a stair making a 180° turn, consisting of three straight flights connected by two quarterspace landings. the direction of the turns is determined by the walking line"@en ,
                                              "http://bsdd.buildingsmart.org/#concept/details/0mW4DtraD3SA57fcejW4cS"@en ;
                                 rdfs:label "Two Quarter Turn Stair"@en ;
                                 rdfs:seeAlso ifc:IfcStairEnumType .


###  http://pi.pauwel.be/voc/buildingelement#Stair-TWO_QUARTER_WINDING_STAIR
beo:Stair-TWO_QUARTER_WINDING_STAIR rdf:type owl:Class ;
                                    rdfs:subClassOf beo:Stair ;
                                    rdfs:comment "http://bsdd.buildingsmart.org/#concept/details/3SSlfuJ_nA49lzIOhda6Xr"@en ;
                                    rdfs:label "Two Quarter Winding Stair"@en ;
                                    rdfs:seeAlso ifc:IfcStairEnumType .


###  http://pi.pauwel.be/voc/buildingelement#Stair-TWO_STRAIGHT_RUN_STAIR
beo:Stair-TWO_STRAIGHT_RUN_STAIR rdf:type owl:Class ;
                                 rdfs:subClassOf beo:Stair ;
                                 rdfs:comment "a straight stair consisting of two straight flights without turns but with one landing."@en ,
                                              "http://bsdd.buildingsmart.org/#concept/details/3VuqGJNz160B87TSrFhrM4"@en ;
                                 rdfs:label "Two Straight Run Stair"@en ;
                                 rdfs:seeAlso ifc:IfcStairEnumType .


###  http://pi.pauwel.be/voc/buildingelement#StairFlight
beo:StairFlight rdf:type owl:Class ;
                rdfs:subClassOf beo:BuildingElement ;
                rdfs:comment "An assembly of building components in a single \"run\" of stair steps (not interrupted by a landing)."@en ,
                             "http://bsdd.buildingsmart.org/#concept/details/0pceq0qWqHuO00025QrE$V"@en ;
                rdfs:label "Stair Flight"@en ,
                           "Volée d'escalier"@fr-fr ,
                           "trap"@nl-nl ,
                           "trapp"@nb-no ,
                           "trapslag"@nl-nl ,
                           "treppenlauf"@de-de ;
                rdfs:seeAlso ifc:IfcStairFlight .


###  http://pi.pauwel.be/voc/buildingelement#StairFlight-CURVED
beo:StairFlight-CURVED rdf:type owl:Class ;
                       rdfs:subClassOf beo:StairFlight ;
                       rdfs:comment "http://bsdd.buildingsmart.org/#concept/details/2DeCDqEVHDjwFaGVpyNC89"@en ;
                       rdfs:label "Curved"@en ,
                                  "trapp - kurvet"@nb-no ;
                       rdfs:seeAlso ifc:IfcStairFlightEnumType .


###  http://pi.pauwel.be/voc/buildingelement#StairFlight-FREEFORM
beo:StairFlight-FREEFORM rdf:type owl:Class ;
                         rdfs:subClassOf beo:StairFlight ;
                         rdfs:comment "http://bsdd.buildingsmart.org/#concept/details/0uFuIDRO1EZPmcL8pEkVU$"@en ;
                         rdfs:label "Freeform" ,
                                    "friform"@nb-no ,
                                    "friform tak"@nb-no ;
                         rdfs:seeAlso ifc:IfcStairFlightEnumType .


###  http://pi.pauwel.be/voc/buildingelement#StairFlight-SPIRAL
beo:StairFlight-SPIRAL rdf:type owl:Class ;
                       rdfs:subClassOf beo:StairFlight ;
                       rdfs:comment "http://bsdd.buildingsmart.org/#concept/details/1zj3DVJij6IBVuIqOLbi46"@en ;
                       rdfs:label "Spiral"@en ,
                                  "scroll"@en ,
                                  "spiral"@nb-no ,
                                  "vindel"@nb-no ;
                       rdfs:seeAlso ifc:IfcStairFlightEnumType .


###  http://pi.pauwel.be/voc/buildingelement#StairFlight-STRAIGHT
beo:StairFlight-STRAIGHT rdf:type owl:Class ;
                         rdfs:subClassOf beo:StairFlight ;
                         rdfs:comment "http://bsdd.buildingsmart.org/#concept/details/247CeErMz16BZyRhwbAOdR"@en ;
                         rdfs:label "Straight"@en ,
                                    "rett"@nb-no ;
                         rdfs:seeAlso ifc:IfcStairFlightEnumType .


###  http://pi.pauwel.be/voc/buildingelement#StairFlight-WINDER
beo:StairFlight-WINDER rdf:type owl:Class ;
                       rdfs:subClassOf beo:StairFlight ;
                       rdfs:comment "http://bsdd.buildingsmart.org/#concept/details/3XVLP1SZf8YQfshhp0Vjph"@en ;
                       rdfs:label "Winder"@en ,
                                  "svingtrapp"@nb-no ;
                       rdfs:seeAlso ifc:IfcStairFlightEnumType .


###  http://pi.pauwel.be/voc/buildingelement#Tendon
beo:Tendon rdf:type owl:Class ;
           rdfs:subClassOf beo:ReinforcingElement ;
           rdfs:comment "a tendon is a steel element such as a wire, cable, bar, rod or strand used to impart prestress to concrete when the element is tensioned."@en ,
                        "http://bsdd.buildingsmart.org/#concept/details/0GEDRkhJ9DdQ2MRE_CaSCF"@en ;
           rdfs:label "Spannglied"@de-de ,
                      "Tendon"@en ,
                      "cable"@fr-fr ;
           rdfs:seeAlso ifc:IfcTendon .


###  http://pi.pauwel.be/voc/buildingelement#Tendon-BAR
beo:Tendon-BAR rdf:type owl:Class ;
               rdfs:subClassOf beo:Tendon ;
               rdfs:comment "http://bsdd.buildingsmart.org/#concept/details/3seMZXSSH4YfQCPjOcaoZG"@en ;
               rdfs:label "Bar"@en ;
               rdfs:seeAlso ifc:IfcTendonEnumType .


###  http://pi.pauwel.be/voc/buildingelement#Tendon-COATED
beo:Tendon-COATED rdf:type owl:Class ;
                  rdfs:subClassOf beo:Tendon ;
                  rdfs:comment "http://bsdd.buildingsmart.org/#concept/details/1WLzEVaRD77A5KPd3$v9DB"@en ;
                  rdfs:label "Coated"@en ;
                  rdfs:seeAlso ifc:IfcTendonEnumType .


###  http://pi.pauwel.be/voc/buildingelement#Tendon-STRAND
beo:Tendon-STRAND rdf:type owl:Class ;
                  rdfs:subClassOf beo:Tendon ;
                  rdfs:comment "http://bsdd.buildingsmart.org/#concept/details/1d4UrJXi92ivdu3FflJ62n"@en ;
                  rdfs:label "Strand"@en ;
                  rdfs:seeAlso ifc:IfcTendonEnumType .


###  http://pi.pauwel.be/voc/buildingelement#Tendon-WIRE
beo:Tendon-WIRE rdf:type owl:Class ;
                rdfs:subClassOf beo:Tendon ;
                rdfs:comment "http://bsdd.buildingsmart.org/#concept/details/1NCnQvMs9AaRqwexu7DofF"@en ;
                rdfs:label "Wire"@en ;
                rdfs:seeAlso ifc:IfcTendonEnumType .


###  http://pi.pauwel.be/voc/buildingelement#TendonAnchor
beo:TendonAnchor rdf:type owl:Class ;
                 rdfs:subClassOf beo:ReinforcingElement ;
                 rdfs:comment "a tendon anchor is the end connection for tendons in prestressed or posttensioned concrete."@en ,
                              "http://bsdd.buildingsmart.org/#concept/details/0Z116ntsH6xBFYGYsNg38f"@en ;
                 rdfs:label "Spanngliedanker"@de-de ,
                            "Tendon Anchor"@en ,
                            "ancrage"@fr-fr ;
                 rdfs:seeAlso ifc:IfcTendonAnchor .


###  http://pi.pauwel.be/voc/buildingelement#TendonAnchor-COUPLER
beo:TendonAnchor-COUPLER rdf:type owl:Class ;
                         rdfs:subClassOf beo:TendonAnchor ;
                         rdfs:comment "http://bsdd.buildingsmart.org/#concept/details/2yrjArQAnBL9EdTqIc7Uv7"@en ;
                         rdfs:label "Coupler"@en ;
                         rdfs:seeAlso ifc:IfcTendonAnchorEnumType .


###  http://pi.pauwel.be/voc/buildingelement#TendonAnchor-FIXED_END
beo:TendonAnchor-FIXED_END rdf:type owl:Class ;
                           rdfs:subClassOf beo:TendonAnchor ;
                           rdfs:comment "http://bsdd.buildingsmart.org/#concept/details/133YYoKAv8mBxccTJtzWju"@en ;
                           rdfs:label "Fixed End"@en ;
                           rdfs:seeAlso ifc:IfcTendonAnchorEnumType .


###  http://pi.pauwel.be/voc/buildingelement#TendonAnchor-TENSIONING_END
beo:TendonAnchor-TENSIONING_END rdf:type owl:Class ;
                                rdfs:subClassOf beo:TendonAnchor ;
                                rdfs:comment "http://bsdd.buildingsmart.org/#concept/details/2Bp8P7qwn1Hg1BaRHyCQP4"@en ;
                                rdfs:label "Tensioning End"@en ;
                                rdfs:seeAlso ifc:IfcTendonAnchorEnumType .


###  http://pi.pauwel.be/voc/buildingelement#TransportElement
beo:TransportElement rdf:type owl:Class ;
                     rdfs:subClassOf <https://schema.org/Product> ;
                     rdfs:comment "A generalization of all transport related objects that move people, animals or goods within a building or building complex. Include elevator (lift), escalator, moving walkway, etc."@en ,
                                  """An element type defined by commonly shared information for occurrences of transport elements. The set of shared information may include:
common properties within shared property sets
common material information
common shape representations
It is used to define a transport element specification (i.e. the specific product information that is common to all occurrences of that beam type). """@en ,
                                  "http://bsdd.buildingsmart.org/#concept/details/3ZSVc0qX4HuO00025QrE$V"@en ;
                     rdfs:label "Beförderungsgerät"@de-de ,
                                "Equipement de transport"@fr-fr ,
                                "Transport Element"@en ,
                                "transportelement"@nb-no ;
                     rdfs:seeAlso ifc:IfcTransportElement .


###  http://pi.pauwel.be/voc/buildingelement#TransportElement-CRANEWAY
beo:TransportElement-CRANEWAY rdf:type owl:Class ;
                              rdfs:subClassOf beo:TransportElement ;
                              rdfs:comment "An artefact for raising, shifting and lowering heavy weights by means of a projecting swinging arm or with hoisting mechanism supported on an overhead track.        "@en ,
                                           "a crane way system, normally including the crane rails, fasteners and the crane. it is primarily used to move heavy goods in a factory or other industry buildings"@en ,
                                           "a crane way system, normally including the crane rails, fasteners and the crane. it is primarily used to move heavy goods in a factory or other industry buildings"@en-gb ,
                                           "http://bsdd.buildingsmart.org/#concept/details/087V4aTMPA09OItHDUip4G"@en ;
                              rdfs:label "Craneway"@en ,
                                         "kran"@nb-no ,
                                         "kranbane"@nb-no ;
                              rdfs:seeAlso ifc:IfcTransportElementEnumType .


###  http://pi.pauwel.be/voc/buildingelement#TransportElement-ELEVATOR
beo:TransportElement-ELEVATOR rdf:type owl:Class ;
                              rdfs:subClassOf beo:TransportElement ;
                              rdfs:comment "a permanent lifting equipment serving defined landing levels, comprising a car, whose dimensions and means of construction clearly permit the access of persons; running at least partially between rigid vertical guides or guides whose inclination to the ve"@en ,
                                           "http://bsdd.buildingsmart.org/#concept/details/2qanav0WDASA8V5to62fCx"@en ,
                                           "http://bsdd.buildingsmart.org/#concept/details/3vHX1_oT0Hsm00051Mm008"@en ,
                                           "permanent løfteutstyr som betjener definerte etasjenivåer, og som består av en stol hvis dimensjoner og konstruksjonsmåte klart gir adgang for personer, og som minst delvis beveger seg mellom stive, vertikale føringsskinner eller føringer hvor hellingen f"@nb-no ;
                              rdfs:label "Aufzug"@de-de ,
                                         "Elevator" ,
                                         "Elevator"@en ,
                                         "ascenseur"@fr-fr ,
                                         "heis"@nb-no ,
                                         "lift"@en ;
                              rdfs:seeAlso ifc:IfcTransportElementEnumType .


###  http://pi.pauwel.be/voc/buildingelement#TransportElement-ESCALATOR
beo:TransportElement-ESCALATOR rdf:type owl:Class ;
                               rdfs:subClassOf beo:TransportElement ;
                               rdfs:comment "http://bsdd.buildingsmart.org/#concept/details/377eo0WJOHu000025QrE$V"@en ,
                                            "http://bsdd.buildingsmart.org/#concept/details/3vHZncoT0Hsm00051Mm008"@en ,
                                            "power-driven, inclined, continuous moving stairway used for raising or lowering persons in which the user carrying surface (e.g. steps) remains horizontal"@en ;
                               rdfs:label "Escalator" ,
                                          "Fahrtreppe"@de-de ,
                                          "Roltrap"@nl-nl ,
                                          "escalier roulant"@fr-fr ,
                                          "rulletrapp"@nb-no ;
                               rdfs:seeAlso ifc:IfcTransportElementEnumType .


###  http://pi.pauwel.be/voc/buildingelement#TransportElement-LIFTINGGEAR
beo:TransportElement-LIFTINGGEAR rdf:type owl:Class ;
                                 rdfs:subClassOf beo:TransportElement ;
                                 rdfs:comment "a device used for lifting or lowering heavy goods. It may be manually operated or electrically or pneumatically driven"@en ,
                                              "a device used for lifting or lowering heavy goods. It may be manually operated or electrically or pneumatically driven"@en-gb ,
                                              "http://bsdd.buildingsmart.org/#concept/details/3qsVNaK3r6Uw2tccQdpTmo"@en ;
                                 rdfs:label "Lifting Gear"@en ,
                                            "løfteinretning"@nb-no ;
                                 rdfs:seeAlso ifc:IfcTransportElementEnumType .


###  http://pi.pauwel.be/voc/buildingelement#TransportElement-MOVINGWALKWAY
beo:TransportElement-MOVINGWALKWAY rdf:type owl:Class ;
                                   rdfs:subClassOf beo:TransportElement ;
                                   rdfs:comment "http://bsdd.buildingsmart.org/#concept/details/0Fn7lcsC5As81fnfma0hsy"@en ;
                                   rdfs:label "Moving Walkway"@en ,
                                              "rullebånd"@nb-no ;
                                   rdfs:seeAlso ifc:IfcTransportElementEnumType .


###  http://pi.pauwel.be/voc/buildingelement#VibrationIsolator
beo:VibrationIsolator rdf:type owl:Class ;
                      rdfs:subClassOf beo:ElementComponent ;
                      rdfs:comment "A device used to minimize the effects of vibration transmissibility in a building."@en ,
                                   "http://bsdd.buildingsmart.org/#concept/details/0Oy60xvFT7TO70hyDzhWWZ"@en ;
                      rdfs:label "Schwingungsisolator"@de-de ,
                                 "Vibration Isolator"@en ,
                                 "isolateur de vibrations"@fr-fr ,
                                 "isolation anti-vibratoire"@fr-fr ,
                                 "trillingsisolator"@nl-nl ,
                                 "vibrasjonsisolator"@nb-no ;
                      rdfs:seeAlso ifc:IfcVibrationIsolator .


###  http://pi.pauwel.be/voc/buildingelement#VibrationIsolator-COMPRESSION
beo:VibrationIsolator-COMPRESSION rdf:type owl:Class ;
                                  rdfs:subClassOf beo:VibrationIsolator ;
                                  rdfs:comment "compression type vibration isolator"@en ,
                                               "compression type vibration isolator"@en-gb ,
                                               "http://bsdd.buildingsmart.org/#concept/details/0EwSGR8PX1z9zHS_KHBRcA"@en ;
                                  rdfs:label "Compression-based vibration isolator" ,
                                             "kompresjon"@nb-no ;
                                  rdfs:seeAlso ifc:IfcVibrationIsolatorEnumType .


###  http://pi.pauwel.be/voc/buildingelement#VibrationIsolator-SPRING
beo:VibrationIsolator-SPRING rdf:type owl:Class ;
                             rdfs:subClassOf beo:VibrationIsolator ;
                             rdfs:comment "http://bsdd.buildingsmart.org/#concept/details/3cKim0GJf3mxz7EqVVfQ8u"@en ,
                                          "spring type vibration isolator"@en ,
                                          "spring type vibration isolator"@en-gb ;
                             rdfs:label "Spring"@en ,
                                        "fjær"@nb-no ;
                             rdfs:seeAlso ifc:IfcVibrationIsolatorEnumType .


###  http://pi.pauwel.be/voc/buildingelement#Wall
beo:Wall rdf:type owl:Class ;
         rdfs:subClassOf beo:BuildingElement ;
         rdfs:comment "A vertical construction that bounds or subdivides spaces. Usually vertical, or nearly vertical, planar elements, often designed to bear structural loads. However not required to be load bearing."@en ,
                      "http://bsdd.buildingsmart.org/#concept/details/2Xuqs0qXKHuO00025QrE$V"@en ;
         rdfs:label "Muur"@nl ,
                    "Væg"@da ,
                    "Wall"@en ,
                    "Wand"@de-de ,
                    "mur"@fr-fr ,
                    "vegg"@nb-no ,
                    "wall"@en ;
         rdfs:seeAlso ifc:IfcWall .


###  http://pi.pauwel.be/voc/buildingelement#Wall-ELEMENTEDWALL
beo:Wall-ELEMENTEDWALL rdf:type owl:Class ;
                       rdfs:subClassOf beo:Wall ;
                       rdfs:comment "a stud wall framed with studs and faced with sheetings, sidings, wallboard, or plasterwork"@en ,
                                    "a stud wall framed with studs and faced with sheetings, sidings, wallboard, or plasterwork"@en-gb ,
                                    "http://bsdd.buildingsmart.org/#concept/details/0sVBQjaqvEcAVsdRJorFkQ"@en ;
                       rdfs:label "Elemented Wall"@en ,
                                  "elementvegg"@nb-no ,
                                  "systemvegg"@nb-no ;
                       rdfs:seeAlso ifc:IfcWallEnumType .


###  http://pi.pauwel.be/voc/buildingelement#Wall-MOVABLE
beo:Wall-MOVABLE rdf:type owl:Class ;
                 rdfs:subClassOf beo:Wall ;
                 rdfs:comment "http://bsdd.buildingsmart.org/#concept/details/2nSQnTH_18RB$MO5daYxD0"@en ;
                 rdfs:label "Flyttbar"@nb-no ,
                            "Movable Wall"@en ;
                 rdfs:seeAlso ifc:IfcWallEnumType .


###  http://pi.pauwel.be/voc/buildingelement#Wall-PARAPET
beo:Wall-PARAPET rdf:type owl:Class ;
                 rdfs:subClassOf beo:Wall ;
                 rdfs:comment """Parapet/brystning
Opphøyet kant som stikker opp over tak"""@nb-no ,
                              "http://bsdd.buildingsmart.org/#concept/details/1uS$40WJmHu000025QrE$V"@en ,
                              "http://bsdd.buildingsmart.org/#concept/details/2BlEUUV2L2BBUdnPO3PtnQ"@en ;
                 rdfs:label "Balustrade"@nl-nl ,
                            "Borstwering"@nl-nl ,
                            "Parapet Wall"@en ,
                            "balustrade"@en ,
                            "parapet"@en ,
                            "parapet"@nb-no ;
                 rdfs:seeAlso ifc:IfcWallEnumType .


###  http://pi.pauwel.be/voc/buildingelement#Wall-PARTITIONING
beo:Wall-PARTITIONING rdf:type owl:Class ;
                      rdfs:subClassOf beo:Wall ;
                      rdfs:comment "http://bsdd.buildingsmart.org/#concept/details/3DBpG2jff4GAXiQp8trskt"@en ;
                      rdfs:label "Partitioning Wall"@en ,
                                 "skillevegg"@nb-no ;
                      rdfs:seeAlso ifc:IfcWallEnumType .


###  http://pi.pauwel.be/voc/buildingelement#Wall-PLUMBINGWALL
beo:Wall-PLUMBINGWALL rdf:type owl:Class ;
                      rdfs:subClassOf beo:Wall ;
                      rdfs:comment "http://bsdd.buildingsmart.org/#concept/details/1YFt0DFB99uxbJnz4oFiew"@en ;
                      rdfs:label "Plumbing Wall"@en ,
                                 "rør i vegg"@nb-no ;
                      rdfs:seeAlso ifc:IfcWallEnumType .


###  http://pi.pauwel.be/voc/buildingelement#Wall-POLYGONAL
beo:Wall-POLYGONAL rdf:type owl:Class ;
                   rdfs:subClassOf beo:Wall ;
                   rdfs:comment "a polygonal wall, extruded vertically, where the wall thickness varies along the wall path"@en ,
                                "a polygonal wall, extruded vertically, where the wall thickness varies along the wall path"@en-gb ,
                                "http://bsdd.buildingsmart.org/#concept/details/0cJEMJHYj6Hh7Q1xNPsiIf"@en ;
                   rdfs:label "Polygonal Wall"@en ,
                              "mangekantet"@nb-no ;
                   rdfs:seeAlso ifc:IfcWallEnumType .


###  http://pi.pauwel.be/voc/buildingelement#Wall-SHEAR
beo:Wall-SHEAR rdf:type owl:Class ;
               rdfs:subClassOf beo:Wall ;
               rdfs:comment "http://bsdd.buildingsmart.org/#concept/details/0MAk1miOTAJQpI0VGyMnjS"@en ;
               rdfs:label "Shear Wall"@en ,
                          "skive"@nb-no ;
               rdfs:seeAlso ifc:IfcWallEnumType .


###  http://pi.pauwel.be/voc/buildingelement#Wall-SOLIDWALL
beo:Wall-SOLIDWALL rdf:type owl:Class ;
                   rdfs:subClassOf beo:Wall ;
                   rdfs:comment "http://bsdd.buildingsmart.org/#concept/details/2J1xt_ADz7heqvTyh5YGEM"@en ;
                   rdfs:label "Solid Wall"@en ,
                              "massiv vegg"@nb-no ;
                   rdfs:seeAlso ifc:IfcWallEnumType .


###  http://pi.pauwel.be/voc/buildingelement#Wall-STANDARD
beo:Wall-STANDARD rdf:type owl:Class ;
                  rdfs:subClassOf beo:Wall ;
                  rdfs:comment "http://bsdd.buildingsmart.org/#concept/details/2HWHt8Yiz4m9UzhlqVFLeO"@en ;
                  rdfs:label "Standard Wall"@en ;
                  rdfs:seeAlso ifc:IfcWallEnumType .


###  http://pi.pauwel.be/voc/buildingelement#WallElementedCase
beo:WallElementedCase rdf:type owl:Class ;
                      rdfs:subClassOf beo:Wall ;
                      rdfs:comment "A wall with certain constraints for the provision of its components."@en ,
                                   "http://bsdd.buildingsmart.org/#concept/details/2dG9W0qXKHuO00025QrE$V"@en ;
                      rdfs:label "Elemented Wall Case"@en ,
                                 "Mur composite"@fr-fr ,
                                 "Wand elementiert"@de-de ;
                      rdfs:seeAlso ifc:IfcWallElementedCase .


###  http://pi.pauwel.be/voc/buildingelement#Window
beo:Window rdf:type owl:Class ;
           rdfs:subClassOf beo:BuildingElement ;
           rdfs:comment "Abertura destinada a iluminar e ventilar os ambientes internos, além de facilitar a visão do exterior."@pt-br ,
                        "Bauteil zum Schließen einer Öffnung in einer Wand oder Satteldach, das Licht durchlassen und Belüftung ermöglichen kann"@de-de ,
                        "building component for closing an opening in a wall or pitched roof that will admit light and may provide ventilation"@en ,
                        "building component for closing an opening in a wall or pitched roof that will admit light and may provide ventilation"@en-gb ,
                        "byggelement som används för att stänga en öppning i en vägg eller ett sadeltak som kan släppa in ljus och bidra med ventilation"@sv-se ,
                        "componente costruttivo atto a chiudere un'apertura in un muro o in un tetto a spiovente che ammetta la luce e possa fornire ventilazione"@it-it ,
                        "componente de construcción para cerrar una abertura en una pared o techo a dos aguas que deja pasar la luz y puede proporcionar ventilación"@es-es ,
                        "construction for closing a vertical or near-vertical opening in a wall or pitched roof which will admit light and may provide ventilation. Often a pane of glass framed and mounted to permit opening and closing"@en ,
                        "construction for closing a vertical or near-vertical opening in a wall or pitched roof which will admit light and may provide ventilation. Often a pane of glass framed and mounted to permit opening and closing"@en-gb ,
                        "ein konstruksjon som står i ei opning som i ein vegg eller tak og som normalt er dekt av glas, med det føremålet å sleppa inn lys og luft. | konstruksjon for *lukking av ein vertikal eller nesten vertikal opning i ein vegg eller eit skråtak som skal sleppa igjennom lys kan gje ventilasjon. Ofte ei glasrute *innrammet og montert for å gjera muleg opning og lukking"@nn-no ,
                        "element budynku służący do zamykania i otwierania, osadzony w ścianie lub w dachu dwuspadowym, przepuszczający światło i mogący zapewniać wentylację"@pl-pl ,
                        "en konstruksjon som står i en åpning som i en vegg eller tak og som normalt er dekket av glass, med det formål å slippe inn lys og luft."@nb-no ,
                        "http://bsdd.buildingsmart.org/#concept/details/3vHUaooT0Hsm00051Mm008"@en ,
                        "konstruksjon for lukking av en vertikal eller nesten vertikal åpning i en vegg eller et skråtak som skal slippe igjennom lys kan gi ventilasjon. Ofte en glassrute innrammet og montert for å muliggjøre åpning og lukking"@nb-no ,
                        "konstruktion til lukning af en lodret eller næsten lodret åbning i en mur eller skråt tag, der lader lys trænge igennem og kan muliggøre ventilation. Ofte en rude i en karm og monteret, så den kan åbnes og lukkes"@dk-dk ,
                        "seinä- tai kattoaukon sulkeva, valoa läpipäästävä rakenneosa varustettuna mahdollisin ilmanvaihto-ominaisuuksin"@fi-fi ,
                        "une construction destinée à fermer une ouverture verticale ou quasi-verticale dans un mur ou un toit en pente qui laissera passer la lumière et pourra fournir une ventilation. souvent constituée d'un panneau vitré monté sur un châssis permettant son ouverture et sa fermeture."@fr-fr ,
                        "строителен компонент за затваряне на отвор в стена или скатен покрив, който служи за осветяване и евентуално за проветряване"@bg-bg ;
           rdfs:label "Fenster"@de-de ,
                      "Raam"@nl ,
                      "Raam"@nl-nl ,
                      "Vindue"@da ,
                      "Window"@en ,
                      "fenêtre"@fr-fr ,
                      "finestra"@it-it ,
                      "fönster"@sv-se ,
                      "ikkuna"@fi-fi ,
                      "janela"@pt-br ,
                      "okna"@pl-pl ,
                      "ventana"@es-es ,
                      "vindauge"@nn-no ,
                      "vindu"@nb-no ,
                      "vindue"@dk-dk ,
                      "window"@en-gb ,
                      "windowset"@en ,
                      "прозорец"@bg-bg ,
                      "نافذة"@ar-sa ,
                      "窓"@ja-jp ;
           rdfs:seeAlso ifc:IfcWindow .


###  http://pi.pauwel.be/voc/buildingelement#Window-LIGHTDOME
beo:Window-LIGHTDOME rdf:type owl:Class ;
                     rdfs:subClassOf beo:Window ;
                     rdfs:comment "a special window that lies horizonally in a roof slab opening"@en ,
                                  "http://bsdd.buildingsmart.org/#concept/details/3aXmro5wX3FeEqYU7Y7w5X"@en ;
                     rdfs:label "Light dome"@en ,
                                "lyskuppel"@nb-no ;
                     rdfs:seeAlso ifc:IfcWindowEnumType .


###  http://pi.pauwel.be/voc/buildingelement#Window-SKYLIGHT
beo:Window-SKYLIGHT rdf:type owl:Class ;
                    rdfs:subClassOf beo:Window ;
                    rdfs:comment "Overlys"@nb-no ,
                                 "construction for closing an opening in a flat roof or low pitched roof, intended primarily for lighting and consisting of a frame and glazing"@en ,
                                 "http://bsdd.buildingsmart.org/#concept/details/1irgDncIrAVQwjja3JEbnb"@en ;
                    rdfs:label "Daklicht"@nl-nl ,
                               "Skylight"@en ,
                               "overlys"@nb-no ;
                    rdfs:seeAlso ifc:IfcWindowEnumType .


###  http://pi.pauwel.be/voc/buildingelement#Window-WINDOW
beo:Window-WINDOW rdf:type owl:Class ;
                  rdfs:subClassOf beo:Window ;
                  rdfs:comment """A building element that is predominately used to provide natural light and fresh air. It includes vertical opening but also horizontal opening such as skylights or light domes. It includes constructions with swinging, pivoting, sliding, or revolving panels and fixed panels. A window consists of a lining and one or several panels.
NOTE  Definition according to ISO 6707-1
Construction for closing a vertical or near vertical opening in a wall or pitched roof that will admit light and may admit fresh air."""@ifc-2x4 ,
                               "Abertura destinada a iluminar e ventilar os ambientes internos, além de facilitar a visão do exterior."@pt-br ,
                               "Bauteil zum Schließen einer Öffnung in einer Wand oder Satteldach, das Licht durchlassen und Belüftung ermöglichen kann"@de-de ,
                               "Een raam is een constructie met een scheidingsfunctie en een lichttoetredingsfunctie."@nl-nl ,
                               "building component for closing an opening in a wall or pitched roof that will admit light and may provide ventilation"@en ,
                               "building component for closing an opening in a wall or pitched roof that will admit light and may provide ventilation"@en-gb ,
                               "byggelement som används för att stänga en öppning i en vägg eller ett sadeltak som kan släppa in ljus och bidra med ventilation"@sv-se ,
                               "componente costruttivo atto a chiudere un'apertura in un muro o in un tetto a spiovente che ammetta la luce e possa fornire ventilazione"@it-it ,
                               "componente de construcción para cerrar una abertura en una pared o techo a dos aguas que deja pasar la luz y puede proporcionar ventilación"@es-es ,
                               "construction for closing a vertical or near-vertical opening in a wall or pitched roof which will admit light and may provide ventilation. Often a pane of glass framed and mounted to permit opening and closing"@en ,
                               "construction for closing a vertical or near-vertical opening in a wall or pitched roof which will admit light and may provide ventilation. Often a pane of glass framed and mounted to permit opening and closing"@en-gb ,
                               "ein konstruksjon som står i ei opning som i ein vegg eller tak og som normalt er dekt av glas, med det føremålet å sleppa inn lys og luft. | konstruksjon for *lukking av ein vertikal eller nesten vertikal opning i ein vegg eller eit skråtak som skal sleppa igjennom lys kan gje ventilasjon. Ofte ei glasrute *innrammet og montert for å gjera muleg opning og lukking"@nn-no ,
                               "element budynku służący do zamykania i otwierania, osadzony w ścianie lub w dachu dwuspadowym, przepuszczający światło i mogący zapewniać wentylację"@pl-pl ,
                               "en konstruksjon som står i en åpning som i en vegg eller tak og som normalt er dekket av glass, med det formål å slippe inn lys og luft."@nb-no ,
                               "http://bsdd.buildingsmart.org/#concept/details/3QkFVA4cD3YvP3Y3zVGFc3"@en ,
                               "konstruksjon for lukking av en vertikal eller nesten vertikal åpning i en vegg eller et skråtak som skal slippe igjennom lys kan gi ventilasjon. Ofte en glassrute innrammet og montert for å muliggjøre åpning og lukking"@nb-no ,
                               "konstruktion til lukning af en lodret eller næsten lodret åbning i en mur eller skråt tag, der lader lys trænge igennem og kan muliggøre ventilation. Ofte en rude i en karm og monteret, så den kan åbnes og lukkes"@dk-dk ,
                               "objekt för tillträde till utrymme för enbart ljus"@sv-se ,
                               "seinä- tai kattoaukon sulkeva, valoa läpipäästävä rakenneosa varustettuna mahdollisin ilmanvaihto-ominaisuuksin"@fi-fi ,
                               "space access object for light entry only"@en ,
                               "une construction destinée à fermer une ouverture verticale ou quasi-verticale dans un mur ou un toit en pente qui laissera passer la lumière et pourra fournir une ventilation. souvent constituée d'un panneau vitré monté sur un châssis permettant son ouverture et sa fermeture."@fr-fr ,
                               "строителен компонент за затваряне на отвор в стена или скатен покрив, който служи за осветяване и евентуално за проветряване"@bg-bg ;
                  rdfs:label "Fenster"@de-de ,
                             "Raam"@nl-nl ,
                             "Window" ,
                             "fenster"@de-ch ,
                             "fenêtre"@fr-fr ,
                             "finestra"@it-it ,
                             "fönster"@sv-se ,
                             "ikkuna"@fi-fi ,
                             "janela"@pt-br ,
                             "okna"@pl-pl ,
                             "ventana"@es-es ,
                             "vindauge"@nn-no ,
                             "vindu"@nb-no ,
                             "vindue"@dk-dk ,
                             "window"@en-gb ,
                             "прозорец"@bg-bg ,
                             "نافذة"@ar-sa ,
                             "窓"@ja-jp ;
                  rdfs:seeAlso ifc:IfcWindowEnumType .


###  http://purl.org/vocommons/voaf#Vocabulary
voaf:Vocabulary rdf:type owl:Class .


###  http://xmlns.com/foaf/0.1/Person
foaf:Person rdf:type owl:Class .


###  https://schema.org/Product
<https://schema.org/Product> rdf:type owl:Class .


#################################################################
#    Individuals
#################################################################

###  http://pi.pauwel.be/voc/buildingelement#
beo: rdf:type owl:NamedIndividual ,
              voaf:Vocabulary .


[ rdf:type foaf:Person ;
  foaf:name "Pieter Pauwels"
] .

[ rdf:type foaf:Person ;
   foaf:name "Pieter Pauwels"
 ] .

###  Generated by the OWL API (version 4.5.7.2018-12-02T02:23:35Z) https://github.com/owlcs/owlapi
