@prefix : <http://pi.pauwel.be/voc/distributionelement#> .
@prefix vs: <http://www.w3.org/2003/06/sw-vocab-status/ns#> .
@prefix dce: <http://purl.org/dc/elements/1.1/> .
@prefix ifc: <http://www.buildingsmart-tech.org/ifcOWL/IFC4_ADD2#> .
@prefix mep: <http://pi.pauwel.be/voc/distributionelement#> .
@prefix owl: <http://www.w3.org/2002/07/owl#> .
@prefix rdf: <http://www.w3.org/1999/02/22-rdf-syntax-ns#> .
@prefix xml: <http://www.w3.org/XML/1998/namespace> .
@prefix xsd: <http://www.w3.org/2001/XMLSchema#> .
@prefix foaf: <http://xmlns.com/foaf/0.1/> .
@prefix rdfs: <http://www.w3.org/2000/01/rdf-schema#> .
@prefix skos: <http://www.w3.org/2004/02/skos/core#> .
@prefix vann: <http://purl.org/vocab/vann/> .
@prefix voaf: <http://purl.org/vocommons/voaf#> .
@prefix dcterms: <http://purl.org/dc/terms/> .
@base <http://pi.pauwel.be/voc/distributionelement#> .

<http://pi.pauwel.be/voc/buildingelement> rdf:type owl:Ontology ;
                                           dce:Language "en" ;
                                           dce:description "The Distribution Element Ontology provides an ontology based on the IfcDistributionElement subtree in the IFC specification, containing a taxonomy of classes that allow to define common distribution elements (actuators, flowterminals, ...)."@en ;
                                           dce:modified "January 28th 2019" ;
                                           dce:title "Distribution Element Ontology" ;
                                           dcterms:creator [ rdf:type foaf:Person ;
                                                             foaf:name "Pieter Pauwels"
                                                           ] ;
                                           dcterms:description "The Distribution Element Ontology provides an ontology based on the IfcDistributionElement subtree in the IFC specification, containing a taxonomy of classes that allow to define common distribution elements (actuators, flowterminals, ...)."@en ;
                                           dcterms:issued "2019-01-28"^^xsd:date ;
                                           dcterms:license <https://creativecommons.org/licenses/by/1.0/> ;
                                           dcterms:title "Distribution Element Ontology"@en ;
                                           vann:preferredNamespacePrefix "mep" ;
                                           vann:preferredNamespaceUri mep: ;
                                           owl:versionInfo "January 28th 2019" ,
                                                           "v0.1.0" .

#################################################################
#    Annotation properties
#################################################################

###  http://purl.org/dc/terms/contributor
dcterms:contributor rdf:type owl:AnnotationProperty .


###  http://purl.org/dc/terms/creator
dcterms:creator rdf:type owl:AnnotationProperty .


###  http://purl.org/dc/terms/description
dcterms:description rdf:type owl:AnnotationProperty .


###  http://purl.org/dc/terms/issued
dcterms:issued rdf:type owl:AnnotationProperty .


###  http://purl.org/dc/terms/license
dcterms:license rdf:type owl:AnnotationProperty .


###  http://purl.org/dc/terms/modified
dcterms:modified rdf:type owl:AnnotationProperty .


###  http://purl.org/dc/terms/title
dcterms:title rdf:type owl:AnnotationProperty .


###  http://purl.org/vocab/vann/preferredNamespacePrefix
vann:preferredNamespacePrefix rdf:type owl:AnnotationProperty .


###  http://purl.org/vocab/vann/preferredNamespaceUri
vann:preferredNamespaceUri rdf:type owl:AnnotationProperty .


###  http://www.w3.org/2003/06/sw-vocab-status/ns#term_status
vs:term_status rdf:type owl:AnnotationProperty .


#################################################################
#    Data properties
#################################################################

###  http://xmlns.com/foaf/0.1/name
foaf:name rdf:type owl:DatatypeProperty .


#################################################################
#    Classes
#################################################################

###  http://purl.org/vocommons/voaf#Vocabulary
voaf:Vocabulary rdf:type owl:Class .


###  http://xmlns.com/foaf/0.1/Person
foaf:Person rdf:type owl:Class .

###  https://schema.org/Product
<https://schema.org/Product> rdf:type owl:Class .


###  http://pi.pauwel.be/voc/distributionelement#Actuator
mep:Actuator rdf:type owl:Class ;
             rdfs:subClassOf mep:DistributionControlElement ;
             rdfs:comment "A mechanical device for moving or controlling a mechanism or system. An actuator takes energy, usually created by air, electricity, or liquid, and converts that into some kind of motion."@en ,
                          "An artefact intended to convert energy (electric, pneumatic, hydraulic) from an external source to kinetic energy in response to a signal..                "@en ,
                          "http://bsdd.buildingsmart.org/#concept/details/14RHCzJ6j6MOcOYy1uRfnX"@en ;
             rdfs:label "Actuator"@en ,
                        "actionneur"@fr-fr ,
                        "aktor"@de-de ,
                        "aktuator"@nb-no ,
                        "antrieb"@de-de ,
                        "appareillage de commande"@fr-fr ,
                        "utløser"@nb-no ;
             rdfs:seeAlso ifc:IfcActuator .


###  http://pi.pauwel.be/voc/distributionelement#Actuator-ELECTRICACTUATOR
mep:Actuator-ELECTRICACTUATOR rdf:type owl:Class ;
                              rdfs:subClassOf mep:Actuator ;
                              rdfs:comment "a device that electrically actuates a control element"@en ,
                                           "http://bsdd.buildingsmart.org/#concept/details/0_R289D0r6oPsUChqMMWr1"@en ;
                              rdfs:label "Electric Actuator"@en ,
                                         "elektrisk aktuator"@nb-no ;
                              rdfs:seeAlso ifc:IfcActuatorEnumType .


###  http://pi.pauwel.be/voc/distributionelement#Actuator-HANDOPERATEDACTUATOR
mep:Actuator-HANDOPERATEDACTUATOR rdf:type owl:Class ;
                                  rdfs:subClassOf mep:Actuator ;
                                  rdfs:comment "http://bsdd.buildingsmart.org/#concept/details/0FuSpPYcbBcAKNNq77IEUN"@en ;
                                  rdfs:label "Hand-Operated Actuator"@en ;
                                  rdfs:seeAlso ifc:IfcActuatorEnumType .


###  http://pi.pauwel.be/voc/distributionelement#Actuator-HYDRAULICACTUATOR
mep:Actuator-HYDRAULICACTUATOR rdf:type owl:Class ;
                               rdfs:subClassOf mep:Actuator ;
                               rdfs:comment "http://bsdd.buildingsmart.org/#concept/details/23inrfSJTEjPmdb42m6RPS"@en ;
                               rdfs:label "Hydraulic Actuator"@en ;
                               rdfs:seeAlso ifc:IfcActuatorEnumType .


###  http://pi.pauwel.be/voc/distributionelement#Actuator-PNEUMATICACTUATOR
mep:Actuator-PNEUMATICACTUATOR rdf:type owl:Class ;
                               rdfs:subClassOf mep:Actuator ;
                               rdfs:comment "http://bsdd.buildingsmart.org/#concept/details/1An85fZE5EZuDCIYomL2WH"@en ;
                               rdfs:label "Pneumatic Actuator"@en ;
                               rdfs:seeAlso ifc:IfcActuatorEnumType .


###  http://pi.pauwel.be/voc/distributionelement#Actuator-THERMOSTATICACTUATOR
mep:Actuator-THERMOSTATICACTUATOR rdf:type owl:Class ;
                                  rdfs:subClassOf mep:Actuator ;
                                  rdfs:comment "http://bsdd.buildingsmart.org/#concept/details/3dkx9QS9HB_emzU3ErhfqY"@en ;
                                  rdfs:label "Thermostatic Actuator"@en ;
                                  rdfs:seeAlso ifc:IfcActuatorEnumType .


###  http://pi.pauwel.be/voc/distributionelement#AirTerminal
mep:AirTerminal rdf:type owl:Class ;
                rdfs:subClassOf mep:FlowTerminal ;
                rdfs:comment "A terminal terminating or origination point for the transfer of air between distribution system(s) and one or more spaces. It can also be used for the transfer of air between adjacent spaces."@en ,
                             "http://bsdd.buildingsmart.org/#concept/details/3ydOg0qRuHuO00025QrE$V"@en ;
                rdfs:label "Air Terminal"@en ,
                           "Luftauslass"@de-de ,
                           "entrée ou sortie d'air"@fr-fr ,
                           "ventilasjonsterminal"@nb-no ;
                rdfs:seeAlso ifc:IfcAirTerminal .


###  http://pi.pauwel.be/voc/distributionelement#AirTerminal-DIFFUSER
mep:AirTerminal-DIFFUSER rdf:type owl:Class ;
                         rdfs:subClassOf mep:AirTerminal ;
                         rdfs:comment "http://bsdd.buildingsmart.org/#concept/details/1FTT5hVkDA$QvjrFJNJEnI"@en ;
                         rdfs:label "Diffuser"@en ,
                                    "luftterminal - diffusor"@nb-no ;
                         rdfs:seeAlso ifc:IfcAirTerminalEnumType .


###  http://pi.pauwel.be/voc/distributionelement#AirTerminal-GRILLE
mep:AirTerminal-GRILLE rdf:type owl:Class ;
                       rdfs:subClassOf mep:AirTerminal ;
                       rdfs:comment "a covering for any area through which air passes."@en ,
                                    "http://bsdd.buildingsmart.org/#concept/details/2hjaxvDcLE49ehxXYke964"@en ;
                       rdfs:label "Grille"@en ,
                                  "gitter"@nb-no ,
                                  "grille"@fr-fr ;
                       rdfs:seeAlso ifc:IfcAirTerminalEnumType .


###  http://pi.pauwel.be/voc/distributionelement#AirTerminal-LOUVRE
mep:AirTerminal-LOUVRE rdf:type owl:Class ;
                       rdfs:subClassOf mep:AirTerminal ;
                       rdfs:comment "a rectilinear louvre."@en ,
                                    "http://bsdd.buildingsmart.org/#concept/details/0cCEo7qnfDSgG93nJsd3eQ"@en ;
                       rdfs:label "Louvre"@en ,
                                  "rist"@nb-no ;
                       rdfs:seeAlso ifc:IfcAirTerminalEnumType .


###  http://pi.pauwel.be/voc/distributionelement#AirTerminal-REGISTER
mep:AirTerminal-REGISTER rdf:type owl:Class ;
                         rdfs:subClassOf mep:AirTerminal ;
                         rdfs:comment "a grille typically equipped with a damper or control valve."@en ,
                                      "http://bsdd.buildingsmart.org/#concept/details/3PWMnCjqP5peD0PtO2aiy5"@en ;
                         rdfs:label "Register"@en ,
                                    "register"@nb-no ;
                         rdfs:seeAlso ifc:IfcAirTerminalEnumType .


###  http://pi.pauwel.be/voc/distributionelement#AirTerminalBox
mep:AirTerminalBox rdf:type owl:Class ;
                   rdfs:subClassOf mep:FlowController ;
                   rdfs:comment "A terminal box in an HVAC duct distribution system and is used to control or modulate the amount of air delivered to its downstream ductwork. Often referred to as an 'air flow regulator'."@en ,
                                "http://bsdd.buildingsmart.org/#concept/details/0zPqWPJST5LRtUuSJBlWpM"@en ;
                   rdfs:label "Air Terminal Box"@en ,
                              "Diffuseur d'air"@fr-fr ,
                              "Volumenstromregler"@de-de ,
                              "plenumskammer"@nb-no ;
                   rdfs:seeAlso ifc:IfcAirTerminalBox .


###  http://pi.pauwel.be/voc/distributionelement#AirTerminalBox-CONSTANTFLOW
mep:AirTerminalBox-CONSTANTFLOW rdf:type owl:Class ;
                                rdfs:subClassOf mep:AirTerminalBox ;
                                rdfs:comment "http://bsdd.buildingsmart.org/#concept/details/0dsGGCiP10ouwdibwvCd4F"@en ;
                                rdfs:label "Constant Flow Air Terminal Box"@en ;
                                rdfs:seeAlso ifc:IfcAirTerminalBoxEnumType .


###  http://pi.pauwel.be/voc/distributionelement#AirTerminalBox-VARIABLEFLOWPRESSUREDEPENDANT
mep:AirTerminalBox-VARIABLEFLOWPRESSUREDEPENDANT rdf:type owl:Class ;
                                                 rdfs:subClassOf mep:AirTerminalBox ;
                                                 rdfs:comment "http://bsdd.buildingsmart.org/#concept/details/2EJZMcPDLDIvG04WI9UZaC"@en ;
                                                 rdfs:label "Variable Flow Pressure Dependent Air Terminal Box"@en ;
                                                 rdfs:seeAlso ifc:IfcAirTerminalBoxEnumType .


###  http://pi.pauwel.be/voc/distributionelement#AirTerminalBox-VARIABLEFLOWPRESSUREINDEPENDANT
mep:AirTerminalBox-VARIABLEFLOWPRESSUREINDEPENDANT rdf:type owl:Class ;
                                                   rdfs:subClassOf mep:AirTerminalBox ;
                                                   rdfs:comment "http://bsdd.buildingsmart.org/#concept/details/2zgc7TxXP2igAw6tyDqxcB"@en ;
                                                   rdfs:label "Variable Flow Pressure Independent Air Terminal Box"@en ;
                                                   rdfs:seeAlso ifc:IfcAirTerminalBoxEnumType .


###  http://pi.pauwel.be/voc/distributionelement#AirToAirHeatRecovery
mep:AirToAirHeatRecovery rdf:type owl:Class ;
                         rdfs:subClassOf mep:EnergyConversionDevice ;
                         rdfs:comment "A counter-flow heat exchanger between inbound and outbound air flow. Typically used to transfer heat from warmer air in one chamber to cooler air in the second chamber (i.e., typically used to recover heat from the conditioned air being exhausted and the outside air being supplied to a building), resulting in energy savings from reduced heating (or cooling) requirements."@en ,
                                      "http://bsdd.buildingsmart.org/#concept/details/2NT_DsArH7_Q5msK_YfU$N"@en ;
                         rdfs:label "Air-to-Air Heat Recovery"@en ,
                                    "Echangeur air-air"@fr-fr ,
                                    "Wärmerückgewinner"@de-de ,
                                    "luft/luft-varmegjenvinningsanlegg"@nb-no ;
                         rdfs:seeAlso ifc:IfcAirToAirHeatRecovery .


###  http://pi.pauwel.be/voc/distributionelement#AirToAirHeatRecovery-FIXEDPLATECOUNTERFLOWEXCHANGER
mep:AirToAirHeatRecovery-FIXEDPLATECOUNTERFLOWEXCHANGER rdf:type owl:Class ;
                                                        rdfs:subClassOf mep:AirToAirHeatRecovery ;
                                                        rdfs:comment "heat exchanger with moving parts and alternate layers of plates, separated and sealed from the exhaust and supply air stream passages with primary air entering at secondary air outlet location and exiting at secondary air inlet location"@en ,
                                                                     "heat exchanger with moving parts and alternate layers of plates, separated and sealed from the exhaust and supply air stream passages with primary air entering at secondary air outlet location and exiting at secondary air inlet location"@en-gb ,
                                                                     "http://bsdd.buildingsmart.org/#concept/details/32kk64JBbDDPM$6p$uBj_5"@en ;
                                                        rdfs:label "Fixed-Plate Counter-Flow Exchanger"@en ,
                                                                   "fast plate motstrømsveksler"@nb-no ;
                                                        rdfs:seeAlso ifc:IfcAirToAirHeatRecoveryEnumType .


###  http://pi.pauwel.be/voc/distributionelement#AirToAirHeatRecovery-FIXEDPLATECROSSFLOWEXCHANGER
mep:AirToAirHeatRecovery-FIXEDPLATECROSSFLOWEXCHANGER rdf:type owl:Class ;
                                                      rdfs:subClassOf mep:AirToAirHeatRecovery ;
                                                      rdfs:comment "http://bsdd.buildingsmart.org/#concept/details/2LTpG80kz5Oh41Z0r9nlld"@en ,
                                                                   "not available"@en ;
                                                      rdfs:label "Fixed-Plate Cross-Flow Exchanger"@en ;
                                                      rdfs:seeAlso ifc:IfcAirToAirHeatRecoveryEnumType .


###  http://pi.pauwel.be/voc/distributionelement#AirToAirHeatRecovery-FIXEDPLATEPARALLELFLOWEXCHANGER
mep:AirToAirHeatRecovery-FIXEDPLATEPARALLELFLOWEXCHANGER rdf:type owl:Class ;
                                                         rdfs:subClassOf mep:AirToAirHeatRecovery ;
                                                         rdfs:comment "http://bsdd.buildingsmart.org/#concept/details/2miQYyrOfDkQ3LRDmm98s2"@en ;
                                                         rdfs:label "Fixed-Plate Parallel-Flow Exchanger"@en ;
                                                         rdfs:seeAlso ifc:IfcAirToAirHeatRecoveryEnumType .


###  http://pi.pauwel.be/voc/distributionelement#AirToAirHeatRecovery-HEATPIPE
mep:AirToAirHeatRecovery-HEATPIPE rdf:type owl:Class ;
                                  rdfs:subClassOf mep:AirToAirHeatRecovery ;
                                  rdfs:comment "a passive energy recovery device with a heat pipe divided into evaporator and condenser sections"@en ,
                                               "a passive energy recovery device with a heat pipe divided into evaporator and condenser sections"@en-gb ,
                                               "http://bsdd.buildingsmart.org/#concept/details/3g4XqNsbDCXxINl9l4yi1C"@en ;
                                  rdfs:label "Heat Pipe"@en ,
                                             "varmerør"@nb-no ;
                                  rdfs:seeAlso ifc:IfcAirToAirHeatRecoveryEnumType .


###  http://pi.pauwel.be/voc/distributionelement#AirToAirHeatRecovery-ROTARYWHEEL
mep:AirToAirHeatRecovery-ROTARYWHEEL rdf:type owl:Class ;
                                     rdfs:subClassOf mep:AirToAirHeatRecovery ;
                                     rdfs:comment "a heat wheel with a revolving cylinder filled with an air-permeable medium having a large internal surface area"@en ,
                                                  "a heat wheel with a revolving cylinder filled with an air-permeable medium having a large internal surface area"@en-gb ,
                                                  "http://bsdd.buildingsmart.org/#concept/details/1jrV4bYDD3JfDdNo49vivZ"@en ;
                                     rdfs:label "Rotary Wheel"@en ,
                                                "dreiehjul"@nb-no ;
                                     rdfs:seeAlso ifc:IfcAirToAirHeatRecoveryEnumType .


###  http://pi.pauwel.be/voc/distributionelement#AirToAirHeatRecovery-RUNAROUNDCOILLOOP
mep:AirToAirHeatRecovery-RUNAROUNDCOILLOOP rdf:type owl:Class ;
                                           rdfs:subClassOf mep:AirToAirHeatRecovery ;
                                           rdfs:comment "http://bsdd.buildingsmart.org/#concept/details/2cqFu4yIn4g8zaq7Ari71H"@en ;
                                           rdfs:label "Run-Around Coil Loop"@en ;
                                           rdfs:seeAlso ifc:IfcAirToAirHeatRecoveryEnumType .


###  http://pi.pauwel.be/voc/distributionelement#AirToAirHeatRecovery-THERMOSIPHONCOILTYPEHEATEXCHANGERS
mep:AirToAirHeatRecovery-THERMOSIPHONCOILTYPEHEATEXCHANGERS rdf:type owl:Class ;
                                                            rdfs:subClassOf mep:AirToAirHeatRecovery ;
                                                            rdfs:comment "http://bsdd.buildingsmart.org/#concept/details/1tRIVmPDzFEwR3BpMALcZq"@en ;
                                                            rdfs:label "Thermosiphon Coil-Type Heat Exchangers"@en ;
                                                            rdfs:seeAlso ifc:IfcAirToAirHeatRecoveryEnumType .


###  http://pi.pauwel.be/voc/distributionelement#AirToAirHeatRecovery-THERMOSIPHONSEALEDTUBEHEATEXCHANGERS
mep:AirToAirHeatRecovery-THERMOSIPHONSEALEDTUBEHEATEXCHANGERS rdf:type owl:Class ;
                                                              rdfs:subClassOf mep:AirToAirHeatRecovery ;
                                                              rdfs:comment "http://bsdd.buildingsmart.org/#concept/details/3sRN7JNafC$OyVXS$9WPxV"@en ;
                                                              rdfs:label "Thermosiphon Sealed-Tube Heat Exchanger"@en ;
                                                              rdfs:seeAlso ifc:IfcAirToAirHeatRecoveryEnumType .


###  http://pi.pauwel.be/voc/distributionelement#AirToAirHeatRecovery-TWINTOWERENTHALPYRECOVERYLOOPS
mep:AirToAirHeatRecovery-TWINTOWERENTHALPYRECOVERYLOOPS rdf:type owl:Class ;
                                                        rdfs:subClassOf mep:AirToAirHeatRecovery ;
                                                        rdfs:comment "http://bsdd.buildingsmart.org/#concept/details/0LF0EN7b17KRgoO5lIZDTY"@en ;
                                                        rdfs:label "Twin Tower Enthalpy Recovery Loop"@en ;
                                                        rdfs:seeAlso ifc:IfcAirToAirHeatRecoveryEnumType .


###  http://pi.pauwel.be/voc/distributionelement#Alarm
mep:Alarm rdf:type owl:Class ;
          rdfs:subClassOf mep:DistributionControlElement ;
          rdfs:comment "device, which may be connected into a transmission path of a fire detection and fire alarm system, to limit the consequences of low parallel resistance faults between the lines of this transmission path"@en ,
                       "http://bsdd.buildingsmart.org/#concept/details/1lb9XO$N58HxZ1Bunuwfkb"@en ;
          rdfs:label "Alarm"@en ,
                     "brannalarm - kortslutningsisolator"@nb-no ;
          rdfs:seeAlso ifc:IfcAlarm .


###  http://pi.pauwel.be/voc/distributionelement#Alarm-BELL
mep:Alarm-BELL rdf:type owl:Class ;
               rdfs:subClassOf mep:Alarm ;
               rdfs:comment "an audible alarm"@en ,
                            "http://bsdd.buildingsmart.org/#concept/details/2iAce1_ub4pRT_gbGydGqi"@en ;
               rdfs:label "Bell"@en ,
                          "bjelle"@nb-no ;
               rdfs:seeAlso ifc:IfcAlarmEnumType .


###  http://pi.pauwel.be/voc/distributionelement#Alarm-BREAKGLASSBUTTON
mep:Alarm-BREAKGLASSBUTTON rdf:type owl:Class ;
                           rdfs:subClassOf mep:Alarm ;
                           rdfs:comment "an alarm activation mechanism in which a protective glass has to be broken to enable a button to be pressed"@en ,
                                        "an alarm activation mechanism in which a protective glass has to be broken to enable a button to be pressed"@en-gb ,
                                        "http://bsdd.buildingsmart.org/#concept/details/1PccK35QXEef9_Kn79zIxl"@en ;
                           rdfs:label "Break Glass Button"@en ,
                                      "brannvarslingsknapp"@nb-no ;
                           rdfs:seeAlso ifc:IfcAlarmEnumType .


###  http://pi.pauwel.be/voc/distributionelement#Alarm-LIGHT
mep:Alarm-LIGHT rdf:type owl:Class ;
                rdfs:subClassOf mep:Alarm ;
                rdfs:comment "a visual alarm"@en ,
                             "http://bsdd.buildingsmart.org/#concept/details/3S8_P1o2L01Ozx8doI6nGk"@en ;
                rdfs:label "Licht"@de-de ,
                           "Light"@en ,
                           "lys"@nb-no ;
                rdfs:seeAlso ifc:IfcAlarmEnumType .


###  http://pi.pauwel.be/voc/distributionelement#Alarm-MANUALPULLBOX
mep:Alarm-MANUALPULLBOX rdf:type owl:Class ;
                        rdfs:subClassOf mep:Alarm ;
                        rdfs:comment "http://bsdd.buildingsmart.org/#concept/details/3zt85EwTXD_QTso9MWvKcg"@en ;
                        rdfs:label "Manual Pullbox"@en ,
                                   "manuell trekkeboks"@nb-no ;
                        rdfs:seeAlso ifc:IfcAlarmEnumType .


###  http://pi.pauwel.be/voc/distributionelement#Alarm-SIREN
mep:Alarm-SIREN rdf:type owl:Class ;
                rdfs:subClassOf mep:Alarm ;
                rdfs:comment "an audible alarm"@en ,
                             "http://bsdd.buildingsmart.org/#concept/details/1UTy6cbg964OXOMBBCXymq"@en ;
                rdfs:label "Siren"@en ,
                           "sirene"@nb-no ;
                rdfs:seeAlso ifc:IfcAlarmEnumType .


###  http://pi.pauwel.be/voc/distributionelement#Alarm-WHISTLE
mep:Alarm-WHISTLE rdf:type owl:Class ;
                  rdfs:subClassOf mep:Alarm ;
                  rdfs:comment "an audible alarm"@en ,
                               "http://bsdd.buildingsmart.org/#concept/details/2AoyxzFcb3MB1ULS_ZzZZX"@en ;
                  rdfs:label "Whistle"@en ,
                             "fløyte"@nb-no ;
                  rdfs:seeAlso ifc:IfcAlarmEnumType .


###  http://pi.pauwel.be/voc/distributionelement#AudioVisualAppliance
mep:AudioVisualAppliance rdf:type owl:Class ;
                         rdfs:subClassOf mep:FlowTerminal ;
                         rdfs:comment """A device that displays, captures, transmits, or receives audio or video.
Audio-visual appliances may be fixed in place or may be able to be moved from one space to another. They may require an electrical supply that may be supplied either by an electrical circuit or provided from a local battery source. Audio-visual appliances may be connected to data circuits including specialist circuits for audio visual purposes only."""@en ,
                                      "http://bsdd.buildingsmart.org/#concept/details/2ZaJrCZM56p8CnFEqtkRj5"@en ;
                         rdfs:label "Audio Visual Appliance"@en ,
                                    "appareil audiovisuel"@fr-fr ,
                                    "audiovisuell enheten"@nb-no ,
                                    "audiovisuelles Gerät"@de-de ;
                         rdfs:seeAlso ifc:IfcAudioVisualAppliance .


###  http://pi.pauwel.be/voc/distributionelement#AudioVisualAppliance-AMPLIFIER
mep:AudioVisualAppliance-AMPLIFIER rdf:type owl:Class ;
                                   rdfs:subClassOf mep:AudioVisualAppliance ;
                                   rdfs:comment "device for boosting audio signal power by means of auxiliary power"@en ,
                                                "device for boosting audio signal power by means of auxiliary power"@en-gb ,
                                                "http://bsdd.buildingsmart.org/#concept/details/3wRrr4McP2IPDX2xDHWMb5"@en ;
                                   rdfs:label "Amplifier"@en ,
                                              "forsterker"@nb-no ;
                                   rdfs:seeAlso ifc:IfcAudioVisualApplianceEnumType .


###  http://pi.pauwel.be/voc/distributionelement#AudioVisualAppliance-CAMERA
mep:AudioVisualAppliance-CAMERA rdf:type owl:Class ;
                                rdfs:subClassOf mep:AudioVisualAppliance ;
                                rdfs:comment "a device that records images, either as a still photograph or as moving images known as videos or movies. Note that a camera may operate with light from the visible spectrum or from other parts of the electromagnetic spectrum such as infrared or ultraviolet."@en ,
                                             "a device that records images, either as a still photograph or as moving images known as videos or movies. Note that a camera may operate with light from the visible spectrum or from other parts of the electromagnetic spectrum such as infrared or ultraviolet."@en-gb ,
                                             "http://bsdd.buildingsmart.org/#concept/details/0Iits$HO92OhljjIcBPane"@en ;
                                rdfs:label "Camera"@en ,
                                           "Camera"@nl-nl ,
                                           "kamera"@nb-no ;
                                rdfs:seeAlso ifc:IfcAudioVisualApplianceEnumType .


###  http://pi.pauwel.be/voc/distributionelement#AudioVisualAppliance-DISPLAY
mep:AudioVisualAppliance-DISPLAY rdf:type owl:Class ;
                                 rdfs:subClassOf mep:AudioVisualAppliance ;
                                 rdfs:comment "an electronic device that represents information in visual form such as a flat-panel display or television."@en ,
                                              "http://bsdd.buildingsmart.org/#concept/details/3zbk7NQJzCte2YLviWyYiT"@en ;
                                 rdfs:label "Display"@en ,
                                            "viser"@nb-no ;
                                 rdfs:seeAlso ifc:IfcAudioVisualApplianceEnumType .


###  http://pi.pauwel.be/voc/distributionelement#AudioVisualAppliance-MICROPHONE
mep:AudioVisualAppliance-MICROPHONE rdf:type owl:Class ;
                                    rdfs:subClassOf mep:AudioVisualAppliance ;
                                    rdfs:comment "an instrument for converting sound waves into electrical energy variations which may then be amplified, transmitted, or recorded"@en ,
                                                 "an instrument for converting sound waves into electrical energy variations which may then be amplified, transmitted, or recorded"@en-gb ,
                                                 "http://bsdd.buildingsmart.org/#concept/details/2L42aAWJmHu000025QrE$V"@en ;
                                    rdfs:label "Microfoon"@nl-nl ,
                                               "Microphone"@en ,
                                               "mikrofon"@nb-no ;
                                    rdfs:seeAlso ifc:IfcAudioVisualApplianceEnumType .


###  http://pi.pauwel.be/voc/distributionelement#AudioVisualAppliance-PLAYER
mep:AudioVisualAppliance-PLAYER rdf:type owl:Class ;
                                rdfs:subClassOf mep:AudioVisualAppliance ;
                                rdfs:comment "a device for playing recorded music"@en ,
                                             "a device for playing recorded music"@en-gb ,
                                             "http://bsdd.buildingsmart.org/#concept/details/3eOLloUdbACBmRDqUZRsWN"@en ;
                                rdfs:label "Player"@en ,
                                           "avspiller"@nb-no ;
                                rdfs:seeAlso ifc:IfcAudioVisualApplianceEnumType .


###  http://pi.pauwel.be/voc/distributionelement#AudioVisualAppliance-PROJECTOR
mep:AudioVisualAppliance-PROJECTOR rdf:type owl:Class ;
                                   rdfs:subClassOf mep:AudioVisualAppliance ;
                                   rdfs:comment "a device that is used to project rays of light, especially an apparatus with a system of lenses for projecting slides or film on to a screen"@en ,
                                                "a device that is used to project rays of light, especially an apparatus with a system of lenses for projecting slides or film on to a screen"@en-gb ,
                                                "http://bsdd.buildingsmart.org/#concept/details/3PFxyF66H6Awpa8qVklE0D"@en ;
                                   rdfs:label "Projector"@en ,
                                              "prosjektor"@nb-no ;
                                   rdfs:seeAlso ifc:IfcAudioVisualApplianceEnumType .


###  http://pi.pauwel.be/voc/distributionelement#AudioVisualAppliance-RECEIVER
mep:AudioVisualAppliance-RECEIVER rdf:type owl:Class ;
                                  rdfs:subClassOf mep:AudioVisualAppliance ;
                                  rdfs:comment "http://bsdd.buildingsmart.org/#concept/details/0f5ylhxBD1hxZPMi642Cwa"@en ,
                                               "the part of a telephone apparatus contained in the earpiece, in which electrical signals are converted into sounds"@en ,
                                               "the part of a telephone apparatus contained in the earpiece, in which electrical signals are converted into sounds"@en-gb ;
                                  rdfs:label "Receiver"@en ,
                                             "mottaker"@nb-no ;
                                  rdfs:seeAlso ifc:IfcAudioVisualApplianceEnumType .


###  http://pi.pauwel.be/voc/distributionelement#AudioVisualAppliance-SPEAKER
mep:AudioVisualAppliance-SPEAKER rdf:type owl:Class ;
                                 rdfs:subClassOf mep:AudioVisualAppliance ;
                                 rdfs:comment "an apparatus that converts electrical impulses into sound, typically as part of a public address system"@en ,
                                              "an apparatus that converts electrical impulses into sound, typically as part of a public address system"@en-gb ,
                                              "http://bsdd.buildingsmart.org/#concept/details/3VXQt2hgT5iRydKNBGNLUm"@en ;
                                 rdfs:label "Speaker"@en ,
                                            "haut-parleur"@fr-fr ,
                                            "høytaler"@nb-no ,
                                            "høyttaler"@nb-no ;
                                 rdfs:seeAlso ifc:IfcAudioVisualApplianceEnumType .


###  http://pi.pauwel.be/voc/distributionelement#AudioVisualAppliance-SWITCHER
mep:AudioVisualAppliance-SWITCHER rdf:type owl:Class ;
                                  rdfs:subClassOf mep:AudioVisualAppliance ;
                                  rdfs:comment "a piece of electronic equipment used to select or combine different video and audio signals"@en ,
                                               "a piece of electronic equipment used to select or combine different video and audio signals"@en-gb ,
                                               "http://bsdd.buildingsmart.org/#concept/details/15RfXB4Cf9VOzccs$seVij"@en ;
                                  rdfs:label "Switcher"@en ,
                                             "bryter"@nb-no ;
                                  rdfs:seeAlso ifc:IfcAudioVisualApplianceEnumType .


###  http://pi.pauwel.be/voc/distributionelement#AudioVisualAppliance-TELEPHONE
mep:AudioVisualAppliance-TELEPHONE rdf:type owl:Class ;
                                   rdfs:subClassOf mep:AudioVisualAppliance ;
                                   rdfs:comment "http://bsdd.buildingsmart.org/#concept/details/3LvBfsxh5A9OLMJxpzp_5P"@en ;
                                   rdfs:label "Telephone"@en ,
                                              "telefon"@nb-no ;
                                   rdfs:seeAlso ifc:IfcAudioVisualApplianceEnumType .


###  http://pi.pauwel.be/voc/distributionelement#AudioVisualAppliance-TUNER
mep:AudioVisualAppliance-TUNER rdf:type owl:Class ;
                               rdfs:subClassOf mep:AudioVisualAppliance ;
                               rdfs:comment "an electronic device for varying the frequency to which a radio or television is tuned"@en ,
                                            "an electronic device for varying the frequency to which a radio or television is tuned"@en-gb ,
                                            "http://bsdd.buildingsmart.org/#concept/details/0sGM9efvTEy8OclWcCNG6k"@en ;
                               rdfs:label "Tuner"@en ,
                                          "tuner"@nb-no ;
                               rdfs:seeAlso ifc:IfcAudioVisualApplianceEnumType .


###  http://pi.pauwel.be/voc/distributionelement#Boiler
mep:Boiler rdf:type owl:Class ;
           rdfs:subClassOf mep:EnergyConversionDevice ;
           rdfs:comment "A closed, pressure-rated vessel in which water or other fluid is heated using an energy source such as natural gas, heating oil, or electricity. "@en ,
                        "http://bsdd.buildingsmart.org/#concept/details/2n42GxcQv3ZeE_LK7_FaP7"@en ;
           rdfs:label "Boiler"@en ,
                      "Boiler"@nl-nl ,
                      "Chaudière"@fr-fr ,
                      "Heizkessel"@de-de ,
                      "Warmwater voorraadtoestel"@nl-nl ,
                      "Warmwatertoestel"@nl-nl ,
                      "kjel"@nb-no ,
                      "water boiler"@en ;
           rdfs:seeAlso ifc:IfcBoiler .


###  http://pi.pauwel.be/voc/distributionelement#Boiler-STEAM
mep:Boiler-STEAM rdf:type owl:Class ;
                 rdfs:subClassOf mep:Boiler ;
                 rdfs:comment "The amount of steam consumed during the period specified in the time series."@ifc-2x4 ,
                              "http://bsdd.buildingsmart.org/#concept/details/3r3yMQaETCj9yTgeFnY6eO"@en ;
                 rdfs:label "Steam Boiler"@en ,
                            "dampkjel"@nb-no ;
                 rdfs:seeAlso ifc:IfcBoilerEnumType .


###  http://pi.pauwel.be/voc/distributionelement#Boiler-WATER
mep:Boiler-WATER rdf:type owl:Class ;
                 rdfs:subClassOf mep:Boiler ;
                 rdfs:comment "http://bsdd.buildingsmart.org/#concept/details/3vHZlaoT0Hsm00051Mm008"@en ;
                 rdfs:label "Water Boiler"@en ;
                 rdfs:seeAlso ifc:IfcBoilerEnumType .


###  http://pi.pauwel.be/voc/distributionelement#Burner
mep:Burner rdf:type owl:Class ;
           rdfs:subClassOf mep:EnergyConversionDevice ;
           rdfs:comment "A device that converts fuel into heat through combustion."@en ,
                        "http://bsdd.buildingsmart.org/#concept/details/3eaWqihr5FfBQB2Eu0SSfd"@en ;
           rdfs:label "Brenner"@de-de ,
                      "Brûleur"@fr-fr ,
                      "Burner"@en ,
                      "brenner"@nb-no ;
           rdfs:seeAlso ifc:IfcBurner .


###  http://pi.pauwel.be/voc/distributionelement#CableCarrierFitting
mep:CableCarrierFitting rdf:type owl:Class ;
                        rdfs:subClassOf mep:FlowFitting ;
                        rdfs:comment "A fitting that is placed at junction or transition in a cable carrier system."@en ,
                                     "http://bsdd.buildingsmart.org/#concept/details/1UxFU0Z7L3wgssm2xurkpg"@en ;
                        rdfs:label "Cable Carrier Fitting"@en ,
                                   "Kabelträger Passstück"@de-de ,
                                   "Raccord de chemin de cable"@fr-fr ,
                                   "kabelføringskobling"@nb-no ;
                        rdfs:seeAlso ifc:IfcCableCarrierFitting .


###  http://pi.pauwel.be/voc/distributionelement#CableCarrierFitting-BEND
mep:CableCarrierFitting-BEND rdf:type owl:Class ;
                             rdfs:subClassOf mep:CableCarrierFitting ;
                             rdfs:comment "a fitting that changes the route of the cable carrier."@en ,
                                          "a fitting that changes the route of the cable carrier."@en-gb ,
                                          "http://bsdd.buildingsmart.org/#concept/details/02T1S3SGrDMBMfyCIF7X4E"@en ;
                             rdfs:label "Bend"@en ,
                                        "bend"@nb-no ;
                             rdfs:seeAlso ifc:IfcCableCarrierFittingEnumType .


###  http://pi.pauwel.be/voc/distributionelement#CableCarrierFitting-CROSS
mep:CableCarrierFitting-CROSS rdf:type owl:Class ;
                              rdfs:subClassOf mep:CableCarrierFitting ;
                              rdfs:comment "a fitting at which two branches are taken from the main route of the cable carrier simultaneously."@en ,
                                           "http://bsdd.buildingsmart.org/#concept/details/0Nz$21cnn4VwLtD25_Kdcr"@en ;
                              rdfs:label "Cross"@en ,
                                         "kryss"@nb-no ;
                              rdfs:seeAlso ifc:IfcCableCarrierFittingEnumType .


###  http://pi.pauwel.be/voc/distributionelement#CableCarrierFitting-REDUCER
mep:CableCarrierFitting-REDUCER rdf:type owl:Class ;
                                rdfs:subClassOf mep:CableCarrierFitting ;
                                rdfs:comment "http://bsdd.buildingsmart.org/#concept/details/3$DOQ8x9jEFehexpevTRMs"@en ;
                                rdfs:label "Reducer"@en ,
                                           "reduksjon"@nb-no ;
                                rdfs:seeAlso ifc:IfcCableCarrierFittingEnumType .


###  http://pi.pauwel.be/voc/distributionelement#CableCarrierFitting-TEE
mep:CableCarrierFitting-TEE rdf:type owl:Class ;
                            rdfs:subClassOf mep:CableCarrierFitting ;
                            rdfs:comment "a fitting at which a branch is taken from the main route of the cable carrier."@en ,
                                         "http://bsdd.buildingsmart.org/#concept/details/2qYrhIwZ1BQgGx_wwRrFAA"@en ;
                            rdfs:label "T-rør"@nb-no ,
                                       "Tee"@en ;
                            rdfs:seeAlso ifc:IfcCableCarrierFittingEnumType .


###  http://pi.pauwel.be/voc/distributionelement#CableCarrierSegment
mep:CableCarrierSegment rdf:type owl:Class ;
                        rdfs:subClassOf mep:FlowSegment ;
                        rdfs:comment "A flow segment that is specifically used to carry and support cabling."@en ,
                                     "http://bsdd.buildingsmart.org/#concept/details/0wEcZCe1zEsO4LVirAd0ZF"@en ;
                        rdfs:label "Cable Carrier Segment"@en ,
                                   "Kabelträgersegment"@de-de ,
                                   "Segment de chemin de cable"@fr-fr ,
                                   "kabelføringssegment"@nb-no ;
                        rdfs:seeAlso ifc:IfcCableCarrierSegment .


###  http://pi.pauwel.be/voc/distributionelement#CableCarrierSegment-CABLELADDERSEGMENT
mep:CableCarrierSegment-CABLELADDERSEGMENT rdf:type owl:Class ;
                                           rdfs:subClassOf mep:CableCarrierSegment ;
                                           rdfs:comment "http://bsdd.buildingsmart.org/#concept/details/0FImfTYGb48ursCbLXsTCr"@en ;
                                           rdfs:label "Cable Ladder Segment"@en ;
                                           rdfs:seeAlso ifc:IfcCableCarrierSegmentEnumType .


###  http://pi.pauwel.be/voc/distributionelement#CableCarrierSegment-CABLETRAYSEGMENT
mep:CableCarrierSegment-CABLETRAYSEGMENT rdf:type owl:Class ;
                                         rdfs:subClassOf mep:CableCarrierSegment ;
                                         rdfs:comment "http://bsdd.buildingsmart.org/#concept/details/3t8hY0ZCvEj8gC2KrGLxGu"@en ;
                                         rdfs:label "Cable Tray Segment"@en ;
                                         rdfs:seeAlso ifc:IfcCableCarrierSegmentEnumType .


###  http://pi.pauwel.be/voc/distributionelement#CableCarrierSegment-CABLETRUNKINGSEGMENT
mep:CableCarrierSegment-CABLETRUNKINGSEGMENT rdf:type owl:Class ;
                                             rdfs:subClassOf mep:CableCarrierSegment ;
                                             rdfs:comment "http://bsdd.buildingsmart.org/#concept/details/0bkSD8Eh1ByuLzjMf5xfTq"@en ;
                                             rdfs:label "Cable Trunk Segment"@en ;
                                             rdfs:seeAlso ifc:IfcCableCarrierSegmentEnumType .


###  http://pi.pauwel.be/voc/distributionelement#CableCarrierSegment-CONDUITSEGMENT
mep:CableCarrierSegment-CONDUITSEGMENT rdf:type owl:Class ;
                                       rdfs:subClassOf mep:CableCarrierSegment ;
                                       rdfs:comment "http://bsdd.buildingsmart.org/#concept/details/3MuSnBn2PFkfAY3gBeVAlk"@en ;
                                       rdfs:label "Conduit Segment"@en ;
                                       rdfs:seeAlso ifc:IfcCableCarrierSegmentEnumType .


###  http://pi.pauwel.be/voc/distributionelement#CableFitting
mep:CableFitting rdf:type owl:Class ;
                 rdfs:subClassOf mep:FlowFitting ;
                 rdfs:comment "A fitting that is placed at a junction, transition or termination in a cable system."@en ,
                              "http://bsdd.buildingsmart.org/#concept/details/27LUFoJu97RuNCAIoglvnW"@en ;
                 rdfs:label "Cable Fitting"@en ,
                            "Kabelverbinder"@de-de ,
                            "Kabelverbinder - Typ"@de-de ;
                 rdfs:seeAlso ifc:IfcCableFitting .


###  http://pi.pauwel.be/voc/distributionelement#CableFitting-CONNECTOR
mep:CableFitting-CONNECTOR rdf:type owl:Class ;
                           rdfs:subClassOf mep:CableFitting ;
                           rdfs:comment "a device for keeping two parts of an electric circuit in contact"@en ,
                                        "a device for keeping two parts of an electric circuit in contact"@en-gb ,
                                        "http://bsdd.buildingsmart.org/#concept/details/1xjOGZ4kX1g8pvaS5Bd5bG"@en ;
                           rdfs:label "Connector"@en ,
                                      "connecteur"@fr-fr ,
                                      "forbindelse"@nb-no ;
                           rdfs:seeAlso ifc:IfcCableFittingEnumType .


###  http://pi.pauwel.be/voc/distributionelement#CableFitting-ENTRY
mep:CableFitting-ENTRY rdf:type owl:Class ;
                       rdfs:subClassOf mep:CableFitting ;
                       rdfs:comment "a fitting that begins a cable segment at a non-electrical element such as a grounding clamp attached to a pipe"@en ,
                                    "http://bsdd.buildingsmart.org/#concept/details/07gAPw_U1EguTzO5UilotA"@en ;
                       rdfs:label "Entry"@en ,
                                  "inngang"@nb-no ;
                       rdfs:seeAlso ifc:IfcCableFittingEnumType .


###  http://pi.pauwel.be/voc/distributionelement#CableFitting-EXIT
mep:CableFitting-EXIT rdf:type owl:Class ;
                      rdfs:subClassOf mep:CableFitting ;
                      rdfs:comment "http://bsdd.buildingsmart.org/#concept/details/1_YaBIQW905QZ9AjtoPTNy"@en ;
                      rdfs:label "Exit"@en ,
                                 "utgang"@nb-no ;
                      rdfs:seeAlso ifc:IfcCableFittingEnumType .


###  http://pi.pauwel.be/voc/distributionelement#CableFitting-JUNCTION
mep:CableFitting-JUNCTION rdf:type owl:Class ;
                          rdfs:subClassOf mep:CableFitting ;
                          rdfs:comment "a fitting that joins three or more segments of arbitrary connector types for signal splitting or multiplexing."@en ,
                                       "a fitting that joins three or more segments of arbitrary connector types for signal splitting or multiplexing."@en-gb ,
                                       "http://bsdd.buildingsmart.org/#concept/details/1RPq5LwjT7VwBv_u4OjJrf"@en ;
                          rdfs:label "Junction"@en ,
                                     "gren"@nb-no ;
                          rdfs:seeAlso ifc:IfcCableFittingEnumType .


###  http://pi.pauwel.be/voc/distributionelement#CableFitting-TRANSITION
mep:CableFitting-TRANSITION rdf:type owl:Class ;
                            rdfs:subClassOf mep:CableFitting ;
                            rdfs:comment "http://bsdd.buildingsmart.org/#concept/details/2H3YKfRzn2u9Nog81SAl8k"@en ;
                            rdfs:label "Transition"@en ,
                                       "overgang"@nb-no ;
                            rdfs:seeAlso ifc:IfcCableFittingEnumType .


###  http://pi.pauwel.be/voc/distributionelement#CableSegment
mep:CableSegment rdf:type owl:Class ;
                 rdfs:subClassOf mep:FlowSegment ;
                 rdfs:comment "A flow segment used to carry electrical power, data, or telecommunications signals."@en ,
                              "http://bsdd.buildingsmart.org/#concept/details/26thIKCK1FhfE8oeEPRbVn"@en ;
                 rdfs:label "Cable Segment"@en ,
                            "Kabelsegment"@de-de ,
                            "Segment de câble"@fr-fr ;
                 rdfs:seeAlso ifc:IfcCableSegment .


###  http://pi.pauwel.be/voc/distributionelement#CableSegment-BUSBARSEGMENT
mep:CableSegment-BUSBARSEGMENT rdf:type owl:Class ;
                               rdfs:subClassOf mep:CableSegment ;
                               rdfs:comment "http://bsdd.buildingsmart.org/#concept/details/0uFCFVhl53Re8TGtNoQbaU"@en ;
                               rdfs:label "Busbar Segment"@en ;
                               rdfs:seeAlso ifc:IfcCableSegmentEnumType .


###  http://pi.pauwel.be/voc/distributionelement#CableSegment-CONDUCTORSEGMENT
mep:CableSegment-CONDUCTORSEGMENT rdf:type owl:Class ;
                                  rdfs:subClassOf mep:CableSegment ;
                                  rdfs:comment "http://bsdd.buildingsmart.org/#concept/details/2dlPSgGMHCnu9mfLG8gZtL"@en ;
                                  rdfs:label "Conductor Segment"@en ;
                                  rdfs:seeAlso ifc:IfcCableSegmentEnumType .


###  http://pi.pauwel.be/voc/distributionelement#CableSegment-CORESEGMENT
mep:CableSegment-CORESEGMENT rdf:type owl:Class ;
                             rdfs:subClassOf mep:CableSegment ;
                             rdfs:comment "http://bsdd.buildingsmart.org/#concept/details/2AYnQG0vTDUwn_LR9znomO"@en ;
                             rdfs:label "Core Segment"@en ;
                             rdfs:seeAlso ifc:IfcCableSegmentEnumType .


###  http://pi.pauwel.be/voc/distributionelement#Chiller
mep:Chiller rdf:type owl:Class ;
            rdfs:subClassOf mep:EnergyConversionDevice ;
            rdfs:comment "A device used to remove heat from a liquid via a vapor-compression or absorption refrigeration cycle to cool a fluid, typically water or a mixture of water and glycol."@en ,
                         "http://bsdd.buildingsmart.org/#concept/details/1Zpzuw4lf8p9CkbZR8gJou"@en ;
            rdfs:label "Chiller"@en ,
                       "Kältemaschine"@de-de ,
                       "Refroidisseur"@fr-fr ,
                       "kjøler"@nb-no ,
                       "kylare"@sv-se ,
                       "refrigeratore"@it-it ;
            rdfs:seeAlso ifc:IfcChiller .


###  http://pi.pauwel.be/voc/distributionelement#Chiller-AIRCOOLED
mep:Chiller-AIRCOOLED rdf:type owl:Class ;
                      rdfs:subClassOf mep:Chiller ;
                      rdfs:comment "air cooled chiller"@en ,
                                   "air cooled chiller"@en-gb ,
                                   "http://bsdd.buildingsmart.org/#concept/details/0Tmp5umYX80uDxxCJQrW$a"@en ;
                      rdfs:label "Air-Cooled Chiller"@en ,
                                 "luftkjølt kjøler"@nb-no ;
                      rdfs:seeAlso ifc:IfcChillerEnumType .


###  http://pi.pauwel.be/voc/distributionelement#Chiller-HEATRECOVERY
mep:Chiller-HEATRECOVERY rdf:type owl:Class ;
                         rdfs:subClassOf mep:Chiller ;
                         rdfs:comment "heat recovery chiller."@en ,
                                      "http://bsdd.buildingsmart.org/#concept/details/30ALQiOHn5LetyiGCdujt6"@en ;
                         rdfs:label "Heat Recovery Chiller"@en ,
                                    "varmegjenvinning"@nb-no ;
                         rdfs:seeAlso ifc:IfcChillerEnumType .


###  http://pi.pauwel.be/voc/distributionelement#Chiller-WATERCOOLED
mep:Chiller-WATERCOOLED rdf:type owl:Class ;
                        rdfs:subClassOf mep:Chiller ;
                        rdfs:comment "http://bsdd.buildingsmart.org/#concept/details/1$b15itWrEVeOmpk8LNP3I"@en ,
                                     "water cooled chiller"@en ,
                                     "water cooled chiller"@en-gb ;
                        rdfs:label "Water-Cooled Chiller"@en ,
                                   "vannkjølt"@nb-no ;
                        rdfs:seeAlso ifc:IfcChillerEnumType .


###  http://pi.pauwel.be/voc/distributionelement#Coil
mep:Coil rdf:type owl:Class ;
         rdfs:subClassOf mep:EnergyConversionDevice ;
         rdfs:comment "A device used to provide heat transfer between non-mixing media."@en ,
                      "http://bsdd.buildingsmart.org/#concept/details/1reT_0qSaHuO00025QrE$V"@en ;
         rdfs:label "Bobine"@fr-fr ,
                    "Coil"@en ,
                    "Flade"@da ,
                    "Heiz-Kühlelemente"@de-de ,
                    "spoletype"@nb-no ;
         rdfs:seeAlso ifc:IfcCoil .


###  http://pi.pauwel.be/voc/distributionelement#Coil-DXCOOLINGCOIL
mep:Coil-DXCOOLINGCOIL rdf:type owl:Class ;
                       rdfs:subClassOf mep:Coil ;
                       rdfs:comment "cooling coil using a refrigerant to cool the air stream directly."@en ,
                                    "http://bsdd.buildingsmart.org/#concept/details/1exlqEQr96eATeS6qcQeE3"@en ;
                       rdfs:label "DXCoolingCoil"@en ,
                                  "dx kjølecoil"@nb-no ;
                       rdfs:seeAlso ifc:IfcCoilEnumType .


###  http://pi.pauwel.be/voc/distributionelement#Coil-ELECTRICHEATINGCOIL
mep:Coil-ELECTRICHEATINGCOIL rdf:type owl:Class ;
                             rdfs:subClassOf mep:Coil ;
                             rdfs:comment "heating coil using electricity as a heating source."@en ,
                                          "http://bsdd.buildingsmart.org/#concept/details/1sKDt$czD8mQchRqMMNYlB"@en ;
                             rdfs:label "Electric Heating Coil"@en ,
                                        "varmecoil"@nb-no ;
                             rdfs:seeAlso ifc:IfcCoilEnumType .


###  http://pi.pauwel.be/voc/distributionelement#Coil-GASHEATINGCOIL
mep:Coil-GASHEATINGCOIL rdf:type owl:Class ;
                        rdfs:subClassOf mep:Coil ;
                        rdfs:comment "heating coil using gas as a heating source."@en ,
                                     "http://bsdd.buildingsmart.org/#concept/details/2Y2dXDycvEJe30WIRF8tsM"@en ;
                        rdfs:label "Gas Heating Coil"@en ,
                                   "gassfyring coil"@nb-no ;
                        rdfs:seeAlso ifc:IfcCoilEnumType .


###  http://pi.pauwel.be/voc/distributionelement#Coil-HYDRONICCOIL
mep:Coil-HYDRONICCOIL rdf:type owl:Class ;
                      rdfs:subClassOf mep:Coil ;
                      rdfs:comment "cooling or Heating coil that uses a hydronic fluid as a cooling or heating source."@en ,
                                   "http://bsdd.buildingsmart.org/#concept/details/0KqvZFKzH5SQiVr$vKoSfk"@en ;
                      rdfs:label "Hydronic Coil"@en ,
                                 "vann/luft spole"@nb-no ;
                      rdfs:seeAlso ifc:IfcCoilEnumType .


###  http://pi.pauwel.be/voc/distributionelement#Coil-STEAMHEATINGCOIL
mep:Coil-STEAMHEATINGCOIL rdf:type owl:Class ;
                          rdfs:subClassOf mep:Coil ;
                          rdfs:comment "heating coil using steam as heating source."@en ,
                                       "http://bsdd.buildingsmart.org/#concept/details/2rXlQ3zHz1IwGGCAc5t50T"@en ;
                          rdfs:label "Steam Heating Coil"@en ;
                          rdfs:seeAlso ifc:IfcCoilEnumType .


###  http://pi.pauwel.be/voc/distributionelement#Coil-WATERCOOLINGCOIL
mep:Coil-WATERCOOLINGCOIL rdf:type owl:Class ;
                          rdfs:subClassOf mep:Coil ;
                          rdfs:comment "cooling coil using chilled water. HYDRONICCOIL supercedes this enumerator."@en ,
                                       "http://bsdd.buildingsmart.org/#concept/details/3AbyMrisP4ehArYy89RfYX"@en ;
                          rdfs:label "Water Cooling Coil"@en ,
                                     "vannkjøler - coil"@nb-no ;
                          rdfs:seeAlso ifc:IfcCoilEnumType .


###  http://pi.pauwel.be/voc/distributionelement#Coil-WATERHEATINGCOIL
mep:Coil-WATERHEATINGCOIL rdf:type owl:Class ;
                          rdfs:subClassOf mep:Coil ;
                          rdfs:comment "heating coil using hot water as a heating source. HYDRONICCOIL supercedes this enumerator."@en ,
                                       "http://bsdd.buildingsmart.org/#concept/details/0ZF$5RRJPDkPP$6rdC$LOy"@en ;
                          rdfs:label "Water Heating Coil"@en ,
                                     "vannvarme - coil"@nb-no ;
                          rdfs:seeAlso ifc:IfcCoilEnumType .


###  http://pi.pauwel.be/voc/distributionelement#CommunicationsAppliance
mep:CommunicationsAppliance rdf:type owl:Class ;
                            rdfs:subClassOf mep:FlowTerminal ;
                            rdfs:comment "A communications device transmits and receives electronic or digital information as data or sound."@en ,
                                         "http://bsdd.buildingsmart.org/#concept/details/3dS_KvJn16dgqG0Y8M0_8M"@en ;
                            rdfs:label "Appareil de communications"@fr-fr ,
                                       "Communications Appliance"@en ,
                                       "Kommunikationsgerät"@de-de ,
                                       "kommunikasjonsapparat"@nb-no ;
                            rdfs:seeAlso ifc:IfcCommunicationsAppliance .


###  http://pi.pauwel.be/voc/distributionelement#CommunicationsAppliance-ANTENNA
mep:CommunicationsAppliance-ANTENNA rdf:type owl:Class ;
                                    rdfs:subClassOf mep:CommunicationsAppliance ;
                                    rdfs:comment "a transducer designed to transmit or receive electromagnetic waves."@en ,
                                                 "http://bsdd.buildingsmart.org/#concept/details/0C2VVYeDP29xB3DZDSeUl0"@en ;
                                    rdfs:label "Antenna"@en ,
                                               "antenne"@nb-no ;
                                    rdfs:seeAlso ifc:IfcCommunicationsApplianceEnumType .


###  http://pi.pauwel.be/voc/distributionelement#CommunicationsAppliance-COMPUTER
mep:CommunicationsAppliance-COMPUTER rdf:type owl:Class ;
                                     rdfs:subClassOf mep:CommunicationsAppliance ;
                                     rdfs:comment "an electronic device which is capable of receiving information (data) in a particular form and of performing a sequence of operations in accordance with a predetermined but variable set of procedural instructions (program) to produce a result in the form of information or signals"@en ,
                                                  "an electronic device which is capable of receiving information (data) in a particular form and of performing a sequence of operations in accordance with a predetermined but variable set of procedural instructions (program) to produce a result in the form of information or signals"@en-gb ,
                                                  "http://bsdd.buildingsmart.org/#concept/details/3YJ0SHSxL2Se6$_7rNWY_P"@en ;
                                     rdfs:label "Computer"@en ,
                                                "computer"@nb-no ,
                                                "datagolv"@nb-no ,
                                                "datagulv"@nb-no ,
                                                "datamaskin"@nb-no ,
                                                "gulvsystem datagulv"@nb-no ;
                                     rdfs:seeAlso ifc:IfcCommunicationsApplianceEnumType .


###  http://pi.pauwel.be/voc/distributionelement#CommunicationsAppliance-FAX
mep:CommunicationsAppliance-FAX rdf:type owl:Class ;
                                rdfs:subClassOf mep:CommunicationsAppliance ;
                                rdfs:comment "a machine for transmitting and receiving faxes"@en ,
                                             "a machine for transmitting and receiving faxes"@en-gb ,
                                             "http://bsdd.buildingsmart.org/#concept/details/0rZr4shW90zOb$tqxFAwq_"@en ;
                                rdfs:label "Fax"@en ,
                                           "fax"@nb-no ;
                                rdfs:seeAlso ifc:IfcCommunicationsApplianceEnumType .


###  http://pi.pauwel.be/voc/distributionelement#CommunicationsAppliance-GATEWAY
mep:CommunicationsAppliance-GATEWAY rdf:type owl:Class ;
                                    rdfs:subClassOf mep:CommunicationsAppliance ;
                                    rdfs:comment "a gateway connects multiple network segments with different protocols at all layers (layers 1-7) of the Open Systems Interconnection (OSI) model."@en ,
                                                 "http://bsdd.buildingsmart.org/#concept/details/32NV4lWbbC8fXXlHfMs1EJ"@en ;
                                    rdfs:label "Gateway"@en ,
                                               "gateway"@nb-no ,
                                               "nettgrense - gateway"@nb-no ;
                                    rdfs:seeAlso ifc:IfcCommunicationsApplianceEnumType .


###  http://pi.pauwel.be/voc/distributionelement#CommunicationsAppliance-MODEM
mep:CommunicationsAppliance-MODEM rdf:type owl:Class ;
                                  rdfs:subClassOf mep:CommunicationsAppliance ;
                                  rdfs:comment "a combined device for modulation and demodulation, for example, between the digital data of a computer and the analogue signal of a telephone line"@en ,
                                               "a combined device for modulation and demodulation, for example, between the digital data of a computer and the analogue signal of a telephone line"@en-gb ,
                                               "http://bsdd.buildingsmart.org/#concept/details/0KFUxRBVf7AAcbfoB6t3UZ"@en ;
                                  rdfs:label "Modem"@en ,
                                             "modem"@nb-no ;
                                  rdfs:seeAlso ifc:IfcCommunicationsApplianceEnumType .


###  http://pi.pauwel.be/voc/distributionelement#CommunicationsAppliance-NETWORKAPPLIANCE
mep:CommunicationsAppliance-NETWORKAPPLIANCE rdf:type owl:Class ;
                                             rdfs:subClassOf mep:CommunicationsAppliance ;
                                             rdfs:comment "http://bsdd.buildingsmart.org/#concept/details/2WnZ6tZHfC7gNz8mylrfCG"@en ;
                                             rdfs:label "Network Appliance"@en ;
                                             rdfs:seeAlso ifc:IfcCommunicationsApplianceEnumType .


###  http://pi.pauwel.be/voc/distributionelement#CommunicationsAppliance-NETWORKBRIDGE
mep:CommunicationsAppliance-NETWORKBRIDGE rdf:type owl:Class ;
                                          rdfs:subClassOf mep:CommunicationsAppliance ;
                                          rdfs:comment "http://bsdd.buildingsmart.org/#concept/details/2BwyUI_XTBHhVWLVNXjmP1"@en ;
                                          rdfs:label "Network Bridge"@en ;
                                          rdfs:seeAlso ifc:IfcCommunicationsApplianceEnumType .


###  http://pi.pauwel.be/voc/distributionelement#CommunicationsAppliance-NETWORKHUB
mep:CommunicationsAppliance-NETWORKHUB rdf:type owl:Class ;
                                       rdfs:subClassOf mep:CommunicationsAppliance ;
                                       rdfs:comment "http://bsdd.buildingsmart.org/#concept/details/2isi2CWT5C8hpM6didtFuS"@en ;
                                       rdfs:label "Network Hub"@en ;
                                       rdfs:seeAlso ifc:IfcCommunicationsApplianceEnumType .


###  http://pi.pauwel.be/voc/distributionelement#CommunicationsAppliance-PRINTER
mep:CommunicationsAppliance-PRINTER rdf:type owl:Class ;
                                    rdfs:subClassOf mep:CommunicationsAppliance ;
                                    rdfs:comment "a machine for printing text or pictures, especially one linked to a computer"@en ,
                                                 "a machine for printing text or pictures, especially one linked to a computer"@en-gb ,
                                                 "http://bsdd.buildingsmart.org/#concept/details/2gEEth5ArE5hgXWDZ2HEeu"@en ;
                                    rdfs:label "Printer"@en ,
                                               "printer"@nb-no ;
                                    rdfs:seeAlso ifc:IfcCommunicationsApplianceEnumType .


###  http://pi.pauwel.be/voc/distributionelement#CommunicationsAppliance-REPEATER
mep:CommunicationsAppliance-REPEATER rdf:type owl:Class ;
                                     rdfs:subClassOf mep:CommunicationsAppliance ;
                                     rdfs:comment "a device for the automatic retransmission or amplification of an electrically transmitted message"@en ,
                                                  "a device for the automatic retransmission or amplification of an electrically transmitted message"@en-gb ,
                                                  "http://bsdd.buildingsmart.org/#concept/details/0kMGElI9XD5x0JqYWcVH5G"@en ;
                                     rdfs:label "Repeater"@en ,
                                                "repeater"@nb-no ;
                                     rdfs:seeAlso ifc:IfcCommunicationsApplianceEnumType .


###  http://pi.pauwel.be/voc/distributionelement#CommunicationsAppliance-ROUTER
mep:CommunicationsAppliance-ROUTER rdf:type owl:Class ;
                                   rdfs:subClassOf mep:CommunicationsAppliance ;
                                   rdfs:comment "A router is a networking device whose software and hardware are usually tailored to the tasks of routing and forwarding information. For example, on the Internet, information is directed to various paths by routers."@en ,
                                                "A router is a networking device whose software and hardware are usually tailored to the tasks of routing and forwarding information. For example, on the Internet, information is directed to various paths by routers."@en-gb ,
                                                "http://bsdd.buildingsmart.org/#concept/details/3iPUFOOkn9CR_oYn1_vIJe"@en ;
                                   rdfs:label "Router"@en ,
                                              "nettverksruter"@nb-no ;
                                   rdfs:seeAlso ifc:IfcCommunicationsApplianceEnumType .


###  http://pi.pauwel.be/voc/distributionelement#CommunicationsAppliance-SCANNER
mep:CommunicationsAppliance-SCANNER rdf:type owl:Class ;
                                    rdfs:subClassOf mep:CommunicationsAppliance ;
                                    rdfs:comment "a device that scans documents and converts them into digital data"@en ,
                                                 "a device that scans documents and converts them into digital data"@en-gb ,
                                                 "http://bsdd.buildingsmart.org/#concept/details/3Zb4cC11TBmAB3gBWRepr4"@en ;
                                    rdfs:label "Scanner"@en ,
                                               "scanner"@nb-no ;
                                    rdfs:seeAlso ifc:IfcCommunicationsApplianceEnumType .


###  http://pi.pauwel.be/voc/distributionelement#Compressor
mep:Compressor rdf:type owl:Class ;
               rdfs:subClassOf mep:FlowMovingDevice ;
               rdfs:comment "A device that compresses a fluid typically used in a refrigeration circuit."@en ,
                            "http://bsdd.buildingsmart.org/#concept/details/1Qp4AN19X6Huz0qWsWQk2Q"@en ;
               rdfs:label "Compresseur"@fr-fr ,
                          "Compressor"@en ,
                          "Kompressor"@de-de ;
               rdfs:seeAlso ifc:IfcCompressor .


###  http://pi.pauwel.be/voc/distributionelement#Compressor-BOOSTER
mep:Compressor-BOOSTER rdf:type owl:Class ;
                       rdfs:subClassOf mep:Compressor ;
                       rdfs:comment "http://bsdd.buildingsmart.org/#concept/details/0KvKrF8Vv38QKJC3iDOsZR"@en ,
                                    "positive-displacement reciprocating compressor where pressure is increased by a booster."@en ;
                       rdfs:label "Booster" ,
                                  "forsterker"@nb-no ;
                       rdfs:seeAlso ifc:IfcCompressorEnumType .


###  http://pi.pauwel.be/voc/distributionelement#Compressor-DYNAMIC
mep:Compressor-DYNAMIC rdf:type owl:Class ;
                       rdfs:subClassOf mep:Compressor ;
                       rdfs:comment "http://bsdd.buildingsmart.org/#concept/details/0bjNJRb7f3bOrNnlEVDx$V"@en ,
                                    "the pressure of refrigerant vapor is increased by a continuous transfer of angular momentum from a rotating member to the vapor followed by conversion of this momentum into static pressure."@en ;
                       rdfs:label "Dynamic Compressor"@en ,
                                  "dynamisk"@nb-no ;
                       rdfs:seeAlso ifc:IfcCompressorEnumType .


###  http://pi.pauwel.be/voc/distributionelement#Compressor-HERMETIC
mep:Compressor-HERMETIC rdf:type owl:Class ;
                        rdfs:subClassOf mep:Compressor ;
                        rdfs:comment "http://bsdd.buildingsmart.org/#concept/details/1QxsNyRLjDEfER9sd9a4nA"@en ,
                                     "positive-displacement reciprocating compressor where the motor and compressor are contained within the same housing, with the motor shaft integral with the compressor crankshaft and the motor in contact with refrigerant."@en ;
                        rdfs:label "Hermetic Compressor"@en ,
                                   "lukket"@nb-no ;
                        rdfs:seeAlso ifc:IfcCompressorEnumType .


###  http://pi.pauwel.be/voc/distributionelement#Compressor-OPENTYPE
mep:Compressor-OPENTYPE rdf:type owl:Class ;
                        rdfs:subClassOf mep:Compressor ;
                        rdfs:comment "http://bsdd.buildingsmart.org/#concept/details/35$2VQ6Vf3yAbaBgoiZ_Qy"@en ,
                                     "positive-displacement reciprocating compressor where the shaft extends through a seal in the crankcase for an external drive."@en ;
                        rdfs:label "Open Type Compressor"@en ,
                                   "kompressor - åpen"@nb-no ;
                        rdfs:seeAlso ifc:IfcCompressorEnumType .


###  http://pi.pauwel.be/voc/distributionelement#Compressor-RECIPROCATING
mep:Compressor-RECIPROCATING rdf:type owl:Class ;
                             rdfs:subClassOf mep:Compressor ;
                             rdfs:comment "http://bsdd.buildingsmart.org/#concept/details/1rD1BDTTnA4Opl9hEUzc3J"@en ,
                                          "positive-displacement compressor using a piston driven by a connecting rod from a crankshaft."@en ;
                             rdfs:label "Reciprocating Compressor"@en ,
                                        "stempel"@nb-no ;
                             rdfs:seeAlso ifc:IfcCompressorEnumType .


###  http://pi.pauwel.be/voc/distributionelement#Compressor-ROLLINGPISTON
mep:Compressor-ROLLINGPISTON rdf:type owl:Class ;
                             rdfs:subClassOf mep:Compressor ;
                             rdfs:comment "http://bsdd.buildingsmart.org/#concept/details/25ip$MycH3CApiL8P1Zfua"@en ,
                                          "positive-displacement rotary compressor using a roller mounted on the eccentric of a shaft with a single vane in the nonrotating cylindrical housing."@en ;
                             rdfs:label "Rolling Piston Compressor"@en ,
                                        "rullestempel"@nb-no ;
                             rdfs:seeAlso ifc:IfcCompressorEnumType .


###  http://pi.pauwel.be/voc/distributionelement#Compressor-ROTARY
mep:Compressor-ROTARY rdf:type owl:Class ;
                      rdfs:subClassOf mep:Compressor ;
                      rdfs:comment "http://bsdd.buildingsmart.org/#concept/details/34DscBiG12O81W_KaUsgZs"@en ,
                                   "positive-displacement compressor using a roller or rotor device."@en ;
                      rdfs:label "Rotary Compressor"@en ,
                                 "kompressor - roterende"@nb-no ;
                      rdfs:seeAlso ifc:IfcCompressorEnumType .


###  http://pi.pauwel.be/voc/distributionelement#Compressor-ROTARYVANE
mep:Compressor-ROTARYVANE rdf:type owl:Class ;
                          rdfs:subClassOf mep:Compressor ;
                          rdfs:comment "http://bsdd.buildingsmart.org/#concept/details/3Fnn56$If0Ywd7AMXubW5r"@en ,
                                       "positive-displacement rotary compressor using a roller mounted on the eccentric of a shaft with multiple vanes in the nontotating cylindrical housing."@en ;
                          rdfs:label "Rotary Vane Compressor"@en ,
                                     "kompressor - roterende vinge"@nb-no ;
                          rdfs:seeAlso ifc:IfcCompressorEnumType .


###  http://pi.pauwel.be/voc/distributionelement#Compressor-SCROLL
mep:Compressor-SCROLL rdf:type owl:Class ;
                      rdfs:subClassOf mep:Compressor ;
                      rdfs:comment "http://bsdd.buildingsmart.org/#concept/details/1e5CFyUGv9suZ9ky8c_4Ir"@en ,
                                   "positive-displacement compressor using two inter-fitting, spiral-shaped scroll members."@en ;
                      rdfs:label "Scroll Compressor"@en ,
                                 "spiral"@nb-no ;
                      rdfs:seeAlso ifc:IfcCompressorEnumType .


###  http://pi.pauwel.be/voc/distributionelement#Compressor-SEMIHERMETIC
mep:Compressor-SEMIHERMETIC rdf:type owl:Class ;
                            rdfs:subClassOf mep:Compressor ;
                            rdfs:comment "http://bsdd.buildingsmart.org/#concept/details/0rQK7zwf97_vwAvPlWuuME"@en ,
                                         "positive-displacement reciprocating compressor where the hermetic compressors use bolted construction amenable to field repair."@en ;
                            rdfs:label "Semi Hermetic Compressor"@en ,
                                       "semilukket"@nb-no ;
                            rdfs:seeAlso ifc:IfcCompressorEnumType .


###  http://pi.pauwel.be/voc/distributionelement#Compressor-SINGLESCREW
mep:Compressor-SINGLESCREW rdf:type owl:Class ;
                           rdfs:subClassOf mep:Compressor ;
                           rdfs:comment "http://bsdd.buildingsmart.org/#concept/details/2U43NgKlnBqPnnBLsl6wU4"@en ,
                                        "positive-displacement rotary compressor using a single cylindrical main rotor that works with a pair of gate rotors."@en ;
                           rdfs:label "Single Screw Compressor"@en ,
                                      "enkeltskrue"@nb-no ;
                           rdfs:seeAlso ifc:IfcCompressorEnumType .


###  http://pi.pauwel.be/voc/distributionelement#Compressor-SINGLESTAGE
mep:Compressor-SINGLESTAGE rdf:type owl:Class ;
                           rdfs:subClassOf mep:Compressor ;
                           rdfs:comment "http://bsdd.buildingsmart.org/#concept/details/1sA1FIWkz8SRjvM$gcNai0"@en ,
                                        "positive-displacement reciprocating compressor where vapor is compressed in a single stage."@en ;
                           rdfs:label "Single Stage Compressor"@en ,
                                      "ettrinns"@nb-no ;
                           rdfs:seeAlso ifc:IfcCompressorEnumType .


###  http://pi.pauwel.be/voc/distributionelement#Compressor-TROCHOIDAL
mep:Compressor-TROCHOIDAL rdf:type owl:Class ;
                          rdfs:subClassOf mep:Compressor ;
                          rdfs:comment "http://bsdd.buildingsmart.org/#concept/details/1L2jXYOSr0k980kt8JnyQv"@en ,
                                       "positive-displacement compressor using a rolling motion of one circle outside or inside the circumference of a basic circle and produce either epitrochoids or hypotrochoids."@en ;
                          rdfs:label "Trochoidal Compressor"@en ,
                                     "trokoid"@nb-no ;
                          rdfs:seeAlso ifc:IfcCompressorEnumType .


###  http://pi.pauwel.be/voc/distributionelement#Compressor-TWINSCREW
mep:Compressor-TWINSCREW rdf:type owl:Class ;
                         rdfs:subClassOf mep:Compressor ;
                         rdfs:comment "http://bsdd.buildingsmart.org/#concept/details/3hihvfHSj9h8cGQM0xtKAu"@en ,
                                      "positive-displacement rotary compressor using two mating helically grooved rotors, male (lobes) and female (flutes) in a stationary housing with inlet and outlet gas ports."@en ;
                         rdfs:label "Twin Screw Compressor"@en ,
                                    "dobbelkompressor"@nb-no ;
                         rdfs:seeAlso ifc:IfcCompressorEnumType .


###  http://pi.pauwel.be/voc/distributionelement#Compressor-WELDEDSHELLHERMETIC
mep:Compressor-WELDEDSHELLHERMETIC rdf:type owl:Class ;
                                   rdfs:subClassOf mep:Compressor ;
                                   rdfs:comment "http://bsdd.buildingsmart.org/#concept/details/3YKCxQG3X2xhA2b8$YRmuH"@en ;
                                   rdfs:label "Welded Shell Hermetic Compressor"@en ;
                                   rdfs:seeAlso ifc:IfcCompressorEnumType .


###  http://pi.pauwel.be/voc/distributionelement#Condenser
mep:Condenser rdf:type owl:Class ;
              rdfs:subClassOf mep:EnergyConversionDevice ;
              rdfs:comment "A device that is used to dissipate heat, typically by condensing a substance such as a refrigerant from its gaseous to its liquid state."@en ,
                           "heat exchanger that condenses refrigerant vapour by rejecting heat"@en ,
                           "http://bsdd.buildingsmart.org/#concept/details/2DpcsXxln2WvYyPFOAkV$n"@en ;
              rdfs:label "Condenser"@en ,
                         "Condenseur"@fr-fr ,
                         "Kondensator"@de-de ,
                         "condensatore"@it-it ,
                         "kondensator"@nb-no ;
              rdfs:seeAlso ifc:IfcCondenser .


###  http://pi.pauwel.be/voc/distributionelement#Condenser-AIRCOOLED
mep:Condenser-AIRCOOLED rdf:type owl:Class ;
                        rdfs:subClassOf mep:Condenser ;
                        rdfs:comment "a condenser in which heat is transferred to an air-stream"@en ,
                                     "a condenser in which heat is transferred to an air-stream"@en-gb ,
                                     "http://bsdd.buildingsmart.org/#concept/details/3I1OxJC71BJOJi3xkrXKKM"@en ;
                        rdfs:label "Air Cooled"@en ,
                                   "kondensator luftkjølt"@nb-no ;
                        rdfs:seeAlso ifc:IfcCondenserEnumType .


###  http://pi.pauwel.be/voc/distributionelement#Condenser-EVAPORATIVECOOLED
mep:Condenser-EVAPORATIVECOOLED rdf:type owl:Class ;
                                rdfs:subClassOf mep:Condenser ;
                                rdfs:comment "a condenser that is cooled evaporatively."@en ,
                                             "http://bsdd.buildingsmart.org/#concept/details/1FUPWLndXE$hUQLc0y3Wj6"@en ;
                                rdfs:label "Evaporative Cooled"@en ,
                                           "fordampningkjølt"@nb-no ;
                                rdfs:seeAlso ifc:IfcCondenserEnumType .


###  http://pi.pauwel.be/voc/distributionelement#Condenser-WATERCOOLED
mep:Condenser-WATERCOOLED rdf:type owl:Class ;
                          rdfs:subClassOf mep:Condenser ;
                          rdfs:comment "http://bsdd.buildingsmart.org/#concept/details/1$_Cv8DcnEIhdevMYpgzOs"@en ,
                                       "water-cooled condenser with unspecified operation"@en ,
                                       "water-cooled condenser with unspecified operation"@en-gb ;
                          rdfs:label "Water Cooled"@en ;
                          rdfs:seeAlso ifc:IfcCondenserEnumType .


###  http://pi.pauwel.be/voc/distributionelement#Condenser-WATERCOOLEDBRAZEDPLATE
mep:Condenser-WATERCOOLEDBRAZEDPLATE rdf:type owl:Class ;
                                     rdfs:subClassOf mep:Condenser ;
                                     rdfs:comment "http://bsdd.buildingsmart.org/#concept/details/3DsQKabLb8PuG7s1BwpA5x"@en ,
                                                  "water-cooled condenser condenser with plates brazed together to form an assembly of separate channels."@en ;
                                     rdfs:label "Water Cooled Brazed Plate"@en ;
                                     rdfs:seeAlso ifc:IfcCondenserEnumType .


###  http://pi.pauwel.be/voc/distributionelement#Condenser-WATERCOOLEDSHELLCOIL
mep:Condenser-WATERCOOLEDSHELLCOIL rdf:type owl:Class ;
                                   rdfs:subClassOf mep:Condenser ;
                                   rdfs:comment "http://bsdd.buildingsmart.org/#concept/details/2y2FRrDI58wPQ$P0QmPB4S"@en ,
                                                "water-cooled condenser with cooling water circulated through one or more continuous or assembled coils contained within the shell."@en ;
                                   rdfs:label "Water Cooled Shell Coil"@en ;
                                   rdfs:seeAlso ifc:IfcCondenserEnumType .


###  http://pi.pauwel.be/voc/distributionelement#Condenser-WATERCOOLEDSHELLTUBE
mep:Condenser-WATERCOOLEDSHELLTUBE rdf:type owl:Class ;
                                   rdfs:subClassOf mep:Condenser ;
                                   rdfs:comment "http://bsdd.buildingsmart.org/#concept/details/1v95Mqhl19xxpoA6ogzO73"@en ;
                                   rdfs:label "Water Cooled Shell Tube"@en ;
                                   rdfs:seeAlso ifc:IfcCondenserEnumType .


###  http://pi.pauwel.be/voc/distributionelement#Condenser-WATERCOOLEDTUBEINTUBE
mep:Condenser-WATERCOOLEDTUBEINTUBE rdf:type owl:Class ;
                                    rdfs:subClassOf mep:Condenser ;
                                    rdfs:comment "http://bsdd.buildingsmart.org/#concept/details/2qm75n0SHCbPRb1y1l8QGa"@en ,
                                                 "water-cooled condenser consisting of one or more assemblies of two tubes, one within the other."@en ;
                                    rdfs:label "Water Cooled Tube In Tube"@en ,
                                               "vannkjøler - rør i rør"@nb-no ;
                                    rdfs:seeAlso ifc:IfcCondenserEnumType .


###  http://pi.pauwel.be/voc/distributionelement#Controller
mep:Controller rdf:type owl:Class ;
               rdfs:subClassOf mep:DistributionControlElement ;
               rdfs:comment "A device that monitors inputs and controls outputs within a building automation system."@en ,
                            "http://bsdd.buildingsmart.org/#concept/details/1yoko0qSqHuO00025QrE$V"@en ;
               rdfs:label "Controller"@en ,
                          "Organe de contrôle"@fr-fr ,
                          "Regler"@de-de ;
               rdfs:seeAlso ifc:IfcController .


###  http://pi.pauwel.be/voc/distributionelement#Controller-FLOATING
mep:Controller-FLOATING rdf:type owl:Class ;
                        rdfs:subClassOf mep:Controller ;
                        rdfs:comment "http://bsdd.buildingsmart.org/#concept/details/3v66KyDUH03vDK75zE5Ddn"@en ,
                                     "output increases or decreases at a constant or accelerating rate."@en ;
                        rdfs:label "Floating"@en ,
                                   "flottør"@nb-no ;
                        rdfs:seeAlso ifc:IfcControllerEnumType .


###  http://pi.pauwel.be/voc/distributionelement#Controller-MULTIPOSITION
mep:Controller-MULTIPOSITION rdf:type owl:Class ;
                             rdfs:subClassOf mep:Controller ;
                             rdfs:comment "http://bsdd.buildingsmart.org/#concept/details/2a0hNKxwTAH8HS3TExjKQd"@en ,
                                          "output is discrete value, can be one of three or more values."@en ;
                             rdfs:label "Multi-Position"@en ,
                                        "flerposisjonskontroller"@nb-no ;
                             rdfs:seeAlso ifc:IfcControllerEnumType .


###  http://pi.pauwel.be/voc/distributionelement#Controller-PROGRAMMABLE
mep:Controller-PROGRAMMABLE rdf:type owl:Class ;
                            rdfs:subClassOf mep:Controller ;
                            rdfs:comment "http://bsdd.buildingsmart.org/#concept/details/1UXoUiKJr2XedXgGzf6I3D"@en ,
                                         "programmable logic controller containing interconnected operations and variables."@en ;
                            rdfs:label "Programmable"@en ,
                                       "programerbar kontroller"@nb-no ;
                            rdfs:seeAlso ifc:IfcControllerEnumType .


###  http://pi.pauwel.be/voc/distributionelement#Controller-PROPORTIONAL
mep:Controller-PROPORTIONAL rdf:type owl:Class ;
                            rdfs:subClassOf mep:Controller ;
                            rdfs:comment "http://bsdd.buildingsmart.org/#concept/details/3soSUmco55dRLnyEdLB2Pe"@en ,
                                         "output is proportional to the control error and optionally time integral and derivative."@en ;
                            rdfs:label "Proportional"@en ,
                                       "proporsjonal"@nb-no ;
                            rdfs:seeAlso ifc:IfcControllerEnumType .


###  http://pi.pauwel.be/voc/distributionelement#Controller-TWOPOSITION
mep:Controller-TWOPOSITION rdf:type owl:Class ;
                           rdfs:subClassOf mep:Controller ;
                           rdfs:comment "http://bsdd.buildingsmart.org/#concept/details/3eIN8kftz36v5YeB_hMmzI"@en ;
                           rdfs:label "Two-Position"@en ;
                           rdfs:seeAlso ifc:IfcControllerEnumType .


###  http://pi.pauwel.be/voc/distributionelement#CooledBeam
mep:CooledBeam rdf:type owl:Class ;
               rdfs:subClassOf mep:EnergyConversionDevice ;
               rdfs:comment "A device typically used to cool air by circulating a fluid such as chilled water through exposed finned tubes above a space. Typically mounted overhead near or within a ceiling."@en ,
                            "http://bsdd.buildingsmart.org/#concept/details/1R134kf$f3g9C$U9ACWL3s"@en ;
               rdfs:label "Chilled Beam"@en ,
                          "Cooled Beam"@en ,
                          "Kühlbalken"@de-de ,
                          "Poutre froide"@fr-fr ,
                          "Poutre froide type"@fr-fr ,
                          "kjølekonvektor"@nb-no ;
               rdfs:seeAlso ifc:IfcCooledBeam .


###  http://pi.pauwel.be/voc/distributionelement#CooledBeam-ACTIVE
mep:CooledBeam-ACTIVE rdf:type owl:Class ;
                      rdfs:subClassOf mep:CooledBeam ;
                      rdfs:comment "an active or ventilated cooled beam provides cooling (and heating) but can also function as an air terminal in a ventilation system"@en ,
                                   "an active or ventilated cooled beam provides cooling (and heating) but can also function as an air terminal in a ventilation system"@en-gb ,
                                   "http://bsdd.buildingsmart.org/#concept/details/366WDqf6H92RxKizKbtgeZ"@en ;
                      rdfs:label "Active"@en ,
                                 "kjølekonvektor - aktiv"@nb-no ;
                      rdfs:seeAlso ifc:IfcCooledBeamEnumType .


###  http://pi.pauwel.be/voc/distributionelement#CooledBeam-PASSIVE
mep:CooledBeam-PASSIVE rdf:type owl:Class ;
                       rdfs:subClassOf mep:CooledBeam ;
                       rdfs:comment "http://bsdd.buildingsmart.org/#concept/details/2xz0NcLlr5_O7fEPShW1WV"@en ;
                       rdfs:label "Passive"@en ,
                                  "passiv"@nb-no ;
                       rdfs:seeAlso ifc:IfcCooledBeamEnumType .


###  http://pi.pauwel.be/voc/distributionelement#CoolingTower
mep:CoolingTower rdf:type owl:Class ;
                 rdfs:subClassOf mep:EnergyConversionDevice ;
                 rdfs:comment "A device which rejects heat to ambient air by circulating a fluid such as water through it to reduce its temperature by partial evaporation."@en ,
                              "http://bsdd.buildingsmart.org/#concept/details/0ExTiEVwf5eBdOlVt_Lyd0"@en ;
                 rdfs:label "Cooling Tower"@en ,
                            "Kühlturm"@de-de ,
                            "Tour de refroidissement"@fr-fr ,
                            "kjøletårn"@nb-no ;
                 rdfs:seeAlso ifc:IfcCoolingTower .


###  http://pi.pauwel.be/voc/distributionelement#CoolingTower-MECHANICALFORCEDDRAFT
mep:CoolingTower-MECHANICALFORCEDDRAFT rdf:type owl:Class ;
                                       rdfs:subClassOf mep:CoolingTower ;
                                       rdfs:comment "air flow is produced by a mechanical device, typically one or more fans, located on the inlet air side of the cooling tower."@en ,
                                                    "http://bsdd.buildingsmart.org/#concept/details/3dU1hLD$n4bwQx_$PVTTC6"@en ;
                                       rdfs:label "Mechanical Forced Draft"@en ,
                                                  "mekanisk utkast"@nb-no ;
                                       rdfs:seeAlso ifc:IfcCoolingTowerEnumType .


###  http://pi.pauwel.be/voc/distributionelement#CoolingTower-MECHANICALINDUCEDDRAFT
mep:CoolingTower-MECHANICALINDUCEDDRAFT rdf:type owl:Class ;
                                        rdfs:subClassOf mep:CoolingTower ;
                                        rdfs:comment "air flow is produced by a mechanical device, typically one or more fans, located on the air outlet side of the cooling tower."@en ,
                                                     "http://bsdd.buildingsmart.org/#concept/details/2aEmlXSRL6hO5XcfF8JxRk"@en ;
                                        rdfs:label "Mechanical Induced Draft"@en ,
                                                   "mekanisk indusert utkast"@nb-no ;
                                        rdfs:seeAlso ifc:IfcCoolingTowerEnumType .


###  http://pi.pauwel.be/voc/distributionelement#CoolingTower-NATURALDRAFT
mep:CoolingTower-NATURALDRAFT rdf:type owl:Class ;
                              rdfs:subClassOf mep:CoolingTower ;
                              rdfs:comment "air flow is produced naturally."@en ,
                                           "http://bsdd.buildingsmart.org/#concept/details/3O4_SVPPzB3881fdAXOU7s"@en ;
                              rdfs:label "Natural Draft"@en ,
                                         "naturlig trekk"@nb-no ;
                              rdfs:seeAlso ifc:IfcCoolingTowerEnumType .


###  http://pi.pauwel.be/voc/distributionelement#Damper
mep:Damper rdf:type owl:Class ;
           rdfs:subClassOf mep:FlowController ;
           rdfs:comment "A flow controller in an HVAC duct distribution system and is used to control or modulate the flow of air."@en ,
                        "http://bsdd.buildingsmart.org/#concept/details/2lAXa0qT0HuO00025QrE$V"@en ,
                        "innretning som brukes til å redusere støt eller vibrasjoner med energiabsorberende metoder"@nb-no ;
           rdfs:label "Damper"@en ,
                      "Détecteur d'incendie"@fr-fr ,
                      "Regelklappe"@de-de ,
                      "Spjæld"@da ,
                      "serranda"@it-it ,
                      "spjeld"@nb-no ;
           rdfs:seeAlso ifc:IfcDamper .


###  http://pi.pauwel.be/voc/distributionelement#Damper-BACKDRAFTDAMPER
mep:Damper-BACKDRAFTDAMPER rdf:type owl:Class ;
                           rdfs:subClassOf mep:Damper ;
                           rdfs:comment "http://bsdd.buildingsmart.org/#concept/details/0g_pG9hAD1XgJ8pML2mm5H"@en ;
                           rdfs:label "Back Draft Damper"@en ,
                                      "baktrekk demper"@nb-no ;
                           rdfs:seeAlso ifc:IfcDamperEnumType .


###  http://pi.pauwel.be/voc/distributionelement#Damper-BALANCINGDAMPER
mep:Damper-BALANCINGDAMPER rdf:type owl:Class ;
                           rdfs:subClassOf mep:Damper ;
                           rdfs:comment "http://bsdd.buildingsmart.org/#concept/details/2p0wEtbSj4gxlyI6mhADq2"@en ;
                           rdfs:label "Balancing Damper"@en ,
                                      "utjevningsspjeld"@nb-no ;
                           rdfs:seeAlso ifc:IfcDamperEnumType .


###  http://pi.pauwel.be/voc/distributionelement#Damper-BLASTDAMPER
mep:Damper-BLASTDAMPER rdf:type owl:Class ;
                       rdfs:subClassOf mep:Damper ;
                       rdfs:comment "http://bsdd.buildingsmart.org/#concept/details/369EqwVYL9pfnNqcXnoDHU"@en ;
                       rdfs:label "Blast Damper"@en ,
                                  "eksplosjon spjeld"@nb-no ;
                       rdfs:seeAlso ifc:IfcDamperEnumType .


###  http://pi.pauwel.be/voc/distributionelement#Damper-CONTROLDAMPER
mep:Damper-CONTROLDAMPER rdf:type owl:Class ;
                         rdfs:subClassOf mep:Damper ;
                         rdfs:comment "http://bsdd.buildingsmart.org/#concept/details/2rVf7QFRTEWOLI2fZJuW7H"@en ;
                         rdfs:label "Control Damper"@en ;
                         rdfs:seeAlso ifc:IfcDamperEnumType .


###  http://pi.pauwel.be/voc/distributionelement#Damper-FIREDAMPER
mep:Damper-FIREDAMPER rdf:type owl:Class ;
                      rdfs:subClassOf mep:Damper ;
                      rdfs:comment "http://bsdd.buildingsmart.org/#concept/details/3mqiUJIz57JBFFnuqvB3qT"@en ;
                      rdfs:label "Fire Damper"@en ;
                      rdfs:seeAlso ifc:IfcDamperEnumType .


###  http://pi.pauwel.be/voc/distributionelement#Damper-FIRESMOKEDAMPER
mep:Damper-FIRESMOKEDAMPER rdf:type owl:Class ;
                           rdfs:subClassOf mep:Damper ;
                           rdfs:comment "http://bsdd.buildingsmart.org/#concept/details/3fTPn78FL2kPB6iokOAbpY"@en ;
                           rdfs:label "Fire Smoke Damper"@en ;
                           rdfs:seeAlso ifc:IfcDamperEnumType .


###  http://pi.pauwel.be/voc/distributionelement#Damper-FUMEHOODEXHAUST
mep:Damper-FUMEHOODEXHAUST rdf:type owl:Class ;
                           rdfs:subClassOf mep:Damper ;
                           rdfs:comment "http://bsdd.buildingsmart.org/#concept/details/1U6ESQrqDFCPr0rdPKWCka"@en ;
                           rdfs:label "Fume Hood Exhaust"@en ,
                                      "røykhette"@nb-no ;
                           rdfs:seeAlso ifc:IfcDamperEnumType .


###  http://pi.pauwel.be/voc/distributionelement#Damper-GRAVITYDAMPER
mep:Damper-GRAVITYDAMPER rdf:type owl:Class ;
                         rdfs:subClassOf mep:Damper ;
                         rdfs:comment "http://bsdd.buildingsmart.org/#concept/details/1A$dgK16XE_x2gK7uacSn3"@en ;
                         rdfs:label "Gravity Damper"@en ;
                         rdfs:seeAlso ifc:IfcDamperEnumType .


###  http://pi.pauwel.be/voc/distributionelement#Damper-GRAVITYRELIEFDAMPER
mep:Damper-GRAVITYRELIEFDAMPER rdf:type owl:Class ;
                               rdfs:subClassOf mep:Damper ;
                               rdfs:comment "http://bsdd.buildingsmart.org/#concept/details/26urqKngv5ve948m7Tso_5"@en ;
                               rdfs:label "Gravity Relief Damper"@en ;
                               rdfs:seeAlso ifc:IfcDamperEnumType .


###  http://pi.pauwel.be/voc/distributionelement#Damper-RELIEFDAMPER
mep:Damper-RELIEFDAMPER rdf:type owl:Class ;
                        rdfs:subClassOf mep:Damper ;
                        rdfs:comment "http://bsdd.buildingsmart.org/#concept/details/0CQxb8jqP12etStsVhj0a2"@en ;
                        rdfs:label "Relief Damper"@en ,
                                   "relieff spjeld"@nb-no ;
                        rdfs:seeAlso ifc:IfcDamperEnumType .


###  http://pi.pauwel.be/voc/distributionelement#Damper-SMOKEDAMPER
mep:Damper-SMOKEDAMPER rdf:type owl:Class ;
                       rdfs:subClassOf mep:Damper ;
                       rdfs:comment "http://bsdd.buildingsmart.org/#concept/details/1vKdAZIn1BaBKbLSz3Ygwn"@en ;
                       rdfs:label "Smoke Damper"@en ,
                                  "røyspjeld"@nb-no ;
                       rdfs:seeAlso ifc:IfcDamperEnumType .


###  http://pi.pauwel.be/voc/distributionelement#DistributionChamberElement
mep:DistributionChamberElement rdf:type owl:Class ;
                               rdfs:subClassOf mep:DistributionFlowElement ;
                               rdfs:comment "A place at which distribution systems and their constituent elements may be inspected or through which they may travel."@en ,
                                            "http://bsdd.buildingsmart.org/#concept/details/1D7kC0qTCHuO00025QrE$V"@en ;
                               rdfs:label "Distribution Chamber Element"@en ,
                                          "Elément de chambre de distribution"@fr-fr ,
                                          "Schacht / Graben / Revisionsschacht"@de-de ,
                                          "distribusjonskammer element"@nb-no ;
                               rdfs:seeAlso ifc:IfcDistributionChamberElement .


###  http://pi.pauwel.be/voc/distributionelement#DistributionChamberElement-FORMEDDUCT
mep:DistributionChamberElement-FORMEDDUCT rdf:type owl:Class ;
                                          rdfs:subClassOf mep:DistributionChamberElement ;
                                          rdfs:comment "http://bsdd.buildingsmart.org/#concept/details/02IcnFZFL5vOjShoJLi_XK"@en ;
                                          rdfs:label "Formed Duct"@en ;
                                          rdfs:seeAlso ifc:IfcDistributionChamberElementEnumType .


###  http://pi.pauwel.be/voc/distributionelement#DistributionChamberElement-INSPECTIONCHAMBER
mep:DistributionChamberElement-INSPECTIONCHAMBER rdf:type owl:Class ;
                                                 rdfs:subClassOf mep:DistributionChamberElement ;
                                                 rdfs:comment "chamber constructed on a drain, sewer or pipeline with a removable cover that permits visble inspection"@en ,
                                                              "chamber constructed on a drain, sewer or pipeline with a removable cover that permits visble inspection"@en-gb ,
                                                              "http://bsdd.buildingsmart.org/#concept/details/0XN2ZdAhP8tPdjsk4V3170"@en ;
                                                 rdfs:label "Inspection Chamber"@en ,
                                                            "inspeksjonskammer"@nb-no ;
                                                 rdfs:seeAlso ifc:IfcDistributionChamberElementEnumType .


###  http://pi.pauwel.be/voc/distributionelement#DistributionChamberElement-INSPECTIONPIT
mep:DistributionChamberElement-INSPECTIONPIT rdf:type owl:Class ;
                                             rdfs:subClassOf mep:DistributionChamberElement ;
                                             rdfs:comment "http://bsdd.buildingsmart.org/#concept/details/05cbWWHhL7kgrWsi2U6_yV"@en ,
                                                          "recess or chamber formed to permit access for inspection of substructure and services"@en ,
                                                          "recess or chamber formed to permit access for inspection of substructure and services"@en-gb ;
                                             rdfs:label "Inspection Pit"@en ,
                                                        "inspeksjonsbrønn"@nb-no ;
                                             rdfs:seeAlso ifc:IfcDistributionChamberElementEnumType .


###  http://pi.pauwel.be/voc/distributionelement#DistributionChamberElement-MANHOLE
mep:DistributionChamberElement-MANHOLE rdf:type owl:Class ;
                                       rdfs:subClassOf mep:DistributionChamberElement ;
                                       rdfs:comment "http://bsdd.buildingsmart.org/#concept/details/1bbvZoH6X72QXL2iztFvrY"@en ;
                                       rdfs:label "Manhole"@en ,
                                                  "kum"@nb-no ;
                                       rdfs:seeAlso ifc:IfcDistributionChamberElementEnumType .


###  http://pi.pauwel.be/voc/distributionelement#DistributionChamberElement-METERCHAMBER
mep:DistributionChamberElement-METERCHAMBER rdf:type owl:Class ;
                                            rdfs:subClassOf mep:DistributionChamberElement ;
                                            rdfs:comment "chamber that houses a meter(s)"@en ,
                                                         "chamber that houses a meter(s)"@en-gb ,
                                                         "http://bsdd.buildingsmart.org/#concept/details/2t4ttlLaz5zerB1pgSekJt"@en ;
                                            rdfs:label "Meter Chamber"@en ,
                                                       "målekammer"@nb-no ;
                                            rdfs:seeAlso ifc:IfcDistributionChamberElementEnumType .


###  http://pi.pauwel.be/voc/distributionelement#DistributionChamberElement-SUMP
mep:DistributionChamberElement-SUMP rdf:type owl:Class ;
                                    rdfs:subClassOf mep:DistributionChamberElement ;
                                    rdfs:comment "http://bsdd.buildingsmart.org/#concept/details/013MAut7T66e3F7FQ6GSpz"@en ;
                                    rdfs:label "Sump"@en ,
                                               "drenering"@nb-no ;
                                    rdfs:seeAlso ifc:IfcDistributionChamberElementEnumType .


###  http://pi.pauwel.be/voc/distributionelement#DistributionChamberElement-TRENCH
mep:DistributionChamberElement-TRENCH rdf:type owl:Class ;
                                      rdfs:subClassOf mep:DistributionChamberElement ;
                                      rdfs:comment "http://bsdd.buildingsmart.org/#concept/details/2yGBCxZDXDlBMJTgQNqhCM"@en ;
                                      rdfs:label "Trench"@en ,
                                                 "grøft"@nb-no ;
                                      rdfs:seeAlso ifc:IfcDistributionChamberElementEnumType .


###  http://pi.pauwel.be/voc/distributionelement#DistributionChamberElement-VALVECHAMBER
mep:DistributionChamberElement-VALVECHAMBER rdf:type owl:Class ;
                                            rdfs:subClassOf mep:DistributionChamberElement ;
                                            rdfs:comment "http://bsdd.buildingsmart.org/#concept/details/1JHK2axxvBXQ7W3Ey18QZW"@en ;
                                            rdfs:label "Valve Chamber"@en ;
                                            rdfs:seeAlso ifc:IfcDistributionChamberElementEnumType .


###  http://pi.pauwel.be/voc/distributionelement#DistributionControlElement
mep:DistributionControlElement rdf:type owl:Class ;
                               rdfs:subClassOf mep:DistributionElement ;
                               rdfs:comment "http://bsdd.buildingsmart.org/#concept/details/3U4sRnv$D80uOqEQZrMx_Z"@en ,
                                            "the distribution element ifcdistributioncontrolelement defines occurrence elements of a building automation control system that are used to impart control over elements of a distribution system. ifcdistributioncontrolelement defines elements of a building automation control system. these are typically used to control distribution system elements to maintain variables such as temperature, humidity, pressure, flow, power or lighting levels, through the modulation, staging or sequencing of mechanical or electrical devices. the three general functional categories of control elements are as follows: impart control over flow control elements (ifcflowcontroller) in a distribution system such as dampers, valves or relays, typically through the use of actuation (ifcactuator)., sensing elements (ifcsensor) that measure changes in the controlled variable such as temperature, humidity, pressure or flow., controllers (ifccontroller) typically classified according to the control action they seek to perform and generally responsible for making decisions about the elements under control.. since ifcdistributioncontrolelement and its subtypes typically relate to many different distribution flow elements (ifcdistributionflowelement), the objectified relationship ifcrelflowcontrolelements has been provided to relate control and flow elements as required. the key distinction between ifcdistributionflowelement and ifcdistributioncontrolelement is whether it is internal or external to the flow system, respectively. for example, the distinction between ifcflowmeter (subtype of ifcdistributionflowelement measuring a flow quantity) and ifcflowinstrument (subtype of ifcdistributioncontrolelement measuring a flow quality), is based on this principal. a physical device that connects within the flow system in which it measures (having inlet/outlet pipes for the measured substance) follows the ifcdistributionflowelement hierarchy (and therefore ifcflowmeter which measures the flow internally). otherwise, if it monitors/controls but does not connect inline within the flow system (it is external or is a component of another device), then it follows the ifcdistributioncontrolelement hierarchy (and therefore ifcflowinstrument which may display various attributes through connected sensors)."@en ;
                               rdfs:label "Distribution Control Element"@en ,
                                          "Komponente der Gebäudeautomation (allgemein)"@de-de ,
                                          "distribusjon manøvreringsorgan"@nb-no ,
                                          "Élément de circuit de distribution"@fr-fr ;
                               rdfs:seeAlso ifc:IfcDistributionControlElement .


###  http://pi.pauwel.be/voc/distributionelement#DistributionElement
mep:DistributionElement rdf:type owl:Class ;
                        rdfs:subClassOf <https://schema.org/Product>, <http://purl.org/goodrelations/v1#SomeItems> ;
                        rdfs:comment "A generalization of all elements that participate in a distribution system. "@en ,
                                     """A generalization of all elements that participate in a distribution system. Typical examples :
building service elements within a heating systems, cooling system, ventilation system, plumbing system
or electrical elements within a communication network"""@ifc-2x4 ,
                                     "http://bsdd.buildingsmart.org/#concept/details/1UHiGqJXTCL9Ds53EKce2Y"@en ;
                        rdfs:label "Distribution Element"@en ,
                                   "Elément de distribution"@fr-fr ,
                                   "haustechnische Komponente (allgemein)"@de-de ;
                        rdfs:seeAlso ifc:IfcDistributionElement .


###  http://pi.pauwel.be/voc/distributionelement#DistributionFlowElement
mep:DistributionFlowElement rdf:type owl:Class ;
                            rdfs:subClassOf mep:DistributionElement ;
                            rdfs:comment """A distribution element defined by occurrence elements of a distribution system that facilitate the distribution of energy or matter, such as air, water or power.
Examples are ducts, pipes, wires, fittings, and equipment."""@en ,
                                         "http://bsdd.buildingsmart.org/#concept/details/2Ci$80qWWHuO00025QrE$V"@en ;
                            rdfs:label "Distribution Flow Element"@en ,
                                       "Elément de distribution de fluide"@fr-fr ,
                                       "Komponente der TGA (allgemein)"@de-de ,
                                       "distribusjonsrørelement"@nb-no ;
                            rdfs:seeAlso ifc:IfcDistributionFlowElement .


###  http://pi.pauwel.be/voc/distributionelement#DuctFitting
mep:DuctFitting rdf:type owl:Class ;
                rdfs:subClassOf mep:FlowFitting ;
                rdfs:comment "A junction or transition in a ducted flow distribution system or used to connect duct segments, resulting in changes in flow characteristics to the fluid such as direction and flow rate."@en ,
                             "http://bsdd.buildingsmart.org/#concept/details/3UarA0qTqHuO00025QrE$V"@en ;
                rdfs:label "Duct Fitting"@en ,
                           "Kanaalverbindingshulpstuk"@nl-nl ,
                           "Kanalverbinder"@de-de ,
                           "Raccord de gaine"@fr-fr ,
                           "kanalfeste"@nb-no ;
                rdfs:seeAlso ifc:IfcDuctFitting .


###  http://pi.pauwel.be/voc/distributionelement#DuctFitting-BEND
mep:DuctFitting-BEND rdf:type owl:Class ;
                     rdfs:subClassOf mep:DuctFitting ;
                     rdfs:comment "a fitting with typically two ports used to change the direction of flow between connected elements"@en ,
                                  "a fitting with typically two ports used to change the direction of flow between connected elements"@en-gb ,
                                  "http://bsdd.buildingsmart.org/#concept/details/0TRO3rI8H6H9tkJsr0U5Zs"@en ;
                     rdfs:label "Bend"@en ,
                                "bend"@nb-no ;
                     rdfs:seeAlso ifc:IfcDuctFittingEnumType .


###  http://pi.pauwel.be/voc/distributionelement#DuctFitting-CONNECTOR
mep:DuctFitting-CONNECTOR rdf:type owl:Class ;
                          rdfs:subClassOf mep:DuctFitting ;
                          rdfs:comment "http://bsdd.buildingsmart.org/#concept/details/2uxftRh$fAkhgUKLmF1KRz"@en ;
                          rdfs:label "Connector"@en ,
                                     "connecteur"@fr-fr ,
                                     "forbindelse"@nb-no ;
                          rdfs:seeAlso ifc:IfcDuctFittingEnumType .


###  http://pi.pauwel.be/voc/distributionelement#DuctFitting-ENTRY
mep:DuctFitting-ENTRY rdf:type owl:Class ;
                      rdfs:subClassOf mep:DuctFitting ;
                      rdfs:comment "entry fitting, typically unconnected at one port and connected to a flow distribution system at the other (e.g., an outside air duct system intake opening)"@en ,
                                   "entry fitting, typically unconnected at one port and connected to a flow distribution system at the other (e.g., an outside air duct system intake opening)"@en-gb ,
                                   "http://bsdd.buildingsmart.org/#concept/details/05vd0J9Jv4yf_lzDUNR9nD"@en ;
                      rdfs:label "Entry"@en ,
                                 "inngang"@nb-no ;
                      rdfs:seeAlso ifc:IfcDuctFittingEnumType .


###  http://pi.pauwel.be/voc/distributionelement#DuctFitting-EXIT
mep:DuctFitting-EXIT rdf:type owl:Class ;
                     rdfs:subClassOf mep:DuctFitting ;
                     rdfs:comment "http://bsdd.buildingsmart.org/#concept/details/0VmlPFMi57uO7GMaLeI9HP"@en ;
                     rdfs:label "Exit"@en ,
                                "utgang"@nb-no ;
                     rdfs:seeAlso ifc:IfcDuctFittingEnumType .


###  http://pi.pauwel.be/voc/distributionelement#DuctFitting-JUNCTION
mep:DuctFitting-JUNCTION rdf:type owl:Class ;
                         rdfs:subClassOf mep:DuctFitting ;
                         rdfs:comment "a fitting with typically more than two ports used to redistribute flow among the ports and/or to change the direction of flow between connected elements (e.g, tee, cross, wye, etc.)"@en ,
                                      "a fitting with typically more than two ports used to redistribute flow among the ports and/or to change the direction of flow between connected elements (e.g, tee, cross, wye, etc.)."@en-gb ,
                                      "http://bsdd.buildingsmart.org/#concept/details/0UePnHIHn9vvttWhkbxrCv"@en ;
                         rdfs:label "Junction"@en ,
                                    "grenrør"@nb-no ,
                                    "kryss"@nb-no ;
                         rdfs:seeAlso ifc:IfcDuctFittingEnumType .


###  http://pi.pauwel.be/voc/distributionelement#DuctFitting-OBSTRUCTION
mep:DuctFitting-OBSTRUCTION rdf:type owl:Class ;
                            rdfs:subClassOf mep:DuctFitting ;
                            rdfs:comment "http://bsdd.buildingsmart.org/#concept/details/0_eTgdHQn7MwoGtRPOoi4r"@en ;
                            rdfs:label "Obstruction"@en ,
                                       "hindring"@nb-no ;
                            rdfs:seeAlso ifc:IfcDuctFittingEnumType .


###  http://pi.pauwel.be/voc/distributionelement#DuctFitting-TRANSITION
mep:DuctFitting-TRANSITION rdf:type owl:Class ;
                           rdfs:subClassOf mep:DuctFitting ;
                           rdfs:comment "http://bsdd.buildingsmart.org/#concept/details/1JknxHMCfDq9zypxDIsX5P"@en ;
                           rdfs:label "Transition"@en ,
                                      "overgang"@nb-no ;
                           rdfs:seeAlso ifc:IfcDuctFittingEnumType .


###  http://pi.pauwel.be/voc/distributionelement#DuctSegment
mep:DuctSegment rdf:type owl:Class ;
                rdfs:subClassOf mep:FlowSegment ;
                rdfs:comment "Used to typically join two sections of duct network."@en ,
                             "http://bsdd.buildingsmart.org/#concept/details/0i3x_0qTuHuO00025QrE$V"@en ;
                rdfs:label "Duct Segment"@en ,
                           "Kanal"@de-de ,
                           "Tronçon de gaine"@fr-fr ,
                           "kanalsegment"@nb-no ;
                rdfs:seeAlso ifc:IfcDuctSegment .


###  http://pi.pauwel.be/voc/distributionelement#DuctSegment-FLEXIBLESEGMENT
mep:DuctSegment-FLEXIBLESEGMENT rdf:type owl:Class ;
                                rdfs:subClassOf mep:DuctSegment ;
                                rdfs:comment "http://bsdd.buildingsmart.org/#concept/details/2nqUfs2mn9YQ_jGNKRyiPP"@en ;
                                rdfs:label "Flexible Duct Segment"@en ,
                                           "fleksibel delflate"@nb-no ,
                                           "fleksibel rørdel"@nb-no ;
                                rdfs:seeAlso ifc:IfcDuctSegmentEnumType .


###  http://pi.pauwel.be/voc/distributionelement#DuctSegment-RIGIDSEGMENT
mep:DuctSegment-RIGIDSEGMENT rdf:type owl:Class ;
                             rdfs:subClassOf mep:DuctSegment ;
                             rdfs:comment "a rigid segment is a continuous linear segment of duct that cannot be deformed"@en ,
                                          "a rigid segment is a continuous linear segment of duct that cannot be deformed"@en-gb ,
                                          "http://bsdd.buildingsmart.org/#concept/details/0Wy45YhJ1Bee5B_Ev4IySE"@en ;
                             rdfs:label "Rigid Duct Segment"@en ,
                                        "stiv delflate"@nb-no ;
                             rdfs:seeAlso ifc:IfcDuctSegmentEnumType .


###  http://pi.pauwel.be/voc/distributionelement#DuctSilencer
mep:DuctSilencer rdf:type owl:Class ;
                 rdfs:subClassOf mep:FlowTreatmentDevice ;
                 rdfs:comment "A device that is typically installed inside a duct distribution system for the purpose of reducing the noise levels from air movement, fan noise, etc. in the adjacent space or downstream of the duct silencer device."@en ,
                              "http://bsdd.buildingsmart.org/#concept/details/2htluultzBmQOOYxoTJ2k5"@en ;
                 rdfs:label "Duct Silencer"@en ,
                            "Kanaalgeluiddemper"@nl-nl ,
                            "Kanalschalldämpfer"@de-de ,
                            "Silencieux circulaire"@fr-fr ;
                 rdfs:seeAlso ifc:IfcDuctSilencer .


###  http://pi.pauwel.be/voc/distributionelement#DuctSilencer-FLATOVAL
mep:DuctSilencer-FLATOVAL rdf:type owl:Class ;
                          rdfs:subClassOf mep:DuctSilencer ;
                          rdfs:comment "http://bsdd.buildingsmart.org/#concept/details/0VN55_f5zDDwQXiRI$8Z_y"@en ;
                          rdfs:label "Flat Oval Duct Silencer"@en ,
                                     "flatoval"@nb-no ;
                          rdfs:seeAlso ifc:IfcDuctSilencerEnumType .


###  http://pi.pauwel.be/voc/distributionelement#DuctSilencer-RECTANGULAR
mep:DuctSilencer-RECTANGULAR rdf:type owl:Class ;
                             rdfs:subClassOf mep:DuctSilencer ;
                             rdfs:comment "http://bsdd.buildingsmart.org/#concept/details/3NtvXddFX5JRlghR5mPion"@en ;
                             rdfs:label "Rectangular Duct Silencer"@en ,
                                        "rektangulær"@nb-no ;
                             rdfs:seeAlso ifc:IfcDuctSilencerEnumType .


###  http://pi.pauwel.be/voc/distributionelement#DuctSilencer-ROUND
mep:DuctSilencer-ROUND rdf:type owl:Class ;
                       rdfs:subClassOf mep:DuctSilencer ;
                       rdfs:comment "http://bsdd.buildingsmart.org/#concept/details/0Pab9zW$v0E8Xbyt9Joo2A"@en ;
                       rdfs:label "Round Duct Silencer"@en ,
                                  "sirkulær"@nb-no ;
                       rdfs:seeAlso ifc:IfcDuctSilencerEnumType .


###  http://pi.pauwel.be/voc/distributionelement#ElectricAppliance
mep:ElectricAppliance rdf:type owl:Class ;
                      rdfs:subClassOf mep:FlowTerminal ;
                      rdfs:comment """A device intended for consumer usage that is powered by electricity.
May be fixed in place or able to be moved from one space to another. Requires an electrical supply that may be supplied either by an electrical circuit or provided from a local battery source."""@en ,
                                   "http://bsdd.buildingsmart.org/#concept/details/3YTFM$9GvByR7HJawXiG4V"@en ;
                      rdfs:label "Appareil électrique"@fr-fr ,
                                 "Electric Appliance"@en ,
                                 "Elektrisches Gerät"@de-de ,
                                 "elektrisk innretning"@nb-no ;
                      rdfs:seeAlso ifc:IfcElectricAppliance .


###  http://pi.pauwel.be/voc/distributionelement#ElectricAppliance-DISHWASHER
mep:ElectricAppliance-DISHWASHER rdf:type owl:Class ;
                                 rdfs:subClassOf mep:ElectricAppliance ;
                                 rdfs:comment "an appliance that has the primary function of washing dishes"@en ,
                                              "an appliance that has the primary function of washing dishes"@en-gb ,
                                              "appliance for washing dishes"@en ,
                                              "diskmaskin"@sv-se ,
                                              "http://bsdd.buildingsmart.org/#concept/details/02NUQ13z56XvvUbtiIY3SW"@en ;
                                 rdfs:label "Dishwasher"@en ,
                                            "Geschirrspülmaschine"@de-de ,
                                            "diskmaskin"@sv-se ,
                                            "machine à laver la vaisselle"@fr-fr ,
                                            "oppvaskmaskin"@nb-no ;
                                 rdfs:seeAlso ifc:IfcElectricApplianceEnumType .


###  http://pi.pauwel.be/voc/distributionelement#ElectricAppliance-ELECTRICCOOKER
mep:ElectricAppliance-ELECTRICCOOKER rdf:type owl:Class ;
                                     rdfs:subClassOf mep:ElectricAppliance ;
                                     rdfs:comment "an electrical appliance that has the primary function of cooking food (including oven, hob, grill)"@en ,
                                                  "an electrical appliance that has the primary function of cooking food (including oven, hob, grill)"@en-gb ,
                                                  "http://bsdd.buildingsmart.org/#concept/details/1fQUOe4mvC$PVZhL6$zYMj"@en ;
                                     rdfs:label "Electric Cooker"@en ,
                                                "kokeplate"@nb-no ;
                                     rdfs:seeAlso ifc:IfcElectricApplianceEnumType .


###  http://pi.pauwel.be/voc/distributionelement#ElectricAppliance-FREESTANDINGELECTRICHEATER
mep:ElectricAppliance-FREESTANDINGELECTRICHEATER rdf:type owl:Class ;
                                                 rdfs:subClassOf mep:ElectricAppliance ;
                                                 rdfs:comment "http://bsdd.buildingsmart.org/#concept/details/2vmsBMt5f6vOIJtsLV43C5"@en ;
                                                 rdfs:label "Free Standing Electric Heater"@en ;
                                                 rdfs:seeAlso ifc:IfcElectricApplianceEnumType .


###  http://pi.pauwel.be/voc/distributionelement#ElectricAppliance-FREESTANDINGFAN
mep:ElectricAppliance-FREESTANDINGFAN rdf:type owl:Class ;
                                      rdfs:subClassOf mep:ElectricAppliance ;
                                      rdfs:comment "http://bsdd.buildingsmart.org/#concept/details/1sbx$V$pfE3gA1HPGomlqC"@en ;
                                      rdfs:label "Free Standing Fan"@en ;
                                      rdfs:seeAlso ifc:IfcElectricApplianceEnumType .


###  http://pi.pauwel.be/voc/distributionelement#ElectricAppliance-FREESTANDINGWATERCOOLER
mep:ElectricAppliance-FREESTANDINGWATERCOOLER rdf:type owl:Class ;
                                              rdfs:subClassOf mep:ElectricAppliance ;
                                              rdfs:comment "http://bsdd.buildingsmart.org/#concept/details/2GNk4XczH2a9Bo486M2Dhf"@en ;
                                              rdfs:label "Free Standing Water Cooler"@en ;
                                              rdfs:seeAlso ifc:IfcElectricApplianceEnumType .


###  http://pi.pauwel.be/voc/distributionelement#ElectricAppliance-FREESTANDINGWATERHEATER
mep:ElectricAppliance-FREESTANDINGWATERHEATER rdf:type owl:Class ;
                                              rdfs:subClassOf mep:ElectricAppliance ;
                                              rdfs:comment "a small, local electrical appliance for heating water. a freestanding water heater is a 'plugged' appliance whose load may be removed from an electric circuit"@en ,
                                                           "a small, local electrical appliance for heating water. a freestanding water heater is a 'plugged' appliance whose load may be removed from an electric circuit"@en-gb ,
                                                           "http://bsdd.buildingsmart.org/#concept/details/0hmcm_zGD2HuO7SHEfEIAX"@en ;
                                              rdfs:label "Free Standing Water Heater"@en ,
                                                         "varmtvannsbereder"@nb-no ;
                                              rdfs:seeAlso ifc:IfcElectricApplianceEnumType .


###  http://pi.pauwel.be/voc/distributionelement#ElectricAppliance-FREEZER
mep:ElectricAppliance-FREEZER rdf:type owl:Class ;
                              rdfs:subClassOf mep:ElectricAppliance ;
                              rdfs:comment "an electrical appliance that has the primary function of storing food at temperatures below the freezing point of water"@en ,
                                           "an electrical appliance that has the primary function of storing food at temperatures below the freezing point of water"@en-gb ,
                                           "http://bsdd.buildingsmart.org/#concept/details/2lufsAWJmHu000025QrE$V"@en ;
                              rdfs:label "Freezer"@en ,
                                         "Vrieskast"@nl-nl ,
                                         "fryser"@nb-no ;
                              rdfs:seeAlso ifc:IfcElectricApplianceEnumType .


###  http://pi.pauwel.be/voc/distributionelement#ElectricAppliance-FRIDGE_FREEZER
mep:ElectricAppliance-FRIDGE_FREEZER rdf:type owl:Class ;
                                     rdfs:subClassOf mep:ElectricAppliance ;
                                     rdfs:comment "http://bsdd.buildingsmart.org/#concept/details/2$l6h0fcP1u9I_bcu2_2t0"@en ;
                                     rdfs:label "Fridge Freezer"@en ;
                                     rdfs:seeAlso ifc:IfcElectricApplianceEnumType .


###  http://pi.pauwel.be/voc/distributionelement#ElectricAppliance-HANDDRYER
mep:ElectricAppliance-HANDDRYER rdf:type owl:Class ;
                                rdfs:subClassOf mep:ElectricAppliance ;
                                rdfs:comment "http://bsdd.buildingsmart.org/#concept/details/0MdGYaJi90Ugvs9F4IBH45"@en ;
                                rdfs:label "Hand Dryer"@en ;
                                rdfs:seeAlso ifc:IfcElectricApplianceEnumType .


###  http://pi.pauwel.be/voc/distributionelement#ElectricAppliance-KITCHENMACHINE
mep:ElectricAppliance-KITCHENMACHINE rdf:type owl:Class ;
                                     rdfs:subClassOf mep:ElectricAppliance ;
                                     rdfs:comment "a specialized appliance used in commercial kitchens such as a mixer"@en ,
                                                  "a specialized appliance used in commercial kitchens such as a mixer"@en-gb ,
                                                  "http://bsdd.buildingsmart.org/#concept/details/3jScF9EaLB6wWXD1wgq6DV"@en ;
                                     rdfs:label "Kitchen Machine"@en ,
                                                "kjøkkenmaskin"@nb-no ;
                                     rdfs:seeAlso ifc:IfcElectricApplianceEnumType .


###  http://pi.pauwel.be/voc/distributionelement#ElectricAppliance-MICROWAVE
mep:ElectricAppliance-MICROWAVE rdf:type owl:Class ;
                                rdfs:subClassOf mep:ElectricAppliance ;
                                rdfs:comment "an electrical appliance that has the primary function of cooking food using microwaves"@en ,
                                             "an electrical appliance that has the primary function of cooking food using microwaves"@en-gb ,
                                             "http://bsdd.buildingsmart.org/#concept/details/3aYGRc49PF4AXOOV4IRJxc"@en ;
                                rdfs:label "MicroWave"@en ,
                                           "mikrobølge"@nb-no ;
                                rdfs:seeAlso ifc:IfcElectricApplianceEnumType .


###  http://pi.pauwel.be/voc/distributionelement#ElectricAppliance-PHOTOCOPIER
mep:ElectricAppliance-PHOTOCOPIER rdf:type owl:Class ;
                                  rdfs:subClassOf mep:ElectricAppliance ;
                                  rdfs:comment "a machine that has the primary function of reproduction of printed matter"@en ,
                                               "a machine that has the primary function of reproduction of printed matter"@en-gb ,
                                               "http://bsdd.buildingsmart.org/#concept/details/3f7QlBmRH8ixz3XB$p1vFX"@en ;
                                  rdfs:label "Photocopier"@en ,
                                             "kopimaskin"@nb-no ;
                                  rdfs:seeAlso ifc:IfcElectricApplianceEnumType .


###  http://pi.pauwel.be/voc/distributionelement#ElectricAppliance-REFRIGERATOR
mep:ElectricAppliance-REFRIGERATOR rdf:type owl:Class ;
                                   rdfs:subClassOf mep:ElectricAppliance ;
                                   rdfs:comment "http://bsdd.buildingsmart.org/#concept/details/2lIWS0WJmHu000025QrE$V"@en ;
                                   rdfs:label "Koelkast"@nl-nl ,
                                              "Refrigerator"@en ,
                                              "kjøleskap"@nb-no ;
                                   rdfs:seeAlso ifc:IfcElectricApplianceEnumType .


###  http://pi.pauwel.be/voc/distributionelement#ElectricAppliance-TUMBLEDRYER
mep:ElectricAppliance-TUMBLEDRYER rdf:type owl:Class ;
                                  rdfs:subClassOf mep:ElectricAppliance ;
                                  rdfs:comment "http://bsdd.buildingsmart.org/#concept/details/3vHWUCoT0Hsm00051Mm008"@en ;
                                  rdfs:label "Tumble Dryer"@en ,
                                             "Wäschetrockner"@de-de ,
                                             "dryer"@en ,
                                             "machine séchante"@fr-fr ,
                                             "tørketrommel"@nb-no ;
                                  rdfs:seeAlso ifc:IfcElectricApplianceEnumType .


###  http://pi.pauwel.be/voc/distributionelement#ElectricAppliance-VENDINGMACHINE
mep:ElectricAppliance-VENDINGMACHINE rdf:type owl:Class ;
                                     rdfs:subClassOf mep:ElectricAppliance ;
                                     rdfs:comment "http://bsdd.buildingsmart.org/#concept/details/3a1GPgbGb4HhfJfWNNnwRG"@en ;
                                     rdfs:label "Vending Machine"@en ;
                                     rdfs:seeAlso ifc:IfcElectricApplianceEnumType .


###  http://pi.pauwel.be/voc/distributionelement#ElectricAppliance-WASHINGMACHINE
mep:ElectricAppliance-WASHINGMACHINE rdf:type owl:Class ;
                                     rdfs:subClassOf mep:ElectricAppliance ;
                                     rdfs:comment "http://bsdd.buildingsmart.org/#concept/details/3nK_JH93v5JRpo7imsOJm6"@en ;
                                     rdfs:label "Washing Machine"@en ;
                                     rdfs:seeAlso ifc:IfcElectricApplianceEnumType .


###  http://pi.pauwel.be/voc/distributionelement#ElectricDistributionBoard
mep:ElectricDistributionBoard rdf:type owl:Class ;
                              rdfs:subClassOf mep:FlowController ;
                              rdfs:comment "A flow controller in which instances of electrical devices are brought together at a single place for a particular purpose. A distribution provides a housing for connected electrical distribution elements so that they can be viewed, operated or acted upon from a single place. Each connected item may have its own geometric representation and location."@en ,
                                           "http://bsdd.buildingsmart.org/#concept/details/1NTXNvjYPEHAEdF4$lUOA4"@en ;
                              rdfs:label "Electric Distribution Board"@en ,
                                         "Elektrischer Verteilungsregler"@de-de ,
                                         "Tableau de distribution électrique"@fr-fr ;
                              rdfs:seeAlso ifc:IfcElectricDistributionBoard .


###  http://pi.pauwel.be/voc/distributionelement#ElectricDistributionBoard-CONSUMERUNIT
mep:ElectricDistributionBoard-CONSUMERUNIT rdf:type owl:Class ;
                                           rdfs:subClassOf mep:ElectricDistributionBoard ;
                                           rdfs:comment "http://bsdd.buildingsmart.org/#concept/details/02vRNiXL17Ng6A0tyY3IZm"@en ;
                                           rdfs:label "Consumer Unit"@en ;
                                           rdfs:seeAlso ifc:IfcElectricDistributionBoardEnumType .


###  http://pi.pauwel.be/voc/distributionelement#ElectricDistributionBoard-DISTRIBUTIONBOARD
mep:ElectricDistributionBoard-DISTRIBUTIONBOARD rdf:type owl:Class ;
                                                rdfs:subClassOf mep:ElectricDistributionBoard ;
                                                rdfs:comment "http://bsdd.buildingsmart.org/#concept/details/2t_kmsr_9FbOzG08gdq5sn"@en ;
                                                rdfs:label "Distribution Board"@en ;
                                                rdfs:seeAlso ifc:IfcElectricDistributionBoardEnumType .


###  http://pi.pauwel.be/voc/distributionelement#ElectricDistributionBoard-MOTORCONTROLCENTRE
mep:ElectricDistributionBoard-MOTORCONTROLCENTRE rdf:type owl:Class ;
                                                 rdfs:subClassOf mep:ElectricDistributionBoard ;
                                                 rdfs:comment "http://bsdd.buildingsmart.org/#concept/details/23gvwO2$16qPz5TGUDljzB"@en ;
                                                 rdfs:label "Motor Control Centre"@en ;
                                                 rdfs:seeAlso ifc:IfcElectricDistributionBoardEnumType .


###  http://pi.pauwel.be/voc/distributionelement#ElectricDistributionBoard-SWITCHBOARD
mep:ElectricDistributionBoard-SWITCHBOARD rdf:type owl:Class ;
                                          rdfs:subClassOf mep:ElectricDistributionBoard ;
                                          rdfs:comment "http://bsdd.buildingsmart.org/#concept/details/3XP0I3Joj7y8AYq9ASPean"@en ;
                                          rdfs:label "Switch Board"@en ;
                                          rdfs:seeAlso ifc:IfcElectricDistributionBoardEnumType .


###  http://pi.pauwel.be/voc/distributionelement#ElectricFlowStorageDevice
mep:ElectricFlowStorageDevice rdf:type owl:Class ;
                              rdfs:subClassOf mep:FlowStorageDevice ;
                              rdfs:comment "A device in which electrical energy is stored and from which energy may be progressively released."@en ,
                                           "http://bsdd.buildingsmart.org/#concept/details/1QtwhR5Zn328NFUBlGt0yh"@en ;
                              rdfs:label "Electric Flow Storage Device"@en ,
                                         "Elektrisches Speichergerät"@de-de ,
                                         "strømlagringsenhet"@nb-no ;
                              rdfs:seeAlso ifc:IfcElectricFlowStorageDevice .


###  http://pi.pauwel.be/voc/distributionelement#ElectricFlowStorageDevice-BATTERY
mep:ElectricFlowStorageDevice-BATTERY rdf:type owl:Class ;
                                      rdfs:subClassOf mep:ElectricFlowStorageDevice ;
                                      rdfs:comment "a device for storing energy in chemical form so that it can be released as electrical energy"@en ,
                                                   "a device for storing energy in chemical form so that it can be released as electrical energy"@en-gb ,
                                                   "http://bsdd.buildingsmart.org/#concept/details/2SgW4DbB93yuwE75nOI9iX"@en ;
                                      rdfs:label "Battery"@en ,
                                                 "batteri"@nb-no ;
                                      rdfs:seeAlso ifc:IfcElectricFlowStorageDeviceEnumType .


###  http://pi.pauwel.be/voc/distributionelement#ElectricFlowStorageDevice-CAPACITORBANK
mep:ElectricFlowStorageDevice-CAPACITORBANK rdf:type owl:Class ;
                                            rdfs:subClassOf mep:ElectricFlowStorageDevice ;
                                            rdfs:comment "a device that stores electrical energy when an external power supply is present using the electrical property of capacitance"@en ,
                                                         "a device that stores electrical energy when an external power supply is present using the electrical property of capacitance"@en-gb ,
                                                         "http://bsdd.buildingsmart.org/#concept/details/3T$uPXx997$B5skfKbEgBk"@en ;
                                            rdfs:label "Capacitor Bank"@en ,
                                                       "kapasitetsbank"@nb-no ;
                                            rdfs:seeAlso ifc:IfcElectricFlowStorageDeviceEnumType .


###  http://pi.pauwel.be/voc/distributionelement#ElectricFlowStorageDevice-HARMONICFILTER
mep:ElectricFlowStorageDevice-HARMONICFILTER rdf:type owl:Class ;
                                             rdfs:subClassOf mep:ElectricFlowStorageDevice ;
                                             rdfs:comment "http://bsdd.buildingsmart.org/#concept/details/3CCGbA$dfCHxGIK0Zz2C08"@en ;
                                             rdfs:label "Harmonic Filter"@en ;
                                             rdfs:seeAlso ifc:IfcElectricFlowStorageDeviceEnumType .


###  http://pi.pauwel.be/voc/distributionelement#ElectricFlowStorageDevice-INDUCTORBANK
mep:ElectricFlowStorageDevice-INDUCTORBANK rdf:type owl:Class ;
                                           rdfs:subClassOf mep:ElectricFlowStorageDevice ;
                                           rdfs:comment "http://bsdd.buildingsmart.org/#concept/details/0s_ACAnfD8YAPin0isHx0d"@en ;
                                           rdfs:label "Inductor Bank"@en ;
                                           rdfs:seeAlso ifc:IfcElectricFlowStorageDeviceEnumType .


###  http://pi.pauwel.be/voc/distributionelement#ElectricFlowStorageDevice-UPS
mep:ElectricFlowStorageDevice-UPS rdf:type owl:Class ;
                                  rdfs:subClassOf mep:ElectricFlowStorageDevice ;
                                  rdfs:comment "a device that provides a time limited alternative source of power supply in the event of failure of the main supply"@en ,
                                               "a device that provides a time limited alternative source of power supply in the event of failure of the main supply"@en-gb ,
                                               "combination of convertors, switches and energy storage devices (for example batteries), constituting a power system for maintaining continuity of load power in case of input power failure."@en ,
                                               "http://bsdd.buildingsmart.org/#concept/details/1ru5tvtfLE7g$pBOrRs6g$"@en ;
                                  rdfs:label "UPS"@en ,
                                             "UPS"@nb-no ,
                                             "uninterruptible power supply"@en ,
                                             "uninterruptible power system"@en ;
                                  rdfs:seeAlso ifc:IfcElectricFlowStorageDeviceEnumType .


###  http://pi.pauwel.be/voc/distributionelement#ElectricGenerator
mep:ElectricGenerator rdf:type owl:Class ;
                      rdfs:subClassOf mep:EnergyConversionDevice ;
                      rdfs:comment "An engine that is a machine for converting mechanical energy into electrical energy."@en ,
                                   "http://bsdd.buildingsmart.org/#concept/details/1xmminhSL6bhcxZRNY$u6Z"@en ;
                      rdfs:label "Electric Generator"@en ,
                                 "Elektrogenerator"@de-de ,
                                 "elektrogenerator"@nb-no ,
                                 "générateur électrique"@fr-fr ;
                      rdfs:seeAlso ifc:IfcElectricGenerator .


###  http://pi.pauwel.be/voc/distributionelement#ElectricGenerator-CHP
mep:ElectricGenerator-CHP rdf:type owl:Class ;
                          rdfs:subClassOf mep:ElectricGenerator ;
                          rdfs:comment "combined heat and power supply, used not only as a source of electric energy but also as a heating source for the building. it may therefore be not only part of an electrical system but also of a heating system"@en ,
                                       "combined heat and power supply, used not only as a source of electric energy but also as a heating source for the building. it may therefore be not only part of an electrical system but also of a heating system"@en-gb ,
                                       "http://bsdd.buildingsmart.org/#concept/details/2vNA8q44vBZRsy_n0gsv2T"@en ;
                          rdfs:label "CHP"@en ,
                                     "kraftvarmeverk"@nb-no ;
                          rdfs:seeAlso ifc:IfcElectricGeneratorEnumType .


###  http://pi.pauwel.be/voc/distributionelement#ElectricGenerator-ENGINEGENERATOR
mep:ElectricGenerator-ENGINEGENERATOR rdf:type owl:Class ;
                                      rdfs:subClassOf mep:ElectricGenerator ;
                                      rdfs:comment "electrical generator with a fuel-driven engine, for example a diesel-driven emergency power supply"@en ,
                                                   "electrical generator with a fuel-driven engine, for example a diesel-driven emergency power supply"@en-gb ,
                                                   "http://bsdd.buildingsmart.org/#concept/details/1cgIU0HJT6GuV3i$OWzcqr"@en ;
                                      rdfs:label "Engine Generator"@en ,
                                                 "motorgenerator"@nb-no ;
                                      rdfs:seeAlso ifc:IfcElectricGeneratorEnumType .


###  http://pi.pauwel.be/voc/distributionelement#ElectricGenerator-STANDALONE
mep:ElectricGenerator-STANDALONE rdf:type owl:Class ;
                                 rdfs:subClassOf mep:ElectricGenerator ;
                                 rdfs:comment "electrical generator which does not include its source of kinetic energy, that is, a motor, engine, or turbine are all modeled separately"@en ,
                                              "electrical generator which does not include its source of kinetic energy, that is, a motor, engine, or turbine are all modeled separately"@en-gb ,
                                              "http://bsdd.buildingsmart.org/#concept/details/385E6cNGD9CAcjlAWZNrUW"@en ;
                                 rdfs:label "Standalone Generator"@en ,
                                            "frittstående"@nb-no ;
                                 rdfs:seeAlso ifc:IfcElectricGeneratorEnumType .


###  http://pi.pauwel.be/voc/distributionelement#ElectricMotor
mep:ElectricMotor rdf:type owl:Class ;
                  rdfs:subClassOf mep:EnergyConversionDevice ;
                  rdfs:comment "An engine that is a machine for converting electrical energy into mechanical energy."@en ,
                               "An engine that is a machine for converting electrical energy into mechanical energy."@ifc-2x4 ,
                               "http://bsdd.buildingsmart.org/#concept/details/3_kLW3eI10Xem4Z9zSCTzp"@en ;
                  rdfs:label "Electric Motor"@en ,
                             "Elektromotor"@de-de ,
                             "Moteur électrique"@fr-fr ,
                             "elektrisk motor"@nb-no ,
                             "elektromotor"@nl-nl ;
                  rdfs:seeAlso ifc:IfcElectricMotor .


###  http://pi.pauwel.be/voc/distributionelement#ElectricMotor-DC
mep:ElectricMotor-DC rdf:type owl:Class ;
                     rdfs:subClassOf mep:ElectricMotor ;
                     rdfs:comment "a motor using either generated or rectified Direct Current (DC) power"@en ,
                                  "a motor using either generated or rectified Direct Current (DC) power"@en-gb ,
                                  "http://bsdd.buildingsmart.org/#concept/details/3FK3hjao1DDw14M1qybLxa"@en ;
                     rdfs:label "DC - motor"@nb-no ,
                                "DC-motor"@en ;
                     rdfs:seeAlso ifc:IfcElectricMotorEnumType .


###  http://pi.pauwel.be/voc/distributionelement#ElectricMotor-INDUCTION
mep:ElectricMotor-INDUCTION rdf:type owl:Class ;
                            rdfs:subClassOf mep:ElectricMotor ;
                            rdfs:comment "an alternating current motor in which the primary winding on one member (usually the stator) is connected to the power source and a secondary winding or a squirrel-cage secondary winding on the other member (usually the rotor) carries the induced current. there is no physical electrical connection to the secondary winding, its current is induced"@en ,
                                         "an alternating current motor in which the primary winding on one member (usually the stator) is connected to the power source and a secondary winding or a squirrel-cage secondary winding on the other member (usually the rotor) carries the induced current. there is no physical electrical connection to the secondary winding, its current is induced"@en-gb ,
                                         "http://bsdd.buildingsmart.org/#concept/details/3OYMbkndX6lxYQ5WInnHhX"@en ;
                            rdfs:label "Induction Motor"@en ,
                                       "induksjon"@nb-no ;
                            rdfs:seeAlso ifc:IfcElectricMotorEnumType .


###  http://pi.pauwel.be/voc/distributionelement#ElectricMotor-POLYPHASE
mep:ElectricMotor-POLYPHASE rdf:type owl:Class ;
                            rdfs:subClassOf mep:ElectricMotor ;
                            rdfs:comment "a two or three-phase induction motor in which the windings, one for each phase, are evenly divided by the same number of electrical degrees"@en ,
                                         "a two or three-phase induction motor in which the windings, one for each phase, are evenly divided by the same number of electrical degrees"@en-gb ,
                                         "http://bsdd.buildingsmart.org/#concept/details/1US3A1hwXBIA9FaVqUl3HY"@en ;
                            rdfs:label "Polyphase Motor"@en ,
                                       "flerfasmotor"@nb-no ;
                            rdfs:seeAlso ifc:IfcElectricMotorEnumType .


###  http://pi.pauwel.be/voc/distributionelement#ElectricMotor-RELUCTANCESYNCHRONOUS
mep:ElectricMotor-RELUCTANCESYNCHRONOUS rdf:type owl:Class ;
                                        rdfs:subClassOf mep:ElectricMotor ;
                                        rdfs:comment "http://bsdd.buildingsmart.org/#concept/details/2lD9V5iynEBB3XgItdjfos"@en ;
                                        rdfs:label "Reluctance Synchronous Motor"@en ;
                                        rdfs:seeAlso ifc:IfcElectricMotorEnumType .


###  http://pi.pauwel.be/voc/distributionelement#ElectricMotor-SYNCHRONOUS
mep:ElectricMotor-SYNCHRONOUS rdf:type owl:Class ;
                              rdfs:subClassOf mep:ElectricMotor ;
                              rdfs:comment "a motor that operates at a constant speed up to full load. the rotor speed is equal to the speed of the rotating magnetic field of the stator; there is no slip"@en ,
                                           "a motor that operates at a constant speed up to full load. the rotor speed is equal to the speed of the rotating magnetic field of the stator; there is no slip"@en-gb ,
                                           "http://bsdd.buildingsmart.org/#concept/details/3aYFsz0Ij95vr3j85mOzlh"@en ;
                              rdfs:label "Synchronous Motor"@en ,
                                         "synkromotor"@nb-no ;
                              rdfs:seeAlso ifc:IfcElectricMotorEnumType .


###  http://pi.pauwel.be/voc/distributionelement#ElectricTimeControl
mep:ElectricTimeControl rdf:type owl:Class ;
                        rdfs:subClassOf mep:FlowController ;
                        rdfs:comment "A device that applies control to the provision or flow of electrical energy over time."@en ,
                                     "http://bsdd.buildingsmart.org/#concept/details/34zeeiRU160PRfc1BOv2UT"@en ;
                        rdfs:label "Electric Time Control"@en ,
                                   "Elektrische Zeitsteuerung"@de-de ,
                                   "elektronisk tidskontroll"@nb-no ;
                        rdfs:seeAlso ifc:IfcElectricTimeControl .


###  http://pi.pauwel.be/voc/distributionelement#ElectricTimeControl-RELAY
mep:ElectricTimeControl-RELAY rdf:type owl:Class ;
                              rdfs:subClassOf mep:ElectricTimeControl ;
                              rdfs:comment "electromagnetically operated contactor for making or breaking a control circuit"@en ,
                                           "electromagnetically operated contactor for making or breaking a control circuit"@en-gb ,
                                           "http://bsdd.buildingsmart.org/#concept/details/1uMPSl_pL5eufzS8GVHHU$"@en ;
                              rdfs:label "Relay"@en ,
                                         "relais"@fr-fr ,
                                         "relè"@nb-no ,
                                         "relé"@nb-no ;
                              rdfs:seeAlso ifc:IfcElectricTimeControlEnumType .


###  http://pi.pauwel.be/voc/distributionelement#ElectricTimeControl-TIMECLOCK
mep:ElectricTimeControl-TIMECLOCK rdf:type owl:Class ;
                                  rdfs:subClassOf mep:ElectricTimeControl ;
                                  rdfs:comment "http://bsdd.buildingsmart.org/#concept/details/3_BiobHgL589mZt5gGZ6vc"@en ;
                                  rdfs:label "Time Clock"@en ;
                                  rdfs:seeAlso ifc:IfcElectricTimeControlEnumType .


###  http://pi.pauwel.be/voc/distributionelement#ElectricTimeControl-TIMEDELAY
mep:ElectricTimeControl-TIMEDELAY rdf:type owl:Class ;
                                  rdfs:subClassOf mep:ElectricTimeControl ;
                                  rdfs:comment "http://bsdd.buildingsmart.org/#concept/details/1frllCTITFVANbn$YJ11RW"@en ;
                                  rdfs:label "Time Delay"@en ;
                                  rdfs:seeAlso ifc:IfcElectricTimeControlEnumType .


###  http://pi.pauwel.be/voc/distributionelement#EnergyConversionDevice
mep:EnergyConversionDevice rdf:type owl:Class ;
                           rdfs:subClassOf mep:DistributionFlowElement ;
                           rdfs:comment "http://bsdd.buildingsmart.org/#concept/details/1VQ1GZZDD2pvhjZ8ZKtCoL"@en ,
                                        "the distribution flow element ifcenergyconversiondevice defines the occurrence of a device used to perform energy conversion or heat transfer and typically participates in a flow distribution system. its type is defined by ifcenergyconversiondevicetype or its subtypes."@en ;
                           rdfs:label "Energiewandler"@de-de ,
                                      "Energy Conversion Device"@en ,
                                      "aggregat frys"@nb-no ,
                                      "aggregat kjøl virksomhet"@nb-no ,
                                      "aggregate freezer"@en ,
                                      "aggregate refrigirator industry"@en ,
                                      "dispositif de conversion d'énergie"@fr-fr ,
                                      "kjøleaggregat"@nb-no ;
                           rdfs:seeAlso ifc:IfcEnergyConversionDevice .


###  http://pi.pauwel.be/voc/distributionelement#Engine
mep:Engine rdf:type owl:Class ;
           rdfs:subClassOf mep:EnergyConversionDevice ;
           rdfs:comment "A device that converts fuel into mechanical energy through combustion."@en ,
                        "http://bsdd.buildingsmart.org/#concept/details/2Z1mXqriH13epQNHSH0Q6U"@en ;
           rdfs:label "Engine"@en ,
                      "Moteur"@fr-fr ,
                      "Motor"@de-de ,
                      "motor"@nb-no ;
           rdfs:seeAlso ifc:IfcEngine .


###  http://pi.pauwel.be/voc/distributionelement#Engine-EXTERNALCOMBUSTION
mep:Engine-EXTERNALCOMBUSTION rdf:type owl:Class ;
                              rdfs:subClassOf mep:Engine ;
                              rdfs:comment "combustion is external"@en ,
                                           "combustion is external"@en-gb ,
                                           "http://bsdd.buildingsmart.org/#concept/details/2NLKuMKf91wviDc2F5qWzU"@en ;
                              rdfs:label "External Combustion Engine"@en ,
                                         "utvendig forbrenning"@nb-no ;
                              rdfs:seeAlso ifc:IfcEngineEnumType .


###  http://pi.pauwel.be/voc/distributionelement#Engine-INTERNALCOMBUSTION
mep:Engine-INTERNALCOMBUSTION rdf:type owl:Class ;
                              rdfs:subClassOf mep:Engine ;
                              rdfs:comment "combustion is internal"@en ,
                                           "combustion is internal"@en-gb ,
                                           "http://bsdd.buildingsmart.org/#concept/details/2Tx86TGHX9mfF61hssJ$wH"@en ;
                              rdfs:label "Internal Combustion Engine"@en ,
                                         "forbrenningsmotor"@nb-no ;
                              rdfs:seeAlso ifc:IfcEngineEnumType .


###  http://pi.pauwel.be/voc/distributionelement#EvaporativeCooler
mep:EvaporativeCooler rdf:type owl:Class ;
                      rdfs:subClassOf mep:EnergyConversionDevice ;
                      rdfs:comment "A device that cools air by saturating it with water vapor."@en ,
                                   "http://bsdd.buildingsmart.org/#concept/details/3q9N4QJHXEvB$P7TiIBB3x"@en ;
                      rdfs:label "Evaporative Cooler"@en ,
                                 "Refroidisseur évaporatif"@fr-fr ,
                                 "Verdunstungskühler"@de-de ,
                                 "fordampningskjøler"@nb-no ,
                                 "verdampingskoeler"@nl-nl ;
                      rdfs:seeAlso ifc:IfcEvaporativeCooler .


###  http://pi.pauwel.be/voc/distributionelement#EvaporativeCooler-DIRECTEVAPORATIVEAIRWASHER
mep:EvaporativeCooler-DIRECTEVAPORATIVEAIRWASHER rdf:type owl:Class ;
                                                 rdfs:subClassOf mep:EvaporativeCooler ;
                                                 rdfs:comment "http://bsdd.buildingsmart.org/#concept/details/1mfNeZzsr75wDjPDHJlb4H"@en ;
                                                 rdfs:label "Direct Evaporative Air Washer"@en ,
                                                            "direkte luftfukter - luftvasker"@nb-no ;
                                                 rdfs:seeAlso ifc:IfcEvaporativeCoolerEnumType .


###  http://pi.pauwel.be/voc/distributionelement#EvaporativeCooler-DIRECTEVAPORATIVEPACKAGEDROTARYAIRCOOLER
mep:EvaporativeCooler-DIRECTEVAPORATIVEPACKAGEDROTARYAIRCOOLER rdf:type owl:Class ;
                                                               rdfs:subClassOf mep:EvaporativeCooler ;
                                                               rdfs:comment "http://bsdd.buildingsmart.org/#concept/details/1cj7p5WhDB_xBonDIVd_4z"@en ;
                                                               rdfs:label "Direct Evaporative Packaged Rotary Air Cooler"@en ;
                                                               rdfs:seeAlso ifc:IfcEvaporativeCoolerEnumType .


###  http://pi.pauwel.be/voc/distributionelement#EvaporativeCooler-DIRECTEVAPORATIVERANDOMMEDIAAIRCOOLER
mep:EvaporativeCooler-DIRECTEVAPORATIVERANDOMMEDIAAIRCOOLER rdf:type owl:Class ;
                                                            rdfs:subClassOf mep:EvaporativeCooler ;
                                                            rdfs:comment "http://bsdd.buildingsmart.org/#concept/details/0UORhKPhjCL85YKa2Bnb3r"@en ;
                                                            rdfs:label "Direct Evaporative Random Media Air Cooler"@en ;
                                                            rdfs:seeAlso ifc:IfcEvaporativeCoolerEnumType .


###  http://pi.pauwel.be/voc/distributionelement#EvaporativeCooler-DIRECTEVAPORATIVERIGIDMEDIAAIRCOOLER
mep:EvaporativeCooler-DIRECTEVAPORATIVERIGIDMEDIAAIRCOOLER rdf:type owl:Class ;
                                                           rdfs:subClassOf mep:EvaporativeCooler ;
                                                           rdfs:comment "http://bsdd.buildingsmart.org/#concept/details/0MWgqKd0z5GPNm6aaAnj5C"@en ;
                                                           rdfs:label "Direct Evaporative Rigid Media Air Cooler"@en ;
                                                           rdfs:seeAlso ifc:IfcEvaporativeCoolerEnumType .


###  http://pi.pauwel.be/voc/distributionelement#EvaporativeCooler-DIRECTEVAPORATIVESLINGERSPACKAGEDAIRCOOLER
mep:EvaporativeCooler-DIRECTEVAPORATIVESLINGERSPACKAGEDAIRCOOLER rdf:type owl:Class ;
                                                                 rdfs:subClassOf mep:EvaporativeCooler ;
                                                                 rdfs:comment "http://bsdd.buildingsmart.org/#concept/details/16b3LdCezBDPr$dY5Jspfu"@en ;
                                                                 rdfs:label "Direct Evaporative Slingers Packaged Air Cooler"@en ;
                                                                 rdfs:seeAlso ifc:IfcEvaporativeCoolerEnumType .


###  http://pi.pauwel.be/voc/distributionelement#EvaporativeCooler-INDIRECTDIRECTCOMBINATION
mep:EvaporativeCooler-INDIRECTDIRECTCOMBINATION rdf:type owl:Class ;
                                                rdfs:subClassOf mep:EvaporativeCooler ;
                                                rdfs:comment "http://bsdd.buildingsmart.org/#concept/details/0m3PNQ2HLCZxrflh7tIhW4"@en ;
                                                rdfs:label "Indirect Direct Combination"@en ,
                                                           "kombinasjonskjøler"@nb-no ;
                                                rdfs:seeAlso ifc:IfcEvaporativeCoolerEnumType .


###  http://pi.pauwel.be/voc/distributionelement#EvaporativeCooler-INDIRECTEVAPORATIVECOOLINGTOWERORCOILCOOLER
mep:EvaporativeCooler-INDIRECTEVAPORATIVECOOLINGTOWERORCOILCOOLER rdf:type owl:Class ;
                                                                  rdfs:subClassOf mep:EvaporativeCooler ;
                                                                  rdfs:comment "http://bsdd.buildingsmart.org/#concept/details/2NrTpcYUv9zg$5$$fO_19L"@en ;
                                                                  rdfs:label "Indirect Evaporative Cooling Tower Or Coil Cooler"@en ,
                                                                             "indirekte damp kjøletårn"@nb-no ;
                                                                  rdfs:seeAlso ifc:IfcEvaporativeCoolerEnumType .


###  http://pi.pauwel.be/voc/distributionelement#EvaporativeCooler-INDIRECTEVAPORATIVEPACKAGEAIRCOOLER
mep:EvaporativeCooler-INDIRECTEVAPORATIVEPACKAGEAIRCOOLER rdf:type owl:Class ;
                                                          rdfs:subClassOf mep:EvaporativeCooler ;
                                                          rdfs:comment "http://bsdd.buildingsmart.org/#concept/details/0jmwDswxz4_AQl2__GUqUv"@en ;
                                                          rdfs:label "Indirect Evaporative Package Air Cooler"@en ,
                                                                     "indirekte dampkjøler"@nb-no ;
                                                          rdfs:seeAlso ifc:IfcEvaporativeCoolerEnumType .


###  http://pi.pauwel.be/voc/distributionelement#EvaporativeCooler-INDIRECTEVAPORATIVEWETCOIL
mep:EvaporativeCooler-INDIRECTEVAPORATIVEWETCOIL rdf:type owl:Class ;
                                                 rdfs:subClassOf mep:EvaporativeCooler ;
                                                 rdfs:comment "http://bsdd.buildingsmart.org/#concept/details/1LV$DC3_H2PQ4WPTuDrKrT"@en ;
                                                 rdfs:label "Indirect Evaporative Wet Coil"@en ,
                                                            "indirekte damp coil"@nb-no ;
                                                 rdfs:seeAlso ifc:IfcEvaporativeCoolerEnumType .


###  http://pi.pauwel.be/voc/distributionelement#Evaporator
mep:Evaporator rdf:type owl:Class ;
               rdfs:subClassOf mep:EnergyConversionDevice ;
               rdfs:comment "A liquid refrigerant is vaporized and absorbs heat from the surrounding fluid."@en ,
                            "In heat transfer systems, a evaporator is a device used to turn a liquid into its gaseous form"@en ,
                            "http://bsdd.buildingsmart.org/#concept/details/1b85u16kXAuQVMX36yZmUh"@en ;
               rdfs:label "Evaporateur"@fr-fr ,
                          "Evaporator"@en ,
                          "kjøleelement"@nb-no ,
                          "luftfukter"@nb-no ,
                          "verdamper"@nl-nl ,
                          "verdampfer"@de-de ,
                          "évaporateur"@fr-fr ;
               rdfs:seeAlso ifc:IfcEvaporator .


###  http://pi.pauwel.be/voc/distributionelement#Evaporator-DIRECTEXPANSION
mep:Evaporator-DIRECTEXPANSION rdf:type owl:Class ;
                               rdfs:subClassOf mep:Evaporator ;
                               rdfs:comment "http://bsdd.buildingsmart.org/#concept/details/09VTDOubL8rQM9Zzgh3ZOX"@en ;
                               rdfs:label "Direct Expansion"@en ,
                                          "direkte ekspansjon"@nb-no ;
                               rdfs:seeAlso ifc:IfcEvaporatorEnumType .


###  http://pi.pauwel.be/voc/distributionelement#Evaporator-DIRECTEXPANSIONBRAZEDPLATE
mep:Evaporator-DIRECTEXPANSIONBRAZEDPLATE rdf:type owl:Class ;
                                          rdfs:subClassOf mep:Evaporator ;
                                          rdfs:comment "http://bsdd.buildingsmart.org/#concept/details/1T3UjVbrn8GRRfXuXNLYnr"@en ;
                                          rdfs:label "Direct Expansion Brazed Plate"@en ,
                                                     "direkte ekspansjon loddeplate"@nb-no ;
                                          rdfs:seeAlso ifc:IfcEvaporatorEnumType .


###  http://pi.pauwel.be/voc/distributionelement#Evaporator-DIRECTEXPANSIONSHELLANDTUBE
mep:Evaporator-DIRECTEXPANSIONSHELLANDTUBE rdf:type owl:Class ;
                                           rdfs:subClassOf mep:Evaporator ;
                                           rdfs:comment "http://bsdd.buildingsmart.org/#concept/details/1u9oqdehL1dgBJ6OLyn3QA"@en ;
                                           rdfs:label "Direct Expansion Shell And Tube"@en ,
                                                      "direkte ekspansjon rette rør"@nb-no ;
                                           rdfs:seeAlso ifc:IfcEvaporatorEnumType .


###  http://pi.pauwel.be/voc/distributionelement#Evaporator-DIRECTEXPANSIONTUBEINTUBE
mep:Evaporator-DIRECTEXPANSIONTUBEINTUBE rdf:type owl:Class ;
                                         rdfs:subClassOf mep:Evaporator ;
                                         rdfs:comment "http://bsdd.buildingsmart.org/#concept/details/3sib_FFsX9OPAtp2_avAxn"@en ;
                                         rdfs:label "Direct Expansion Tube In Tube"@en ,
                                                    "direkte ekspansjon rør-i-rør"@nb-no ;
                                         rdfs:seeAlso ifc:IfcEvaporatorEnumType .


###  http://pi.pauwel.be/voc/distributionelement#Evaporator-FLOODEDSHELLANDTUBE
mep:Evaporator-FLOODEDSHELLANDTUBE rdf:type owl:Class ;
                                   rdfs:subClassOf mep:Evaporator ;
                                   rdfs:comment "http://bsdd.buildingsmart.org/#concept/details/0ccrsyQl54TBm8fRTQgQ74"@en ;
                                   rdfs:label "Flooded Shell And Tube"@en ;
                                   rdfs:seeAlso ifc:IfcEvaporatorEnumType .


###  http://pi.pauwel.be/voc/distributionelement#Evaporator-SHELLANDCOIL
mep:Evaporator-SHELLANDCOIL rdf:type owl:Class ;
                            rdfs:subClassOf mep:Evaporator ;
                            rdfs:comment "http://bsdd.buildingsmart.org/#concept/details/30V2jCzRrB$APJOlZf7jhx"@en ;
                            rdfs:label "Shell And Coil"@en ;
                            rdfs:seeAlso ifc:IfcEvaporatorEnumType .


###  http://pi.pauwel.be/voc/distributionelement#Fan
mep:Fan rdf:type owl:Class ;
        rdfs:subClassOf mep:FlowMovingDevice ;
        rdfs:comment "A device which imparts mechanical work on a gas. A typical usage of a fan is to induce airflow in a building services air distribution system."@en ,
                     "A machine for the movement of air that has a rotating impeller, often for cooling."@en ,
                     "An artefact which delivers or exhausts volumes of air or gas at low differential pressure.       "@en ,
                     "funksjonsdel for bevegelse av luft med roterende element, ofte brukt til kjøling."@nb-no ,
                     "http://bsdd.buildingsmart.org/#concept/details/1ugSc0qUCHuO00025QrE$V"@en ;
        rdfs:label "Fan"@en ,
                   "Ventilator"@de-de ,
                   "ventilateur"@fr-fr ,
                   "vifte"@nb-no ;
        rdfs:seeAlso ifc:IfcFan .


###  http://pi.pauwel.be/voc/distributionelement#Fan-CENTRIFUGALAIRFOIL
mep:Fan-CENTRIFUGALAIRFOIL rdf:type owl:Class ;
                           rdfs:subClassOf mep:Fan ;
                           rdfs:comment "http://bsdd.buildingsmart.org/#concept/details/2b2DdpoeD2DebGtqb8$WWB"@en ;
                           rdfs:label "Centrifugal Air Foil"@en ;
                           rdfs:seeAlso ifc:IfcFanEnumType .


###  http://pi.pauwel.be/voc/distributionelement#Fan-CENTRIFUGALBACKWARDINCLINEDCURVED
mep:Fan-CENTRIFUGALBACKWARDINCLINEDCURVED rdf:type owl:Class ;
                                          rdfs:subClassOf mep:Fan ;
                                          rdfs:comment "http://bsdd.buildingsmart.org/#concept/details/2947TJClP4iRuoq1E3mkRW"@en ;
                                          rdfs:label "Centrifugal Backward Inclined Curved Fan"@en ;
                                          rdfs:seeAlso ifc:IfcFanEnumType .


###  http://pi.pauwel.be/voc/distributionelement#Fan-CENTRIFUGALFORWARDCURVED
mep:Fan-CENTRIFUGALFORWARDCURVED rdf:type owl:Class ;
                                 rdfs:subClassOf mep:Fan ;
                                 rdfs:comment "http://bsdd.buildingsmart.org/#concept/details/2BtF98qKP9pAJgsmJrKTcX"@en ;
                                 rdfs:label "Centrifugal Forward Curved Fan"@en ;
                                 rdfs:seeAlso ifc:IfcFanEnumType .


###  http://pi.pauwel.be/voc/distributionelement#Fan-CENTRIFUGALRADIAL
mep:Fan-CENTRIFUGALRADIAL rdf:type owl:Class ;
                          rdfs:subClassOf mep:Fan ;
                          rdfs:comment "http://bsdd.buildingsmart.org/#concept/details/3ZTCLrBaz0NwkdZhJ1jzAB"@en ;
                          rdfs:label "Centrifugal Radial Fan"@en ;
                          rdfs:seeAlso ifc:IfcFanEnumType .


###  http://pi.pauwel.be/voc/distributionelement#Fan-PROPELLORAXIAL
mep:Fan-PROPELLORAXIAL rdf:type owl:Class ;
                       rdfs:subClassOf mep:Fan ;
                       rdfs:comment "http://bsdd.buildingsmart.org/#concept/details/0B7IEewCf7DPbZs58QORZ_"@en ;
                       rdfs:label "Propellor Axial Fan"@en ;
                       rdfs:seeAlso ifc:IfcFanEnumType .


###  http://pi.pauwel.be/voc/distributionelement#Fan-TUBEAXIAL
mep:Fan-TUBEAXIAL rdf:type owl:Class ;
                  rdfs:subClassOf mep:Fan ;
                  rdfs:comment "air flows through the impeller axially with reduced tip clearance and operating at higher tip speeds"@en ,
                               "http://bsdd.buildingsmart.org/#concept/details/0uYC2U15n0ggOtHNsP3kmN"@en ;
                  rdfs:label "Tube Axial Fan"@en ,
                             "tube aksialvifte"@nb-no ;
                  rdfs:seeAlso ifc:IfcFanEnumType .


###  http://pi.pauwel.be/voc/distributionelement#Fan-VANEAXIAL
mep:Fan-VANEAXIAL rdf:type owl:Class ;
                  rdfs:subClassOf mep:Fan ;
                  rdfs:comment "air flows through the impeller axially with guide vanes and reduced running blade tip clearance"@en ,
                               "air flows through the impeller axially with guide vanes and reduced running blade tip clearance"@en-gb ,
                               "http://bsdd.buildingsmart.org/#concept/details/2W_hdCD6D3DPaj$HRNjU0Z"@en ;
                  rdfs:label "Vane Axial Fan"@en ,
                             "lamellaksial vifte"@nb-no ;
                  rdfs:seeAlso ifc:IfcFanEnumType .


###  http://pi.pauwel.be/voc/distributionelement#Filter
mep:Filter rdf:type owl:Class ;
           rdfs:subClassOf mep:FlowTreatmentDevice ;
           rdfs:comment "An apparatus used to remove particulate or gaseous matter from fluids and gases"@en ,
                        "http://bsdd.buildingsmart.org/#concept/details/07moCBVkH3OhoQDperZAGA"@en ;
           rdfs:label "Filter"@en ,
                      "filtre"@fr-fr ;
           rdfs:seeAlso ifc:IfcFilter .


###  http://pi.pauwel.be/voc/distributionelement#Filter-AIRPARTICLEFILTER
mep:Filter-AIRPARTICLEFILTER rdf:type owl:Class ;
                             rdfs:subClassOf mep:Filter ;
                             rdfs:comment "http://bsdd.buildingsmart.org/#concept/details/2ha4cuVrn2CO6DtVG5m_2l"@en ;
                             rdfs:label "Air Particle Filter"@en ,
                                        "støvutskiller (filter)"@nb-no ;
                             rdfs:seeAlso ifc:IfcFilterEnumType .


###  http://pi.pauwel.be/voc/distributionelement#Filter-COMPRESSEDAIRFILTER
mep:Filter-COMPRESSEDAIRFILTER rdf:type owl:Class ;
                               rdfs:subClassOf mep:Filter ;
                               rdfs:comment "http://bsdd.buildingsmart.org/#concept/details/3eXdymzEL2WwWgDskL3E7I"@en ;
                               rdfs:label "Compressed Air Filter"@en ;
                               rdfs:seeAlso ifc:IfcFilterEnumType .


###  http://pi.pauwel.be/voc/distributionelement#Filter-ODORFILTER
mep:Filter-ODORFILTER rdf:type owl:Class ;
                      rdfs:subClassOf mep:Filter ;
                      rdfs:comment "http://bsdd.buildingsmart.org/#concept/details/0Nh$mYaRT13xMPbS$8vqwW"@en ;
                      rdfs:label "Odor Filter"@en ;
                      rdfs:seeAlso ifc:IfcFilterEnumType .


###  http://pi.pauwel.be/voc/distributionelement#Filter-OILFILTER
mep:Filter-OILFILTER rdf:type owl:Class ;
                     rdfs:subClassOf mep:Filter ;
                     rdfs:comment "a filter used to remove particulates from oil"@en ,
                                  "a filter used to remove particulates from oil"@en-gb ,
                                  "http://bsdd.buildingsmart.org/#concept/details/0HemsvirL2luh4LogPKmfT"@en ;
                     rdfs:label "Oil Filter"@en ,
                                "oljefilter"@nb-no ;
                     rdfs:seeAlso ifc:IfcFilterEnumType .


###  http://pi.pauwel.be/voc/distributionelement#Filter-STRAINER
mep:Filter-STRAINER rdf:type owl:Class ;
                    rdfs:subClassOf mep:Filter ;
                    rdfs:comment "A fitting for preventing that leaves enters the down-pipe"@en ,
                                 "En innretning som hindrer løv og annet nedfall i å komme inn i nedløpsrøret"@nb-no ,
                                 "device that prevents solid matter from entering a pipe, pump, valve or meter"@en ,
                                 "http://bsdd.buildingsmart.org/#concept/details/30aQppcM58MR6pxe6iVccR"@en ;
                    rdfs:label "Siebe"@de-de ,
                               "Strainer"@en ,
                               "filtre"@fr-fr ,
                               "løvrist"@nb-no ,
                               "sil"@nb-no ;
                    rdfs:seeAlso ifc:IfcFilterEnumType .


###  http://pi.pauwel.be/voc/distributionelement#Filter-WATERFILTER
mep:Filter-WATERFILTER rdf:type owl:Class ;
                       rdfs:subClassOf mep:Filter ;
                       rdfs:comment "http://bsdd.buildingsmart.org/#concept/details/3IqBAp0Tv5HxjI8BQo7oFW"@en ;
                       rdfs:label "Water Filter"@en ,
                                  "vannfilter"@nb-no ;
                       rdfs:seeAlso ifc:IfcFilterEnumType .


###  http://pi.pauwel.be/voc/distributionelement#FireSuppressionTerminal
mep:FireSuppressionTerminal rdf:type owl:Class ;
                            rdfs:subClassOf mep:FlowTerminal ;
                            rdfs:comment """A suppression terminal has the purpose of delivering a fluid (gas or liquid) that will suppress a fire.
Provides for all forms of sprinkler, spreader and other form of terminal that is connected to a pipework system and intended to act in the role of suppressing a fire."""@en ,
                                         "http://bsdd.buildingsmart.org/#concept/details/1P1aiBVvPDjPVBP4TWbJw6"@en ;
                            rdfs:label "Appareil terminal d'extinction d'incendie"@fr-fr ,
                                       "Feuerlöscheinrichtung"@de-de ,
                                       "Fire Suppression Terminal"@en ,
                                       "brannundertrykkelsessystem"@nb-no ;
                            rdfs:seeAlso ifc:IfcFireSuppressionTerminal .


###  http://pi.pauwel.be/voc/distributionelement#FireSuppressionTerminal-BREECHINGINLET
mep:FireSuppressionTerminal-BREECHINGINLET rdf:type owl:Class ;
                                           rdfs:subClassOf mep:FireSuppressionTerminal ;
                                           rdfs:comment "http://bsdd.buildingsmart.org/#concept/details/00IdsJ7iT7Nx$veMrXzcqM"@en ;
                                           rdfs:label "Breeching Inlet"@en ;
                                           rdfs:seeAlso ifc:IfcFireSuppressionTerminalEnumType .


###  http://pi.pauwel.be/voc/distributionelement#FireSuppressionTerminal-FIREHYDRANT
mep:FireSuppressionTerminal-FIREHYDRANT rdf:type owl:Class ;
                                        rdfs:subClassOf mep:FireSuppressionTerminal ;
                                        rdfs:comment "http://bsdd.buildingsmart.org/#concept/details/1esoBNGDb2wOo3IcBnG9Zv"@en ;
                                        rdfs:label "Fire Hydrant"@en ;
                                        rdfs:seeAlso ifc:IfcFireSuppressionTerminalEnumType .


###  http://pi.pauwel.be/voc/distributionelement#FireSuppressionTerminal-HOSEREEL
mep:FireSuppressionTerminal-HOSEREEL rdf:type owl:Class ;
                                     rdfs:subClassOf mep:FireSuppressionTerminal ;
                                     rdfs:comment "http://bsdd.buildingsmart.org/#concept/details/3BjPDggX5A1uWncjNaSpTp"@en ;
                                     rdfs:label "Hosereel"@en ;
                                     rdfs:seeAlso ifc:IfcFireSuppressionTerminalEnumType .


###  http://pi.pauwel.be/voc/distributionelement#FireSuppressionTerminal-SPRINKLER
mep:FireSuppressionTerminal-SPRINKLER rdf:type owl:Class ;
                                      rdfs:subClassOf mep:FireSuppressionTerminal ;
                                      rdfs:comment "http://bsdd.buildingsmart.org/#concept/details/09wWrp7P91aASjo0_dry01"@en ,
                                                   "nozzle with a thermally sensitive sealing device which opens to discharge water for fire fighting"@en ;
                                      rdfs:label "Sprinkler"@en ,
                                                 "Sprinkler"@nl-nl ,
                                                 "fire sprinkler"@en ,
                                                 "sprinkler"@nb-no ;
                                      rdfs:seeAlso ifc:IfcFireSuppressionTerminalEnumType .


###  http://pi.pauwel.be/voc/distributionelement#FireSuppressionTerminal-SPRINKLERDEFLECTOR
mep:FireSuppressionTerminal-SPRINKLERDEFLECTOR rdf:type owl:Class ;
                                               rdfs:subClassOf mep:FireSuppressionTerminal ;
                                               rdfs:comment "http://bsdd.buildingsmart.org/#concept/details/2LU6yVzZT7U8X4VneBA$Bh"@en ;
                                               rdfs:label "Sprinkler Deflector"@en ;
                                               rdfs:seeAlso ifc:IfcFireSuppressionTerminalEnumType .


###  http://pi.pauwel.be/voc/distributionelement#FlowController
mep:FlowController rdf:type owl:Class ;
                   rdfs:subClassOf mep:DistributionFlowElement ;
                   rdfs:comment "http://bsdd.buildingsmart.org/#concept/details/1iDky6Xqz0NhbMNjWBjWCy"@en ,
                                "the distribution flow element ifcflowcontroller defines the occurrence of elements of a distribution system that are used to regulate flow through a distribution system. examples include dampers, valves, switches, and relays. its type is defined by ifcflowcontrollertype or subtypes."@en ;
                   rdfs:label "Flow Controller"@en ,
                              "Regler (allgemein)"@de-de ,
                              "contrôleur de débit"@fr-fr ,
                              "vannmengderegulator"@nb-no ;
                   rdfs:seeAlso ifc:IfcFlowController .


###  http://pi.pauwel.be/voc/distributionelement#FlowFitting
mep:FlowFitting rdf:type owl:Class ;
                rdfs:subClassOf mep:DistributionFlowElement ;
                rdfs:comment "Elkraftfordeling til driftstekniske installasjoner"@nb-no ,
                             "Elkraftfordeling til virksomhet"@nb-no ,
                             "http://bsdd.buildingsmart.org/#concept/details/0QXNqIaY58ARlIeBKvxECI"@en ,
                             "the distribution flow element ifcflowfitting defines the occurrence of a junction or transition in a flow distribution system, such as an elbow or tee. its type is defined by ifcflowfittingtype or its subtypes."@en ;
                rdfs:label "Flow Fitting"@en ,
                           "Verbinder / Formstück (allgemein)"@de-de ,
                           "koblinger driftsteknisk"@nb-no ,
                           "koblinger virksomhet"@nb-no ,
                           "raccord d'installation fluides"@fr-fr ;
                rdfs:seeAlso ifc:IfcFlowFitting .


###  http://pi.pauwel.be/voc/distributionelement#FlowInstrument
mep:FlowInstrument rdf:type owl:Class ;
                   rdfs:subClassOf mep:DistributionControlElement ;
                   rdfs:comment """An instrument reads and displays the flow value of a particular property of a system at a point, or displays the difference in the value of a property between two points.
Typically for the purpose of determining the value of the property at a point in time. Includes  forms of mechanical flow instrument (thermometers, pressure gauges etc.) and electrical flow instruments (ammeters, voltmeters etc.)"""@en ,
                                "http://bsdd.buildingsmart.org/#concept/details/11jUOktIH3ZBjsCen5K$76"@en ;
                   rdfs:label "Flow Instrument"@en ,
                              "Instrument d'installation fluides"@fr-fr ,
                              "Messinstrument (allgemein)"@de-de ,
                              "strømningsinstrument"@nb-no ;
                   rdfs:seeAlso ifc:IfcFlowInstrument .


###  http://pi.pauwel.be/voc/distributionelement#FlowInstrument-AMMETER
mep:FlowInstrument-AMMETER rdf:type owl:Class ;
                           rdfs:subClassOf mep:FlowInstrument ;
                           rdfs:comment "a device that reads and displays the current flow in a circuit"@en ,
                                        "a device that reads and displays the current flow in a circuit"@en-gb ,
                                        "http://bsdd.buildingsmart.org/#concept/details/1ZnXtG18TFxghzaROUOOEo"@en ;
                           rdfs:label "AMMeter"@en ,
                                      "amperemeter"@nb-no ;
                           rdfs:seeAlso ifc:IfcFlowInstrumentEnumType .


###  http://pi.pauwel.be/voc/distributionelement#FlowInstrument-FREQUENCYMETER
mep:FlowInstrument-FREQUENCYMETER rdf:type owl:Class ;
                                  rdfs:subClassOf mep:FlowInstrument ;
                                  rdfs:comment "a device that reads and displays the electrical frequency of an alternating current circuit."@en ,
                                               "http://bsdd.buildingsmart.org/#concept/details/01E8ZEHkn6nuRHiPM5blVG"@en ;
                                  rdfs:label "Frequency Meter"@en ,
                                             "frekvensmåler"@nb-no ;
                                  rdfs:seeAlso ifc:IfcFlowInstrumentEnumType .


###  http://pi.pauwel.be/voc/distributionelement#FlowInstrument-PHASEANGLEMETER
mep:FlowInstrument-PHASEANGLEMETER rdf:type owl:Class ;
                                   rdfs:subClassOf mep:FlowInstrument ;
                                   rdfs:comment "a device that reads and displays the phase angle of a phase in a polyphase electrical circuit"@en ,
                                                "a device that reads and displays the phase angle of a phase in a polyphase electrical circuit"@en-gb ,
                                                "http://bsdd.buildingsmart.org/#concept/details/3Gf7_xpUn18gOIu3amQEQH"@en ;
                                   rdfs:label "Phase-Angle Meter"@en ,
                                              "fasevinkelmåler"@nb-no ;
                                   rdfs:seeAlso ifc:IfcFlowInstrumentEnumType .


###  http://pi.pauwel.be/voc/distributionelement#FlowInstrument-POWERFACTORMETER
mep:FlowInstrument-POWERFACTORMETER rdf:type owl:Class ;
                                    rdfs:subClassOf mep:FlowInstrument ;
                                    rdfs:comment "http://bsdd.buildingsmart.org/#concept/details/1P$PbnF35AFwKgPqjZPzC0"@en ;
                                    rdfs:label "Power Factor Meter"@en ;
                                    rdfs:seeAlso ifc:IfcFlowInstrumentEnumType .


###  http://pi.pauwel.be/voc/distributionelement#FlowInstrument-PRESSUREGAUGE
mep:FlowInstrument-PRESSUREGAUGE rdf:type owl:Class ;
                                 rdfs:subClassOf mep:FlowInstrument ;
                                 rdfs:comment "http://bsdd.buildingsmart.org/#concept/details/0OE6$aHKjCBBgczwu$WIy0"@en ;
                                 rdfs:label "Pressure Gauge"@en ;
                                 rdfs:seeAlso ifc:IfcFlowInstrumentEnumType .


###  http://pi.pauwel.be/voc/distributionelement#FlowInstrument-THERMOMETER
mep:FlowInstrument-THERMOMETER rdf:type owl:Class ;
                               rdfs:subClassOf mep:FlowInstrument ;
                               rdfs:comment "Måler og viser temperatur analogt"@nb-no ,
                                            "a device that reads and displays a temperature value at a point"@en ,
                                            "a device that reads and displays a temperature value at a point"@en-gb ,
                                            "http://bsdd.buildingsmart.org/#concept/details/3vHXe6oT0Hsm00051Mm008"@en ;
                               rdfs:label "Temperaturmeßgerät"@de-de ,
                                          "Thermometer"@en ,
                                          "Thermometer"@nl-nl ,
                                          "termometer"@nb-no ,
                                          "thermomètre"@fr-fr ;
                               rdfs:seeAlso ifc:IfcFlowInstrumentEnumType .


###  http://pi.pauwel.be/voc/distributionelement#FlowInstrument-VOLTMETER_PEAK
mep:FlowInstrument-VOLTMETER_PEAK rdf:type owl:Class ;
                                  rdfs:subClassOf mep:FlowInstrument ;
                                  rdfs:comment "a device that reads and displays the peak voltage in an electrical circuit"@en ,
                                               "a device that reads and displays the peak voltage in an electrical circuit"@en-gb ,
                                               "http://bsdd.buildingsmart.org/#concept/details/3HJn6Sn$TBNQmm9Dwrzknj"@en ;
                                  rdfs:label "Peak Volt Meter"@en ,
                                             "toppverdi voltmeter"@nb-no ;
                                  rdfs:seeAlso ifc:IfcFlowInstrumentEnumType .


###  http://pi.pauwel.be/voc/distributionelement#FlowInstrument-VOLTMETER_RMS
mep:FlowInstrument-VOLTMETER_RMS rdf:type owl:Class ;
                                 rdfs:subClassOf mep:FlowInstrument ;
                                 rdfs:comment "a device that reads and displays the RMS (mean) voltage in an electrical circuit"@en ,
                                              "a device that reads and displays the RMS (mean) voltage in an electrical circuit"@en-gb ,
                                              "http://bsdd.buildingsmart.org/#concept/details/2rsw3JDZn4yRFLbTU1Aq7v"@en ;
                                 rdfs:label "RMS Volt Meter"@en ,
                                            "rms voltmeter"@nb-no ;
                                 rdfs:seeAlso ifc:IfcFlowInstrumentEnumType .


###  http://pi.pauwel.be/voc/distributionelement#FlowMeter
mep:FlowMeter rdf:type owl:Class ;
              rdfs:subClassOf mep:FlowController ;
              rdfs:comment "A device that is used to measure the flow rate in a system."@en ,
                           "http://bsdd.buildingsmart.org/#concept/details/3lICO0qUSHuO00025QrE$V"@en ;
              rdfs:label "Appareil de mesure de débit"@fr-fr ,
                         "Flow Meter"@en ,
                         "Zähler (allgemein)"@de-de ,
                         "flytmåler"@nb-no ,
                         "vannmengdemåler"@nb-no ;
              rdfs:seeAlso ifc:IfcFlowMeter .


###  http://pi.pauwel.be/voc/distributionelement#FlowMeter-ENERGYMETER
mep:FlowMeter-ENERGYMETER rdf:type owl:Class ;
                          rdfs:subClassOf mep:FlowMeter ;
                          rdfs:comment "device that measures, indicates and sometimes records, the energy usage in a system"@en ,
                                       "device that measures, indicates and sometimes records, the energy usage in a system"@en-gb ,
                                       "http://bsdd.buildingsmart.org/#concept/details/0dqsT4P2DFmvAItnTOiex9"@en ;
                          rdfs:label "Energy Meter"@en ,
                                     "energimåler"@nb-no ;
                          rdfs:seeAlso ifc:IfcFlowMeterEnumType .


###  http://pi.pauwel.be/voc/distributionelement#FlowMeter-GASMETER
mep:FlowMeter-GASMETER rdf:type owl:Class ;
                       rdfs:subClassOf mep:FlowMeter ;
                       rdfs:comment "device that measures, indicates and sometimes records, the volume of gas that passes through it without interrupting the flow"@en ,
                                    "device that measures, indicates and sometimes records, the volume of gas that passes through it without interrupting the flow"@en-gb ,
                                    "http://bsdd.buildingsmart.org/#concept/details/2d9Kt_TA9Dww_aaJ0$7nqk"@en ;
                       rdfs:label "Gas Meter"@en ,
                                  "gassmåler"@nb-no ;
                       rdfs:seeAlso ifc:IfcFlowMeterEnumType .


###  http://pi.pauwel.be/voc/distributionelement#FlowMeter-OILMETER
mep:FlowMeter-OILMETER rdf:type owl:Class ;
                       rdfs:subClassOf mep:FlowMeter ;
                       rdfs:comment "http://bsdd.buildingsmart.org/#concept/details/2HD3O5A6XAmQiJv54wilAx"@en ,
                                    "not available"@en ;
                       rdfs:label "Oil Meter"@en ,
                                  "oljemåler"@nb-no ;
                       rdfs:seeAlso ifc:IfcFlowMeterEnumType .


###  http://pi.pauwel.be/voc/distributionelement#FlowMeter-WATERMETER
mep:FlowMeter-WATERMETER rdf:type owl:Class ;
                         rdfs:subClassOf mep:FlowMeter ;
                         rdfs:comment "http://bsdd.buildingsmart.org/#concept/details/2bpgnuN4XCdOPs0pKS1wP1"@en ;
                         rdfs:label "Water Meter"@en ;
                         rdfs:seeAlso ifc:IfcFlowMeterEnumType .


###  http://pi.pauwel.be/voc/distributionelement#FlowMovingDevice
mep:FlowMovingDevice rdf:type owl:Class ;
                     rdfs:subClassOf mep:DistributionFlowElement ;
                     rdfs:comment "http://bsdd.buildingsmart.org/#concept/details/1z188Qjir3JArIaN1C$Jlp"@en ,
                                  "the distribution flow element ifcflowmovingdevice defines the occurrence of an apparatus used to distribute, circulate or perform conveyance of fluids, including liquids and gases (such as a pump or fan), and typically participates in a flow distribution system. its type is defined by ifcflowmovingdevicetype or its subtypes."@en ;
                     rdfs:label "Flow Moving Device"@en ,
                                "Strömungsmaschine (allgemein)"@de-de ,
                                "dispositif de circulation de fluide"@fr-fr ,
                                "flow moving device type"@en ,
                                "strømførende enhet"@nb-no ;
                     rdfs:seeAlso ifc:IfcFlowMovingDevice .


###  http://pi.pauwel.be/voc/distributionelement#FlowSegment
mep:FlowSegment rdf:type owl:Class ;
                rdfs:subClassOf mep:DistributionFlowElement ;
                rdfs:comment "http://bsdd.buildingsmart.org/#concept/details/3pgLxEkmTCmg6JWI8OZE4J"@en ,
                             "the distribution flow element ifcflowsegment defines the occurrence of a segment of a flow distribution system. the ifcflowsegment defines a particular occurrence of a segment inserted in the spatial context of a project. the parameters defining the type of the segment and/or its shape are defined by the ifcflowsegmenttype, which is related by the inverse relationship isdefinedby pointing to ifcreldefinesbytype."@en ;
                rdfs:label "Flow Segment"@en ,
                           "Verteiler (allgemein)"@de-de ,
                           "strømførende segment"@nb-no ,
                           "tronçon d'installation fluides"@fr-fr ;
                rdfs:seeAlso ifc:IfcFlowSegment .


###  http://pi.pauwel.be/voc/distributionelement#FlowStorageDevice
mep:FlowStorageDevice rdf:type owl:Class ;
                      rdfs:subClassOf mep:DistributionFlowElement ;
                      rdfs:comment "http://bsdd.buildingsmart.org/#concept/details/32pa_OQBP6exzNXNT$7YTr"@en ,
                                   "the distribution flow element ifcflowstoragedevice defines the occurrence of a device that participates in a distribution system and is used for temporary storage (such as a tank). its type is defined by ifcflowstoragedevicetype or its subtypes."@en ;
                      rdfs:label "Flow Storage Device"@en ,
                                 "Speicher (allgemein)"@de-de ,
                                 "appareil de stockage de fluide"@fr-fr ,
                                 "strømlagrende enhet"@nb-no ;
                      rdfs:seeAlso ifc:IfcFlowStorageDevice .


###  http://pi.pauwel.be/voc/distributionelement#FlowTerminal
mep:FlowTerminal rdf:type owl:Class ;
                 rdfs:subClassOf mep:DistributionFlowElement ;
                 rdfs:comment "http://bsdd.buildingsmart.org/#concept/details/2zsZIJsQfBq98RWGNFmix9"@en ,
                              "the distribution flow element ifcflowterminal defines the occurrence of a permanently attached element that acts as a terminus or beginning of a distribution system (such as an air outlet, drain, water closet or sink). a terminal is typically a point at which a system interfaces with an external environment. its type is defined by ifcflowterminaltype or its subtypes."@en ;
                 rdfs:label "Endgerät (allgemein)"@de-de ,
                            "Flow Terminal"@en ,
                            "elément terminal d'installation fluides"@fr-fr ,
                            "strømterminal"@nb-no ;
                 rdfs:seeAlso ifc:IfcFlowTerminal .


###  http://pi.pauwel.be/voc/distributionelement#FlowTreatmentDevice
mep:FlowTreatmentDevice rdf:type owl:Class ;
                        rdfs:subClassOf mep:DistributionFlowElement ;
                        rdfs:comment "http://bsdd.buildingsmart.org/#concept/details/358GrBQjP36vPq9aYtgYQa"@en ,
                                     "the distribution flow element ifcflowtreatmentdevice defines the occurrence of a device typically used to remove unwanted matter from a fluid, either liquid or gas, and typically participates in a flow distribution system. its type is defined by ifcflowtreatmentdevicetype or its subtypes."@en ;
                        rdfs:label "Filter"@de-de ,
                                   "Flow Treatment Device"@en ,
                                   "appareil de traitement de fluide"@fr-fr ,
                                   "strømbehandlingsenhet"@nb-no ;
                        rdfs:seeAlso ifc:IfcFlowTreatmentDevice .


###  http://pi.pauwel.be/voc/distributionelement#HeatExchanger
mep:HeatExchanger rdf:type owl:Class ;
                  rdfs:subClassOf mep:EnergyConversionDevice ;
                  rdfs:comment "A device used to provide heat transfer between non-mixing media such as plate and shell and tube heat exchangers. Commonly used on water-side distribution systems to recover energy from a liquid to another liquid (typically water-based)."@en ,
                               "An artefact intended for transferring thermal energy from one fluid to another.        "@en ,
                               "http://bsdd.buildingsmart.org/#concept/details/3WpPiXIp5Bf89w8w0QL9_r"@en ;
                  rdfs:label "Echangeur de chaleur"@fr-fr ,
                             "Heat Exchanger"@en ,
                             "Varmeveksler"@da ,
                             "Warmtewisselaar"@nl ,
                             "Warmtewisselaar"@nl-nl ,
                             "Wärmetauscher"@de-de ,
                             "varmeveksler"@nb-no ;
                  rdfs:seeAlso ifc:IfcHeatExchanger .


###  http://pi.pauwel.be/voc/distributionelement#HeatExchanger-PLATE
mep:HeatExchanger-PLATE rdf:type owl:Class ;
                        rdfs:subClassOf mep:HeatExchanger ;
                        rdfs:comment "http://bsdd.buildingsmart.org/#concept/details/2pALi8Jfv7Se_pR4H3dTaH"@en ;
                        rdfs:label "Plate Heat Exchanger"@en ,
                                   "platevarmeveksler"@nb-no ;
                        rdfs:seeAlso ifc:IfcHeatExchangerEnumType .


###  http://pi.pauwel.be/voc/distributionelement#HeatExchanger-SHELLANDTUBE
mep:HeatExchanger-SHELLANDTUBE rdf:type owl:Class ;
                               rdfs:subClassOf mep:HeatExchanger ;
                               rdfs:comment "http://bsdd.buildingsmart.org/#concept/details/1h3yHT$MPE0BoJuFFtf4$5"@en ;
                               rdfs:label "Shell And Tube Heat Exchanger"@en ,
                                          "varmeveksler med rette rør"@nb-no ;
                               rdfs:seeAlso ifc:IfcHeatExchangerEnumType .


###  http://pi.pauwel.be/voc/distributionelement#Humidifier
mep:Humidifier rdf:type owl:Class ;
               rdfs:subClassOf mep:EnergyConversionDevice ;
               rdfs:comment "A device that adds moisture into the air."@en ,
                            "http://bsdd.buildingsmart.org/#concept/details/1FcXNG5qj2GQITbOwXrOIF"@en ;
               rdfs:label "Befeuchter"@de-de ,
                          "Befugter"@da ,
                          "Humidifier"@en ,
                          "humidificateur"@fr-fr ,
                          "luftfukter"@nb-no ;
               rdfs:seeAlso ifc:IfcHumidifier .


###  http://pi.pauwel.be/voc/distributionelement#Humidifier-ADIABATICAIRWASHER
mep:Humidifier-ADIABATICAIRWASHER rdf:type owl:Class ;
                                  rdfs:subClassOf mep:Humidifier ;
                                  rdfs:comment "http://bsdd.buildingsmart.org/#concept/details/2MNV0vgOv328qlczPJ03OC"@en ;
                                  rdfs:label "Adiabatic Air Washer"@en ,
                                             "adiabatisk luftvasker"@nb-no ;
                                  rdfs:seeAlso ifc:IfcHumidifierEnumType .


###  http://pi.pauwel.be/voc/distributionelement#Humidifier-ADIABATICATOMIZING
mep:Humidifier-ADIABATICATOMIZING rdf:type owl:Class ;
                                  rdfs:subClassOf mep:Humidifier ;
                                  rdfs:comment "http://bsdd.buildingsmart.org/#concept/details/1K4HZEHEv1wQ19Vzk48Sgn"@en ,
                                               "water vapor is added into the airstream through adiabatic evaporation using an atomizing element"@en ,
                                               "water vapor is added into the airstream through adiabatic evaporation using an atomizing element"@en-gb ;
                                  rdfs:label "Adiabatic Atomizing"@en ,
                                             "adiabatisk forstøver"@nb-no ;
                                  rdfs:seeAlso ifc:IfcHumidifierEnumType .


###  http://pi.pauwel.be/voc/distributionelement#Humidifier-ADIABATICCOMPRESSEDAIRNOZZLE
mep:Humidifier-ADIABATICCOMPRESSEDAIRNOZZLE rdf:type owl:Class ;
                                            rdfs:subClassOf mep:Humidifier ;
                                            rdfs:comment "http://bsdd.buildingsmart.org/#concept/details/2HCfOW4In2BREPSqe5Ms$p"@en ,
                                                         "water vapor is added into the airstream through adiabatic evaporation using a compressed air nozzle"@en ,
                                                         "water vapor is added into the airstream through adiabatic evaporation using a compressed air nozzle"@en-gb ;
                                            rdfs:label "Adiabatic Compressed Air Nozzle"@en ,
                                                       "adiabatisk trykkluftdyse"@nb-no ;
                                            rdfs:seeAlso ifc:IfcHumidifierEnumType .


###  http://pi.pauwel.be/voc/distributionelement#Humidifier-ADIABATICPAN
mep:Humidifier-ADIABATICPAN rdf:type owl:Class ;
                            rdfs:subClassOf mep:Humidifier ;
                            rdfs:comment "http://bsdd.buildingsmart.org/#concept/details/3d9dTNKyPFRRor9abHmtji"@en ;
                            rdfs:label "Adiabatic Pan"@en ,
                                       "adiabatisk kar"@nb-no ;
                            rdfs:seeAlso ifc:IfcHumidifierEnumType .


###  http://pi.pauwel.be/voc/distributionelement#Humidifier-ADIABATICRIGIDMEDIA
mep:Humidifier-ADIABATICRIGIDMEDIA rdf:type owl:Class ;
                                   rdfs:subClassOf mep:Humidifier ;
                                   rdfs:comment "http://bsdd.buildingsmart.org/#concept/details/0RD4N$yNr7jQPEzfNuNDtm"@en ,
                                                "water vapor is added into the airstream through adiabatic evaporation using a rigid media"@en ,
                                                "water vapor is added into the airstream through adiabatic evaporation using a rigid media"@en-gb ;
                                   rdfs:label "Adiabatic Rigid Media"@en ,
                                              "adiabatisk rigid medium"@nb-no ;
                                   rdfs:seeAlso ifc:IfcHumidifierEnumType .


###  http://pi.pauwel.be/voc/distributionelement#Humidifier-ADIABATICULTRASONIC
mep:Humidifier-ADIABATICULTRASONIC rdf:type owl:Class ;
                                   rdfs:subClassOf mep:Humidifier ;
                                   rdfs:comment "http://bsdd.buildingsmart.org/#concept/details/0LHdcNpKzA9fe_4pzr59WD"@en ,
                                                "water vapor is added into the airstream through adiabatic evaporation using an ultrasonic element"@en ,
                                                "water vapor is added into the airstream through adiabatic evaporation using an ultrasonic element"@en-gb ;
                                   rdfs:label "Adiabatic Ultra Sonic"@en ,
                                              "adiabatisk ultralyd"@nb-no ;
                                   rdfs:seeAlso ifc:IfcHumidifierEnumType .


###  http://pi.pauwel.be/voc/distributionelement#Humidifier-ADIABATICWETTEDELEMENT
mep:Humidifier-ADIABATICWETTEDELEMENT rdf:type owl:Class ;
                                      rdfs:subClassOf mep:Humidifier ;
                                      rdfs:comment "http://bsdd.buildingsmart.org/#concept/details/3K$6EMdYfCzPmmFTgegHDy"@en ;
                                      rdfs:label "Adiabatic Wetted Element"@en ,
                                                 "adiabatisk våtelement"@nb-no ;
                                      rdfs:seeAlso ifc:IfcHumidifierEnumType .


###  http://pi.pauwel.be/voc/distributionelement#Humidifier-ASSISTEDBUTANE
mep:Humidifier-ASSISTEDBUTANE rdf:type owl:Class ;
                              rdfs:subClassOf mep:Humidifier ;
                              rdfs:comment "http://bsdd.buildingsmart.org/#concept/details/2VKdEEkCn1ghIvaWPax9j3"@en ,
                                           "water vapor is added into the airstream through water heated evaporation using a butane heater"@en ,
                                           "water vapor is added into the airstream through water heated evaporation using a butane heater"@en-gb ;
                              rdfs:label "Assisted Butane"@en ,
                                         "assistert butan"@nb-no ;
                              rdfs:seeAlso ifc:IfcHumidifierEnumType .


###  http://pi.pauwel.be/voc/distributionelement#Humidifier-ASSISTEDELECTRIC
mep:Humidifier-ASSISTEDELECTRIC rdf:type owl:Class ;
                                rdfs:subClassOf mep:Humidifier ;
                                rdfs:comment "http://bsdd.buildingsmart.org/#concept/details/157UtcquX8d8khI$Nxg6Dg"@en ,
                                             "water vapor is added into the airstream through water heated evaporation using an electric heater"@en ,
                                             "water vapor is added into the airstream through water heated evaporation using an electric heater"@en-gb ;
                                rdfs:label "Assisted Electric"@en ,
                                           "assistert elektrisitet"@nb-no ;
                                rdfs:seeAlso ifc:IfcHumidifierEnumType .


###  http://pi.pauwel.be/voc/distributionelement#Humidifier-ASSISTEDNATURALGAS
mep:Humidifier-ASSISTEDNATURALGAS rdf:type owl:Class ;
                                  rdfs:subClassOf mep:Humidifier ;
                                  rdfs:comment "http://bsdd.buildingsmart.org/#concept/details/2y1ecVVOv7Lfs9vbXts2uj"@en ;
                                  rdfs:label "Assisted Natural Gas"@en ,
                                             "assistert naturgass"@nb-no ;
                                  rdfs:seeAlso ifc:IfcHumidifierEnumType .


###  http://pi.pauwel.be/voc/distributionelement#Humidifier-ASSISTEDPROPANE
mep:Humidifier-ASSISTEDPROPANE rdf:type owl:Class ;
                               rdfs:subClassOf mep:Humidifier ;
                               rdfs:comment "http://bsdd.buildingsmart.org/#concept/details/1Byt2bBk58pg9rdsh_tvnd"@en ,
                                            "water vapor is added into the airstream through water heated evaporation using a propane heater"@en ,
                                            "water vapor is added into the airstream through water heated evaporation using a propane heater"@en-gb ;
                               rdfs:label "Assisted Propane"@en ,
                                          "assistert propan"@nb-no ;
                               rdfs:seeAlso ifc:IfcHumidifierEnumType .


###  http://pi.pauwel.be/voc/distributionelement#Humidifier-ASSISTEDSTEAM
mep:Humidifier-ASSISTEDSTEAM rdf:type owl:Class ;
                             rdfs:subClassOf mep:Humidifier ;
                             rdfs:comment "http://bsdd.buildingsmart.org/#concept/details/2INKwOIaXFgxGMKSsCa2Lm"@en ,
                                          "water vapor is added into the airstream through water heated evaporation using a steam heater"@en ,
                                          "water vapor is added into the airstream through water heated evaporation using a steam heater"@en-gb ;
                             rdfs:label "Assisted Steam"@en ,
                                        "assistert damp"@nb-no ;
                             rdfs:seeAlso ifc:IfcHumidifierEnumType .


###  http://pi.pauwel.be/voc/distributionelement#Humidifier-STEAMINJECTION
mep:Humidifier-STEAMINJECTION rdf:type owl:Class ;
                              rdfs:subClassOf mep:Humidifier ;
                              rdfs:comment "http://bsdd.buildingsmart.org/#concept/details/05OOwwH2b5pwbQqrAayAR1"@en ,
                                           "water vapor is added into the airstream through direct steam injection"@en ,
                                           "water vapor is added into the airstream through direct steam injection"@en-gb ;
                              rdfs:label "Steam Injection"@en ,
                                         "dampinjeksjon"@nb-no ;
                              rdfs:seeAlso ifc:IfcHumidifierEnumType .


###  http://pi.pauwel.be/voc/distributionelement#Interceptor
mep:Interceptor rdf:type owl:Class ;
                rdfs:subClassOf mep:FlowTreatmentDevice ;
                rdfs:comment "A device designed and installed in order to separate and retain deleterious, hazardous or undesirable matter while permitting normal sewage or liquids to discharge into a collection system by gravity."@en ,
                             "http://bsdd.buildingsmart.org/#concept/details/11vN9pRrz0KQUNzVQ5_2RM"@en ;
                rdfs:label "Abscheider"@de-de ,
                           "Interceptor"@en ;
                rdfs:seeAlso ifc:IfcInterceptor .


###  http://pi.pauwel.be/voc/distributionelement#Interceptor-CYCLONIC
mep:Interceptor-CYCLONIC rdf:type owl:Class ;
                         rdfs:subClassOf mep:Interceptor ;
                         rdfs:comment "http://bsdd.buildingsmart.org/#concept/details/2RxuKardj99Q$KLR33Cbq6"@en ,
                                      "removes larger liquid drops or larger solid particles"@en ,
                                      "removes larger liquid drops or larger solid particles"@en-gb ;
                         rdfs:label "Cyclonic Interceptor"@en ,
                                    "syklonisk"@nb-no ;
                         rdfs:seeAlso ifc:IfcInterceptorEnumType .


###  http://pi.pauwel.be/voc/distributionelement#Interceptor-GREASE
mep:Interceptor-GREASE rdf:type owl:Class ;
                       rdfs:subClassOf mep:Interceptor ;
                       rdfs:comment "chamber, on the line of a drain or discharge pipe, that prevents grease passing into a drainage system"@en ,
                                    "chamber, on the line of a drain or discharge pipe, that prevents grease passing into a drainage system"@en-gb ,
                                    "http://bsdd.buildingsmart.org/#concept/details/3LXDZRMqX6hBYYip97WFpr"@en ;
                       rdfs:label "Grease Interceptor"@en ,
                                  "fett"@nb-no ;
                       rdfs:seeAlso ifc:IfcInterceptorEnumType .


###  http://pi.pauwel.be/voc/distributionelement#Interceptor-OIL
mep:Interceptor-OIL rdf:type owl:Class ;
                    rdfs:subClassOf mep:Interceptor ;
                    rdfs:comment "http://bsdd.buildingsmart.org/#concept/details/0efFn8L559X8O9PLL0mkNu"@en ,
                                 "one or more chambers arranged to prevent the ingress of oil to a drain or sewer that retains the oil for later removal"@en ,
                                 "one or more chambers arranged to prevent the ingress of oil to a drain or sewer that retains the oil for later removal"@en-gb ;
                    rdfs:label "Oil Interceptor"@en ,
                               "olje"@nb-no ;
                    rdfs:seeAlso ifc:IfcInterceptorEnumType .


###  http://pi.pauwel.be/voc/distributionelement#Interceptor-PETROL
mep:Interceptor-PETROL rdf:type owl:Class ;
                       rdfs:subClassOf mep:Interceptor ;
                       rdfs:comment "http://bsdd.buildingsmart.org/#concept/details/3AfygEMd1AwBWNHSyfyIiI"@en ;
                       rdfs:label "Petrol Interceptor"@en ;
                       rdfs:seeAlso ifc:IfcInterceptorEnumType .


###  http://pi.pauwel.be/voc/distributionelement#JunctionBox
mep:JunctionBox rdf:type owl:Class ;
                rdfs:subClassOf mep:FlowFitting ;
                rdfs:comment "An enclosure within which cables are connected. Cables may be members of an electrical circuit (for electrical power systems) or be information carriers (in a telecommunications system). Typically intended to conceal a cable junction from sight, eliminate tampering or provide a safe place for electrical connection."@en ,
                             "http://bsdd.buildingsmart.org/#concept/details/0kaRGER1f0o8KFilly53$b"@en ;
                rdfs:label "Boite de jonction"@fr-fr ,
                           "Junction Box"@en ,
                           "Verbindungsdose"@de-de ;
                rdfs:seeAlso ifc:IfcJunctionBox .


###  http://pi.pauwel.be/voc/distributionelement#JunctionBox-DATA
mep:JunctionBox-DATA rdf:type owl:Class ;
                     rdfs:subClassOf mep:JunctionBox ;
                     rdfs:comment "contains cables, outlets, and/or switches for communications use"@en ,
                                  "contains cables, outlets, and/or switches for communications use"@en-gb ,
                                  "http://bsdd.buildingsmart.org/#concept/details/1mq782MKb1ZxoRYPK9Umy2"@en ;
                     rdfs:label "Data"@en ,
                                "data"@nb-no ;
                     rdfs:seeAlso ifc:IfcJunctionBoxEnumType .


###  http://pi.pauwel.be/voc/distributionelement#JunctionBox-POWER
mep:JunctionBox-POWER rdf:type owl:Class ;
                      rdfs:subClassOf mep:JunctionBox ;
                      rdfs:comment "http://bsdd.buildingsmart.org/#concept/details/2rfL__S75EcOfkEgBpZV_b"@en ;
                      rdfs:label "Power"@en ,
                                 "strømtilførsel"@nb-no ;
                      rdfs:seeAlso ifc:IfcJunctionBoxEnumType .


###  http://pi.pauwel.be/voc/distributionelement#Lamp
mep:Lamp rdf:type owl:Class ;
         rdfs:subClassOf mep:FlowTerminal ;
         rdfs:comment "An artificial light source such as a light bulb or tube."@en ,
                      "http://bsdd.buildingsmart.org/#concept/details/0ETiMxiX14xwxiqYleSsxj"@en ;
         rdfs:label "Lamp"@en ,
                    "Lampe"@de-de ,
                    "Leuchtmittel"@de-de ,
                    "lampe"@fr-fr ;
         rdfs:seeAlso ifc:IfcLamp .


###  http://pi.pauwel.be/voc/distributionelement#Lamp-COMPACTFLUORESCENT
mep:Lamp-COMPACTFLUORESCENT rdf:type owl:Class ;
                            rdfs:subClassOf mep:Lamp ;
                            rdfs:comment "http://bsdd.buildingsmart.org/#concept/details/3zxJlrQUXE3BF9p3XFK9sV"@en ;
                            rdfs:label "Compact Fluorescent"@en ;
                            rdfs:seeAlso ifc:IfcLampEnumType .


###  http://pi.pauwel.be/voc/distributionelement#Lamp-FLUORESCENT
mep:Lamp-FLUORESCENT rdf:type owl:Class ;
                     rdfs:subClassOf mep:Lamp ;
                     rdfs:comment "a typically tubular discharge lamp in which most of the light is emitted by one or several layers of phosphors excited by ultraviolet radiation from the discharge."@en ,
                                  "a typically tubular discharge lamp in which most of the light is emitted by one or several layers of phosphors excited by ultraviolet radiation from the discharge."@en-gb ,
                                  "http://bsdd.buildingsmart.org/#concept/details/0V1bibu4L13Bts98Ganx3k"@en ;
                     rdfs:label "Fluorescent"@en ,
                                "fluoriserende lampe"@nb-no ;
                     rdfs:seeAlso ifc:IfcLampEnumType .


###  http://pi.pauwel.be/voc/distributionelement#Lamp-HALOGEN
mep:Lamp-HALOGEN rdf:type owl:Class ;
                 rdfs:subClassOf mep:Lamp ;
                 rdfs:comment "a gas-filled, high-intensity incandescent lamp containing a small amount of a halogen"@en ,
                              "http://bsdd.buildingsmart.org/#concept/details/2EGers_2r5rBBnldpP0G_o"@en ;
                 rdfs:label "Halogen"@en ,
                            "halogen"@nb-no ;
                 rdfs:seeAlso ifc:IfcLampEnumType .


###  http://pi.pauwel.be/voc/distributionelement#Lamp-HIGHPRESSUREMERCURY
mep:Lamp-HIGHPRESSUREMERCURY rdf:type owl:Class ;
                             rdfs:subClassOf mep:Lamp ;
                             rdfs:comment "a discharge lamp in which most of the light is emitted by exciting mercury at high pressure"@en ,
                                          "a discharge lamp in which most of the light is emitted by exciting mercury at high pressure"@en-gb ,
                                          "http://bsdd.buildingsmart.org/#concept/details/2QODll5IXBLOrmpb298AP_"@en ;
                             rdfs:label "High Pressure Mercury"@en ,
                                        "høytrykk - bly lampe"@nb-no ;
                             rdfs:seeAlso ifc:IfcLampEnumType .


###  http://pi.pauwel.be/voc/distributionelement#Lamp-HIGHPRESSURESODIUM
mep:Lamp-HIGHPRESSURESODIUM rdf:type owl:Class ;
                            rdfs:subClassOf mep:Lamp ;
                            rdfs:comment "a discharge lamp in which most of the light is emitted by exciting sodium at high pressure"@en ,
                                         "a discharge lamp in which most of the light is emitted by exciting sodium at high pressure"@en-gb ,
                                         "http://bsdd.buildingsmart.org/#concept/details/1vX9Auimj7BfAyryFJkgkm"@en ;
                            rdfs:label "High Pressure Sodium"@en ,
                                       "høytrykk - sodium"@nb-no ;
                            rdfs:seeAlso ifc:IfcLampEnumType .


###  http://pi.pauwel.be/voc/distributionelement#Lamp-LED
mep:Lamp-LED rdf:type owl:Class ;
             rdfs:subClassOf mep:Lamp ;
             rdfs:comment "a light-emitting diode (LED) is a semiconductor device that emits visible light when an electric current passes through it."@en ,
                          "http://bsdd.buildingsmart.org/#concept/details/2mULGMKGf1cRYOSiyAofvb"@en ;
             rdfs:label "LED"@en ,
                        "LED"@nb-no ;
             rdfs:seeAlso ifc:IfcLampEnumType .


###  http://pi.pauwel.be/voc/distributionelement#Lamp-METALHALIDE
mep:Lamp-METALHALIDE rdf:type owl:Class ;
                     rdfs:subClassOf mep:Lamp ;
                     rdfs:comment "http://bsdd.buildingsmart.org/#concept/details/3esdl$BJXD9htEWoSEpsDg"@en ;
                     rdfs:label "Metal Halide"@en ;
                     rdfs:seeAlso ifc:IfcLampEnumType .


###  http://pi.pauwel.be/voc/distributionelement#Lamp-OLED
mep:Lamp-OLED rdf:type owl:Class ;
              rdfs:subClassOf mep:Lamp ;
              rdfs:comment "a solid state lamp that uses light-emitting diodes as the source of light whose emissive electroluminescent layer is composed of a film of organic compounds"@en ,
                           "a solid state lamp that uses light-emitting diodes as the source of light whose emissive electroluminescent layer is composed of a film of organic compounds"@en-gb ,
                           "http://bsdd.buildingsmart.org/#concept/details/2ga1cHzm5D$fItBN2Tozo9"@en ;
              rdfs:label "OLED"@en ,
                         "oled"@nb-no ;
              rdfs:seeAlso ifc:IfcLampEnumType .


###  http://pi.pauwel.be/voc/distributionelement#Lamp-TUNGSTENFILAMENT
mep:Lamp-TUNGSTENFILAMENT rdf:type owl:Class ;
                          rdfs:subClassOf mep:Lamp ;
                          rdfs:comment "http://bsdd.buildingsmart.org/#concept/details/3n5ZYbHnnBuhtIMoheS78j"@en ;
                          rdfs:label "Tungsten Filament"@en ;
                          rdfs:seeAlso ifc:IfcLampEnumType .


###  http://pi.pauwel.be/voc/distributionelement#LightFixture
mep:LightFixture rdf:type owl:Class ;
                 rdfs:subClassOf mep:FlowTerminal ;
                 rdfs:comment "A container that is designed for the purpose of housing one or more lamps and optionally devices that control, restrict or vary their emission."@en ,
                              "http://bsdd.buildingsmart.org/#concept/details/1sxtfF6Gb1ieWm5Xy9aa5C"@en ;
                 rdfs:label "Fixation de lampe"@fr-fr ,
                            "Leuchte"@de-de ,
                            "Light Fixture"@en ,
                            "Verlichtingsarmatuur"@nl-nl ,
                            "lysarmatur"@nb-no ;
                 rdfs:seeAlso ifc:IfcLightFixture .


###  http://pi.pauwel.be/voc/distributionelement#LightFixture-DIRECTIONSOURCE
mep:LightFixture-DIRECTIONSOURCE rdf:type owl:Class ;
                                 rdfs:subClassOf mep:LightFixture ;
                                 rdfs:comment "a light fixture that is considered to have a length or surface area from which it emits light in a direction. a light fixture containing one or more fluorescent lamps is an example of a direction source"@en ,
                                              "a light fixture that is considered to have a length or surface area from which it emits light in a direction. a light fixture containing one or more fluorescent lamps is an example of a direction source"@en-gb ,
                                              "http://bsdd.buildingsmart.org/#concept/details/0XEOjAoQb8nAOs58mf0C7S"@en ;
                                 rdfs:label "Direction Source"@en ,
                                            "kilderetning"@nb-no ;
                                 rdfs:seeAlso ifc:IfcLightFixtureEnumType .


###  http://pi.pauwel.be/voc/distributionelement#LightFixture-POINTSOURCE
mep:LightFixture-POINTSOURCE rdf:type owl:Class ;
                             rdfs:subClassOf mep:LightFixture ;
                             rdfs:comment "http://bsdd.buildingsmart.org/#concept/details/1bOvnRIgnDhuRposkK0D7b"@en ;
                             rdfs:label "Point Source"@en ;
                             rdfs:seeAlso ifc:IfcLightFixtureEnumType .


###  http://pi.pauwel.be/voc/distributionelement#LightFixture-SECURITYLIGHTING
mep:LightFixture-SECURITYLIGHTING rdf:type owl:Class ;
                                  rdfs:subClassOf mep:LightFixture ;
                                  rdfs:comment "a light fixture having specific purpose of directing occupants in an emergency, such as an illuminated exit sign or emergency flood light"@en ,
                                               "a light fixture having specific purpose of directing occupants in an emergency, such as an illuminated exit sign or emergency flood light"@en-gb ,
                                               "http://bsdd.buildingsmart.org/#concept/details/3r7SZninH9Uh6FH$yz54Pl"@en ;
                                  rdfs:label "Security Lighting"@en ,
                                             "sikkerhetsbelysning"@nb-no ;
                                  rdfs:seeAlso ifc:IfcLightFixtureEnumType .


###  http://pi.pauwel.be/voc/distributionelement#MedicalDevice
mep:MedicalDevice rdf:type owl:Class ;
                  rdfs:subClassOf mep:FlowTerminal ;
                  rdfs:comment "A device is attached to a medical piping system and operates upon medical gases to perform a specific function. Medical gases include medical air, medical vacuum, oxygen, carbon dioxide, nitrogen, and nitrous oxide."@en ,
                               "http://bsdd.buildingsmart.org/#concept/details/1AkDu7dZb8l8V$ZCIldlOl"@en ;
                  rdfs:label "Equipement médical"@fr-fr ,
                             "Medical Device"@en ,
                             "Medizinisches Gerät"@de-de ,
                             "medisinsk utstyr"@nb-no ;
                  rdfs:seeAlso ifc:IfcMedicalDevice .


###  http://pi.pauwel.be/voc/distributionelement#MedicalDevice-AIRSTATION
mep:MedicalDevice-AIRSTATION rdf:type owl:Class ;
                             rdfs:subClassOf mep:MedicalDevice ;
                             rdfs:comment "device that provides purified medical air, composed of an air compressor and air treatment line"@en ,
                                          "device that provides purified medical air, composed of an air compressor and air treatment line"@en-gb ,
                                          "http://bsdd.buildingsmart.org/#concept/details/3o0TKF$jb4JfwCg4jNP8QH"@en ;
                             rdfs:label "Air Station"@en ,
                                        "luftstasjon"@nb-no ;
                             rdfs:seeAlso ifc:IfcMedicalDeviceEnumType .


###  http://pi.pauwel.be/voc/distributionelement#MedicalDevice-FEEDAIRUNIT
mep:MedicalDevice-FEEDAIRUNIT rdf:type owl:Class ;
                              rdfs:subClassOf mep:MedicalDevice ;
                              rdfs:comment "http://bsdd.buildingsmart.org/#concept/details/0L4vXkvln2MRDKPQngnIZ1"@en ;
                              rdfs:label "Feed Air Unit"@en ;
                              rdfs:seeAlso ifc:IfcMedicalDeviceEnumType .


###  http://pi.pauwel.be/voc/distributionelement#MedicalDevice-OXYGENGENERATOR
mep:MedicalDevice-OXYGENGENERATOR rdf:type owl:Class ;
                                  rdfs:subClassOf mep:MedicalDevice ;
                                  rdfs:comment "device that generates oxygen from air"@en ,
                                               "device that generates oxygen from air"@en-gb ,
                                               "http://bsdd.buildingsmart.org/#concept/details/2beptDYcnFLwdWqGq$GWRC"@en ;
                                  rdfs:label "Oxygen Generator"@en ,
                                             "oksygengenerator"@nb-no ;
                                  rdfs:seeAlso ifc:IfcMedicalDeviceEnumType .


###  http://pi.pauwel.be/voc/distributionelement#MedicalDevice-OXYGENPLANT
mep:MedicalDevice-OXYGENPLANT rdf:type owl:Class ;
                              rdfs:subClassOf mep:MedicalDevice ;
                              rdfs:comment "device that combines a feed air unit, oxygen generator, and backup oxygen cylinders"@en ,
                                           "http://bsdd.buildingsmart.org/#concept/details/2Z$pgegmf8Bv9ktRxYuUY7"@en ;
                              rdfs:label "Oxygen Plant"@en ,
                                         "oksygenanlegg"@nb-no ;
                              rdfs:seeAlso ifc:IfcMedicalDeviceEnumType .


###  http://pi.pauwel.be/voc/distributionelement#MedicalDevice-VACUUMSTATION
mep:MedicalDevice-VACUUMSTATION rdf:type owl:Class ;
                                rdfs:subClassOf mep:MedicalDevice ;
                                rdfs:comment "device that provides suction, composed of a vacuum pump and bacterial filtration line"@en ,
                                             "device that provides suction, composed of a vacuum pump and bacterial filtration line"@en-gb ,
                                             "http://bsdd.buildingsmart.org/#concept/details/2qtw8iOMD6aQlRYJeE54Oe"@en ;
                                rdfs:label "Vacuum Station"@en ,
                                           "vakuumstasjon"@nb-no ;
                                rdfs:seeAlso ifc:IfcMedicalDeviceEnumType .


###  http://pi.pauwel.be/voc/distributionelement#MotorConnection
mep:MotorConnection rdf:type owl:Class ;
                    rdfs:subClassOf mep:EnergyConversionDevice ;
                    rdfs:comment "The means for connecting a motor as the driving device to the driven device."@en ,
                                 "http://bsdd.buildingsmart.org/#concept/details/1uD4xpI6rB28wdUvR8Y86u"@en ;
                    rdfs:label "Connection du moteur"@fr-fr ,
                               "Motor Connection"@en ,
                               "Motoranschluss"@de-de ,
                               "Motorkoppeling"@nl-nl ,
                               "motorkobling"@nb-no ;
                    rdfs:seeAlso ifc:IfcMotorConnection .


###  http://pi.pauwel.be/voc/distributionelement#MotorConnection-BELTDRIVE
mep:MotorConnection-BELTDRIVE rdf:type owl:Class ;
                              rdfs:subClassOf mep:MotorConnection ;
                              rdfs:comment "an indirect connection made through the medium of a shaped, flexible continuous loop"@en ,
                                           "an indirect connection made through the medium of a shaped, flexible continuous loop"@en-gb ,
                                           "http://bsdd.buildingsmart.org/#concept/details/337StHg8r5XxwkyT3aqNfr"@en ;
                              rdfs:label "Belt Drive Motor Connection"@en ,
                                         "beltedrevet"@nb-no ,
                                         "drivbelte"@nb-no ;
                              rdfs:seeAlso ifc:IfcMotorConnectionEnumType .


###  http://pi.pauwel.be/voc/distributionelement#MotorConnection-COUPLING
mep:MotorConnection-COUPLING rdf:type owl:Class ;
                             rdfs:subClassOf mep:MotorConnection ;
                             rdfs:comment "an indirect connection made through the medium of the viscosity of a fluid"@en ,
                                          "http://bsdd.buildingsmart.org/#concept/details/2ztf_P39HBTfamG9J37o0l"@en ;
                             rdfs:label "Coupling Motor Connection"@en ,
                                        "kopling"@nb-no ;
                             rdfs:seeAlso ifc:IfcMotorConnectionEnumType .


###  http://pi.pauwel.be/voc/distributionelement#MotorConnection-DIRECTDRIVE
mep:MotorConnection-DIRECTDRIVE rdf:type owl:Class ;
                                rdfs:subClassOf mep:MotorConnection ;
                                rdfs:comment "a direct, physical connection made between the motor and the driven device"@en ,
                                             "a direct, physical connection made between the motor and the driven device"@en-gb ,
                                             "http://bsdd.buildingsmart.org/#concept/details/26AgedTrrEsuQRrx2V_DY3"@en ;
                                rdfs:label "Direct Drive Motor Connection"@en ,
                                           "direktedrevet motor"@nb-no ;
                                rdfs:seeAlso ifc:IfcMotorConnectionEnumType .


###  http://pi.pauwel.be/voc/distributionelement#Outlet
mep:Outlet rdf:type owl:Class ;
           rdfs:subClassOf mep:FlowTerminal ;
           rdfs:comment """A device installed at a point to receive one or more inserted plugs for electrical power or communications.
"""@en ,
                        "http://bsdd.buildingsmart.org/#concept/details/28QPmBjcbAuOHAWzJovXA6"@en ;
           rdfs:label "Dose"@de-de ,
                      "Outlet"@en ,
                      "Steckdose"@de-de ,
                      "prise"@fr-fr ,
                      "uttak"@nb-no ;
           rdfs:seeAlso ifc:IfcOutlet .


###  http://pi.pauwel.be/voc/distributionelement#Outlet-AUDIOVISUALOUTLET
mep:Outlet-AUDIOVISUALOUTLET rdf:type owl:Class ;
                             rdfs:subClassOf mep:Outlet ;
                             rdfs:comment "an outlet used for an audio or visual device"@en ,
                                          "an outlet used for an audio or visual device"@en-gb ,
                                          "http://bsdd.buildingsmart.org/#concept/details/0lKEDMjxLFNxLZF0uvQXvQ"@en ;
                             rdfs:label "Audiovisual Outlet"@en ,
                                        "audiovisuelt utgang"@nb-no ;
                             rdfs:seeAlso ifc:IfcOutletEnumType .


###  http://pi.pauwel.be/voc/distributionelement#Outlet-COMMUNICATIONSOUTLET
mep:Outlet-COMMUNICATIONSOUTLET rdf:type owl:Class ;
                                rdfs:subClassOf mep:Outlet ;
                                rdfs:comment "an outlet used for connecting communications equipment"@en ,
                                             "an outlet used for connecting communications equipment"@en-gb ,
                                             "http://bsdd.buildingsmart.org/#concept/details/3LRis6YOnAhO_2qLThy$7d"@en ;
                                rdfs:label "Communications Outlet"@en ,
                                           "kommunikasjonuttak"@nb-no ;
                                rdfs:seeAlso ifc:IfcOutletEnumType .


###  http://pi.pauwel.be/voc/distributionelement#Outlet-DATAOUTLET
mep:Outlet-DATAOUTLET rdf:type owl:Class ;
                      rdfs:subClassOf mep:Outlet ;
                      rdfs:comment "an outlet used for connecting data communications equipment"@en ,
                                   "an outlet used for connecting data communications equipment"@en-gb ,
                                   "http://bsdd.buildingsmart.org/#concept/details/2nLbYVXBz2iPUzoVG9MSjL"@en ;
                      rdfs:label "Data Outlet"@en ,
                                 "datautgang"@nb-no ;
                      rdfs:seeAlso ifc:IfcOutletEnumType .


###  http://pi.pauwel.be/voc/distributionelement#Outlet-POWEROUTLET
mep:Outlet-POWEROUTLET rdf:type owl:Class ;
                       rdfs:subClassOf mep:Outlet ;
                       rdfs:comment "an outlet used for connecting electrical devices requiring power"@en ,
                                    "an outlet used for connecting electrical devices requiring power"@en-gb ,
                                    "http://bsdd.buildingsmart.org/#concept/details/1VO3tI1Bn2AO1KWd3ZVGi6"@en ;
                       rdfs:label "Power Outlet"@en ,
                                  "strømuttak"@nb-no ;
                       rdfs:seeAlso ifc:IfcOutletEnumType .


###  http://pi.pauwel.be/voc/distributionelement#Outlet-TELEPHONEOUTLET
mep:Outlet-TELEPHONEOUTLET rdf:type owl:Class ;
                           rdfs:subClassOf mep:Outlet ;
                           rdfs:comment "an outlet used for connecting telephone communications equipment"@en ,
                                        "an outlet used for connecting telephone communications equipment"@en-gb ,
                                        "http://bsdd.buildingsmart.org/#concept/details/3sQmISw8154AzAhVrfw8CI"@en ;
                           rdfs:label "Telephone Outlet"@en ,
                                      "telekommunikasjonsuttak"@nb-no ;
                           rdfs:seeAlso ifc:IfcOutletEnumType .


###  http://pi.pauwel.be/voc/distributionelement#PipeFitting
mep:PipeFitting rdf:type owl:Class ;
                rdfs:subClassOf mep:FlowFitting ;
                rdfs:comment "A junction or transition in a piping flow distribution system used to connect pipe segments, resulting in changes in flow characteristics to the fluid such as direction or flow rate. Includes elbows, junctions, manifolds, and plumbing boxes."@en ,
                             "http://bsdd.buildingsmart.org/#concept/details/36UVu0qV8HuO00025QrE$V"@en ;
                rdfs:label "Pipe Fitting"@en ,
                           "Rohrverbinder"@de-de ,
                           "raccord de tuyauterie"@fr-fr ,
                           "rørdel"@nb-no ;
                rdfs:seeAlso ifc:IfcPipeFitting .


###  http://pi.pauwel.be/voc/distributionelement#PipeFitting-BEND
mep:PipeFitting-BEND rdf:type owl:Class ;
                     rdfs:subClassOf mep:PipeFitting ;
                     rdfs:comment "A fitting for joining the down-pipe in different angles pass blockings"@en ,
                                  "Bend albue"@nb-no ,
                                  "Bend, albue"@nb-no ,
                                  "En innretning for å skjøte nedløpsrøret i ulike vinkler forbi hindringer"@nb-no ,
                                  "a fitting with typically two ports used to change the direction of flow between connected elements"@en ,
                                  "a fitting with typically two ports used to change the direction of flow between connected elements"@en-gb ,
                                  "http://bsdd.buildingsmart.org/#concept/details/0_1uLp$45FjOqNjel4YBnY"@en ,
                                  "http://bsdd.buildingsmart.org/#concept/details/11IUzA0c9C9gGPcD6wjcm8"@en ,
                                  "http://bsdd.buildingsmart.org/#concept/details/2ScGOKl0TF58sYPFb6KHbc"@en ,
                                  "http://bsdd.buildingsmart.org/#concept/details/2VSwjMBw1DguPAi2T4j5Vo"@en ,
                                  "http://bsdd.buildingsmart.org/#concept/details/2Wxblu6ePDPQ1joWCcVscx"@en ,
                                  "http://bsdd.buildingsmart.org/#concept/details/3$QIJ5gKv4hPazehz8XSJr"@en ,
                                  "http://bsdd.buildingsmart.org/#concept/details/3qojuW1k5C89_5p3vK7la0"@en ,
                                  "http://bsdd.buildingsmart.org/#concept/details/3vHSO0oT0Hsm00051Mm008"@en ;
                     rdfs:label "Bend"@en ,
                                "Krümmer"@de-de ,
                                "bend"@nb-no ,
                                "bend brannslokking inertgass"@nb-no ,
                                "bend brannslukking vann"@nb-no ,
                                "bend bunnledning sanitær"@nb-no ,
                                "bend gassinstallasjon"@nb-no ,
                                "bend gassinstallasjon virksomhet"@nb-no ,
                                "bend pipeline sanitation"@en ,
                                "bend sanitær"@nb-no ,
                                "brannslokkingbend for tåke"@nb-no ,
                                "brannslukkingbend for sprinkler"@nb-no ,
                                "coude"@fr-fr ,
                                "elbows"@en ,
                                "rørbend"@nb-no ,
                                "tee gas installation"@en ;
                     rdfs:seeAlso ifc:IfcPipeFittingEnumType .


###  http://pi.pauwel.be/voc/distributionelement#PipeFitting-CONNECTOR
mep:PipeFitting-CONNECTOR rdf:type owl:Class ;
                          rdfs:subClassOf mep:PipeFitting ;
                          rdfs:comment "device generally consisting of a plate, toothed-plate or ring which, when partly embedded in each or in one of the contact faces of two members and held together by a connecting bolt, is capable of transmitting a load from one member to another"@en ,
                                       "http://bsdd.buildingsmart.org/#concept/details/3tvMvSswv0Dw7HoTwOQYKj"@en ,
                                       "innretning som vanligvis består av en plate, en fortannet plate eller en ring, og som, når den er delvis trengt inn i alle eller i en av kontaktflatene på to komponenter og holdt sammen med en bolt, er i stand til å overføre en last fra en komponent til e"@nb-no ;
                          rdfs:label "Connector"@en ,
                                     "Dübel"@de-de ,
                                     "connecteur"@fr-fr ,
                                     "forbindelse"@nb-no ,
                                     "forbindelsesledd"@nb-no ,
                                     "forbinder"@nb-no ;
                          rdfs:seeAlso ifc:IfcPipeFittingEnumType .


###  http://pi.pauwel.be/voc/distributionelement#PipeFitting-ENTRY
mep:PipeFitting-ENTRY rdf:type owl:Class ;
                      rdfs:subClassOf mep:PipeFitting ;
                      rdfs:comment "entry fitting, typically unconnected at one port and connected to a flow distribution system at the other (e.g., a breeching inlet)"@en ,
                                   "entry fitting, typically unconnected at one port and connected to a flow distribution system at the other (e.g., a breeching inlet)"@en-gb ,
                                   "entry fitting, typically unconnected at one port and connected to a flow distribution system at the other (e.g., an outside air duct system intake opening)"@en ,
                                   "entry fitting, typically unconnected at one port and connected to a flow distribution system at the other (e.g., an outside air duct system intake opening)"@en-gb ,
                                   "http://bsdd.buildingsmart.org/#concept/details/3iMmwy9iv0SBFB7w4cNsVs"@en ;
                      rdfs:label "Entry"@en ,
                                 "inngang"@nb-no ;
                      rdfs:seeAlso ifc:IfcPipeFittingEnumType .


###  http://pi.pauwel.be/voc/distributionelement#PipeFitting-EXIT
mep:PipeFitting-EXIT rdf:type owl:Class ;
                     rdfs:subClassOf mep:PipeFitting ;
                     rdfs:comment "http://bsdd.buildingsmart.org/#concept/details/1vLJsY3MX6I8Ss72zp5sN_"@en ;
                     rdfs:label "Exit"@en ,
                                "utgang"@nb-no ;
                     rdfs:seeAlso ifc:IfcPipeFittingEnumType .


###  http://pi.pauwel.be/voc/distributionelement#PipeFitting-JUNCTION
mep:PipeFitting-JUNCTION rdf:type owl:Class ;
                         rdfs:subClassOf mep:PipeFitting ;
                         rdfs:comment "a fitting with typically more than two ports used to redistribute flow among the ports and/or to change the direction of flow between connected elements (e.g, tee, cross, wye, etc.)"@en ,
                                      "a fitting with typically more than two ports used to redistribute flow among the ports and/or to change the direction of flow between connected elements (e.g, tee, cross, wye, etc.)."@en-gb ,
                                      "http://bsdd.buildingsmart.org/#concept/details/2OzMql95b8ouXEzC1oYarB"@en ;
                         rdfs:label "Junction"@en ,
                                    "gren"@nb-no ,
                                    "grenrør"@nb-no ,
                                    "kryss"@nb-no ;
                         rdfs:seeAlso ifc:IfcPipeFittingEnumType .


###  http://pi.pauwel.be/voc/distributionelement#PipeFitting-OBSTRUCTION
mep:PipeFitting-OBSTRUCTION rdf:type owl:Class ;
                            rdfs:subClassOf mep:PipeFitting ;
                            rdfs:comment "http://bsdd.buildingsmart.org/#concept/details/2gXay6NOz7NPfYIUbDxtmF"@en ;
                            rdfs:label "Obstruction"@en ,
                                       "hindring"@nb-no ;
                            rdfs:seeAlso ifc:IfcPipeFittingEnumType .


###  http://pi.pauwel.be/voc/distributionelement#PipeFitting-TRANSITION
mep:PipeFitting-TRANSITION rdf:type owl:Class ;
                           rdfs:subClassOf mep:PipeFitting ;
                           rdfs:comment "http://bsdd.buildingsmart.org/#concept/details/0mLpncHvn8AguL5g1sYDP7"@en ;
                           rdfs:label "Transition"@en ,
                                      "overgang"@nb-no ;
                           rdfs:seeAlso ifc:IfcPipeFittingEnumType .


###  http://pi.pauwel.be/voc/distributionelement#PipeSegment
mep:PipeSegment rdf:type owl:Class ;
                rdfs:subClassOf mep:FlowSegment ;
                rdfs:comment "A segment is used to typically join two sections of a piping network."@en ,
                             "http://bsdd.buildingsmart.org/#concept/details/27v4E0qV8HuO00025QrE$V"@en ;
                rdfs:label "Pipe Segment"@en ,
                           "Rohr"@de-de ,
                           "Tronçon de tuyauterie"@fr-fr ,
                           "rørdel"@nb-no ;
                rdfs:seeAlso ifc:IfcPipeSegment .


###  http://pi.pauwel.be/voc/distributionelement#PipeSegment-CULVERT
mep:PipeSegment-CULVERT rdf:type owl:Class ;
                        rdfs:subClassOf mep:PipeSegment ;
                        rdfs:comment "http://bsdd.buildingsmart.org/#concept/details/0kbHQAKHrDHfD6TQOe$Myu"@en ;
                        rdfs:label "Culvert"@en ,
                                   "kulvert"@nb-no ;
                        rdfs:seeAlso ifc:IfcPipeSegmentEnumType .


###  http://pi.pauwel.be/voc/distributionelement#PipeSegment-FLEXIBLESEGMENT
mep:PipeSegment-FLEXIBLESEGMENT rdf:type owl:Class ;
                                rdfs:subClassOf mep:PipeSegment ;
                                rdfs:comment "http://bsdd.buildingsmart.org/#concept/details/0bMKZ$AyPEsOOwHPCXcOcT"@en ;
                                rdfs:label "Flexible Pipe Segment"@en ,
                                           "fleksibel delflate"@nb-no ,
                                           "fleksibel rørdel"@nb-no ;
                                rdfs:seeAlso ifc:IfcPipeSegmentEnumType .


###  http://pi.pauwel.be/voc/distributionelement#PipeSegment-GUTTER
mep:PipeSegment-GUTTER rdf:type owl:Class ;
                       rdfs:subClassOf mep:PipeSegment ;
                       rdfs:comment "A gutter situated outside the building and supported by brackets"@en ,
                                    "En renne som støttes av rennekroker og som er plassert på utsiden av bygningen for å lede bort regnvann."@nb-no ,
                                    "Takrenne"@nb-no ,
                                    "http://bsdd.buildingsmart.org/#concept/details/2deKArJfvCcR42exJCfGfR"@en ;
                       rdfs:label "Gutter"@en ,
                                  "eaves gutter"@en ,
                                  "renne"@nb-no ,
                                  "takrenne"@nb-no ;
                       rdfs:seeAlso ifc:IfcPipeSegmentEnumType .


###  http://pi.pauwel.be/voc/distributionelement#PipeSegment-RIGIDSEGMENT
mep:PipeSegment-RIGIDSEGMENT rdf:type owl:Class ;
                             rdfs:subClassOf mep:PipeSegment ;
                             rdfs:comment "a rigid segment is a continuous linear segment of pipe that cannot be deformed"@en ,
                                          "a rigid segment is a continuous linear segment of pipe that cannot be deformed"@en-gb ,
                                          "http://bsdd.buildingsmart.org/#concept/details/0oZaW79IT5rfrDH337Wczh"@en ;
                             rdfs:label "Rigid Pipe Segment"@en ,
                                        "stiv delflate"@nb-no ;
                             rdfs:seeAlso ifc:IfcPipeSegmentEnumType .


###  http://pi.pauwel.be/voc/distributionelement#PipeSegment-SPOOL
mep:PipeSegment-SPOOL rdf:type owl:Class ;
                      rdfs:subClassOf mep:PipeSegment ;
                      rdfs:comment "a type of rigid segment that is typically shorter and used for providing connectivity within a piping network"@en ,
                                   "a type of rigid segment that is typically shorter and used for providing connectivity within a piping network"@en-gb ,
                                   "http://bsdd.buildingsmart.org/#concept/details/1XnqgBB0b5Ehi3OXV3HNVt"@en ;
                      rdfs:label "Spool"@en ;
                      rdfs:seeAlso ifc:IfcPipeSegmentEnumType .


###  http://pi.pauwel.be/voc/distributionelement#ProtectiveDevice
mep:ProtectiveDevice rdf:type owl:Class ;
                     rdfs:subClassOf mep:FlowController ;
                     rdfs:comment """A device breaks an electrical circuit when a stated electric current that passes through it is exceeded.
Provides protection against electrical current only (not as a general protective device)."""@en ,
                                  "http://bsdd.buildingsmart.org/#concept/details/127XSeDXvD5haPLRkC8eyd"@en ;
                     rdfs:label "Protective Device"@en ,
                                "Sicherung"@de-de ,
                                "beskyttende enhet"@nb-no ,
                                "équipement de protection"@fr-fr ;
                     rdfs:seeAlso ifc:IfcProtectiveDevice .


###  http://pi.pauwel.be/voc/distributionelement#ProtectiveDevice-CIRCUITBREAKER
mep:ProtectiveDevice-CIRCUITBREAKER rdf:type owl:Class ;
                                    rdfs:subClassOf mep:ProtectiveDevice ;
                                    rdfs:comment "http://bsdd.buildingsmart.org/#concept/details/3EWAB3Ur5Cng3zn8b4wZEE"@en ;
                                    rdfs:label "Circuit Breaker"@en ,
                                               "strømbryter"@nb-no ;
                                    rdfs:seeAlso ifc:IfcProtectiveDeviceEnumType .


###  http://pi.pauwel.be/voc/distributionelement#ProtectiveDevice-EARTHINGSWITCH
mep:ProtectiveDevice-EARTHINGSWITCH rdf:type owl:Class ;
                                    rdfs:subClassOf mep:ProtectiveDevice ;
                                    rdfs:comment "a safety device used to open or close a circuit when there is no current. used to isolate a part of a circuit, a machine, a part of an overhead line or an underground line so that maintenance can be safely conducted"@en ,
                                                 "a safety device used to open or close a circuit when there is no current. used to isolate a part of a circuit, a machine, a part of an overhead line or an underground line so that maintenance can be safely conducted"@en-gb ,
                                                 "http://bsdd.buildingsmart.org/#concept/details/2q5Q9N9Az1Oh7iRLNISzdt"@en ;
                                    rdfs:label "Earthing Switch"@en ,
                                               "jordingsbryter"@nb-no ;
                                    rdfs:seeAlso ifc:IfcProtectiveDeviceEnumType .


###  http://pi.pauwel.be/voc/distributionelement#ProtectiveDevice-EARTHLEAKAGECIRCUITBREAKER
mep:ProtectiveDevice-EARTHLEAKAGECIRCUITBREAKER rdf:type owl:Class ;
                                                rdfs:subClassOf mep:ProtectiveDevice ;
                                                rdfs:comment "a device that opens, closes, or isolates a circuit and has short circuit protection but no overload protection. it attempts to break the circuit when there is a leakage of current from phase to earth, by measuring voltage on the earth conductor"@en ,
                                                             "a device that opens, closes, or isolates a circuit and has short circuit protection but no overload protection. it attempts to break the circuit when there is a leakage of current from phase to earth, by measuring voltage on the earth conductor"@en-gb ,
                                                             "http://bsdd.buildingsmart.org/#concept/details/2h1MphDsfAOOGX2jycslmC"@en ;
                                                rdfs:label "Earth Leakage Circuit Breaker"@en ,
                                                           "lekkstrømsikring"@nb-no ;
                                                rdfs:seeAlso ifc:IfcProtectiveDeviceEnumType .


###  http://pi.pauwel.be/voc/distributionelement#ProtectiveDevice-FUSEDISCONNECTOR
mep:ProtectiveDevice-FUSEDISCONNECTOR rdf:type owl:Class ;
                                      rdfs:subClassOf mep:ProtectiveDevice ;
                                      rdfs:comment "a device that will electrically open the circuit after a period of prolonged, abnormal current flow"@en ,
                                                   "http://bsdd.buildingsmart.org/#concept/details/2TfJqRtl5EbAjQ1_2wg3W9"@en ;
                                      rdfs:label "Fuse Disconnector"@en ,
                                                 "sikringskopling"@nb-no ;
                                      rdfs:seeAlso ifc:IfcProtectiveDeviceEnumType .


###  http://pi.pauwel.be/voc/distributionelement#ProtectiveDevice-RESIDUALCURRENTCIRCUITBREAKER
mep:ProtectiveDevice-RESIDUALCURRENTCIRCUITBREAKER rdf:type owl:Class ;
                                                   rdfs:subClassOf mep:ProtectiveDevice ;
                                                   rdfs:comment "http://bsdd.buildingsmart.org/#concept/details/2RbnT6FAn6fxAlZWiSgJ_I"@en ;
                                                   rdfs:label "Residual Current Circuit Breaker"@en ;
                                                   rdfs:seeAlso ifc:IfcProtectiveDeviceEnumType .


###  http://pi.pauwel.be/voc/distributionelement#ProtectiveDevice-RESIDUALCURRENTSWITCH
mep:ProtectiveDevice-RESIDUALCURRENTSWITCH rdf:type owl:Class ;
                                           rdfs:subClassOf mep:ProtectiveDevice ;
                                           rdfs:comment "a device that opens, closes or isolates a circuit and has no short circuit or overload protection. May also be identified as a 'ground fault switch'"@en ,
                                                        "a device that opens, closes or isolates a circuit and has no short circuit or overload protection. May also be identified as a 'ground fault switch'"@en-gb ,
                                                        "http://bsdd.buildingsmart.org/#concept/details/1P$J7BP319XvA_F1$sO9sN"@en ;
                                           rdfs:label "Residual Current Switch"@en ,
                                                      "reststrømsbryter"@nb-no ;
                                           rdfs:seeAlso ifc:IfcProtectiveDeviceEnumType .


###  http://pi.pauwel.be/voc/distributionelement#ProtectiveDevice-VARISTOR
mep:ProtectiveDevice-VARISTOR rdf:type owl:Class ;
                              rdfs:subClassOf mep:ProtectiveDevice ;
                              rdfs:comment "a high voltage surge protection device"@en ,
                                           "a high voltage surge protection device"@en-gb ,
                                           "http://bsdd.buildingsmart.org/#concept/details/3DtLJ1DjT4LOUFArBkjO_e"@en ;
                              rdfs:label "Varistor"@en ,
                                         "varistor"@nb-no ;
                              rdfs:seeAlso ifc:IfcProtectiveDeviceEnumType .


###  http://pi.pauwel.be/voc/distributionelement#ProtectiveDeviceTrippingUnit
mep:ProtectiveDeviceTrippingUnit rdf:type owl:Class ;
                                 rdfs:subClassOf mep:DistributionControlElement ;
                                 rdfs:comment "A protective device breaks an electrical circuit at a separate breaking unit when a stated electric current that passes through the unit is exceeded."@en ,
                                              "http://bsdd.buildingsmart.org/#concept/details/2XAj9nULf1_vBAY_PiQTNv"@en ;
                                 rdfs:label "Protective Device Tripping Unit"@en ,
                                            "Sicherungsschalter"@de-de ,
                                            "Unité de déclenchement d'équipement de protection"@fr-fr ,
                                            "beskyttende aktiveringsenhet"@nb-no ;
                                 rdfs:seeAlso ifc:IfcProtectiveDeviceTrippingUnit .


###  http://pi.pauwel.be/voc/distributionelement#ProtectiveDeviceTrippingUnit-ELECTROMAGNETIC
mep:ProtectiveDeviceTrippingUnit-ELECTROMAGNETIC rdf:type owl:Class ;
                                                 rdfs:subClassOf mep:ProtectiveDeviceTrippingUnit ;
                                                 rdfs:comment "a tripping unit activated by electromagnetic action"@en ,
                                                              "a tripping unit activated by electromagnetic action"@en-gb ,
                                                              "http://bsdd.buildingsmart.org/#concept/details/1snzfjLSb6VxQ6A4KikKSh"@en ;
                                                 rdfs:label "Electro-magnetic"@en ,
                                                            "elektromagnetisk"@nb-no ;
                                                 rdfs:seeAlso ifc:IfcProtectiveDeviceTrippingUnitEnumType .


###  http://pi.pauwel.be/voc/distributionelement#ProtectiveDeviceTrippingUnit-ELECTRONIC
mep:ProtectiveDeviceTrippingUnit-ELECTRONIC rdf:type owl:Class ;
                                            rdfs:subClassOf mep:ProtectiveDeviceTrippingUnit ;
                                            rdfs:comment "a tripping unit activated by electronic action"@en ,
                                                         "a tripping unit activated by electronic action"@en-gb ,
                                                         "http://bsdd.buildingsmart.org/#concept/details/3LipcBG$z8SuRRCttfOFHZ"@en ;
                                            rdfs:label "Electronic"@en ,
                                                       "elektronisk"@nb-no ;
                                            rdfs:seeAlso ifc:IfcProtectiveDeviceTrippingUnitEnumType .


###  http://pi.pauwel.be/voc/distributionelement#ProtectiveDeviceTrippingUnit-RESIDUALCURRENT
mep:ProtectiveDeviceTrippingUnit-RESIDUALCURRENT rdf:type owl:Class ;
                                                 rdfs:subClassOf mep:ProtectiveDeviceTrippingUnit ;
                                                 rdfs:comment "a tripping unit activated by residual current detection."@en ,
                                                              "http://bsdd.buildingsmart.org/#concept/details/09h4iCV3XArhCUFOXrUJzB"@en ;
                                                 rdfs:label "Residual Current"@en ,
                                                            "jording"@nb-no ;
                                                 rdfs:seeAlso ifc:IfcProtectiveDeviceTrippingUnitEnumType .


###  http://pi.pauwel.be/voc/distributionelement#ProtectiveDeviceTrippingUnit-THERMAL
mep:ProtectiveDeviceTrippingUnit-THERMAL rdf:type owl:Class ;
                                         rdfs:subClassOf mep:ProtectiveDeviceTrippingUnit ;
                                         rdfs:comment "a tripping unit activated by thermal action"@en ,
                                                      "a tripping unit activated by thermal action"@en-gb ,
                                                      "http://bsdd.buildingsmart.org/#concept/details/1xk5ZOrXj7hxv7ViGvtyU$"@en ;
                                         rdfs:label "Thermal"@en ,
                                                    "termisk aktiveringsenhet"@nb-no ;
                                         rdfs:seeAlso ifc:IfcProtectiveDeviceTrippingUnitEnumType .


###  http://pi.pauwel.be/voc/distributionelement#Pump
mep:Pump rdf:type owl:Class ;
         rdfs:subClassOf mep:FlowMovingDevice ;
         rdfs:comment "A device which imparts mechanical work on fluids to move them through a channel or pipe. "@en ,
                      "An equipment driven by a prime mover in which energy is either constantly or periodically added to an amount of pumped liquid in order to increase the pressure requiered for the process in which the pump is in operation.        "@en ,
                      "http://bsdd.buildingsmart.org/#concept/details/1xPUW0qVuHuO00025QrE$V"@en ;
         rdfs:label "Pump"@en ,
                    "Pumpe"@da ,
                    "Pumpe"@de-de ,
                    "pomp"@nl-nl ,
                    "pompe"@fr-fr ,
                    "pump"@en ,
                    "pumpe"@nb-no ;
         rdfs:seeAlso ifc:IfcPump .


###  http://pi.pauwel.be/voc/distributionelement#Pump-CIRCULATOR
mep:Pump-CIRCULATOR rdf:type owl:Class ;
                    rdfs:subClassOf mep:Pump ;
                    rdfs:comment "a circulator pump is a generic low-pressure, low-capacity pump. it may have a wet rotor and may be driven by a flexible-coupled motor"@en ,
                                 "a circulator pump is a generic low-pressure, low-capacity pump. it may have a wet rotor and may be driven by a flexible-coupled motor"@en-gb ,
                                 "http://bsdd.buildingsmart.org/#concept/details/3FNSRucOX3Mfl_kibtqQRr"@en ;
                    rdfs:label "Circulator Pump"@en ,
                               "sirkulasjonspumpe"@nb-no ;
                    rdfs:seeAlso ifc:IfcPumpEnumType .


###  http://pi.pauwel.be/voc/distributionelement#Pump-ENDSUCTION
mep:Pump-ENDSUCTION rdf:type owl:Class ;
                    rdfs:subClassOf mep:Pump ;
                    rdfs:comment "an end suction pump, when mounted horizontally, has a single horizontal inlet on the impeller suction side and a vertical discharge. it may have a direct or close-coupled motor"@en ,
                                 "an end suction pump, when mounted horizontally, has a single horizontal inlet on the impeller suction side and a vertical discharge. it may have a direct or close-coupled motor"@en-gb ,
                                 "http://bsdd.buildingsmart.org/#concept/details/10iAdjK6fEqxsxJnj_WSZS"@en ;
                    rdfs:label "End Suction Pump"@en ,
                               "aksialt innløp"@nb-no ;
                    rdfs:seeAlso ifc:IfcPumpEnumType .


###  http://pi.pauwel.be/voc/distributionelement#Pump-SPLITCASE
mep:Pump-SPLITCASE rdf:type owl:Class ;
                   rdfs:subClassOf mep:Pump ;
                   rdfs:comment "a split case pump, when mounted horizontally, has an inlet and outlet on each side of the impeller. the impeller can be easily accessed by removing the front of the impeller casing. It may have a direct or close-coupled motor"@en ,
                                "a split case pump, when mounted horizontally, has an inlet and outlet on each side of the impeller. the impeller can be easily accessed by removing the front of the impeller casing. It may have a direct or close-coupled motor"@en-gb ,
                                "http://bsdd.buildingsmart.org/#concept/details/3HSu1GQ8T9gQrSbYugJB2f"@en ;
                   rdfs:label "Split Case Pump"@en ,
                              "splitcase pumpe"@nb-no ;
                   rdfs:seeAlso ifc:IfcPumpEnumType .


###  http://pi.pauwel.be/voc/distributionelement#Pump-SUBMERSIBLEPUMP
mep:Pump-SUBMERSIBLEPUMP rdf:type owl:Class ;
                         rdfs:subClassOf mep:Pump ;
                         rdfs:comment "http://bsdd.buildingsmart.org/#concept/details/0rpKGArwf1S8H9bk1lkPiT"@en ;
                         rdfs:label "Submersible Pump"@en ;
                         rdfs:seeAlso ifc:IfcPumpEnumType .


###  http://pi.pauwel.be/voc/distributionelement#Pump-SUMPPUMP
mep:Pump-SUMPPUMP rdf:type owl:Class ;
                  rdfs:subClassOf mep:Pump ;
                  rdfs:comment "a pump designed to sit above a collection tank with a suction inlet extending into the tank"@en ,
                               "a pump designed to sit above a collection tank with a suction inlet extending into the tank"@en-gb ,
                               "http://bsdd.buildingsmart.org/#concept/details/2WUDpiKfDE5u4DZMLBdExr"@en ;
                  rdfs:label "Sump Pump"@en ,
                             "tørroppstilt pumpe"@nb-no ;
                  rdfs:seeAlso ifc:IfcPumpEnumType .


###  http://pi.pauwel.be/voc/distributionelement#Pump-VERTICALINLINE
mep:Pump-VERTICALINLINE rdf:type owl:Class ;
                        rdfs:subClassOf mep:Pump ;
                        rdfs:comment "a vertical Inline pump has the pump and motor close-coupled on the pump casing. the pump depends on the connected, horizontal piping for support, with the suction and discharge along the piping axis"@en ,
                                     "a vertical Inline pump has the pump and motor close-coupled on the pump casing. the pump depends on the connected, horizontal piping for support, with the suction and discharge along the piping axis"@en-gb ,
                                     "http://bsdd.buildingsmart.org/#concept/details/0J3vLYrIDCfQEZZ8ZeRATw"@en ,
                                     "http://bsdd.buildingsmart.org/#concept/details/0VvmpeacrFf8rnDj2jyghe"@en ;
                        rdfs:label "Vertical Inline"@en ,
                                   "vertikallinje"@nb-no ;
                        rdfs:seeAlso ifc:IfcPumpEnumType .


###  http://pi.pauwel.be/voc/distributionelement#Pump-VERTICALTURBINE
mep:Pump-VERTICALTURBINE rdf:type owl:Class ;
                         rdfs:subClassOf mep:Pump ;
                         rdfs:comment "a vertical turbine pump has a motor mounted vertically on the pump casing for either wet-pit sump mounting or dry-well mounting"@en ,
                                      "a vertical turbine pump has a motor mounted vertically on the pump casing for either wet-pit sump mounting or dry-well mounting"@en-gb ,
                                      "http://bsdd.buildingsmart.org/#concept/details/3Ld4kSekL8MOEqs2litt5v"@en ;
                         rdfs:label "Vertical Turbine"@en ,
                                    "vertikalpumpe"@nb-no ;
                         rdfs:seeAlso ifc:IfcPumpEnumType .


###  http://pi.pauwel.be/voc/distributionelement#SanitaryTerminal
mep:SanitaryTerminal rdf:type owl:Class ;
                     rdfs:subClassOf mep:FlowTerminal ;
                     rdfs:comment "A fixed appliance or terminal usually supplied with water and used for drinking, cleaning or foul water disposal or that is an item of equipment directly used with such an appliance or terminal."@en ,
                                  "http://bsdd.buildingsmart.org/#concept/details/2JIcddz_X75xhHc1XUv7d2"@en ;
                     rdfs:label "Equipement sanitaire"@fr-fr ,
                                "Sanitair toestel"@nl-nl ,
                                "Sanitary Terminal"@en ,
                                "Sanitäreinrichtung"@de-de ,
                                "sanitærstasjon"@nb-no ;
                     rdfs:seeAlso ifc:IfcSanitaryTerminal .


###  http://pi.pauwel.be/voc/distributionelement#SanitaryTerminal-BATH
mep:SanitaryTerminal-BATH rdf:type owl:Class ;
                          rdfs:subClassOf mep:SanitaryTerminal ;
                          rdfs:comment "Badekar"@nb-no ,
                                       "Badekar, generisk, modelleres av ARK i tidlig fase"@nb-no ,
                                       "Sanitärobjekt, das der persönlichen Hygiene, vorzugsweise dem Baden und vollständigen Reinigen des menschlichen Körpers dient und mit das Wasser nach dem Gebrauch über ein Ablaufloch abgeleitet werden kann"@de-de ,
                                       "badekar, generisk, arkitekttegnede modeller i tidlige designfaser"@dk-dk ,
                                       "badkar, allmänt, arkitektens modeller under utformningens första steg"@sv-se ,
                                       "baignoire, générique, modeles par l'architecte dans les premières étapes de la conception"@fr-fr ,
                                       "http://bsdd.buildingsmart.org/#concept/details/3obubztQ19OANL1cKUM33Z"@en ,
                                       "sanitary appliance used for partial immersion and washing of the human body or parts of it, and for directing water to a waste outlet after use"@en ,
                                       "sanitary appliance used for partial immersion and washing of the human body or parts of it, and for directing water to a waste outlet after use"@en-gb ,
                                       "sanitærinnretning som brukes for delvis nedsenking og vasking av menneskekropp eller deler av den, og for å lede vann til et avløp etter bruk"@nb-no ,
                                       "varhaisten arkkitehtisuunnitteluvaiheiden yleismalliset kylpyammeet"@fi-fi ;
                          rdfs:label "Badewanne"@de-de ,
                                     "Bath"@en ,
                                     "bad"@dk-dk ,
                                     "bad"@nb-no ,
                                     "bad"@nl-nl ,
                                     "bad"@sv-se ,
                                     "badekar"@nb-no ,
                                     "badekar generisk"@nb-no ,
                                     "baignoire"@fr-fr ,
                                     "bath"@en-gb ,
                                     "bathtub"@en ,
                                     "kylpyamme"@fi-fi ,
                                     "wanna"@pl-pl ;
                          rdfs:seeAlso ifc:IfcSanitaryTerminalEnumType .


###  http://pi.pauwel.be/voc/distributionelement#SanitaryTerminal-BIDET
mep:SanitaryTerminal-BIDET rdf:type owl:Class ;
                           rdfs:subClassOf mep:SanitaryTerminal ;
                           rdfs:comment "Waste water appliance for washing the excretory organs while sitting astride the bowl"@en-gb ,
                                        "http://bsdd.buildingsmart.org/#concept/details/1OsGeXUlz249AKQbE4k_3S"@en ,
                                        "waste water appliance for washing the excretory organs while sitting astride the bowl"@en ;
                           rdfs:label "Bidet"@en ,
                                      "bidè"@nb-no ,
                                      "bidé"@nb-no ;
                           rdfs:seeAlso ifc:IfcSanitaryTerminalEnumType .


###  http://pi.pauwel.be/voc/distributionelement#SanitaryTerminal-CISTERN
mep:SanitaryTerminal-CISTERN rdf:type owl:Class ;
                             rdfs:subClassOf mep:SanitaryTerminal ;
                             rdfs:comment "A water storage unit attached to a sanitary terminal that is fitted with a device, operated automatically or by the user, that discharges water to cleanse a water closet (toilet) pan, urinal or slop hopper"@en ,
                                          "A water storage unit attached to a sanitary terminal that is fitted with a device, operated automatically or by the user, that discharges water to cleanse a water closet (toilet) pan, urinal or slop hopper"@en-gb ,
                                          "http://bsdd.buildingsmart.org/#concept/details/2jTiagbH96wBuf5tVceOCR"@en ;
                             rdfs:label "Cistern"@en ,
                                        "sisterne"@nb-no ;
                             rdfs:seeAlso ifc:IfcSanitaryTerminalEnumType .


###  http://pi.pauwel.be/voc/distributionelement#SanitaryTerminal-SANITARYFOUNTAIN
mep:SanitaryTerminal-SANITARYFOUNTAIN rdf:type owl:Class ;
                                      rdfs:subClassOf mep:SanitaryTerminal ;
                                      rdfs:comment "http://bsdd.buildingsmart.org/#concept/details/3sjNvgHdPAH8fM1jgV3823"@en ;
                                      rdfs:label "Sanitary Fountain"@en ,
                                                 "drikkefontene"@nb-no ;
                                      rdfs:seeAlso ifc:IfcSanitaryTerminalEnumType .


###  http://pi.pauwel.be/voc/distributionelement#SanitaryTerminal-SHOWER
mep:SanitaryTerminal-SHOWER rdf:type owl:Class ;
                            rdfs:subClassOf mep:SanitaryTerminal ;
                            rdfs:comment "Dusj beskyttet med kabinett"@nb-no ,
                                         "Dusjhjørne"@nb-no ,
                                         "Shower installed in its own cabinet"@en ,
                                         "http://bsdd.buildingsmart.org/#concept/details/0epJRcLij1_O8OcMA6Y0WR"@en ;
                            rdfs:label "Shower"@en ,
                                       "dusj"@nb-no ,
                                       "dusjhjørne"@nb-no ,
                                       "dusjkabinett"@nb-no ,
                                       "shower cabinet"@en ;
                            rdfs:seeAlso ifc:IfcSanitaryTerminalEnumType .


###  http://pi.pauwel.be/voc/distributionelement#SanitaryTerminal-SINK
mep:SanitaryTerminal-SINK rdf:type owl:Class ;
                          rdfs:subClassOf mep:SanitaryTerminal ;
                          rdfs:comment "Servant"@nb-no ,
                                       "Servant, generisk, modelleres av ARK i tidlig fase"@nb-no ,
                                       "Vanlig stor"@nb-no ,
                                       "beholder for vann under kran til vasking av hender og ansikt"@nb-no ,
                                       "container for water located below water dispenser, used for washing hands and face"@en ,
                                       "http://bsdd.buildingsmart.org/#concept/details/1SP1BV0Wj9lf1y$D1yvjLF"@en ;
                          rdfs:label "Sink"@en ,
                                     "kjøkken"@nb-no ,
                                     "servant"@nb-no ,
                                     "servant generisk"@nb-no ,
                                     "utslagsvask"@nb-no ,
                                     "vask"@nb-no ,
                                     "wash basin"@en ;
                          rdfs:seeAlso ifc:IfcSanitaryTerminalEnumType .


###  http://pi.pauwel.be/voc/distributionelement#SanitaryTerminal-TOILETPAN
mep:SanitaryTerminal-TOILETPAN rdf:type owl:Class ;
                               rdfs:subClassOf mep:SanitaryTerminal ;
                               rdfs:comment "http://bsdd.buildingsmart.org/#concept/details/2DXU$3jIrFROZFEhM3vmoY"@en ,
                                            "soil appliance for the disposal of excrement"@en ,
                                            "soil appliance for the disposal of excrement"@en-gb ;
                               rdfs:label "Toilet Pan"@en ,
                                          "toalettskål"@nb-no ;
                               rdfs:seeAlso ifc:IfcSanitaryTerminalEnumType .


###  http://pi.pauwel.be/voc/distributionelement#SanitaryTerminal-URINAL
mep:SanitaryTerminal-URINAL rdf:type owl:Class ;
                            rdfs:subClassOf mep:SanitaryTerminal ;
                            rdfs:comment "http://bsdd.buildingsmart.org/#concept/details/2B1zvMQAv9pPzzlnNtd5xA"@en ,
                                         "soil appliance that receives urine and directs it to a waste outlet"@en ,
                                         "soil appliance that receives urine and directs it to a waste outlet"@en-gb ;
                            rdfs:label "Urinal"@en ,
                                       "urinal"@nb-no ;
                            rdfs:seeAlso ifc:IfcSanitaryTerminalEnumType .


###  http://pi.pauwel.be/voc/distributionelement#SanitaryTerminal-WASHHANDBASIN
mep:SanitaryTerminal-WASHHANDBASIN rdf:type owl:Class ;
                                   rdfs:subClassOf mep:SanitaryTerminal ;
                                   rdfs:comment "http://bsdd.buildingsmart.org/#concept/details/2FTLxQE_19NPX9OHQSeAff"@en ,
                                                "waste water appliance for washing the upper parts of the body"@en ,
                                                "waste water appliance for washing the upper parts of the body"@en-gb ;
                                   rdfs:label "Wash Hand Basin"@en ,
                                              "håndvask"@nb-no ;
                                   rdfs:seeAlso ifc:IfcSanitaryTerminalEnumType .


###  http://pi.pauwel.be/voc/distributionelement#SanitaryTerminal-WCSEAT
mep:SanitaryTerminal-WCSEAT rdf:type owl:Class ;
                            rdfs:subClassOf mep:SanitaryTerminal ;
                            rdfs:comment "hinged seat that fits on the top of a water closet (WC) pan"@en ,
                                         "hinged seat that fits on the top of a water closet (WC) pan"@en-gb ,
                                         "http://bsdd.buildingsmart.org/#concept/details/12WSI21rv3UfKISz44T3B5"@en ;
                            rdfs:label "WC Seat"@en ,
                                       "toalettsete"@nb-no ;
                            rdfs:seeAlso ifc:IfcSanitaryTerminalEnumType .


###  http://pi.pauwel.be/voc/distributionelement#Sensor
mep:Sensor rdf:type owl:Class ;
           rdfs:subClassOf mep:DistributionControlElement ;
           rdfs:comment "A device that measures a physical quantity and converts it into a signal which can be read by an observer or by an instrument."@en ,
                        "http://bsdd.buildingsmart.org/#concept/details/0fBybaDK56PuAX2mD3nQsg"@en ;
           rdfs:label "Capteur"@fr-fr ,
                      "Sensor"@de-de ,
                      "Sensor"@en ,
                      "sensor"@nb-no ,
                      "sensor"@nl-nl ;
           rdfs:seeAlso ifc:IfcSensor .


###  http://pi.pauwel.be/voc/distributionelement#Sensor-CO2SENSOR
mep:Sensor-CO2SENSOR rdf:type owl:Class ;
                     rdfs:subClassOf mep:Sensor ;
                     rdfs:label "CO2Sensor"@en ;
                     rdfs:seeAlso ifc:IfcSensorEnumType .


###  http://pi.pauwel.be/voc/distributionelement#Sensor-CONDUCTANCESENSOR
mep:Sensor-CONDUCTANCESENSOR rdf:type owl:Class ;
                             rdfs:subClassOf mep:Sensor ;
                             rdfs:comment "http://bsdd.buildingsmart.org/#concept/details/3B3V_G55z9nPyFZOVtZKu9"@en ;
                             rdfs:label "Conductance Sensor"@en ;
                             rdfs:seeAlso ifc:IfcSensorEnumType .


###  http://pi.pauwel.be/voc/distributionelement#Sensor-CONTACTSENSOR
mep:Sensor-CONTACTSENSOR rdf:type owl:Class ;
                         rdfs:subClassOf mep:Sensor ;
                         rdfs:comment "http://bsdd.buildingsmart.org/#concept/details/37ufVjEi1BZwCCYTaYZdgK"@en ;
                         rdfs:label "Contact Sensor"@en ;
                         rdfs:seeAlso ifc:IfcSensorEnumType .


###  http://pi.pauwel.be/voc/distributionelement#Sensor-FIRESENSOR
mep:Sensor-FIRESENSOR rdf:type owl:Class ;
                      rdfs:subClassOf mep:Sensor ;
                      rdfs:comment "http://bsdd.buildingsmart.org/#concept/details/1uUUJfLpX03uy3ZC8j0YXd"@en ;
                      rdfs:label "Fire Sensor"@en ;
                      rdfs:seeAlso ifc:IfcSensorEnumType .


###  http://pi.pauwel.be/voc/distributionelement#Sensor-FLOWSENSOR
mep:Sensor-FLOWSENSOR rdf:type owl:Class ;
                      rdfs:subClassOf mep:Sensor ;
                      rdfs:comment "http://bsdd.buildingsmart.org/#concept/details/0uovCUrpn9leYila3fCeEN"@en ;
                      rdfs:label "Flow Sensor"@en ;
                      rdfs:seeAlso ifc:IfcSensorEnumType .


###  http://pi.pauwel.be/voc/distributionelement#Sensor-FROSTSENSOR
mep:Sensor-FROSTSENSOR rdf:type owl:Class ;
                       rdfs:subClassOf mep:Sensor ;
                       rdfs:label "Frost Sensor"@en ;
                       rdfs:seeAlso ifc:IfcSensorEnumType .


###  http://pi.pauwel.be/voc/distributionelement#Sensor-GASSENSOR
mep:Sensor-GASSENSOR rdf:type owl:Class ;
                     rdfs:subClassOf mep:Sensor ;
                     rdfs:comment "http://bsdd.buildingsmart.org/#concept/details/2EQoz$FyT5_wpwhtQt6Bt2"@en ;
                     rdfs:label "Gas Sensor"@en ;
                     rdfs:seeAlso ifc:IfcSensorEnumType .


###  http://pi.pauwel.be/voc/distributionelement#Sensor-HEATSENSOR
mep:Sensor-HEATSENSOR rdf:type owl:Class ;
                      rdfs:subClassOf mep:Sensor ;
                      rdfs:comment "http://bsdd.buildingsmart.org/#concept/details/3Op4_nqmj6L96LAusX1Ytq"@en ;
                      rdfs:label "Heat Sensor"@en ;
                      rdfs:seeAlso ifc:IfcSensorEnumType .


###  http://pi.pauwel.be/voc/distributionelement#Sensor-HUMIDITYSENSOR
mep:Sensor-HUMIDITYSENSOR rdf:type owl:Class ;
                          rdfs:subClassOf mep:Sensor ;
                          rdfs:comment "http://bsdd.buildingsmart.org/#concept/details/3Pza_zqrDAwg4Pv44MusVg"@en ;
                          rdfs:label "Humidity Sensor"@en ;
                          rdfs:seeAlso ifc:IfcSensorEnumType .


###  http://pi.pauwel.be/voc/distributionelement#Sensor-IDENTIFIERSENSOR
mep:Sensor-IDENTIFIERSENSOR rdf:type owl:Class ;
                            rdfs:subClassOf mep:Sensor ;
                            rdfs:label "Identifier Sensor"@en ;
                            rdfs:seeAlso ifc:IfcSensorEnumType .


###  http://pi.pauwel.be/voc/distributionelement#Sensor-IONCONCENTRATIONSENSOR
mep:Sensor-IONCONCENTRATIONSENSOR rdf:type owl:Class ;
                                  rdfs:subClassOf mep:Sensor ;
                                  rdfs:comment "http://bsdd.buildingsmart.org/#concept/details/2MglfdfcTCuhCN57KBKgPd"@en ;
                                  rdfs:label "Ion Concentration Sensor"@en ;
                                  rdfs:seeAlso ifc:IfcSensorEnumType .


###  http://pi.pauwel.be/voc/distributionelement#Sensor-LEVELSENSOR
mep:Sensor-LEVELSENSOR rdf:type owl:Class ;
                       rdfs:subClassOf mep:Sensor ;
                       rdfs:comment "http://bsdd.buildingsmart.org/#concept/details/2zHVmDmGT6zBRJIAqmQdkK"@en ;
                       rdfs:label "Level Sensor"@en ;
                       rdfs:seeAlso ifc:IfcSensorEnumType .


###  http://pi.pauwel.be/voc/distributionelement#Sensor-LIGHTSENSOR
mep:Sensor-LIGHTSENSOR rdf:type owl:Class ;
                       rdfs:subClassOf mep:Sensor ;
                       rdfs:comment "http://bsdd.buildingsmart.org/#concept/details/3Y5B9ubBb0xxK9qw_nEkEk"@en ;
                       rdfs:label "Light Sensor"@en ;
                       rdfs:seeAlso ifc:IfcSensorEnumType .


###  http://pi.pauwel.be/voc/distributionelement#Sensor-MOISTURESENSOR
mep:Sensor-MOISTURESENSOR rdf:type owl:Class ;
                          rdfs:subClassOf mep:Sensor ;
                          rdfs:comment "http://bsdd.buildingsmart.org/#concept/details/1LnA01HA5E7fPuuXLI2ZjZ"@en ;
                          rdfs:label "Moisture Sensor"@en ;
                          rdfs:seeAlso ifc:IfcSensorEnumType .


###  http://pi.pauwel.be/voc/distributionelement#Sensor-MOVEMENTSENSOR
mep:Sensor-MOVEMENTSENSOR rdf:type owl:Class ;
                          rdfs:subClassOf mep:Sensor ;
                          rdfs:comment "http://bsdd.buildingsmart.org/#concept/details/2$qvwDkgL0VRFBeuD9w9Si"@en ;
                          rdfs:label "Movement Sensor"@en ;
                          rdfs:seeAlso ifc:IfcSensorEnumType .


###  http://pi.pauwel.be/voc/distributionelement#Sensor-PHSENSOR
mep:Sensor-PHSENSOR rdf:type owl:Class ;
                    rdfs:subClassOf mep:Sensor ;
                    rdfs:comment "http://bsdd.buildingsmart.org/#concept/details/3lwBxJbnL9DAvFoYtIB3Li"@en ;
                    rdfs:label "PH-Sensor"@en ;
                    rdfs:seeAlso ifc:IfcSensorEnumType .


###  http://pi.pauwel.be/voc/distributionelement#Sensor-PRESSURESENSOR
mep:Sensor-PRESSURESENSOR rdf:type owl:Class ;
                          rdfs:subClassOf mep:Sensor ;
                          rdfs:comment "http://bsdd.buildingsmart.org/#concept/details/2RKICtIin2Rw5EFR0Z2J9j"@en ;
                          rdfs:label "Pressure Sensor"@en ;
                          rdfs:seeAlso ifc:IfcSensorEnumType .


###  http://pi.pauwel.be/voc/distributionelement#Sensor-RADIATIONSENSOR
mep:Sensor-RADIATIONSENSOR rdf:type owl:Class ;
                           rdfs:subClassOf mep:Sensor ;
                           rdfs:comment "http://bsdd.buildingsmart.org/#concept/details/3OXFVvFvPCePgxMcTylRzf"@en ;
                           rdfs:label "Radiation Sensor"@en ;
                           rdfs:seeAlso ifc:IfcSensorEnumType .


###  http://pi.pauwel.be/voc/distributionelement#Sensor-RADIOACTIVITYSENSOR
mep:Sensor-RADIOACTIVITYSENSOR rdf:type owl:Class ;
                               rdfs:subClassOf mep:Sensor ;
                               rdfs:comment "http://bsdd.buildingsmart.org/#concept/details/0wp1vLqNP9Lef8Pba4UI6P"@en ;
                               rdfs:label "Radioactivity Sensor"@en ;
                               rdfs:seeAlso ifc:IfcSensorEnumType .


###  http://pi.pauwel.be/voc/distributionelement#Sensor-SMOKESENSOR
mep:Sensor-SMOKESENSOR rdf:type owl:Class ;
                       rdfs:subClassOf mep:Sensor ;
                       rdfs:comment "http://bsdd.buildingsmart.org/#concept/details/05gekqn$D9nA81S2HC8u1E"@en ;
                       rdfs:label "Smoke Sensor"@en ;
                       rdfs:seeAlso ifc:IfcSensorEnumType .


###  http://pi.pauwel.be/voc/distributionelement#Sensor-SOUNDSENSOR
mep:Sensor-SOUNDSENSOR rdf:type owl:Class ;
                       rdfs:subClassOf mep:Sensor ;
                       rdfs:comment "http://bsdd.buildingsmart.org/#concept/details/0OvllOM7fDC8GX67w3ESF6"@en ;
                       rdfs:label "Sound Sensor"@en ;
                       rdfs:seeAlso ifc:IfcSensorEnumType .


###  http://pi.pauwel.be/voc/distributionelement#Sensor-TEMPERATURESENSOR
mep:Sensor-TEMPERATURESENSOR rdf:type owl:Class ;
                             rdfs:subClassOf mep:Sensor ;
                             rdfs:comment "http://bsdd.buildingsmart.org/#concept/details/2SmjV_2JXB4wdmD4Bzr$BP"@en ;
                             rdfs:label "Temperature Sensor"@en ;
                             rdfs:seeAlso ifc:IfcSensorEnumType .


###  http://pi.pauwel.be/voc/distributionelement#Sensor-WINDSENSOR
mep:Sensor-WINDSENSOR rdf:type owl:Class ;
                      rdfs:subClassOf mep:Sensor ;
                      rdfs:comment "http://bsdd.buildingsmart.org/#concept/details/1hMN0c8Rj5dw$7eow$VjWU"@en ;
                      rdfs:label "Wind Sensor"@en ;
                      rdfs:seeAlso ifc:IfcSensorEnumType .


###  http://pi.pauwel.be/voc/distributionelement#SolarDevice
mep:SolarDevice rdf:type owl:Class ;
                rdfs:subClassOf mep:EnergyConversionDevice ;
                rdfs:comment "A device converts solar radiation into other energy such as electric current or thermal energy."@en ,
                             "http://bsdd.buildingsmart.org/#concept/details/10kbcLuh91TeNXCNVtFC6g"@en ;
                rdfs:label "Solar Device"@en ,
                           "Solargerät"@de-de ,
                           "capteur solaire"@fr-fr ,
                           "solenergienhet"@nb-no ;
                rdfs:seeAlso ifc:IfcSolarDevice .


###  http://pi.pauwel.be/voc/distributionelement#SolarDevice-SOLARCOLLECTOR
mep:SolarDevice-SOLARCOLLECTOR rdf:type owl:Class ;
                               rdfs:subClassOf mep:SolarDevice ;
                               rdfs:comment "http://bsdd.buildingsmart.org/#concept/details/0fo0nZHmT5twFp0u9haG2I"@en ;
                               rdfs:label "Solar Collector"@en ;
                               rdfs:seeAlso ifc:IfcSolarDeviceEnumType .


###  http://pi.pauwel.be/voc/distributionelement#SolarDevice-SOLARPANEL
mep:SolarDevice-SOLARPANEL rdf:type owl:Class ;
                           rdfs:subClassOf mep:SolarDevice ;
                           rdfs:comment "a device that converts solar radiation into electric current"@en ,
                                        "a device that converts solar radiation into electric current"@en-gb ,
                                        "http://bsdd.buildingsmart.org/#concept/details/2S$Xvvjqn1GAvVFoENZhtk"@en ;
                           rdfs:label "Solar Panel"@en ,
                                      "solpanel"@nb-no ;
                           rdfs:seeAlso ifc:IfcSolarDeviceEnumType .


###  http://pi.pauwel.be/voc/distributionelement#SpaceHeater
mep:SpaceHeater rdf:type owl:Class ;
                rdfs:subClassOf mep:FlowTerminal ;
                rdfs:comment "Heaters utilize a combination of radiation and/or natural convection using a heating source such as electricity, steam or hot water to heat a limited space or area. Examples of space heaters include radiators, convectors, baseboard and finned-tube heaters."@en ,
                             "http://bsdd.buildingsmart.org/#concept/details/39lbLJ2412vOKf6Cp8ojJd"@en ;
                rdfs:label "Heizkörper"@de-de ,
                           "Space Heater"@en ,
                           "heater"@en ,
                           "kachel"@nl-nl ,
                           "local heating device"@en ,
                           "lokaal verwarmingstoestel"@nl-nl ,
                           "radiateur"@fr-fr ,
                           "ruimteverwarmingstoestel"@nl-nl ,
                           "varmeenhet"@nb-no ;
                rdfs:seeAlso ifc:IfcSpaceHeater .


###  http://pi.pauwel.be/voc/distributionelement#SpaceHeater-CONVECTOR
mep:SpaceHeater-CONVECTOR rdf:type owl:Class ;
                          rdfs:subClassOf mep:SpaceHeater ;
                          rdfs:comment "a heating appliance which emits heat almost entirely by convection. a convector comprises at least a heat emitter and a casing which provides an unheated convective chimney of defined height."@en ,
                                       "http://bsdd.buildingsmart.org/#concept/details/0kMkKT22f00BAkHfSQ7c_B"@en ;
                          rdfs:label "Convector"@en ,
                                     "Convector"@nl-nl ,
                                     "konvektor"@nb-no ,
                                     "varmekonvektor"@nb-no ;
                          rdfs:seeAlso ifc:IfcSpaceHeaterEnumType .


###  http://pi.pauwel.be/voc/distributionelement#SpaceHeater-RADIATOR
mep:SpaceHeater-RADIATOR rdf:type owl:Class ;
                         rdfs:subClassOf mep:SpaceHeater ;
                         rdfs:comment "a heat appliance which emits heat by free convection and radiation"@en ,
                                      "http://bsdd.buildingsmart.org/#concept/details/38a4eei5j5vQs7YtSb7quf"@en ;
                         rdfs:label "Heizkörper"@de-de ,
                                    "Radiator"@de-de ,
                                    "Radiator"@en ,
                                    "radiateur"@fr-fr ,
                                    "radiator"@nb-no ,
                                    "varmelegeme"@nb-no ;
                         rdfs:seeAlso ifc:IfcSpaceHeaterEnumType .


###  http://pi.pauwel.be/voc/distributionelement#StackTerminal
mep:StackTerminal rdf:type owl:Class ;
                  rdfs:subClassOf mep:FlowTerminal ;
                  rdfs:comment "A terminal placed at the top of a ventilating stack (such as to prevent ingress by birds or rainwater) or rainwater pipe (to act as a collector or hopper for discharge from guttering)."@en ,
                               "http://bsdd.buildingsmart.org/#concept/details/0lNPT0EPbBWeJB7HGeHjgH"@en ;
                  rdfs:label "Rohrabdeckung"@de-de ,
                             "Stack Terminal"@en ,
                             "system-terminal"@nb-no ;
                  rdfs:seeAlso ifc:IfcStackTerminal .


###  http://pi.pauwel.be/voc/distributionelement#StackTerminal-BIRDCAGE
mep:StackTerminal-BIRDCAGE rdf:type owl:Class ;
                           rdfs:subClassOf mep:StackTerminal ;
                           rdfs:comment "guard cage, typically wire mesh, at the top of the stack preventing access by birds"@en ,
                                        "guard cage, typically wire mesh, at the top of the stack preventing access by birds"@en-gb ,
                                        "http://bsdd.buildingsmart.org/#concept/details/2yx3o8h5157elNsihhcZZx"@en ;
                           rdfs:label "Birdcage"@en ,
                                      "ventilasjon gitter topp"@nb-no ;
                           rdfs:seeAlso ifc:IfcStackTerminalEnumType .


###  http://pi.pauwel.be/voc/distributionelement#StackTerminal-COWL
mep:StackTerminal-COWL rdf:type owl:Class ;
                       rdfs:subClassOf mep:StackTerminal ;
                       rdfs:comment "air terminal device intended to be installed above a natural ventilation exhaust duct with the aim, by creating negative pressure and depending on wind speed, of avoiding reverse flow and increasing flow rate"@en ,
                                    "http://bsdd.buildingsmart.org/#concept/details/3XIKqh6OnDLvtnQcrmQvo4"@en ;
                       rdfs:label "cowl"@en ,
                                  "hette"@nb-no ,
                                  "vent cap"@en ,
                                  "vent turbine"@en ,
                                  "ventilasjonstopp"@nb-no ;
                       rdfs:seeAlso ifc:IfcStackTerminalEnumType .


###  http://pi.pauwel.be/voc/distributionelement#StackTerminal-RAINWATERHOPPER
mep:StackTerminal-RAINWATERHOPPER rdf:type owl:Class ;
                                  rdfs:subClassOf mep:StackTerminal ;
                                  rdfs:comment "http://bsdd.buildingsmart.org/#concept/details/0tlwEdOcDExuy98lwa6_38"@en ;
                                  rdfs:label "Rainwater Hopper"@en ;
                                  rdfs:seeAlso ifc:IfcStackTerminalEnumType .


###  http://pi.pauwel.be/voc/distributionelement#SwitchingDevice
mep:SwitchingDevice rdf:type owl:Class ;
                    rdfs:subClassOf mep:FlowController ;
                    rdfs:comment "A switch used in a cable distribution system (electrical circuit) to control or modulate the flow of electricity. Include those used for electrical power, communications, audio-visual, or other distribution system types as determined by the available ports."@en ,
                                 "http://bsdd.buildingsmart.org/#concept/details/0JjKezzH55POBG1espn8W$"@en ;
                    rdfs:label "Interrupteur"@fr-fr ,
                               "Schalter"@de-de ,
                               "Switching Device"@en ,
                               "bryter"@nb-no ;
                    rdfs:seeAlso ifc:IfcSwitchingDevice .


###  http://pi.pauwel.be/voc/distributionelement#SwitchingDevice-CONTACTOR
mep:SwitchingDevice-CONTACTOR rdf:type owl:Class ;
                              rdfs:subClassOf mep:SwitchingDevice ;
                              rdfs:comment "http://bsdd.buildingsmart.org/#concept/details/3rxqi3mzn8ovp5j4$AtKpj"@en ,
                                           "mechanical switching device having only one position of rest, operated otherwise than by hand, capable of making, carrying and breaking currents under normal circuit conditions including operating overload conditions"@en ;
                              rdfs:label "Contactor"@en ,
                                         "Contactstop"@nl-nl ,
                                         "kontaktor"@nb-no ;
                              rdfs:seeAlso ifc:IfcSwitchingDeviceEnumType .


###  http://pi.pauwel.be/voc/distributionelement#SwitchingDevice-DIMMERSWITCH
mep:SwitchingDevice-DIMMERSWITCH rdf:type owl:Class ;
                                 rdfs:subClassOf mep:SwitchingDevice ;
                                 rdfs:comment "http://bsdd.buildingsmart.org/#concept/details/2Qsa6P6719HRwY$4OSoDq9"@en ;
                                 rdfs:label "Dimmer Switch"@en ;
                                 rdfs:seeAlso ifc:IfcSwitchingDeviceEnumType .


###  http://pi.pauwel.be/voc/distributionelement#SwitchingDevice-EMERGENCYSTOP
mep:SwitchingDevice-EMERGENCYSTOP rdf:type owl:Class ;
                                  rdfs:subClassOf mep:SwitchingDevice ;
                                  rdfs:comment "http://bsdd.buildingsmart.org/#concept/details/1AkYCx5WrDfQSeajQs4GbK"@en ;
                                  rdfs:label "Emergency Stop"@en ;
                                  rdfs:seeAlso ifc:IfcSwitchingDeviceEnumType .


###  http://pi.pauwel.be/voc/distributionelement#SwitchingDevice-KEYPAD
mep:SwitchingDevice-KEYPAD rdf:type owl:Class ;
                           rdfs:subClassOf mep:SwitchingDevice ;
                           rdfs:comment "http://bsdd.buildingsmart.org/#concept/details/30Wun_rrP3hg09kZxKFSxo"@en ,
                                        "а set of buttons or switches, each potentially applicable to a different device"@en ,
                                        "а set of buttons or switches, each potentially applicable to a different device"@en-gb ;
                           rdfs:label "Keypad"@en ,
                                      "tastatur"@nb-no ;
                           rdfs:seeAlso ifc:IfcSwitchingDeviceEnumType .


###  http://pi.pauwel.be/voc/distributionelement#SwitchingDevice-MOMENTARYSWITCH
mep:SwitchingDevice-MOMENTARYSWITCH rdf:type owl:Class ;
                                    rdfs:subClassOf mep:SwitchingDevice ;
                                    rdfs:comment "http://bsdd.buildingsmart.org/#concept/details/1GXuot6Zv41wgJSbaoN8g7"@en ,
                                                 "а momentary switch has no position, and may trigger some action to occur"@en ,
                                                 "а momentary switch has no position, and may trigger some action to occur"@en-gb ;
                                    rdfs:label "Momentary Switch"@en ,
                                               "momentantbryter"@nb-no ;
                                    rdfs:seeAlso ifc:IfcSwitchingDeviceEnumType .


###  http://pi.pauwel.be/voc/distributionelement#SwitchingDevice-SELECTORSWITCH
mep:SwitchingDevice-SELECTORSWITCH rdf:type owl:Class ;
                                   rdfs:subClassOf mep:SwitchingDevice ;
                                   rdfs:comment "http://bsdd.buildingsmart.org/#concept/details/2WULe4Kq50n8t1M8n_T5Jc"@en ;
                                   rdfs:label "Selector Switch"@en ;
                                   rdfs:seeAlso ifc:IfcSwitchingDeviceEnumType .


###  http://pi.pauwel.be/voc/distributionelement#SwitchingDevice-STARTER
mep:SwitchingDevice-STARTER rdf:type owl:Class ;
                            rdfs:subClassOf mep:SwitchingDevice ;
                            rdfs:comment "http://bsdd.buildingsmart.org/#concept/details/2R7sKp3Zz8EvRVJenaoFA0"@en ,
                                         "а starter is a switch which in the closed position controls the application of power to an electrical device"@en ,
                                         "а starter is a switch which in the closed position controls the application of power to an electrical device"@en-gb ;
                            rdfs:label "Starter"@en ,
                                       "starter"@nb-no ;
                            rdfs:seeAlso ifc:IfcSwitchingDeviceEnumType .


###  http://pi.pauwel.be/voc/distributionelement#SwitchingDevice-SWITCHDISCONNECTOR
mep:SwitchingDevice-SWITCHDISCONNECTOR rdf:type owl:Class ;
                                       rdfs:subClassOf mep:SwitchingDevice ;
                                       rdfs:comment "http://bsdd.buildingsmart.org/#concept/details/2YJHtgvof1aQ6qN28MCYJh"@en ;
                                       rdfs:label "Switch Disconnector"@en ;
                                       rdfs:seeAlso ifc:IfcSwitchingDeviceEnumType .


###  http://pi.pauwel.be/voc/distributionelement#SwitchingDevice-TOGGLESWITCH
mep:SwitchingDevice-TOGGLESWITCH rdf:type owl:Class ;
                                 rdfs:subClassOf mep:SwitchingDevice ;
                                 rdfs:comment "http://bsdd.buildingsmart.org/#concept/details/2OMieHhU5ClBrIpriDbqmz"@en ;
                                 rdfs:label "Toggle Switch"@en ;
                                 rdfs:seeAlso ifc:IfcSwitchingDeviceEnumType .


###  http://pi.pauwel.be/voc/distributionelement#Tank
mep:Tank rdf:type owl:Class ;
         rdfs:subClassOf mep:FlowStorageDevice ;
         rdfs:comment "A vessel or container in which a fluid or gas is stored for later use."@en ,
                      "http://bsdd.buildingsmart.org/#concept/details/2UJCW0qWyHuO00025QrE$V"@en ;
         rdfs:label "Tank"@en ,
                    "réservoir"@fr-fr ,
                    "tank"@nb-no ;
         rdfs:seeAlso ifc:IfcTank .


###  http://pi.pauwel.be/voc/distributionelement#Tank-BASIN
mep:Tank-BASIN rdf:type owl:Class ;
               rdfs:subClassOf mep:Tank ;
               rdfs:comment "an arbitrary open tank type"@en ,
                            "an arbitrary open tank type"@en-gb ,
                            "http://bsdd.buildingsmart.org/#concept/details/2Kr7mfp3HFAfi67PdLwE0L"@en ;
               rdfs:label "Basin"@en ,
                          "servant"@nb-no ,
                          "tank type basseng"@nb-no ;
               rdfs:seeAlso ifc:IfcTankEnumType .


###  http://pi.pauwel.be/voc/distributionelement#Tank-BREAKPRESSURE
mep:Tank-BREAKPRESSURE rdf:type owl:Class ;
                       rdfs:subClassOf mep:Tank ;
                       rdfs:comment "an open container that breaks the hydraulic pressure in a distribution system, typically located between the fluid reservoir and the fluid supply points. a typical break pressure tank allows the flow to discharge into the atmosphere, thereby reducing its hydrostatic pressure to zero"@en ,
                                    "an open container that breaks the hydraulic pressure in a distribution system, typically located between the fluid reservoir and the fluid supply points. a typical break pressure tank allows the flow to discharge into the atmosphere, thereby reducing its hydrostatic pressure to zero"@en-gb ,
                                    "http://bsdd.buildingsmart.org/#concept/details/1uUiVD63rEcPif0cejL9Vx"@en ;
                       rdfs:label "Break Pressure Tank"@en ,
                                  "Bruddtrykk"@nb-no ;
                       rdfs:seeAlso ifc:IfcTankEnumType .


###  http://pi.pauwel.be/voc/distributionelement#Tank-EXPANSION
mep:Tank-EXPANSION rdf:type owl:Class ;
                   rdfs:subClassOf mep:Tank ;
                   rdfs:comment "a closed container used in a closed fluid distribution system to mitigate the effects of thermal expansion or water hammer. the tank is typically constructed with a diaphragm dividing the tank into two sections, with fluid on one side of the diaphragm and air on the other. one example application is when connected to the primary circuit of a hot water system to accommodate the increase in volume of the water when it is heated"@en ,
                                "a closed container used in a closed fluid distribution system to mitigate the effects of thermal expansion or water hammer. the tank is typically constructed with a diaphragm dividing the tank into two sections, with fluid on one side of the diaphragm and air on the other. one example application is when connected to the primary circuit of a hot water system to accommodate the increase in volume of the water when it is heated"@en-gb ,
                                "http://bsdd.buildingsmart.org/#concept/details/1Lw1_wSbzFWe1SaTJeinCg"@en ;
                   rdfs:label "Expansion Tank"@en ,
                              "ekspansjon"@nb-no ;
                   rdfs:seeAlso ifc:IfcTankEnumType .


###  http://pi.pauwel.be/voc/distributionelement#Tank-FEEDANDEXPANSION
mep:Tank-FEEDANDEXPANSION rdf:type owl:Class ;
                          rdfs:subClassOf mep:Tank ;
                          rdfs:comment "http://bsdd.buildingsmart.org/#concept/details/371WHCLHb6vgWMDDSDFW4f"@en ;
                          rdfs:label "Feed And Expansion Tank"@en ,
                                     "mate og ekspansjonstank"@nb-no ;
                          rdfs:seeAlso ifc:IfcTankEnumType .


###  http://pi.pauwel.be/voc/distributionelement#Tank-PRESSUREVESSEL
mep:Tank-PRESSUREVESSEL rdf:type owl:Class ;
                        rdfs:subClassOf mep:Tank ;
                        rdfs:comment "http://bsdd.buildingsmart.org/#concept/details/3pBTMtMgH5UOIRcXURYkQd"@en ;
                        rdfs:label "Pressure Vessel"@en ,
                                   "trykktank"@nb-no ;
                        rdfs:seeAlso ifc:IfcTankEnumType .


###  http://pi.pauwel.be/voc/distributionelement#Tank-STORAGE
mep:Tank-STORAGE rdf:type owl:Class ;
                 rdfs:subClassOf mep:Tank ;
                 rdfs:comment "http://bsdd.buildingsmart.org/#concept/details/36ZG4Tdk1CARQ9FrH0BlZe"@en ;
                 rdfs:label "Storage Tank"@en ,
                            "lagringstank"@nb-no ;
                 rdfs:seeAlso ifc:IfcTankEnumType .


###  http://pi.pauwel.be/voc/distributionelement#Tank-VESSEL
mep:Tank-VESSEL rdf:type owl:Class ;
                rdfs:subClassOf mep:Tank ;
                rdfs:comment "an arbitrary closed tank type"@en ,
                             "an arbitrary closed tank type"@en-gb ,
                             "http://bsdd.buildingsmart.org/#concept/details/2rdBMMRl56p9qdnIOKnbwO"@en ;
                rdfs:label "Vessel"@en ,
                           "beholder"@nb-no ;
                rdfs:seeAlso ifc:IfcTankEnumType .


###  http://pi.pauwel.be/voc/distributionelement#Transformer
mep:Transformer rdf:type owl:Class ;
                rdfs:subClassOf mep:EnergyConversionDevice ;
                rdfs:comment "A artefact that transfers electric energy without change of frequency                "@en ,
                             "An inductive stationary device that transfers electrical energy from one circuit to another."@en ,
                             "Een statische energieomzetter die elektrische energie energie omzet zonder verandering van frequentie."@nl-nl ,
                             "Een toestel dat door elektromagnetische inductie één of meer veranderlijke stromen en spanningen omzet in één of meer verandelijke stromen en spanningen zonder dat voor de omzetting bewegende delen nodig zijn."@nl-nl ,
                             "Een transformator (veelal afgekort tot trafo (NL) of transfo (B)) is een statisch (d.w.z. zonder bewegende onderdelen) elektrisch apparaat, bestaande uit magnetisch gekoppelde spoelen. Stuurt men een veranderlijke stroom door een van de spoelen, de primaire spoel genoemd, dan wordt in de andere spoel(en), de secundaire, een spanning opgewekt."@nl-nl ,
                             "Elektrisch apparaat die elektrische wisselstroomenergie van een bepaald spanningsniveau en aantal fasen via magnetisch gekoppelde spoelen omzet in energie van een ander spanningsniveau, maar met dezelfde frequentie."@nl-nl ,
                             "Elektrisch apparaat waarmee spanning en stroom kunnen worden omgezet van hoge naar lage waarden. In de elektrotechniek een omzetter die elektrische wisselstroomenergie van een bepaald spanningsniveau en aantal fasen omzet in energie van een ander spanningsniveau, maar met dezelfde frequentie."@nl-nl ,
                             "http://bsdd.buildingsmart.org/#concept/details/1d7Az5cjf79B356TXokPOF"@en ,
                             "static piece of apparatus with two or more windings which, by electromagnetic induction, transforms a system of alternating voltage and current into another system of voltage and current usually of different values and at the same frequency for the purpose of transmitting electrical power"@en ,
                             "static piece of apparatus with two or more windings which, by electromagnetic induction, transforms a system of alternating voltage and current into another system of voltage and current usually of different values and at the same frequency for the purpose of transmitting electrical power. (NEN-EN-IEC 61558-1)"@en ;
                rdfs:label "Transformer"@en ,
                           "transformateur"@fr-fr ,
                           "transformator"@de-de ,
                           "transformator"@nb-no ,
                           "transformator"@nl-nl ;
                rdfs:seeAlso ifc:IfcTransformer .


###  http://pi.pauwel.be/voc/distributionelement#Transformer-CURRENT
mep:Transformer-CURRENT rdf:type owl:Class ;
                        rdfs:subClassOf mep:Transformer ;
                        rdfs:comment "a transformer that changes the current between circuits"@en ,
                                     "a transformer that changes the current between circuits"@en-gb ,
                                     "http://bsdd.buildingsmart.org/#concept/details/0S1LeIGoj1CwsRLj4IxJSx"@en ;
                        rdfs:label "Current Transformer"@en ,
                                   "strøm"@nb-no ;
                        rdfs:seeAlso ifc:IfcTransformerEnumType .


###  http://pi.pauwel.be/voc/distributionelement#Transformer-FREQUENCY
mep:Transformer-FREQUENCY rdf:type owl:Class ;
                          rdfs:subClassOf mep:Transformer ;
                          rdfs:comment "a transformer that changes the frequency between circuits"@en ,
                                       "a transformer that changes the frequency between circuits"@en-gb ,
                                       "http://bsdd.buildingsmart.org/#concept/details/1UAFNuQt5E0xPmuu4GQLrJ"@en ;
                          rdfs:label "Frequency Transformer"@en ,
                                     "frekvens"@nb-no ;
                          rdfs:seeAlso ifc:IfcTransformerEnumType .


###  http://pi.pauwel.be/voc/distributionelement#Transformer-INVERTER
mep:Transformer-INVERTER rdf:type owl:Class ;
                         rdfs:subClassOf mep:Transformer ;
                         rdfs:comment "device for the conversion of direct current (DC) to alternating current (AC)"@en ,
                                      "http://bsdd.buildingsmart.org/#concept/details/1JVDHhnQb3Hv0o3sTOfXt3"@en ;
                         rdfs:label "Inverter Transformer"@en ,
                                    "retter"@nb-no ;
                         rdfs:seeAlso ifc:IfcTransformerEnumType .


###  http://pi.pauwel.be/voc/distributionelement#Transformer-RECTIFIER
mep:Transformer-RECTIFIER rdf:type owl:Class ;
                          rdfs:subClassOf mep:Transformer ;
                          rdfs:comment "electric energy converter that changes single-phase or polyphase alternating electric currents to unidirectional current"@en ,
                                       "http://bsdd.buildingsmart.org/#concept/details/0J1BEZtan5FAXomnB0QhUR"@en ;
                          rdfs:label "Rectifier Transformer"@en ,
                                     "likeretter"@nb-no ,
                                     "likeretter - transformator"@nb-no ;
                          rdfs:seeAlso ifc:IfcTransformerEnumType .


###  http://pi.pauwel.be/voc/distributionelement#Transformer-VOLTAGE
mep:Transformer-VOLTAGE rdf:type owl:Class ;
                        rdfs:subClassOf mep:Transformer ;
                        rdfs:comment "a transformer that changes the voltage between circuits"@en ,
                                     "a transformer that changes the voltage between circuits"@en-gb ,
                                     "http://bsdd.buildingsmart.org/#concept/details/1_4pUL3mX9fwVKh_9lcz1S"@en ;
                        rdfs:label "Voltage Transformer"@en ,
                                   "spenning"@nb-no ;
                        rdfs:seeAlso ifc:IfcTransformerEnumType .


###  http://pi.pauwel.be/voc/distributionelement#TubeBundle
mep:TubeBundle rdf:type owl:Class ;
               rdfs:subClassOf mep:EnergyConversionDevice ;
               rdfs:comment "A device consisting of tubes and bundles of tubes used for heat transfer and contained typically within other energy conversion devices, such as a chiller or coil."@en ,
                            "An assembly of tubes constituting a part of a shell and tube heat exchanger. The tubes are in each end collected in a tube sheet.        "@en ,
                            "http://bsdd.buildingsmart.org/#concept/details/2KKY0IUEj0J9jguEJqOHcm"@en ;
               rdfs:label "Buizenregister"@nl-nl ,
                          "Faisceau tubulaire"@fr-fr ,
                          "Rohrbündel"@de-de ,
                          "Tube Bundle"@en ,
                          "rørbunt"@nb-no ;
               rdfs:seeAlso ifc:IfcTubeBundle .


###  http://pi.pauwel.be/voc/distributionelement#TubeBundle-FINNED
mep:TubeBundle-FINNED rdf:type owl:Class ;
                      rdfs:subClassOf mep:TubeBundle ;
                      rdfs:comment "http://bsdd.buildingsmart.org/#concept/details/300_kyP4z8lfGEZ8$LKgLE"@en ;
                      rdfs:label "Finned Tube Bundle"@en ,
                                 "ribberør"@nb-no ;
                      rdfs:seeAlso ifc:IfcTubeBundleEnumType .


###  http://pi.pauwel.be/voc/distributionelement#UnitaryControlElement
mep:UnitaryControlElement rdf:type owl:Class ;
                          rdfs:subClassOf mep:DistributionControlElement ;
                          rdfs:comment """A control element combines a number of control components into a single product, such as a thermostat or humidistat.
Provides a housing for an aggregation of control or electrical distribution elements that, in combination, perform a singular (unitary) purpose. Each item in the aggregation may have its own geometric representation and location."""@en ,
                                       "http://bsdd.buildingsmart.org/#concept/details/1K4LPg0kL5k8UuFp4BB3Q9"@en ;
                          rdfs:label "Einheitsregler"@de-de ,
                                     "Elément de contrôle unitaire"@fr-fr ,
                                     "Unitary Control Element"@en ,
                                     "enhetlig kontroll"@nb-no ;
                          rdfs:seeAlso ifc:IfcUnitaryControlElement .


###  http://pi.pauwel.be/voc/distributionelement#UnitaryControlElement-ALARMPANEL
mep:UnitaryControlElement-ALARMPANEL rdf:type owl:Class ;
                                     rdfs:subClassOf mep:UnitaryControlElement ;
                                     rdfs:comment "http://bsdd.buildingsmart.org/#concept/details/2E$a0foIL9GhqKHxJcRSkz"@en ;
                                     rdfs:label "Alarm Panel"@en ;
                                     rdfs:seeAlso ifc:IfcUnitaryControlElementEnumType .


###  http://pi.pauwel.be/voc/distributionelement#UnitaryControlElement-CONTROLPANEL
mep:UnitaryControlElement-CONTROLPANEL rdf:type owl:Class ;
                                       rdfs:subClassOf mep:UnitaryControlElement ;
                                       rdfs:comment "a control element at which devices that control or monitor the operation of a site, building or part of a building are located"@en ,
                                                    "a control element at which devices that control or monitor the operation of a site, building or part of a building are located"@en-gb ,
                                                    "http://bsdd.buildingsmart.org/#concept/details/0szSYD3cD3$ucQuwpURDzs"@en ;
                                       rdfs:label "Control Panel"@en ,
                                                  "kontrollpanel"@nb-no ;
                                       rdfs:seeAlso ifc:IfcUnitaryControlElementEnumType .


###  http://pi.pauwel.be/voc/distributionelement#UnitaryControlElement-GASDETECTIONPANEL
mep:UnitaryControlElement-GASDETECTIONPANEL rdf:type owl:Class ;
                                            rdfs:subClassOf mep:UnitaryControlElement ;
                                            rdfs:comment "http://bsdd.buildingsmart.org/#concept/details/26McOeRsjAPOMMV393Pkuv"@en ;
                                            rdfs:label "Gas Detection Panel"@en ;
                                            rdfs:seeAlso ifc:IfcUnitaryControlElementEnumType .


###  http://pi.pauwel.be/voc/distributionelement#UnitaryControlElement-HUMIDISTAT
mep:UnitaryControlElement-HUMIDISTAT rdf:type owl:Class ;
                                     rdfs:subClassOf mep:UnitaryControlElement ;
                                     rdfs:comment "a control element that senses and regulates the humidity of a system or space so that the humidity is maintained near a desired setpoint."@en ,
                                                  "http://bsdd.buildingsmart.org/#concept/details/3duRJz_NHBsO8tukebn0Br"@en ;
                                     rdfs:label "Humidistat"@en ,
                                                "hygrostat"@nb-no ;
                                     rdfs:seeAlso ifc:IfcUnitaryControlElementEnumType .


###  http://pi.pauwel.be/voc/distributionelement#UnitaryControlElement-INDICATORPANEL
mep:UnitaryControlElement-INDICATORPANEL rdf:type owl:Class ;
                                         rdfs:subClassOf mep:UnitaryControlElement ;
                                         rdfs:comment "http://bsdd.buildingsmart.org/#concept/details/3wAtS33ID4zuEOa3x02EIn"@en ,
                                                      "а control element at which equipment operational status, condition, safety state or other required parameters are indicated"@en ;
                                         rdfs:label "Indicator Panel"@en ,
                                                    "indikatorpanel"@nb-no ;
                                         rdfs:seeAlso ifc:IfcUnitaryControlElementEnumType .


###  http://pi.pauwel.be/voc/distributionelement#UnitaryControlElement-MIMICPANEL
mep:UnitaryControlElement-MIMICPANEL rdf:type owl:Class ;
                                     rdfs:subClassOf mep:UnitaryControlElement ;
                                     rdfs:comment "http://bsdd.buildingsmart.org/#concept/details/2gW6eFlD1A7Qnqh99Dspb0"@en ,
                                                  "а control element at which information that is available elsewhere is repeated or 'mimicked'"@en ,
                                                  "а control element at which information that is available elsewhere is repeated or 'mimicked'"@en-gb ;
                                     rdfs:label "Mimic Panel"@en ,
                                                "mimikkpanel"@nb-no ;
                                     rdfs:seeAlso ifc:IfcUnitaryControlElementEnumType .


###  http://pi.pauwel.be/voc/distributionelement#UnitaryControlElement-THERMOSTAT
mep:UnitaryControlElement-THERMOSTAT rdf:type owl:Class ;
                                     rdfs:subClassOf mep:UnitaryControlElement ;
                                     rdfs:comment "Is the component of a control system which regulates the temperature of a system so that the system's temperature is maintained near a desired set point temperature"@en ,
                                                  "Temperaturstyrt bryter"@nb-no ,
                                                  "http://bsdd.buildingsmart.org/#concept/details/3MCWw0I6yHuO00025QrE$V"@en ;
                                     rdfs:label "Thermostat"@en ,
                                                "termostat"@nb-no ;
                                     rdfs:seeAlso ifc:IfcUnitaryControlElementEnumType .


###  http://pi.pauwel.be/voc/distributionelement#UnitaryControlElement-WEATHERSTATION
mep:UnitaryControlElement-WEATHERSTATION rdf:type owl:Class ;
                                         rdfs:subClassOf mep:UnitaryControlElement ;
                                         rdfs:comment "a control element that senses multiple climate properties such as temperature, humidity, pressure, wind, and rain"@en ,
                                                      "a control element that senses multiple climate properties such as temperature, humidity, pressure, wind, and rain"@en-gb ,
                                                      "http://bsdd.buildingsmart.org/#concept/details/3d1EK0fY9CfwMNl1j5LmLc"@en ;
                                         rdfs:label "Weather Station"@en ,
                                                    "værstasjon"@nb-no ;
                                         rdfs:seeAlso ifc:IfcUnitaryControlElementEnumType .


###  http://pi.pauwel.be/voc/distributionelement#UnitaryEquipment
mep:UnitaryEquipment rdf:type owl:Class ;
                     rdfs:subClassOf mep:EnergyConversionDevice ;
                     rdfs:comment "A combined of a number of components into a single product, such as air handlers, pre-packaged rooftop air-conditioning units, heat pumps, and split systems."@en ,
                                  "http://bsdd.buildingsmart.org/#concept/details/0mUhAIpDb3mfYfYDW63M7U"@en ;
                     rdfs:label "Einbaufertige Anlage"@de-de ,
                                "Equipement unitaire"@fr-fr ,
                                "Unitary Equipment"@en ,
                                "enhetlig utstyr"@nb-no ;
                     rdfs:seeAlso ifc:IfcUnitaryEquipment .


###  http://pi.pauwel.be/voc/distributionelement#UnitaryEquipment-AIRCONDITIONINGUNIT
mep:UnitaryEquipment-AIRCONDITIONINGUNIT rdf:type owl:Class ;
                                         rdfs:subClassOf mep:UnitaryEquipment ;
                                         rdfs:comment "http://bsdd.buildingsmart.org/#concept/details/1PIU70CHzCMAt_h32UKgoE"@en ;
                                         rdfs:label "Air Conditioning Unit"@en ;
                                         rdfs:seeAlso ifc:IfcUnitaryEquipmentEnumType .


###  http://pi.pauwel.be/voc/distributionelement#UnitaryEquipment-AIRHANDLER
mep:UnitaryEquipment-AIRHANDLER rdf:type owl:Class ;
                                rdfs:subClassOf mep:UnitaryEquipment ;
                                rdfs:comment "http://bsdd.buildingsmart.org/#concept/details/1VnQL7ieb089ehb7syCaMo"@en ;
                                rdfs:label "Air Handler"@en ,
                                           "luftbehandling"@nb-no ;
                                rdfs:seeAlso ifc:IfcUnitaryEquipmentEnumType .


###  http://pi.pauwel.be/voc/distributionelement#UnitaryEquipment-DEHUMIDIFIER
mep:UnitaryEquipment-DEHUMIDIFIER rdf:type owl:Class ;
                                  rdfs:subClassOf mep:UnitaryEquipment ;
                                  rdfs:comment "a unitary packaged dehumidification unit. Note: units supporting multiple modes (dehumidification, cooling, and/or heating) should use AIRCONDITIONINGUNIT"@en ,
                                               "a unitary packaged dehumidification unit. Note: units supporting multiple modes (dehumidification, cooling, and/or heating) should use AIRCONDITIONINGUNIT"@en-gb ,
                                               "http://bsdd.buildingsmart.org/#concept/details/1fDG4loZb609HKaHBIkk_l"@en ;
                                  rdfs:label "Dehumidifier"@en ,
                                             "avfuktingsaggregat"@nb-no ;
                                  rdfs:seeAlso ifc:IfcUnitaryEquipmentEnumType .


###  http://pi.pauwel.be/voc/distributionelement#UnitaryEquipment-ROOFTOPUNIT
mep:UnitaryEquipment-ROOFTOPUNIT rdf:type owl:Class ;
                                 rdfs:subClassOf mep:UnitaryEquipment ;
                                 rdfs:comment "http://bsdd.buildingsmart.org/#concept/details/0yMK$zpZz2Ahk9sfb3u4e7"@en ,
                                              "unitary systems manufactured in various configurations providing single or multi-zone heating, cooling, and ventilation."@en ;
                                 rdfs:label "Rooftop Unit"@en ,
                                            "takenhet"@nb-no ;
                                 rdfs:seeAlso ifc:IfcUnitaryEquipmentEnumType .


###  http://pi.pauwel.be/voc/distributionelement#UnitaryEquipment-SPLITSYSTEM
mep:UnitaryEquipment-SPLITSYSTEM rdf:type owl:Class ;
                                 rdfs:subClassOf mep:UnitaryEquipment ;
                                 rdfs:comment "http://bsdd.buildingsmart.org/#concept/details/2iiBgNKl10ifd$UgILMf64"@en ;
                                 rdfs:label "Split System"@en ,
                                            "delt system"@nb-no ;
                                 rdfs:seeAlso ifc:IfcUnitaryEquipmentEnumType .


###  http://pi.pauwel.be/voc/distributionelement#Valve
mep:Valve rdf:type owl:Class ;
          rdfs:subClassOf mep:FlowController ;
          rdfs:comment "A flow control device used in a building services piping distribution system to control or modulate the flow of the fluid."@en ,
                       "An artefact used to control, i.e. permit, obstruct, regulate or divert a fluid stream.        "@en ,
                       "component isolating or controlling flow and pressure, e.g. isolating valve, control valve, pressure reducing valve, air valve, non-return valve, hydrant"@en ,
                       "http://bsdd.buildingsmart.org/#concept/details/3s7E9HsSHBXejc$aKaBr8N"@en ,
                       "komponent som isolerer eller kontrollerer vannføring og trykk, f.eks. stengeventil, kontrollventil, trykkreduksjonsventil, lufteventil, tilbakeslagsventil, brannventil/hydrant"@nb-no ;
          rdfs:label "Absperrarmatur; Ventil"@de-de ,
                     "Afsluiter"@nl-nl ,
                     "Armatur"@de-de ,
                     "Valve"@en ,
                     "Vanne"@fr-fr ,
                     "Ventil"@da ,
                     "Ventil"@de-de ,
                     "appareil de robinetterie"@fr-fr ,
                     "valve"@en ,
                     "vanne; valve"@fr-fr ,
                     "ventil"@nb-no ;
          rdfs:seeAlso ifc:IfcValve .


###  http://pi.pauwel.be/voc/distributionelement#Valve-AIRRELEASE
mep:Valve-AIRRELEASE rdf:type owl:Class ;
                     rdfs:subClassOf mep:Valve ;
                     rdfs:comment "http://bsdd.buildingsmart.org/#concept/details/3IEYICFuH8M9WXhUv2XVjI"@en ;
                     rdfs:label "Air Release"@en ;
                     rdfs:seeAlso ifc:IfcValveEnumType .


###  http://pi.pauwel.be/voc/distributionelement#Valve-ANTIVACUUM
mep:Valve-ANTIVACUUM rdf:type owl:Class ;
                     rdfs:subClassOf mep:Valve ;
                     rdfs:comment "http://bsdd.buildingsmart.org/#concept/details/3akkmqwTrDKhcl5Sgc6MbM"@en ;
                     rdfs:label "Antivacuum" ;
                     rdfs:seeAlso ifc:IfcValveEnumType .


###  http://pi.pauwel.be/voc/distributionelement#Valve-CHANGEOVER
mep:Valve-CHANGEOVER rdf:type owl:Class ;
                     rdfs:subClassOf mep:Valve ;
                     rdfs:comment "http://bsdd.buildingsmart.org/#concept/details/0EkRKqfjHD0PwOY11Ixaxp"@en ;
                     rdfs:label "Change Over"@en ;
                     rdfs:seeAlso ifc:IfcValveEnumType .


###  http://pi.pauwel.be/voc/distributionelement#Valve-CHECK
mep:Valve-CHECK rdf:type owl:Class ;
                rdfs:subClassOf mep:Valve ;
                rdfs:comment "http://bsdd.buildingsmart.org/#concept/details/39bvtEU9T7Kwb0mdT3F1M9"@en ;
                rdfs:label "Check"@en ;
                rdfs:seeAlso ifc:IfcValveEnumType .


###  http://pi.pauwel.be/voc/distributionelement#Valve-COMMISSIONING
mep:Valve-COMMISSIONING rdf:type owl:Class ;
                        rdfs:subClassOf mep:Valve ;
                        rdfs:comment "http://bsdd.buildingsmart.org/#concept/details/3YmvYjeBXElRSJyWt903HE"@en ;
                        rdfs:label "Commissioning" ;
                        rdfs:seeAlso ifc:IfcValveEnumType .


###  http://pi.pauwel.be/voc/distributionelement#Valve-DIVERTING
mep:Valve-DIVERTING rdf:type owl:Class ;
                    rdfs:subClassOf mep:Valve ;
                    rdfs:comment "http://bsdd.buildingsmart.org/#concept/details/0OsZoKWAP7BBEErvuwAY_x"@en ;
                    rdfs:label "Diverting"@en ;
                    rdfs:seeAlso ifc:IfcValveEnumType .


###  http://pi.pauwel.be/voc/distributionelement#Valve-DOUBLECHECK
mep:Valve-DOUBLECHECK rdf:type owl:Class ;
                      rdfs:subClassOf mep:Valve ;
                      rdfs:comment "http://bsdd.buildingsmart.org/#concept/details/2$M2cKJh50r9iXgcDblZLB"@en ;
                      rdfs:label "DoubleCheck"@en ;
                      rdfs:seeAlso ifc:IfcValveEnumType .


###  http://pi.pauwel.be/voc/distributionelement#Valve-DOUBLEREGULATING
mep:Valve-DOUBLEREGULATING rdf:type owl:Class ;
                           rdfs:subClassOf mep:Valve ;
                           rdfs:comment "http://bsdd.buildingsmart.org/#concept/details/2Y8s3cCGf3WAkyIwDxHfmt"@en ;
                           rdfs:label "Double Regulating"@en ;
                           rdfs:seeAlso ifc:IfcValveEnumType .


###  http://pi.pauwel.be/voc/distributionelement#Valve-DRAWOFFCOCK
mep:Valve-DRAWOFFCOCK rdf:type owl:Class ;
                      rdfs:subClassOf mep:Valve ;
                      rdfs:comment "http://bsdd.buildingsmart.org/#concept/details/1hIDIXF9r7MPfWQSquoEbq"@en ;
                      rdfs:label "Draw Off Cock"@en ;
                      rdfs:seeAlso ifc:IfcValveEnumType .


###  http://pi.pauwel.be/voc/distributionelement#Valve-FAUCET
mep:Valve-FAUCET rdf:type owl:Class ;
                 rdfs:subClassOf mep:Valve ;
                 rdfs:comment "http://bsdd.buildingsmart.org/#concept/details/2j7S2gFkr9VAAkDsk9ttBg"@en ;
                 rdfs:label "Faucet"@en ;
                 rdfs:seeAlso ifc:IfcValveEnumType .


###  http://pi.pauwel.be/voc/distributionelement#Valve-FLUSHING
mep:Valve-FLUSHING rdf:type owl:Class ;
                   rdfs:subClassOf mep:Valve ;
                   rdfs:comment "http://bsdd.buildingsmart.org/#concept/details/3tbXQW_znFmQVfKs3YhQZ_"@en ;
                   rdfs:label "Flushing"@en ;
                   rdfs:seeAlso ifc:IfcValveEnumType .


###  http://pi.pauwel.be/voc/distributionelement#Valve-GASCOCK
mep:Valve-GASCOCK rdf:type owl:Class ;
                  rdfs:subClassOf mep:Valve ;
                  rdfs:comment "http://bsdd.buildingsmart.org/#concept/details/0WwwuPsrfCgv8h5yWR3dKz"@en ;
                  rdfs:label "Gas Cock"@en ;
                  rdfs:seeAlso ifc:IfcValveEnumType .


###  http://pi.pauwel.be/voc/distributionelement#Valve-GASTAP
mep:Valve-GASTAP rdf:type owl:Class ;
                 rdfs:subClassOf mep:Valve ;
                 rdfs:comment "http://bsdd.buildingsmart.org/#concept/details/116lS7JG144hslqbHhbgkA"@en ;
                 rdfs:label "Gas Tap"@en ;
                 rdfs:seeAlso ifc:IfcValveEnumType .


###  http://pi.pauwel.be/voc/distributionelement#Valve-ISOLATING
mep:Valve-ISOLATING rdf:type owl:Class ;
                    rdfs:subClassOf mep:Valve ;
                    rdfs:comment "http://bsdd.buildingsmart.org/#concept/details/3fYepZO51AmflcVtRK9IVO"@en ;
                    rdfs:label "Isolating"@en ;
                    rdfs:seeAlso ifc:IfcValveEnumType .


###  http://pi.pauwel.be/voc/distributionelement#Valve-MIXING
mep:Valve-MIXING rdf:type owl:Class ;
                 rdfs:subClassOf mep:Valve ;
                 rdfs:comment "http://bsdd.buildingsmart.org/#concept/details/3cpFwtq7L1Owmcm7Yxvp05"@en ;
                 rdfs:label "Mixing"@en ;
                 rdfs:seeAlso ifc:IfcValveEnumType .


###  http://pi.pauwel.be/voc/distributionelement#Valve-PRESSUREREDUCING
mep:Valve-PRESSUREREDUCING rdf:type owl:Class ;
                           rdfs:subClassOf mep:Valve ;
                           rdfs:comment "http://bsdd.buildingsmart.org/#concept/details/1P7aHESGb1JxvdNIDc1D9J"@en ;
                           rdfs:label "Pressure Reducing"@en ;
                           rdfs:seeAlso ifc:IfcValveEnumType .


###  http://pi.pauwel.be/voc/distributionelement#Valve-PRESSURERELIEF
mep:Valve-PRESSURERELIEF rdf:type owl:Class ;
                         rdfs:subClassOf mep:Valve ;
                         rdfs:comment "http://bsdd.buildingsmart.org/#concept/details/0Si_BQgDr7f8BoS$bMsnAA"@en ;
                         rdfs:label "Pressure Relief"@en ;
                         rdfs:seeAlso ifc:IfcValveEnumType .


###  http://pi.pauwel.be/voc/distributionelement#Valve-REGULATING
mep:Valve-REGULATING rdf:type owl:Class ;
                     rdfs:subClassOf mep:Valve ;
                     rdfs:comment "http://bsdd.buildingsmart.org/#concept/details/2Y3yA_sy15NRRwfdI7LaxA"@en ;
                     rdfs:label "Regulating"@en ;
                     rdfs:seeAlso ifc:IfcValveEnumType .


###  http://pi.pauwel.be/voc/distributionelement#Valve-SAFETYCUTOFF
mep:Valve-SAFETYCUTOFF rdf:type owl:Class ;
                       rdfs:subClassOf mep:Valve ;
                       rdfs:comment "http://bsdd.buildingsmart.org/#concept/details/2cRQlX33L53gdVBEMFha9_"@en ;
                       rdfs:label "Safety Cut Off"@en ;
                       rdfs:seeAlso ifc:IfcValveEnumType .


###  http://pi.pauwel.be/voc/distributionelement#Valve-STEAMTRAP
mep:Valve-STEAMTRAP rdf:type owl:Class ;
                    rdfs:subClassOf mep:Valve ;
                    rdfs:comment "http://bsdd.buildingsmart.org/#concept/details/1IXcpzdwj4SgIc_5uXMgrX"@en ;
                    rdfs:label "Steam Trap"@en ;
                    rdfs:seeAlso ifc:IfcValveEnumType .


###  http://pi.pauwel.be/voc/distributionelement#Valve-STOPCOCK
mep:Valve-STOPCOCK rdf:type owl:Class ;
                   rdfs:subClassOf mep:Valve ;
                   rdfs:comment "http://bsdd.buildingsmart.org/#concept/details/0dmRan7HrB4v9gh4bkhOo3"@en ;
                   rdfs:label "Stop Cock"@en ;
                   rdfs:seeAlso ifc:IfcValveEnumType .


###  http://pi.pauwel.be/voc/distributionelement#WasteTerminal
mep:WasteTerminal rdf:type owl:Class ;
                  rdfs:subClassOf mep:FlowTerminal ;
                  rdfs:comment """A terminal for the purpose of collecting or intercepting waste from one or more sanitary terminals or other fluid waste generating equipment and discharging it into a single waste/drainage system.
Provides for all forms of trap and waste point that collects discharge from a sanitary terminal and discharges it into a waste/drainage subsystem or that collects waste from several terminals and passes it into a single waste/drainage subsystem. Includes the P and S traps from soil sanitary terminals, sinks, and basins as well as floor wastes and gully traps that provide collection points."""@en ,
                               "http://bsdd.buildingsmart.org/#concept/details/3IXcC8tvn4igBk64SckDjX"@en ;
                  rdfs:label "Ablauf"@de-de ,
                             "Abscheider"@de-de ,
                             "Stockage des déchets"@fr-fr ,
                             "Vuilwaterput"@nl-nl ,
                             "Waste Terminal"@en ,
                             "avfallsterminal"@nb-no ;
                  rdfs:seeAlso ifc:IfcWasteTerminal .


###  http://pi.pauwel.be/voc/distributionelement#WasteTerminal-FLOORTRAP
mep:WasteTerminal-FLOORTRAP rdf:type owl:Class ;
                            rdfs:subClassOf mep:WasteTerminal ;
                            rdfs:comment "http://bsdd.buildingsmart.org/#concept/details/33CCzm2CLBDfHv1gHVU8MC"@en ;
                            rdfs:label "Floor Trap"@en ;
                            rdfs:seeAlso ifc:IfcWasteTerminalEnumType .


###  http://pi.pauwel.be/voc/distributionelement#WasteTerminal-FLOORWASTE
mep:WasteTerminal-FLOORWASTE rdf:type owl:Class ;
                             rdfs:subClassOf mep:WasteTerminal ;
                             rdfs:comment "http://bsdd.buildingsmart.org/#concept/details/0Gg1lQtOn0jv4GqORpX2Y8"@en ;
                             rdfs:label "Floor Waste"@en ;
                             rdfs:seeAlso ifc:IfcWasteTerminalEnumType .


###  http://pi.pauwel.be/voc/distributionelement#WasteTerminal-GULLYSUMP
mep:WasteTerminal-GULLYSUMP rdf:type owl:Class ;
                            rdfs:subClassOf mep:WasteTerminal ;
                            rdfs:comment "http://bsdd.buildingsmart.org/#concept/details/0ZMLzB3o99aurJi3RGmMhG"@en ;
                            rdfs:label "Gully Sump"@en ;
                            rdfs:seeAlso ifc:IfcWasteTerminalEnumType .


###  http://pi.pauwel.be/voc/distributionelement#WasteTerminal-GULLYTRAP
mep:WasteTerminal-GULLYTRAP rdf:type owl:Class ;
                            rdfs:subClassOf mep:WasteTerminal ;
                            rdfs:comment "http://bsdd.buildingsmart.org/#concept/details/1WBoKi2av2NxTXpoB2QfO5"@en ;
                            rdfs:label "Gully Trap"@en ,
                                       "sluklås"@nb-no ;
                            rdfs:seeAlso ifc:IfcWasteTerminalEnumType .


###  http://pi.pauwel.be/voc/distributionelement#WasteTerminal-ROOFDRAIN
mep:WasteTerminal-ROOFDRAIN rdf:type owl:Class ;
                            rdfs:subClassOf mep:WasteTerminal ;
                            rdfs:comment "http://bsdd.buildingsmart.org/#concept/details/0Xkj0nlvX689aFUVxq3IMM"@en ,
                                         "pipe fitting, set into the roof, that collects rainwater for discharge into the rainwater system."@en ;
                            rdfs:label "Roof Drain"@en ,
                                       "taksluk"@nb-no ;
                            rdfs:seeAlso ifc:IfcWasteTerminalEnumType .


###  http://pi.pauwel.be/voc/distributionelement#WasteTerminal-WASTEDISPOSALUNIT
mep:WasteTerminal-WASTEDISPOSALUNIT rdf:type owl:Class ;
                                    rdfs:subClassOf mep:WasteTerminal ;
                                    rdfs:comment "electrically operated device that reduces kitchen or other waste into fragments small enough to be flushed into a drainage system."@en ,
                                                 "http://bsdd.buildingsmart.org/#concept/details/0khvv6MsL5DxzEnCFiP5mr"@en ;
                                    rdfs:label "Waste Disposal Unit"@en ,
                                               "avfallsenhet"@nb-no ;
                                    rdfs:seeAlso ifc:IfcWasteTerminalEnumType .


###  http://pi.pauwel.be/voc/distributionelement#WasteTerminal-WASTETRAP
mep:WasteTerminal-WASTETRAP rdf:type owl:Class ;
                            rdfs:subClassOf mep:WasteTerminal ;
                            rdfs:comment "http://bsdd.buildingsmart.org/#concept/details/1JPv81z_531vDlQ02VFI9a"@en ;
                            rdfs:label "Waste Trap"@en ,
                                       "vannlås"@nb-no ;
                            rdfs:seeAlso ifc:IfcWasteTerminalEnumType .


#################################################################
#    Individuals
#################################################################

###  http://pi.pauwel.be/voc/distributionelement#MEP
<http://pi.pauwel.be/voc/distributionelement#MEP> rdf:type owl:NamedIndividual ,
                                            voaf:Vocabulary .
